<?xml version="1.0"?><rdf:RDF 	xmlns:rdf="http://www.w3.org/1999/02/22-rdf-syntax-ns#" 	xmlns:skos="http://www.w3.org/2004/02/skos/core#" 	xmlns:dc="http://purl.org/dc/terms/" 	xmlns:foaf="http://xmlns.com/foaf/0.1/" 	xmlns:cito="http://purl.org/net/cito/"> <skos:Concept rdf:about="http://cognitiveatlas.org/id/trm_4a3fd79d09b6d"> <dc:identifier>trm_4a3fd79d09b6d</dc:identifier>
		<dc:Title>Cognitive Atlas : Lexicon : backward masking</dc:Title>
		<dc:Description>RDF output for 'backward masking'</dc:Description>
		<dc:Type>InteractiveResource</dc:Type>
		<dc:Publisher>Cognitive Atlas</dc:Publisher>
		<dc:Creator>Cognitive Atlas RDF Generator</dc:Creator>
		<dc:Contributor>Brenda Gregory</dc:Contributor>
		<dc:Date>2011-04-28 16:12:37</dc:Date>
		<dc:Format>text/rdf</dc:Format>
		<dc:Language>en</dc:Language>
		<skos:editorialNote>Generated by testgen.php on Thu Jun 9 14:25:24 PDT 2011.</skos:editorialNote>
		<skos:historyNote>Revision 3: 2 previous definitions.</skos:historyNote>
		<skos:changeNote>See http://cognitiveatlas.org/id/trm_4a3fd79d09b6d for complete revision history.</skos:changeNote>
		<skos:scopeNote>http://www.w3.org/2004/02/skos/core#Concept</skos:scopeNote>
		<skos:Note>SKOS properties defined in http://www.w3.org/TR/skos-primer/#secrel</skos:Note>
		<skos:inScheme rdf:resource="http://cognitiveatlas.org/tasks/"/>
		<skos:definition>a phenomenon wherein presenting one stimulus (a &#34;mask&#34; or &#34;masking stimulus&#34;) immediately after another brief (≤ 50 ms) &#34;target&#34; stimulus leads to a failure to consciously perceive the first stimulus.</skos:definition>
		<skos:prefLabel>backward masking</skos:prefLabel>
		<skos:altLabel></skos:altLabel>
</skos:Concept><skos:Concept rdf:about="http://cognitiveatlas.org/id/trm_4a3fd79d0b3d7"> <dc:identifier>trm_4a3fd79d0b3d7</dc:identifier>
		<dc:Title>Cognitive Atlas : Lexicon : trace conditioning</dc:Title>
		<dc:Description>RDF output for 'trace conditioning'</dc:Description>
		<dc:Type>InteractiveResource</dc:Type>
		<dc:Publisher>Cognitive Atlas</dc:Publisher>
		<dc:Creator>Cognitive Atlas RDF Generator</dc:Creator>
		<dc:Contributor>Brenda Gregory</dc:Contributor>
		<dc:Date>2011-04-29 10:51:16</dc:Date>
		<dc:Format>text/rdf</dc:Format>
		<dc:Language>en</dc:Language>
		<skos:editorialNote>Generated by testgen.php on Thu Jun 9 14:25:24 PDT 2011.</skos:editorialNote>
		<skos:historyNote>Revision 3: 2 previous definitions.</skos:historyNote>
		<skos:changeNote>See http://cognitiveatlas.org/id/trm_4a3fd79d0b3d7 for complete revision history.</skos:changeNote>
		<skos:scopeNote>http://www.w3.org/2004/02/skos/core#Concept</skos:scopeNote>
		<skos:Note>SKOS properties defined in http://www.w3.org/TR/skos-primer/#secrel</skos:Note>
		<skos:inScheme rdf:resource="http://cognitiveatlas.org/tasks/"/>
		<skos:definition>a form of classical conditioning in which the presentation of the conditioned stimulus and the unconditioned stimulus is separated in time by an interstimulus interval.</skos:definition>
		<skos:prefLabel>trace conditioning</skos:prefLabel>
		<skos:altLabel></skos:altLabel>
		<cito:citesForInformation rdf:resource="http://cognitiveatlas.org/citation/id/cit_4dbaf9ccb868b"/>
</skos:Concept><skos:Concept rdf:about="http://cognitiveatlas.org/id/trm_4af89b3a925ca"> <dc:identifier>trm_4af89b3a925ca</dc:identifier>
		<dc:Title>Cognitive Atlas : Lexicon : Vandenberg &amp; Kuse Tasks</dc:Title>
		<dc:Description>RDF output for 'Vandenberg &amp; Kuse Tasks'</dc:Description>
		<dc:Type>InteractiveResource</dc:Type>
		<dc:Publisher>Cognitive Atlas</dc:Publisher>
		<dc:Creator>Cognitive Atlas RDF Generator</dc:Creator>
		<dc:Contributor>Christian Battista</dc:Contributor>
		<dc:Date>2009-11-09 14:44:10</dc:Date>
		<dc:Format>text/rdf</dc:Format>
		<dc:Language>en</dc:Language>
		<skos:editorialNote>Generated by testgen.php on Thu Jun 9 14:25:24 PDT 2011.</skos:editorialNote>
		<skos:historyNote>No previous definition revisions.</skos:historyNote>
		<skos:changeNote>This is the first and only definition provided.</skos:changeNote>
		<skos:scopeNote>http://www.w3.org/2004/02/skos/core#Concept</skos:scopeNote>
		<skos:Note>SKOS properties defined in http://www.w3.org/TR/skos-primer/#secrel</skos:Note>
		<skos:inScheme rdf:resource="http://cognitiveatlas.org/tasks/"/>
		<skos:definition>Paper and pencil Test of mental rotation ability.  Participants must are presented with four 3-D block figures and must select 2 from the group which match a reference figure.  This test is administered under time contraints.  A male advantage is typically seen on this type of task, as measured by test accuracy.</skos:definition>
		<skos:prefLabel>Vandenberg &amp; Kuse Tasks</skos:prefLabel>
		<skos:altLabel></skos:altLabel>
		<cito:citesForInformation rdf:resource="http://cognitiveatlas.org/citation/id/cit_4af89b79c6709"/>
</skos:Concept><skos:Concept rdf:about="http://cognitiveatlas.org/id/trm_4b1968619b00b"> <dc:identifier>trm_4b1968619b00b</dc:identifier>
		<dc:Title>Cognitive Atlas : Lexicon : Color-word Stroop Task</dc:Title>
		<dc:Description>RDF output for 'Color-word Stroop Task'</dc:Description>
		<dc:Type>InteractiveResource</dc:Type>
		<dc:Publisher>Cognitive Atlas</dc:Publisher>
		<dc:Creator>Cognitive Atlas RDF Generator</dc:Creator>
		<dc:Contributor>System Administrator</dc:Contributor>
		<dc:Date>2009-12-04 11:52:20</dc:Date>
		<dc:Format>text/rdf</dc:Format>
		<dc:Language>en</dc:Language>
		<skos:editorialNote>Generated by testgen.php on Thu Jun 9 14:25:24 PDT 2011.</skos:editorialNote>
		<skos:historyNote>Revision 2: 1 previous definitions.</skos:historyNote>
		<skos:changeNote>See http://cognitiveatlas.org/id/trm_4b1968619b00b for complete revision history.</skos:changeNote>
		<skos:scopeNote>http://www.w3.org/2004/02/skos/core#Concept</skos:scopeNote>
		<skos:Note>SKOS properties defined in http://www.w3.org/TR/skos-primer/#secrel</skos:Note>
		<skos:inScheme rdf:resource="http://cognitiveatlas.org/tasks/"/>
		<skos:definition>A task in which single words (including names of colors) are presented in colored ink, and the subject is asked to name the color of the ink as quickly as possible. The ink color may either match or conflict with the color name. Accuracy and response time are measured.</skos:definition>
		<skos:prefLabel>Color-word Stroop Task</skos:prefLabel>
		<skos:altLabel></skos:altLabel>
		<skos:related rdf:resource="http://cognitiveatlas.org/id/trm_4a3fd79d0af66"/>
		<skos:related rdf:resource="http://cognitiveatlas.org/id/trm_4a3fd79d0af66"/>
		<skos:related rdf:resource="http://cognitiveatlas.org/id/trm_4a3fd79d0af66"/>
		<skos:related rdf:resource="http://cognitiveatlas.org/id/tsk_4a57abb949e27"/>
		<skos:related rdf:resource="http://cognitiveatlas.org/id/tsk_4a57abb949e27"/>
		<skos:example>Color-word Stroop Task is descended from Stroop task</skos:example>
		<skos:example>Color-word Stroop Task is a narrower synonym of Stroop task</skos:example>
		<skos:example>response inhibition is measured by the contrast of Incongruent trials in the Color-word Stroop Task</skos:example>
		<skos:example>response inhibition is measured by the contrast of Incongruent - Congruent trials in the Color-word Stroop Task</skos:example>
		<skos:example>response inhibition is measured by the contrast of Incongruent - Neutral trials in the Color-word Stroop Task</skos:example>
		<cito:citesForInformation rdf:resource="http://cognitiveatlas.org/citation/id/cit_4b1968a44c363"/>
		<cito:citesForInformation rdf:resource="http://cognitiveatlas.org/citation/id/cit_4de7ba5e5f0ff"/>
</skos:Concept><skos:Concept rdf:about="http://cognitiveatlas.org/id/trm_4b4a537644d76"> <dc:identifier>trm_4b4a537644d76</dc:identifier>
		<dc:Title>Cognitive Atlas : Lexicon : Continuous Performance Task</dc:Title>
		<dc:Description>RDF output for 'Continuous Performance Task'</dc:Description>
		<dc:Type>InteractiveResource</dc:Type>
		<dc:Publisher>Cognitive Atlas</dc:Publisher>
		<dc:Creator>Cognitive Atlas RDF Generator</dc:Creator>
		<dc:Contributor>Russ Poldrack</dc:Contributor>
		<dc:Date>2010-01-10 14:23:50</dc:Date>
		<dc:Format>text/rdf</dc:Format>
		<dc:Language>en</dc:Language>
		<skos:editorialNote>Generated by testgen.php on Thu Jun 9 14:25:24 PDT 2011.</skos:editorialNote>
		<skos:historyNote>No previous definition revisions.</skos:historyNote>
		<skos:changeNote>This is the first and only definition provided.</skos:changeNote>
		<skos:scopeNote>http://www.w3.org/2004/02/skos/core#Concept</skos:scopeNote>
		<skos:Note>SKOS properties defined in http://www.w3.org/TR/skos-primer/#secrel</skos:Note>
		<skos:inScheme rdf:resource="http://cognitiveatlas.org/tasks/"/>
		<skos:definition>A task in which subjects are presented with a stream of letters, and must respond to one of the letters and refrain from responding to any other letters.</skos:definition>
		<skos:prefLabel>Continuous Performance Task</skos:prefLabel>
		<skos:altLabel></skos:altLabel>
		<skos:related rdf:resource="http://cognitiveatlas.org/id/tsk_4a57abb949bcd"/>
		<skos:related rdf:resource="http://cognitiveatlas.org/id/trm_4c40d22c8a69d"/>
		<skos:related rdf:resource="http://cognitiveatlas.org/id/trm_4a3fd79d0b5ef"/>
		<skos:example>n-back task is descended from Continuous Performance Task</skos:example>
		<skos:example>CPT is an exact synonym of Continuous Performance Task</skos:example>
		<skos:example>attentional focusing is measured by the contrast of Target trials in the Continuous Performance Task</skos:example>
		<cito:citesForInformation rdf:resource="http://cognitiveatlas.org/citation/id/cit_4b50c39646c37"/>
		<cito:citesForInformation rdf:resource="http://cognitiveatlas.org/citation/id/cit_4de7c16c78382"/>
		<cito:citesForInformation rdf:resource="http://cognitiveatlas.org/citation/id/cit_4de7c139bf72e"/>
</skos:Concept><skos:Concept rdf:about="http://cognitiveatlas.org/id/trm_4b4a5ddfb90d0"> <dc:identifier>trm_4b4a5ddfb90d0</dc:identifier>
		<dc:Title>Cognitive Atlas : Lexicon : delayed recognition task</dc:Title>
		<dc:Description>RDF output for 'delayed recognition task'</dc:Description>
		<dc:Type>InteractiveResource</dc:Type>
		<dc:Publisher>Cognitive Atlas</dc:Publisher>
		<dc:Creator>Cognitive Atlas RDF Generator</dc:Creator>
		<dc:Contributor>Russ Poldrack</dc:Contributor>
		<dc:Date>2010-01-10 15:08:15</dc:Date>
		<dc:Format>text/rdf</dc:Format>
		<dc:Language>en</dc:Language>
		<skos:editorialNote>Generated by testgen.php on Thu Jun 9 14:25:24 PDT 2011.</skos:editorialNote>
		<skos:historyNote>No previous definition revisions.</skos:historyNote>
		<skos:changeNote>This is the first and only definition provided.</skos:changeNote>
		<skos:scopeNote>http://www.w3.org/2004/02/skos/core#Concept</skos:scopeNote>
		<skos:Note>SKOS properties defined in http://www.w3.org/TR/skos-primer/#secrel</skos:Note>
		<skos:inScheme rdf:resource="http://cognitiveatlas.org/tasks/"/>
		<skos:definition>The subject is presented with a set of stimuli called the target set, and must maintain those stimuli over a delay.  A probe appears after the delay, and the subject must respond whether the probe was in the target set.</skos:definition>
		<skos:prefLabel>delayed recognition task</skos:prefLabel>
		<skos:altLabel></skos:altLabel>
</skos:Concept><skos:Concept rdf:about="http://cognitiveatlas.org/id/trm_4b65e5e2ab3ca"> <dc:identifier>trm_4b65e5e2ab3ca</dc:identifier>
		<dc:Title>Cognitive Atlas : Lexicon : word-picture verification task</dc:Title>
		<dc:Description>RDF output for 'word-picture verification task'</dc:Description>
		<dc:Type>InteractiveResource</dc:Type>
		<dc:Publisher>Cognitive Atlas</dc:Publisher>
		<dc:Creator>Cognitive Atlas RDF Generator</dc:Creator>
		<dc:Contributor>Joseph Devlin</dc:Contributor>
		<dc:Date>2010-01-31 12:19:46</dc:Date>
		<dc:Format>text/rdf</dc:Format>
		<dc:Language>en</dc:Language>
		<skos:editorialNote>Generated by testgen.php on Thu Jun 9 14:25:24 PDT 2011.</skos:editorialNote>
		<skos:historyNote>No previous definition revisions.</skos:historyNote>
		<skos:changeNote>This is the first and only definition provided.</skos:changeNote>
		<skos:scopeNote>http://www.w3.org/2004/02/skos/core#Concept</skos:scopeNote>
		<skos:Note>SKOS properties defined in http://www.w3.org/TR/skos-primer/#secrel</skos:Note>
		<skos:inScheme rdf:resource="http://cognitiveatlas.org/tasks/"/>
		<skos:definition>is an experimental paradigm where a picture of an object is presented along with either an auditory or written word and participants indicate whether the word and the picture refer to the same concept.  It is typically used as a test of semantic memory integrity.</skos:definition>
		<skos:prefLabel>word-picture verification task</skos:prefLabel>
		<skos:altLabel></skos:altLabel>
</skos:Concept><skos:Concept rdf:about="http://cognitiveatlas.org/id/trm_4b7497a289534"> <dc:identifier>trm_4b7497a289534</dc:identifier>
		<dc:Title>Cognitive Atlas : Lexicon : Block Design Test</dc:Title>
		<dc:Description>RDF output for 'Block Design Test'</dc:Description>
		<dc:Type>InteractiveResource</dc:Type>
		<dc:Publisher>Cognitive Atlas</dc:Publisher>
		<dc:Creator>Cognitive Atlas RDF Generator</dc:Creator>
		<dc:Contributor>Deanna Lau</dc:Contributor>
		<dc:Date>2010-02-11 15:49:54</dc:Date>
		<dc:Format>text/rdf</dc:Format>
		<dc:Language>en</dc:Language>
		<skos:editorialNote>Generated by testgen.php on Thu Jun 9 14:25:24 PDT 2011.</skos:editorialNote>
		<skos:historyNote>No previous definition revisions.</skos:historyNote>
		<skos:changeNote>This is the first and only definition provided.</skos:changeNote>
		<skos:scopeNote>http://www.w3.org/2004/02/skos/core#Concept</skos:scopeNote>
		<skos:Note>SKOS properties defined in http://www.w3.org/TR/skos-primer/#secrel</skos:Note>
		<skos:inScheme rdf:resource="http://cognitiveatlas.org/tasks/"/>
		<skos:definition>The Block Design is a subtest of Perceptual Reasoning index of the Wechsler Adult Intelligence Scale IV. The Block Design test measures spatial perception, visual abstract processing, and problem solving.</skos:definition>
		<skos:prefLabel>Block Design Test</skos:prefLabel>
		<skos:altLabel></skos:altLabel>
		<skos:related rdf:resource="http://cognitiveatlas.org/id/trm_4b82c75498408"/>
		<skos:related rdf:resource="http://cognitiveatlas.org/id/tsk_4a57abb949f12"/>
		<skos:example>Block Design Test is descended from Wechsler Adult Intelligence Scale - Revised</skos:example>
		<skos:example>Central Coherence is measured by the contrast of Unsegmented blocks trials in the Block Design Test</skos:example>
		<cito:citesForInformation rdf:resource="http://cognitiveatlas.org/citation/id/cit_4de680a224fcb"/>
		<cito:citesForInformation rdf:resource="http://cognitiveatlas.org/citation/id/cit_4de6814c280be"/>
		<cito:citesForInformation rdf:resource="http://cognitiveatlas.org/citation/id/cit_4de68240df295"/>
</skos:Concept><skos:Concept rdf:about="http://cognitiveatlas.org/id/trm_4b749b8829eee"> <dc:identifier>trm_4b749b8829eee</dc:identifier>
		<dc:Title>Cognitive Atlas : Lexicon : Embedded Figures Test</dc:Title>
		<dc:Description>RDF output for 'Embedded Figures Test'</dc:Description>
		<dc:Type>InteractiveResource</dc:Type>
		<dc:Publisher>Cognitive Atlas</dc:Publisher>
		<dc:Creator>Cognitive Atlas RDF Generator</dc:Creator>
		<dc:Contributor>Deanna Lau</dc:Contributor>
		<dc:Date>2010-02-11 16:06:32</dc:Date>
		<dc:Format>text/rdf</dc:Format>
		<dc:Language>en</dc:Language>
		<skos:editorialNote>Generated by testgen.php on Thu Jun 9 14:25:24 PDT 2011.</skos:editorialNote>
		<skos:historyNote>No previous definition revisions.</skos:historyNote>
		<skos:changeNote>This is the first and only definition provided.</skos:changeNote>
		<skos:scopeNote>http://www.w3.org/2004/02/skos/core#Concept</skos:scopeNote>
		<skos:Note>SKOS properties defined in http://www.w3.org/TR/skos-primer/#secrel</skos:Note>
		<skos:inScheme rdf:resource="http://cognitiveatlas.org/tasks/"/>
		<skos:definition>In the embedded Figures Test, the research participant is shown a complex background figure and asked to describe it. After this, the participant is shown a target (such as the outline of a triangle) and asked to locate the target amid the background figure.</skos:definition>
		<skos:prefLabel>Embedded Figures Test</skos:prefLabel>
		<skos:altLabel></skos:altLabel>
		<skos:related rdf:resource="http://cognitiveatlas.org/id/trm_4b82c75498408"/>
		<skos:related rdf:resource="http://cognitiveatlas.org/id/trm_4b82c75498408"/>
		<skos:related rdf:resource="http://cognitiveatlas.org/id/trm_4a3fd79d0a81b"/>
		<skos:related rdf:resource="http://cognitiveatlas.org/id/trm_4a3fd79d0a81b"/>
		<skos:related rdf:resource="http://cognitiveatlas.org/id/trm_4a3fd79d0b507"/>
		<skos:related rdf:resource="http://cognitiveatlas.org/id/trm_4a3fd79d0b507"/>
		<skos:example>Central Coherence is measured by the contrast of Segmented blocks trials in the Embedded Figures Test</skos:example>
		<skos:example>Central Coherence is measured by the contrast of Unsegmented blocks trials in the Embedded Figures Test</skos:example>
		<skos:example>logical reasoning is measured by the contrast of Segmented blocks trials in the Embedded Figures Test</skos:example>
		<skos:example>logical reasoning is measured by the contrast of Unsegmented blocks trials in the Embedded Figures Test</skos:example>
		<skos:example>visuospatial sketch pad is measured by the contrast of Segmented blocks trials in the Embedded Figures Test</skos:example>
		<skos:example>visuospatial sketch pad is measured by the contrast of Unsegmented blocks trials in the Embedded Figures Test</skos:example>
		<cito:citesForInformation rdf:resource="http://cognitiveatlas.org/citation/id/cit_4de9659d6844b"/>
		<cito:citesForInformation rdf:resource="http://cognitiveatlas.org/citation/id/cit_4de9667a84427"/>
</skos:Concept><skos:Concept rdf:about="http://cognitiveatlas.org/id/trm_4b75ea4ddd896"> <dc:identifier>trm_4b75ea4ddd896</dc:identifier>
		<dc:Title>Cognitive Atlas : Lexicon : Same-Different Task</dc:Title>
		<dc:Description>RDF output for 'Same-Different Task'</dc:Description>
		<dc:Type>InteractiveResource</dc:Type>
		<dc:Publisher>Cognitive Atlas</dc:Publisher>
		<dc:Creator>Cognitive Atlas RDF Generator</dc:Creator>
		<dc:Contributor>Deanna Lau</dc:Contributor>
		<dc:Date>2010-02-12 15:54:53</dc:Date>
		<dc:Format>text/rdf</dc:Format>
		<dc:Language>en</dc:Language>
		<skos:editorialNote>Generated by testgen.php on Thu Jun 9 14:25:24 PDT 2011.</skos:editorialNote>
		<skos:historyNote>No previous definition revisions.</skos:historyNote>
		<skos:changeNote>This is the first and only definition provided.</skos:changeNote>
		<skos:scopeNote>http://www.w3.org/2004/02/skos/core#Concept</skos:scopeNote>
		<skos:Note>SKOS properties defined in http://www.w3.org/TR/skos-primer/#secrel</skos:Note>
		<skos:inScheme rdf:resource="http://cognitiveatlas.org/tasks/"/>
		<skos:definition>A task which assesses shifting attention. In the computerized version of this task, three spaceships appear on a screen and the participant must determine if the spaceships are all different or all the same. The spaceships can differ in color, size, or shape type. There are three levels of difficulty.  In the first level, the spaceships must all be identical to be considered the same. In the second level of difficulty, the spaceships are considered the same even if they only share two qualities, and in the third difficulty level, the spaceships only need to share one quality to be considered the same. Auditory feedback is given after each response notifying the child whether their answer was correct. </skos:definition>
		<skos:prefLabel>Same-Different Task</skos:prefLabel>
		<skos:altLabel></skos:altLabel>
</skos:Concept><skos:Concept rdf:about="http://cognitiveatlas.org/id/trm_4b843655d5d75"> <dc:identifier>trm_4b843655d5d75</dc:identifier>
		<dc:Title>Cognitive Atlas : Lexicon : Chimeric Animal Stroop Task</dc:Title>
		<dc:Description>RDF output for 'Chimeric Animal Stroop Task'</dc:Description>
		<dc:Type>InteractiveResource</dc:Type>
		<dc:Publisher>Cognitive Atlas</dc:Publisher>
		<dc:Creator>Cognitive Atlas RDF Generator</dc:Creator>
		<dc:Contributor>Deanna Lau</dc:Contributor>
		<dc:Date>2010-02-23 12:11:01</dc:Date>
		<dc:Format>text/rdf</dc:Format>
		<dc:Language>en</dc:Language>
		<skos:editorialNote>Generated by testgen.php on Thu Jun 9 14:25:24 PDT 2011.</skos:editorialNote>
		<skos:historyNote>No previous definition revisions.</skos:historyNote>
		<skos:changeNote>This is the first and only definition provided.</skos:changeNote>
		<skos:scopeNote>http://www.w3.org/2004/02/skos/core#Concept</skos:scopeNote>
		<skos:Note>SKOS properties defined in http://www.w3.org/TR/skos-primer/#secrel</skos:Note>
		<skos:inScheme rdf:resource="http://cognitiveatlas.org/tasks/"/>
		<skos:definition>A task in which participants are shown pictures of chimeric animals (such as a duck&#39;s head attached to a cow&#39;s body) and asked to name animal that the head belongs to while ignoring the identity of the body, or vice versa.  </skos:definition>
		<skos:prefLabel>Chimeric Animal Stroop Task</skos:prefLabel>
		<skos:altLabel></skos:altLabel>
		<skos:related rdf:resource="http://cognitiveatlas.org/id/trm_4a3fd79d0a6ad"/>
		<skos:related rdf:resource="http://cognitiveatlas.org/id/tsk_4a57abb949e27"/>
		<skos:example>Chimeric Animal Stroop Task is descended from Stroop task</skos:example>
		<skos:example>interference is measured by the contrast of Incongruent trials in the Chimeric Animal Stroop Task</skos:example>
		<cito:citesForInformation rdf:resource="http://cognitiveatlas.org/citation/id/cit_4de6bb4540504"/>
</skos:Concept><skos:Concept rdf:about="http://cognitiveatlas.org/id/trm_4b86c2e871b14"> <dc:identifier>trm_4b86c2e871b14</dc:identifier>
		<dc:Title>Cognitive Atlas : Lexicon : Rapid Automatized Naming Test</dc:Title>
		<dc:Description>RDF output for 'Rapid Automatized Naming Test'</dc:Description>
		<dc:Type>InteractiveResource</dc:Type>
		<dc:Publisher>Cognitive Atlas</dc:Publisher>
		<dc:Creator>Cognitive Atlas RDF Generator</dc:Creator>
		<dc:Contributor>Deanna Lau</dc:Contributor>
		<dc:Date>2010-02-25 10:35:20</dc:Date>
		<dc:Format>text/rdf</dc:Format>
		<dc:Language>en</dc:Language>
		<skos:editorialNote>Generated by testgen.php on Thu Jun 9 14:25:24 PDT 2011.</skos:editorialNote>
		<skos:historyNote>No previous definition revisions.</skos:historyNote>
		<skos:changeNote>This is the first and only definition provided.</skos:changeNote>
		<skos:scopeNote>http://www.w3.org/2004/02/skos/core#Concept</skos:scopeNote>
		<skos:Note>SKOS properties defined in http://www.w3.org/TR/skos-primer/#secrel</skos:Note>
		<skos:inScheme rdf:resource="http://cognitiveatlas.org/tasks/"/>
		<skos:definition>A task which involves rapidly naming a series of color blocks, letters, and pictures. </skos:definition>
		<skos:prefLabel>Rapid Automatized Naming Test</skos:prefLabel>
		<skos:altLabel></skos:altLabel>
</skos:Concept><skos:Concept rdf:about="http://cognitiveatlas.org/id/trm_4b86c473a7166"> <dc:identifier>trm_4b86c473a7166</dc:identifier>
		<dc:Title>Cognitive Atlas : Lexicon : Underlining Test</dc:Title>
		<dc:Description>RDF output for 'Underlining Test'</dc:Description>
		<dc:Type>InteractiveResource</dc:Type>
		<dc:Publisher>Cognitive Atlas</dc:Publisher>
		<dc:Creator>Cognitive Atlas RDF Generator</dc:Creator>
		<dc:Contributor>Deanna Lau</dc:Contributor>
		<dc:Date>2010-02-25 10:41:55</dc:Date>
		<dc:Format>text/rdf</dc:Format>
		<dc:Language>en</dc:Language>
		<skos:editorialNote>Generated by testgen.php on Thu Jun 9 14:25:24 PDT 2011.</skos:editorialNote>
		<skos:historyNote>No previous definition revisions.</skos:historyNote>
		<skos:changeNote>This is the first and only definition provided.</skos:changeNote>
		<skos:scopeNote>http://www.w3.org/2004/02/skos/core#Concept</skos:scopeNote>
		<skos:Note>SKOS properties defined in http://www.w3.org/TR/skos-primer/#secrel</skos:Note>
		<skos:inScheme rdf:resource="http://cognitiveatlas.org/tasks/"/>
		<skos:definition>This test involves finding and underlining stimuli that are among other stimuli.  There are four conditions of the test: finding and underlining letters among other letters, drawings among other drawings, real words among nonsense letter strings, and then specific nonsense words among others.  </skos:definition>
		<skos:prefLabel>Underlining Test</skos:prefLabel>
		<skos:altLabel></skos:altLabel>
</skos:Concept><skos:Concept rdf:about="http://cognitiveatlas.org/id/trm_4b86c55f3d5df"> <dc:identifier>trm_4b86c55f3d5df</dc:identifier>
		<dc:Title>Cognitive Atlas : Lexicon : WISC-R Mazes</dc:Title>
		<dc:Description>RDF output for 'WISC-R Mazes'</dc:Description>
		<dc:Type>InteractiveResource</dc:Type>
		<dc:Publisher>Cognitive Atlas</dc:Publisher>
		<dc:Creator>Cognitive Atlas RDF Generator</dc:Creator>
		<dc:Contributor>Deanna Lau</dc:Contributor>
		<dc:Date>2010-02-25 10:45:51</dc:Date>
		<dc:Format>text/rdf</dc:Format>
		<dc:Language>en</dc:Language>
		<skos:editorialNote>Generated by testgen.php on Thu Jun 9 14:25:24 PDT 2011.</skos:editorialNote>
		<skos:historyNote>No previous definition revisions.</skos:historyNote>
		<skos:changeNote>This is the first and only definition provided.</skos:changeNote>
		<skos:scopeNote>http://www.w3.org/2004/02/skos/core#Concept</skos:scopeNote>
		<skos:Note>SKOS properties defined in http://www.w3.org/TR/skos-primer/#secrel</skos:Note>
		<skos:inScheme rdf:resource="http://cognitiveatlas.org/tasks/"/>
		<skos:definition>This task involves completing a series of increasingly complex mazes.  </skos:definition>
		<skos:prefLabel>WISC-R Mazes</skos:prefLabel>
		<skos:altLabel></skos:altLabel>
</skos:Concept><skos:Concept rdf:about="http://cognitiveatlas.org/id/trm_4b86dbcd8ff78"> <dc:identifier>trm_4b86dbcd8ff78</dc:identifier>
		<dc:Title>Cognitive Atlas : Lexicon : Rapid Serial Object Transformation</dc:Title>
		<dc:Description>RDF output for 'Rapid Serial Object Transformation'</dc:Description>
		<dc:Type>InteractiveResource</dc:Type>
		<dc:Publisher>Cognitive Atlas</dc:Publisher>
		<dc:Creator>Cognitive Atlas RDF Generator</dc:Creator>
		<dc:Contributor>Deanna Lau</dc:Contributor>
		<dc:Date>2010-02-25 12:21:33</dc:Date>
		<dc:Format>text/rdf</dc:Format>
		<dc:Language>en</dc:Language>
		<skos:editorialNote>Generated by testgen.php on Thu Jun 9 14:25:24 PDT 2011.</skos:editorialNote>
		<skos:historyNote>No previous definition revisions.</skos:historyNote>
		<skos:changeNote>This is the first and only definition provided.</skos:changeNote>
		<skos:scopeNote>http://www.w3.org/2004/02/skos/core#Concept</skos:scopeNote>
		<skos:Note>SKOS properties defined in http://www.w3.org/TR/skos-primer/#secrel</skos:Note>
		<skos:inScheme rdf:resource="http://cognitiveatlas.org/tasks/"/>
		<skos:definition>A task where two sets of differently colored superimposed patterns of dots rotate in opposite directions.  The participant is asked to pay attention to on set of dots.  One of the sets of dots will then move across the screen and the participant must say which direction the dots are moving.  </skos:definition>
		<skos:prefLabel>Rapid Serial Object Transformation</skos:prefLabel>
		<skos:altLabel></skos:altLabel>
</skos:Concept><skos:Concept rdf:about="http://cognitiveatlas.org/id/trm_4b94affc43245"> <dc:identifier>trm_4b94affc43245</dc:identifier>
		<dc:Title>Cognitive Atlas : Lexicon : Wechsler Abbreviated Scale of Intelligence</dc:Title>
		<dc:Description>RDF output for 'Wechsler Abbreviated Scale of Intelligence'</dc:Description>
		<dc:Type>InteractiveResource</dc:Type>
		<dc:Publisher>Cognitive Atlas</dc:Publisher>
		<dc:Creator>Cognitive Atlas RDF Generator</dc:Creator>
		<dc:Contributor>Nolan Nichols</dc:Contributor>
		<dc:Date>2010-03-08 00:06:20</dc:Date>
		<dc:Format>text/rdf</dc:Format>
		<dc:Language>en</dc:Language>
		<skos:editorialNote>Generated by testgen.php on Thu Jun 9 14:25:24 PDT 2011.</skos:editorialNote>
		<skos:historyNote>No previous definition revisions.</skos:historyNote>
		<skos:changeNote>This is the first and only definition provided.</skos:changeNote>
		<skos:scopeNote>http://www.w3.org/2004/02/skos/core#Concept</skos:scopeNote>
		<skos:Note>SKOS properties defined in http://www.w3.org/TR/skos-primer/#secrel</skos:Note>
		<skos:inScheme rdf:resource="http://cognitiveatlas.org/tasks/"/>
		<skos:definition>The WASI meets the demand for a reliable, brief measure of intellectual ability in clinical, educational and research settings for ages 6 to 89 years.

With parallel forms of WAIS-IIIUK and WISC-IIIUK subtests, it offers the clinician a means of reducing practice effects on repeat testing.

The WASI provides you with more information than is typically available from other brief intelligence tests.

This efficient assessment yields traditional verbal, performance and full scale IQ scores and is linked to the WISC-IIIUK and WAIS-IIIUK.

This linkage allows you to estimate a range of full-scale IQ scores on the comprehensive batteries and increases the WASI&#39;s clinical utility.

While the WASI is not intended to replace detailed assessment using the WISC-IIIUK and WAIS-IIIUK, it is the perfect instrument for quickly measuring an individual&#39;s general level of cognitive functioning.

The WASI is unique because it allows you to choose whether to use the four or two subtest format.

This flexibility provides you with control over administration time and depth of assessment.</skos:definition>
		<skos:prefLabel>Wechsler Abbreviated Scale of Intelligence</skos:prefLabel>
		<skos:altLabel></skos:altLabel>
</skos:Concept><skos:Concept rdf:about="http://cognitiveatlas.org/id/trm_4b94b12bf0eb2"> <dc:identifier>trm_4b94b12bf0eb2</dc:identifier>
		<dc:Title>Cognitive Atlas : Lexicon : Wechsler Memory Scale Fourth Edition</dc:Title>
		<dc:Description>RDF output for 'Wechsler Memory Scale Fourth Edition'</dc:Description>
		<dc:Type>InteractiveResource</dc:Type>
		<dc:Publisher>Cognitive Atlas</dc:Publisher>
		<dc:Creator>Cognitive Atlas RDF Generator</dc:Creator>
		<dc:Contributor>Nolan Nichols</dc:Contributor>
		<dc:Date>2010-03-08 00:11:23</dc:Date>
		<dc:Format>text/rdf</dc:Format>
		<dc:Language>en</dc:Language>
		<skos:editorialNote>Generated by testgen.php on Thu Jun 9 14:25:24 PDT 2011.</skos:editorialNote>
		<skos:historyNote>No previous definition revisions.</skos:historyNote>
		<skos:changeNote>This is the first and only definition provided.</skos:changeNote>
		<skos:scopeNote>http://www.w3.org/2004/02/skos/core#Concept</skos:scopeNote>
		<skos:Note>SKOS properties defined in http://www.w3.org/TR/skos-primer/#secrel</skos:Note>
		<skos:inScheme rdf:resource="http://cognitiveatlas.org/tasks/"/>
		<skos:definition>Areas of Assessment

Updated Test Structure

The WMS-IV has had significant changes to the overall test structure. Based on feedback from customers, we are introducing four new subtests and modifying three existing subtests.

4 subtests were added:

    * Spatial Addition
    * Symbol Span
    * Design Memory
    * General Cognitive Screener

3 subtests retained with modifications:

    * Logical Memory
      Although the stories remain the same as seen in WMS-III for ages 16-69 years old, the repetition trial for Story B has been dropped to increase the consistency with previous editions. For the older age range of 65-90 years old, a new story was developed with content more relevant. The story is shorter and repeated once to enable adequate floor through age 90. You can obtain immediate versus delay and recognition versus delay contrast scores.
    * Verbal Paired Associates
      It now includes a combination of difficult and easy items. For the younger age group (16-69 years) there are 14 items of which 10 are hard. For the older age group (65-90 years), there are 10 items of which six are hard. Delayed Free Recall Trial has been added while Recognition Trial has increased its level of difficulty. You can obtain immediate versus delay and recognition versus delay contrast scores.
    * Visual Reproduction
      While following the same structure and format as seen in WMS-III, there have been a few changes to the subtest. Recognition Trial has been shortened and scoring has been improved. Based on Munro Cullum’s research, scoring is easier and faster than previously experienced and emphasizes recall with less focus on drawing accuracy. You can obtain immediate versus delay and recognition versus delay contrast scores.

8 subtests were eliminated:

    * Information &amp; Orientation
    * Spatial Span
    * Mental Control
    * Faces
    * Digit Span
    * Family Pictures
    * Letter Number
    * Word List (CVLT-II can be entered int</skos:definition>
		<skos:prefLabel>Wechsler Memory Scale Fourth Edition</skos:prefLabel>
		<skos:altLabel></skos:altLabel>
</skos:Concept><skos:Concept rdf:about="http://cognitiveatlas.org/id/trm_4b9568b2865c2"> <dc:identifier>trm_4b9568b2865c2</dc:identifier>
		<dc:Title>Cognitive Atlas : Lexicon : MicroCog</dc:Title>
		<dc:Description>RDF output for 'MicroCog'</dc:Description>
		<dc:Type>InteractiveResource</dc:Type>
		<dc:Publisher>Cognitive Atlas</dc:Publisher>
		<dc:Creator>Cognitive Atlas RDF Generator</dc:Creator>
		<dc:Contributor>Nolan Nichols</dc:Contributor>
		<dc:Date>2010-03-08 13:14:26</dc:Date>
		<dc:Format>text/rdf</dc:Format>
		<dc:Language>en</dc:Language>
		<skos:editorialNote>Generated by testgen.php on Thu Jun 9 14:25:24 PDT 2011.</skos:editorialNote>
		<skos:historyNote>No previous definition revisions.</skos:historyNote>
		<skos:changeNote>This is the first and only definition provided.</skos:changeNote>
		<skos:scopeNote>http://www.w3.org/2004/02/skos/core#Concept</skos:scopeNote>
		<skos:Note>SKOS properties defined in http://www.w3.org/TR/skos-primer/#secrel</skos:Note>
		<skos:inScheme rdf:resource="http://cognitiveatlas.org/tasks/"/>
		<skos:definition>Overview

The first automated neuropsychological battery developed for clinical practice-fast, reliable, extremely efficient

Target specific concerns of cognitive impairment in adults with the updated MicroCog™: Assessment of Cognitive Functioning Windows® Edition (MicroCog™ for Windows®). This version includes significant enhancements and is optimized for Windows®.

Content
This computer administered battery tests individuals with 18 subtests that contribute to summary scores for nine interrelated cognitive areas:
• Attention/Mental Control
• Memory
• Spatial Processing
• Reasoning/Calculation
• Reaction Time
• Information Processing Accuracy
• Information Processing Speed
• Cognitive Functioning
• Cognitive Proficiency

Efficient Screener or Diagnostic Instrument
• Flexible-allows you to choose which subtests to administer
• Provides differential diagnosis across a wide population

Two Forms
• Standard Form (60 to 90 minutes)
• Short Form (30 to 45 minutes)

User Friendly
Most examinees can complete the test quickly and with minimal assistance after a brief orientation by a testing assistant.

Test-Retest, Store Data
MicroCog for Windows® stores test data and is proven effective in testretest situations to monitor a patient&#39;s ongoing cognitive status. A report is automatically provided at the end of each administration.

Other Features and Benefits
• For a broad age range (18-89 years)
• Fast administration time (30 to 90 minutes)
• Results do not vary across cultural differences
• Does not require computer literacy or Internet access (PC-based)
• Report credits embedded in software application (separate use counter not required)

Special Uses
• Screening for dementia or Alzheimer&#39;s
• Determining driving fitness
• Evaluating airline pilots (approved by Federal Aviation Administration for re-certification)
• Testing neurological function of athletes-pre- and post</skos:definition>
		<skos:prefLabel>MicroCog</skos:prefLabel>
		<skos:altLabel></skos:altLabel>
</skos:Concept><skos:Concept rdf:about="http://cognitiveatlas.org/id/trm_4c3e0a9576c3b"> <dc:identifier>trm_4c3e0a9576c3b</dc:identifier>
		<dc:Title>Cognitive Atlas : Lexicon : letter number sequencing</dc:Title>
		<dc:Description>RDF output for 'letter number sequencing'</dc:Description>
		<dc:Type>InteractiveResource</dc:Type>
		<dc:Publisher>Cognitive Atlas</dc:Publisher>
		<dc:Creator>Cognitive Atlas RDF Generator</dc:Creator>
		<dc:Contributor>Russ Poldrack</dc:Contributor>
		<dc:Date>2010-07-14 12:05:57</dc:Date>
		<dc:Format>text/rdf</dc:Format>
		<dc:Language>en</dc:Language>
		<skos:editorialNote>Generated by testgen.php on Thu Jun 9 14:25:24 PDT 2011.</skos:editorialNote>
		<skos:historyNote>No previous definition revisions.</skos:historyNote>
		<skos:changeNote>This is the first and only definition provided.</skos:changeNote>
		<skos:scopeNote>http://www.w3.org/2004/02/skos/core#Concept</skos:scopeNote>
		<skos:Note>SKOS properties defined in http://www.w3.org/TR/skos-primer/#secrel</skos:Note>
		<skos:inScheme rdf:resource="http://cognitiveatlas.org/tasks/"/>
		<skos:definition>a task that requires the reordering of an initially unordered set of letters and numbers</skos:definition>
		<skos:prefLabel>letter number sequencing</skos:prefLabel>
		<skos:altLabel></skos:altLabel>
</skos:Concept><skos:Concept rdf:about="http://cognitiveatlas.org/id/trm_4c3e0add96550"> <dc:identifier>trm_4c3e0add96550</dc:identifier>
		<dc:Title>Cognitive Atlas : Lexicon : oculomotor delayed response</dc:Title>
		<dc:Description>RDF output for 'oculomotor delayed response'</dc:Description>
		<dc:Type>InteractiveResource</dc:Type>
		<dc:Publisher>Cognitive Atlas</dc:Publisher>
		<dc:Creator>Cognitive Atlas RDF Generator</dc:Creator>
		<dc:Contributor>Russ Poldrack</dc:Contributor>
		<dc:Date>2010-07-14 12:07:09</dc:Date>
		<dc:Format>text/rdf</dc:Format>
		<dc:Language>en</dc:Language>
		<skos:editorialNote>Generated by testgen.php on Thu Jun 9 14:25:24 PDT 2011.</skos:editorialNote>
		<skos:historyNote>No previous definition revisions.</skos:historyNote>
		<skos:changeNote>This is the first and only definition provided.</skos:changeNote>
		<skos:scopeNote>http://www.w3.org/2004/02/skos/core#Concept</skos:scopeNote>
		<skos:Note>SKOS properties defined in http://www.w3.org/TR/skos-primer/#secrel</skos:Note>
		<skos:inScheme rdf:resource="http://cognitiveatlas.org/tasks/"/>
		<skos:definition>a task that requires an eye movement to be made to a cued location after a delay</skos:definition>
		<skos:prefLabel>oculomotor delayed response</skos:prefLabel>
		<skos:altLabel></skos:altLabel>
		<cito:citesForInformation rdf:resource="http://cognitiveatlas.org/citation/id/cit_4c9974facbe21"/>
</skos:Concept><skos:Concept rdf:about="http://cognitiveatlas.org/id/trm_4c40d10cd776e"> <dc:identifier>trm_4c40d10cd776e</dc:identifier>
		<dc:Title>Cognitive Atlas : Lexicon : operation span task</dc:Title>
		<dc:Description>RDF output for 'operation span task'</dc:Description>
		<dc:Type>InteractiveResource</dc:Type>
		<dc:Publisher>Cognitive Atlas</dc:Publisher>
		<dc:Creator>Cognitive Atlas RDF Generator</dc:Creator>
		<dc:Contributor>Russ Poldrack</dc:Contributor>
		<dc:Date>2010-07-16 14:37:16</dc:Date>
		<dc:Format>text/rdf</dc:Format>
		<dc:Language>en</dc:Language>
		<skos:editorialNote>Generated by testgen.php on Thu Jun 9 14:25:24 PDT 2011.</skos:editorialNote>
		<skos:historyNote>No previous definition revisions.</skos:historyNote>
		<skos:changeNote>This is the first and only definition provided.</skos:changeNote>
		<skos:scopeNote>http://www.w3.org/2004/02/skos/core#Concept</skos:scopeNote>
		<skos:Note>SKOS properties defined in http://www.w3.org/TR/skos-primer/#secrel</skos:Note>
		<skos:inScheme rdf:resource="http://cognitiveatlas.org/tasks/"/>
		<skos:definition>A task in which subjects are asked to perform a simple mathematical verification (e.g., 4/2 +1 = 3) and then read a word, with a recall test following some number of those verify/read pairs.  The maximum number of words that can be recalled is the &#34;operation span&#34;.</skos:definition>
		<skos:prefLabel>operation span task</skos:prefLabel>
		<skos:altLabel></skos:altLabel>
</skos:Concept><skos:Concept rdf:about="http://cognitiveatlas.org/id/trm_4c40d168898db"> <dc:identifier>trm_4c40d168898db</dc:identifier>
		<dc:Title>Cognitive Atlas : Lexicon : reading span task</dc:Title>
		<dc:Description>RDF output for 'reading span task'</dc:Description>
		<dc:Type>InteractiveResource</dc:Type>
		<dc:Publisher>Cognitive Atlas</dc:Publisher>
		<dc:Creator>Cognitive Atlas RDF Generator</dc:Creator>
		<dc:Contributor>Russ Poldrack</dc:Contributor>
		<dc:Date>2010-07-16 14:38:48</dc:Date>
		<dc:Format>text/rdf</dc:Format>
		<dc:Language>en</dc:Language>
		<skos:editorialNote>Generated by testgen.php on Thu Jun 9 14:25:24 PDT 2011.</skos:editorialNote>
		<skos:historyNote>No previous definition revisions.</skos:historyNote>
		<skos:changeNote>This is the first and only definition provided.</skos:changeNote>
		<skos:scopeNote>http://www.w3.org/2004/02/skos/core#Concept</skos:scopeNote>
		<skos:Note>SKOS properties defined in http://www.w3.org/TR/skos-primer/#secrel</skos:Note>
		<skos:inScheme rdf:resource="http://cognitiveatlas.org/tasks/"/>
		<skos:definition>A task that requires participants to read series of unconnected sentences aloud and to remember the final word of each sentence of a series (grouped according to the total number of sentences). With each sentence presented on a card, participants were cued to recall the memorized end-of-sentence words in their original order by a blank card at the end of a series. The number of sentences of a series was incrementally increased until a participant&#39;s reading span, or the maximum number of final words correctly recalled, was found. (From http://en.wikipedia.org/wiki/Reading_span_task)</skos:definition>
		<skos:prefLabel>reading span task</skos:prefLabel>
		<skos:altLabel></skos:altLabel>
</skos:Concept><skos:Concept rdf:about="http://cognitiveatlas.org/id/trm_4c40d1d16071e"> <dc:identifier>trm_4c40d1d16071e</dc:identifier>
		<dc:Title>Cognitive Atlas : Lexicon : listening span task</dc:Title>
		<dc:Description>RDF output for 'listening span task'</dc:Description>
		<dc:Type>InteractiveResource</dc:Type>
		<dc:Publisher>Cognitive Atlas</dc:Publisher>
		<dc:Creator>Cognitive Atlas RDF Generator</dc:Creator>
		<dc:Contributor>Russ Poldrack</dc:Contributor>
		<dc:Date>2010-07-16 14:40:33</dc:Date>
		<dc:Format>text/rdf</dc:Format>
		<dc:Language>en</dc:Language>
		<skos:editorialNote>Generated by testgen.php on Thu Jun 9 14:25:24 PDT 2011.</skos:editorialNote>
		<skos:historyNote>No previous definition revisions.</skos:historyNote>
		<skos:changeNote>This is the first and only definition provided.</skos:changeNote>
		<skos:scopeNote>http://www.w3.org/2004/02/skos/core#Concept</skos:scopeNote>
		<skos:Note>SKOS properties defined in http://www.w3.org/TR/skos-primer/#secrel</skos:Note>
		<skos:inScheme rdf:resource="http://cognitiveatlas.org/tasks/"/>
		<skos:definition>A task in which subjects must listen to a set of sentences and remember the last word in the sentence.  The number of words that can be recalled is the &#34;listening span.&#34; </skos:definition>
		<skos:prefLabel>listening span task</skos:prefLabel>
		<skos:altLabel></skos:altLabel>
		<skos:related rdf:resource="http://cognitiveatlas.org/id/tsk_4a57abb949d69"/>
		<skos:example>listening span task is a broader synonym of Salthouse and Babcock Listening Span task </skos:example>
</skos:Concept><skos:Concept rdf:about="http://cognitiveatlas.org/id/trm_4c40d22c8a69d"> <dc:identifier>trm_4c40d22c8a69d</dc:identifier>
		<dc:Title>Cognitive Atlas : Lexicon : CPT</dc:Title>
		<dc:Description>RDF output for 'CPT'</dc:Description>
		<dc:Type>InteractiveResource</dc:Type>
		<dc:Publisher>Cognitive Atlas</dc:Publisher>
		<dc:Creator>Cognitive Atlas RDF Generator</dc:Creator>
		<dc:Contributor>Russ Poldrack</dc:Contributor>
		<dc:Date>2010-07-16 14:42:04</dc:Date>
		<dc:Format>text/rdf</dc:Format>
		<dc:Language>en</dc:Language>
		<skos:editorialNote>Generated by testgen.php on Thu Jun 9 14:25:24 PDT 2011.</skos:editorialNote>
		<skos:historyNote>No previous definition revisions.</skos:historyNote>
		<skos:changeNote>This is the first and only definition provided.</skos:changeNote>
		<skos:scopeNote>http://www.w3.org/2004/02/skos/core#Concept</skos:scopeNote>
		<skos:Note>SKOS properties defined in http://www.w3.org/TR/skos-primer/#secrel</skos:Note>
		<skos:inScheme rdf:resource="http://cognitiveatlas.org/tasks/"/>
		<skos:definition>A continuous performance task</skos:definition>
		<skos:prefLabel>CPT</skos:prefLabel>
		<skos:altLabel></skos:altLabel>
		<skos:related rdf:resource="http://cognitiveatlas.org/id/trm_4c40d2a93ea15"/>
		<skos:related rdf:resource="http://cognitiveatlas.org/id/trm_4b4a537644d76"/>
		<skos:example>CPT is an exact synonym of Continuous Performance Task</skos:example>
		<skos:example>AX-CPT task is a narrower synonym of CPT</skos:example>
		<cito:citesForInformation rdf:resource="http://cognitiveatlas.org/citation/id/cit_4de7c139bf72e"/>
		<cito:citesForInformation rdf:resource="http://cognitiveatlas.org/citation/id/cit_4de7c16c78382"/>
</skos:Concept><skos:Concept rdf:about="http://cognitiveatlas.org/id/trm_4c40d2a93ea15"> <dc:identifier>trm_4c40d2a93ea15</dc:identifier>
		<dc:Title>Cognitive Atlas : Lexicon : AX-CPT task</dc:Title>
		<dc:Description>RDF output for 'AX-CPT task'</dc:Description>
		<dc:Type>InteractiveResource</dc:Type>
		<dc:Publisher>Cognitive Atlas</dc:Publisher>
		<dc:Creator>Cognitive Atlas RDF Generator</dc:Creator>
		<dc:Contributor>Russ Poldrack</dc:Contributor>
		<dc:Date>2010-07-16 14:44:09</dc:Date>
		<dc:Format>text/rdf</dc:Format>
		<dc:Language>en</dc:Language>
		<skos:editorialNote>Generated by testgen.php on Thu Jun 9 14:25:24 PDT 2011.</skos:editorialNote>
		<skos:historyNote>No previous definition revisions.</skos:historyNote>
		<skos:changeNote>This is the first and only definition provided.</skos:changeNote>
		<skos:scopeNote>http://www.w3.org/2004/02/skos/core#Concept</skos:scopeNote>
		<skos:Note>SKOS properties defined in http://www.w3.org/TR/skos-primer/#secrel</skos:Note>
		<skos:inScheme rdf:resource="http://cognitiveatlas.org/tasks/"/>
		<skos:definition>A version of the continuous performance task in which subjects are told to make one response for the letter X when it was preceded by the letter A, and another response for all other stimuli.</skos:definition>
		<skos:prefLabel>AX-CPT task</skos:prefLabel>
		<skos:altLabel></skos:altLabel>
		<skos:related rdf:resource="http://cognitiveatlas.org/id/trm_4c40d22c8a69d"/>
		<skos:example>AX-CPT task is a narrower synonym of CPT</skos:example>
		<cito:citesForInformation rdf:resource="http://cognitiveatlas.org/citation/id/cit_4c995f00bcff7"/>
</skos:Concept><skos:Concept rdf:about="http://cognitiveatlas.org/id/trm_4c40d325977f0"> <dc:identifier>trm_4c40d325977f0</dc:identifier>
		<dc:Title>Cognitive Atlas : Lexicon : self-ordered pointing task</dc:Title>
		<dc:Description>RDF output for 'self-ordered pointing task'</dc:Description>
		<dc:Type>InteractiveResource</dc:Type>
		<dc:Publisher>Cognitive Atlas</dc:Publisher>
		<dc:Creator>Cognitive Atlas RDF Generator</dc:Creator>
		<dc:Contributor>Russ Poldrack</dc:Contributor>
		<dc:Date>2010-07-16 14:46:13</dc:Date>
		<dc:Format>text/rdf</dc:Format>
		<dc:Language>en</dc:Language>
		<skos:editorialNote>Generated by testgen.php on Thu Jun 9 14:25:24 PDT 2011.</skos:editorialNote>
		<skos:historyNote>No previous definition revisions.</skos:historyNote>
		<skos:changeNote>This is the first and only definition provided.</skos:changeNote>
		<skos:scopeNote>http://www.w3.org/2004/02/skos/core#Concept</skos:scopeNote>
		<skos:Note>SKOS properties defined in http://www.w3.org/TR/skos-primer/#secrel</skos:Note>
		<skos:inScheme rdf:resource="http://cognitiveatlas.org/tasks/"/>
		<skos:definition>A task in which a set of stimuli is presented, and subjects must point to one stimulus at a time, without ever pointing at the same stimulus twice.</skos:definition>
		<skos:prefLabel>self-ordered pointing task</skos:prefLabel>
		<skos:altLabel></skos:altLabel>
</skos:Concept><skos:Concept rdf:about="http://cognitiveatlas.org/id/trm_4c40d4054f38b"> <dc:identifier>trm_4c40d4054f38b</dc:identifier>
		<dc:Title>Cognitive Atlas : Lexicon : keep-track task</dc:Title>
		<dc:Description>RDF output for 'keep-track task'</dc:Description>
		<dc:Type>InteractiveResource</dc:Type>
		<dc:Publisher>Cognitive Atlas</dc:Publisher>
		<dc:Creator>Cognitive Atlas RDF Generator</dc:Creator>
		<dc:Contributor>Russ Poldrack</dc:Contributor>
		<dc:Date>2010-07-16 14:49:57</dc:Date>
		<dc:Format>text/rdf</dc:Format>
		<dc:Language>en</dc:Language>
		<skos:editorialNote>Generated by testgen.php on Thu Jun 9 14:25:24 PDT 2011.</skos:editorialNote>
		<skos:historyNote>No previous definition revisions.</skos:historyNote>
		<skos:changeNote>This is the first and only definition provided.</skos:changeNote>
		<skos:scopeNote>http://www.w3.org/2004/02/skos/core#Concept</skos:scopeNote>
		<skos:Note>SKOS properties defined in http://www.w3.org/TR/skos-primer/#secrel</skos:Note>
		<skos:inScheme rdf:resource="http://cognitiveatlas.org/tasks/"/>
		<skos:definition>A task in which subjects are first shown a set of categories to keep track of for a particular trial (e.g., animals, colors, and countries).  They are then presented with words (including words from each category), and must remember the last word that was presented from each of the categories and recall those words at the end of the trial.  </skos:definition>
		<skos:prefLabel>keep-track task</skos:prefLabel>
		<skos:altLabel></skos:altLabel>
		<cito:citesForInformation rdf:resource="http://cognitiveatlas.org/citation/id/cit_4c40d41a2ebf1"/>
		<cito:citesForInformation rdf:resource="http://cognitiveatlas.org/citation/id/cit_4df139dd0ea2b"/>
</skos:Concept><skos:Concept rdf:about="http://cognitiveatlas.org/id/trm_4c8989e1f3df7"> <dc:identifier>trm_4c8989e1f3df7</dc:identifier>
		<dc:Title>Cognitive Atlas : Lexicon : Acupuncture Task</dc:Title>
		<dc:Description>RDF output for 'Acupuncture Task'</dc:Description>
		<dc:Type>InteractiveResource</dc:Type>
		<dc:Publisher>Cognitive Atlas</dc:Publisher>
		<dc:Creator>Cognitive Atlas RDF Generator</dc:Creator>
		<dc:Contributor>Brenda Gregory</dc:Contributor>
		<dc:Date>2011-04-28 12:08:19</dc:Date>
		<dc:Format>text/rdf</dc:Format>
		<dc:Language>en</dc:Language>
		<skos:editorialNote>Generated by testgen.php on Thu Jun 9 14:25:24 PDT 2011.</skos:editorialNote>
		<skos:historyNote>Revision 2: 1 previous definitions.</skos:historyNote>
		<skos:changeNote>See http://cognitiveatlas.org/id/trm_4c8989e1f3df7 for complete revision history.</skos:changeNote>
		<skos:scopeNote>http://www.w3.org/2004/02/skos/core#Concept</skos:scopeNote>
		<skos:Note>SKOS properties defined in http://www.w3.org/TR/skos-primer/#secrel</skos:Note>
		<skos:inScheme rdf:resource="http://cognitiveatlas.org/tasks/"/>
		<skos:definition>subjects are stimulated with Chinese acupuncture.</skos:definition>
		<skos:prefLabel>Acupuncture Task</skos:prefLabel>
		<skos:altLabel></skos:altLabel>
</skos:Concept><skos:Concept rdf:about="http://cognitiveatlas.org/id/trm_4c898a20eb254"> <dc:identifier>trm_4c898a20eb254</dc:identifier>
		<dc:Title>Cognitive Atlas : Lexicon : Braille Reading Task</dc:Title>
		<dc:Description>RDF output for 'Braille Reading Task'</dc:Description>
		<dc:Type>InteractiveResource</dc:Type>
		<dc:Publisher>Cognitive Atlas</dc:Publisher>
		<dc:Creator>Cognitive Atlas RDF Generator</dc:Creator>
		<dc:Contributor>Brenda Gregory</dc:Contributor>
		<dc:Date>2011-04-28 12:07:50</dc:Date>
		<dc:Format>text/rdf</dc:Format>
		<dc:Language>en</dc:Language>
		<skos:editorialNote>Generated by testgen.php on Thu Jun 9 14:25:25 PDT 2011.</skos:editorialNote>
		<skos:historyNote>Revision 2: 1 previous definitions.</skos:historyNote>
		<skos:changeNote>See http://cognitiveatlas.org/id/trm_4c898a20eb254 for complete revision history.</skos:changeNote>
		<skos:scopeNote>http://www.w3.org/2004/02/skos/core#Concept</skos:scopeNote>
		<skos:Note>SKOS properties defined in http://www.w3.org/TR/skos-primer/#secrel</skos:Note>
		<skos:inScheme rdf:resource="http://cognitiveatlas.org/tasks/"/>
		<skos:definition>Blind subjects read Braille words with their finger(s).</skos:definition>
		<skos:prefLabel>Braille Reading Task</skos:prefLabel>
		<skos:altLabel></skos:altLabel>
</skos:Concept><skos:Concept rdf:about="http://cognitiveatlas.org/id/trm_4c898a680e424"> <dc:identifier>trm_4c898a680e424</dc:identifier>
		<dc:Title>Cognitive Atlas : Lexicon : Breath-Holding</dc:Title>
		<dc:Description>RDF output for 'Breath-Holding'</dc:Description>
		<dc:Type>InteractiveResource</dc:Type>
		<dc:Publisher>Cognitive Atlas</dc:Publisher>
		<dc:Creator>Cognitive Atlas RDF Generator</dc:Creator>
		<dc:Contributor>Carinna Torgerson</dc:Contributor>
		<dc:Date>2011-06-01 12:58:21</dc:Date>
		<dc:Format>text/rdf</dc:Format>
		<dc:Language>en</dc:Language>
		<skos:editorialNote>Generated by testgen.php on Thu Jun 9 14:25:25 PDT 2011.</skos:editorialNote>
		<skos:historyNote>Revision 3: 2 previous definitions.</skos:historyNote>
		<skos:changeNote>See http://cognitiveatlas.org/id/trm_4c898a680e424 for complete revision history.</skos:changeNote>
		<skos:scopeNote>http://www.w3.org/2004/02/skos/core#Concept</skos:scopeNote>
		<skos:Note>SKOS properties defined in http://www.w3.org/TR/skos-primer/#secrel</skos:Note>
		<skos:inScheme rdf:resource="http://cognitiveatlas.org/tasks/"/>
		<skos:definition>Subjects hold their breath as examiner measures mean blood flow velocity divided by time to find the breath-holding index (BHI). Measures cerebral hemodynamic auto-regulation.</skos:definition>
		<skos:prefLabel>Breath-Holding</skos:prefLabel>
		<skos:altLabel></skos:altLabel>
		<cito:citesForInformation rdf:resource="http://cognitiveatlas.org/citation/id/cit_4de69a7c6da49"/>
		<cito:citesForInformation rdf:resource="http://cognitiveatlas.org/citation/id/cit_4de69c53b79e1"/>
</skos:Concept><skos:Concept rdf:about="http://cognitiveatlas.org/id/trm_4c898a8fd3afb"> <dc:identifier>trm_4c898a8fd3afb</dc:identifier>
		<dc:Title>Cognitive Atlas : Lexicon : Chewing/Swallowing</dc:Title>
		<dc:Description>RDF output for 'Chewing/Swallowing'</dc:Description>
		<dc:Type>InteractiveResource</dc:Type>
		<dc:Publisher>Cognitive Atlas</dc:Publisher>
		<dc:Creator>Cognitive Atlas RDF Generator</dc:Creator>
		<dc:Contributor>Brenda Gregory</dc:Contributor>
		<dc:Date>2011-04-27 15:50:29</dc:Date>
		<dc:Format>text/rdf</dc:Format>
		<dc:Language>en</dc:Language>
		<skos:editorialNote>Generated by testgen.php on Thu Jun 9 14:25:25 PDT 2011.</skos:editorialNote>
		<skos:historyNote>Revision 2: 1 previous definitions.</skos:historyNote>
		<skos:changeNote>See http://cognitiveatlas.org/id/trm_4c898a8fd3afb for complete revision history.</skos:changeNote>
		<skos:scopeNote>http://www.w3.org/2004/02/skos/core#Concept</skos:scopeNote>
		<skos:Note>SKOS properties defined in http://www.w3.org/TR/skos-primer/#secrel</skos:Note>
		<skos:inScheme rdf:resource="http://cognitiveatlas.org/tasks/"/>
		<skos:definition>Subjects chew an oral stimulus that is not food (e.g., gum) or swallow their own saliva.  If the oral stimulus is food or liquid that is swallowed, then the correct paradigm class is Eating/Drinking.</skos:definition>
		<skos:prefLabel>Chewing/Swallowing</skos:prefLabel>
		<skos:altLabel></skos:altLabel>
		<cito:citesForInformation rdf:resource="http://cognitiveatlas.org/citation/id/cit_4de95d166bed4"/>
</skos:Concept><skos:Concept rdf:about="http://cognitiveatlas.org/id/trm_4c898acd1f28e"> <dc:identifier>trm_4c898acd1f28e</dc:identifier>
		<dc:Title>Cognitive Atlas : Lexicon : Classical Conditioning</dc:Title>
		<dc:Description>RDF output for 'Classical Conditioning'</dc:Description>
		<dc:Type>InteractiveResource</dc:Type>
		<dc:Publisher>Cognitive Atlas</dc:Publisher>
		<dc:Creator>Cognitive Atlas RDF Generator</dc:Creator>
		<dc:Contributor>Carinna Torgerson</dc:Contributor>
		<dc:Date>2011-06-01 16:14:39</dc:Date>
		<dc:Format>text/rdf</dc:Format>
		<dc:Language>en</dc:Language>
		<skos:editorialNote>Generated by testgen.php on Thu Jun 9 14:25:25 PDT 2011.</skos:editorialNote>
		<skos:historyNote>Revision 3: 2 previous definitions.</skos:historyNote>
		<skos:changeNote>See http://cognitiveatlas.org/id/trm_4c898acd1f28e for complete revision history.</skos:changeNote>
		<skos:scopeNote>http://www.w3.org/2004/02/skos/core#Concept</skos:scopeNote>
		<skos:Note>SKOS properties defined in http://www.w3.org/TR/skos-primer/#secrel</skos:Note>
		<skos:inScheme rdf:resource="http://cognitiveatlas.org/tasks/"/>
		<skos:definition>Subjects are presented with paired stimuli in an attempt to study associative learning or get a subject to react to the conditioned stimulus in the same manner as the unconditioned stimulus, demonstrating a learned association between the two.</skos:definition>
		<skos:prefLabel>Classical Conditioning</skos:prefLabel>
		<skos:altLabel></skos:altLabel>
		<skos:related rdf:resource="http://cognitiveatlas.org/id/trm_4a3fd79d098c9"/>
		<skos:related rdf:resource="http://cognitiveatlas.org/id/trm_4a3fd79d0ab70"/>
		<skos:related rdf:resource="http://cognitiveatlas.org/id/trm_4a3fd79d0ab70"/>
		<skos:related rdf:resource="http://cognitiveatlas.org/id/trm_4a3fd79d0ab70"/>
		<skos:related rdf:resource="http://cognitiveatlas.org/id/trm_4a3fd79d0ab70"/>
		<skos:related rdf:resource="http://cognitiveatlas.org/id/trm_4a3fd79d0a637"/>
		<skos:related rdf:resource="http://cognitiveatlas.org/id/trm_4a3fd79d09b28"/>
		<skos:related rdf:resource="http://cognitiveatlas.org/id/trm_4a3fd79d09b28"/>
		<skos:related rdf:resource="http://cognitiveatlas.org/id/trm_4a3fd79d09b28"/>
		<skos:example>association learning is measured by the contrast of conditioned response trials in the Classical Conditioning</skos:example>
		<skos:example>pavlovian conditioning is measured by the contrast of conditioned stimulus trials in the Classical Conditioning</skos:example>
		<skos:example>pavlovian conditioning is measured by the contrast of unconditioned stimulus trials in the Classical Conditioning</skos:example>
		<skos:example>pavlovian conditioning is measured by the contrast of unconditioned response trials in the Classical Conditioning</skos:example>
		<skos:example>pavlovian conditioning is measured by the contrast of conditioned response trials in the Classical Conditioning</skos:example>
		<skos:example>instinct is measured by the contrast of unconditioned stimulus trials in the Classical Conditioning</skos:example>
		<skos:example>automaticity is measured by the contrast of unconditioned stimulus trials in the Classical Conditioning</skos:example>
		<skos:example>automaticity is measured by the contrast of unconditioned response trials in the Classical Conditioning</skos:example>
		<skos:example>automaticity is measured by the contrast of conditioned response trials in the Classical Conditioning</skos:example>
		<cito:citesForInformation rdf:resource="http://cognitiveatlas.org/citation/id/cit_4de6cb32edf13"/>
		<cito:citesForInformation rdf:resource="http://cognitiveatlas.org/citation/id/cit_4de6cbabc885d"/>
		<cito:citesForInformation rdf:resource="http://cognitiveatlas.org/citation/id/cit_4de6cc590c7ea"/>
</skos:Concept><skos:Concept rdf:about="http://cognitiveatlas.org/id/trm_4c898b02722d2"> <dc:identifier>trm_4c898b02722d2</dc:identifier>
		<dc:Title>Cognitive Atlas : Lexicon : Counting/Calculation</dc:Title>
		<dc:Description>RDF output for 'Counting/Calculation'</dc:Description>
		<dc:Type>InteractiveResource</dc:Type>
		<dc:Publisher>Cognitive Atlas</dc:Publisher>
		<dc:Creator>Cognitive Atlas RDF Generator</dc:Creator>
		<dc:Contributor>Brenda Gregory</dc:Contributor>
		<dc:Date>2011-04-27 15:46:15</dc:Date>
		<dc:Format>text/rdf</dc:Format>
		<dc:Language>en</dc:Language>
		<skos:editorialNote>Generated by testgen.php on Thu Jun 9 14:25:25 PDT 2011.</skos:editorialNote>
		<skos:historyNote>Revision 2: 1 previous definitions.</skos:historyNote>
		<skos:changeNote>See http://cognitiveatlas.org/id/trm_4c898b02722d2 for complete revision history.</skos:changeNote>
		<skos:scopeNote>http://www.w3.org/2004/02/skos/core#Concept</skos:scopeNote>
		<skos:Note>SKOS properties defined in http://www.w3.org/TR/skos-primer/#secrel</skos:Note>
		<skos:inScheme rdf:resource="http://cognitiveatlas.org/tasks/"/>
		<skos:definition>Subjects count, add, subtract, multiply, or divide various stimuli (numbers, bars, dots, etc).</skos:definition>
		<skos:prefLabel>Counting/Calculation</skos:prefLabel>
		<skos:altLabel></skos:altLabel>
		<cito:citesForInformation rdf:resource="http://cognitiveatlas.org/citation/id/cit_4de7c9250d6a4"/>
		<cito:citesForInformation rdf:resource="http://cognitiveatlas.org/citation/id/cit_4de7ccf4107f0"/>
		<cito:citesForInformation rdf:resource="http://cognitiveatlas.org/citation/id/cit_4de7ce1dbd04d"/>
</skos:Concept><skos:Concept rdf:about="http://cognitiveatlas.org/id/trm_4c898b29660b0"> <dc:identifier>trm_4c898b29660b0</dc:identifier>
		<dc:Title>Cognitive Atlas : Lexicon : Cued Explicit Recognition</dc:Title>
		<dc:Description>RDF output for 'Cued Explicit Recognition'</dc:Description>
		<dc:Type>InteractiveResource</dc:Type>
		<dc:Publisher>Cognitive Atlas</dc:Publisher>
		<dc:Creator>Cognitive Atlas RDF Generator</dc:Creator>
		<dc:Contributor>Brenda Gregory</dc:Contributor>
		<dc:Date>2011-04-27 15:45:43</dc:Date>
		<dc:Format>text/rdf</dc:Format>
		<dc:Language>en</dc:Language>
		<skos:editorialNote>Generated by testgen.php on Thu Jun 9 14:25:25 PDT 2011.</skos:editorialNote>
		<skos:historyNote>Revision 2: 1 previous definitions.</skos:historyNote>
		<skos:changeNote>See http://cognitiveatlas.org/id/trm_4c898b29660b0 for complete revision history.</skos:changeNote>
		<skos:scopeNote>http://www.w3.org/2004/02/skos/core#Concept</skos:scopeNote>
		<skos:Note>SKOS properties defined in http://www.w3.org/TR/skos-primer/#secrel</skos:Note>
		<skos:inScheme rdf:resource="http://cognitiveatlas.org/tasks/"/>
		<skos:definition>Subjects view a list of items (words, pictures, sounds, or abstract patterns) prior to scanning.  During scanning, probe words are presented and subject recall if the words are familiar or unfamiliar.</skos:definition>
		<skos:prefLabel>Cued Explicit Recognition</skos:prefLabel>
		<skos:altLabel></skos:altLabel>
		<skos:related rdf:resource="http://cognitiveatlas.org/id/trm_4a3fd79d0b58f"/>
		<skos:related rdf:resource="http://cognitiveatlas.org/id/trm_4a3fd79d0b908"/>
		<skos:related rdf:resource="http://cognitiveatlas.org/id/tsk_4a57abb9499c7"/>
		<skos:example>Cued Explicit Recognition is related to continuous recognition paradigm</skos:example>
		<skos:example>word recognition is measured by the contrast of hit rate (number of correct recognitions) trials in the Cued Explicit Recognition</skos:example>
		<skos:example>forgetting is measured by the contrast of miss rate (number of items subject failed to recognize) trials in the Cued Explicit Recognition</skos:example>
		<cito:citesForInformation rdf:resource="http://cognitiveatlas.org/citation/id/cit_4de7d0dee02b1"/>
		<cito:citesForInformation rdf:resource="http://cognitiveatlas.org/citation/id/cit_4de7d120be9c2"/>
</skos:Concept><skos:Concept rdf:about="http://cognitiveatlas.org/id/trm_4c898b4b463aa"> <dc:identifier>trm_4c898b4b463aa</dc:identifier>
		<dc:Title>Cognitive Atlas : Lexicon : Deception Task</dc:Title>
		<dc:Description>RDF output for 'Deception Task'</dc:Description>
		<dc:Type>InteractiveResource</dc:Type>
		<dc:Publisher>Cognitive Atlas</dc:Publisher>
		<dc:Creator>Cognitive Atlas RDF Generator</dc:Creator>
		<dc:Contributor>Brenda Gregory</dc:Contributor>
		<dc:Date>2011-04-27 15:45:13</dc:Date>
		<dc:Format>text/rdf</dc:Format>
		<dc:Language>en</dc:Language>
		<skos:editorialNote>Generated by testgen.php on Thu Jun 9 14:25:25 PDT 2011.</skos:editorialNote>
		<skos:historyNote>Revision 2: 1 previous definitions.</skos:historyNote>
		<skos:changeNote>See http://cognitiveatlas.org/id/trm_4c898b4b463aa for complete revision history.</skos:changeNote>
		<skos:scopeNote>http://www.w3.org/2004/02/skos/core#Concept</skos:scopeNote>
		<skos:Note>SKOS properties defined in http://www.w3.org/TR/skos-primer/#secrel</skos:Note>
		<skos:inScheme rdf:resource="http://cognitiveatlas.org/tasks/"/>
		<skos:definition>Subjects are asked to perform a task and either lie or be truthful in their responses.</skos:definition>
		<skos:prefLabel>Deception Task</skos:prefLabel>
		<skos:altLabel></skos:altLabel>
		<skos:related rdf:resource="http://cognitiveatlas.org/id/trm_4a3fd79d0b392"/>
		<skos:related rdf:resource="http://cognitiveatlas.org/id/trm_4a3fd79d0b392"/>
		<skos:related rdf:resource="http://cognitiveatlas.org/id/trm_4a3fd79d0a02c"/>
		<skos:example>theory of mind is measured by the contrast of object occlusion and misinformation scores trials in the Deception Task</skos:example>
		<skos:example>theory of mind is measured by the contrast of accuracy trials in the Deception Task</skos:example>
		<skos:example>deception is measured by the contrast of hider trials in the Deception Task</skos:example>
		<cito:citesForInformation rdf:resource="http://cognitiveatlas.org/citation/id/cit_4de7db8fec7a0"/>
		<cito:citesForInformation rdf:resource="http://cognitiveatlas.org/citation/id/cit_4de7db976e852"/>
		<cito:citesForInformation rdf:resource="http://cognitiveatlas.org/citation/id/cit_4de7dea05cb2d"/>
</skos:Concept><skos:Concept rdf:about="http://cognitiveatlas.org/id/trm_4c898b8c2d071"> <dc:identifier>trm_4c898b8c2d071</dc:identifier>
		<dc:Title>Cognitive Atlas : Lexicon : Deductive Reasoning Task</dc:Title>
		<dc:Description>RDF output for 'Deductive Reasoning Task'</dc:Description>
		<dc:Type>InteractiveResource</dc:Type>
		<dc:Publisher>Cognitive Atlas</dc:Publisher>
		<dc:Creator>Cognitive Atlas RDF Generator</dc:Creator>
		<dc:Contributor>Carinna Torgerson</dc:Contributor>
		<dc:Date>2011-06-02 12:27:28</dc:Date>
		<dc:Format>text/rdf</dc:Format>
		<dc:Language>en</dc:Language>
		<skos:editorialNote>Generated by testgen.php on Thu Jun 9 14:25:25 PDT 2011.</skos:editorialNote>
		<skos:historyNote>Revision 3: 2 previous definitions.</skos:historyNote>
		<skos:changeNote>See http://cognitiveatlas.org/id/trm_4c898b8c2d071 for complete revision history.</skos:changeNote>
		<skos:scopeNote>http://www.w3.org/2004/02/skos/core#Concept</skos:scopeNote>
		<skos:Note>SKOS properties defined in http://www.w3.org/TR/skos-primer/#secrel</skos:Note>
		<skos:inScheme rdf:resource="http://cognitiveatlas.org/tasks/"/>
		<skos:definition>Participants generate or evaluate conclusions based on given or well-known premises.</skos:definition>
		<skos:prefLabel>Deductive Reasoning Task</skos:prefLabel>
		<skos:altLabel></skos:altLabel>
		<skos:related rdf:resource="http://cognitiveatlas.org/id/trm_4a3fd79d09ece"/>
		<skos:related rdf:resource="http://cognitiveatlas.org/id/trm_4a3fd79d0a80f"/>
		<skos:related rdf:resource="http://cognitiveatlas.org/id/trm_4a3fd79d0a80f"/>
		<skos:related rdf:resource="http://cognitiveatlas.org/id/trm_4a3fd79d0a81b"/>
		<skos:related rdf:resource="http://cognitiveatlas.org/id/trm_4a3fd79d0a81b"/>
		<skos:related rdf:resource="http://cognitiveatlas.org/id/trm_4a3fd79d0a827"/>
		<skos:related rdf:resource="http://cognitiveatlas.org/id/trm_4a3fd79d0a827"/>
		<skos:related rdf:resource="http://cognitiveatlas.org/id/trm_4a3fd79d09e07"/>
		<skos:related rdf:resource="http://cognitiveatlas.org/id/trm_4a3fd79d0a072"/>
		<skos:related rdf:resource="http://cognitiveatlas.org/id/trm_4a3fd79d0a072"/>
		<skos:related rdf:resource="http://cognitiveatlas.org/id/trm_4a3fd79d0aec1"/>
		<skos:related rdf:resource="http://cognitiveatlas.org/id/trm_4a3fd79d0aec1"/>
		<skos:example>convergent thinking is measured by the contrast of valid trials in the Deductive Reasoning Task</skos:example>
		<skos:example>logic is measured by the contrast of valid trials in the Deductive Reasoning Task</skos:example>
		<skos:example>logic is measured by the contrast of invalid trials in the Deductive Reasoning Task</skos:example>
		<skos:example>logical reasoning is measured by the contrast of valid trials in the Deductive Reasoning Task</skos:example>
		<skos:example>logical reasoning is measured by the contrast of invalid trials in the Deductive Reasoning Task</skos:example>
		<skos:example>logical thinking is measured by the contrast of valid trials in the Deductive Reasoning Task</skos:example>
		<skos:example>logical thinking is measured by the contrast of invalid trials in the Deductive Reasoning Task</skos:example>
		<skos:example>conditional reasoning is measured by the contrast of valid trials in the Deductive Reasoning Task</skos:example>
		<skos:example>deductive reasoning is measured by the contrast of valid trials in the Deductive Reasoning Task</skos:example>
		<skos:example>deductive reasoning is measured by the contrast of invalid trials in the Deductive Reasoning Task</skos:example>
		<skos:example>reasoning is measured by the contrast of valid trials in the Deductive Reasoning Task</skos:example>
		<skos:example>reasoning is measured by the contrast of invalid trials in the Deductive Reasoning Task</skos:example>
		<cito:citesForInformation rdf:resource="http://cognitiveatlas.org/citation/id/cit_4de7e35975765"/>
		<cito:citesForInformation rdf:resource="http://cognitiveatlas.org/citation/id/cit_4de7e5ab750f3"/>
</skos:Concept><skos:Concept rdf:about="http://cognitiveatlas.org/id/trm_4c898bbab4fd4"> <dc:identifier>trm_4c898bbab4fd4</dc:identifier>
		<dc:Title>Cognitive Atlas : Lexicon : Divided Auditory Attention</dc:Title>
		<dc:Description>RDF output for 'Divided Auditory Attention'</dc:Description>
		<dc:Type>InteractiveResource</dc:Type>
		<dc:Publisher>Cognitive Atlas</dc:Publisher>
		<dc:Creator>Cognitive Atlas RDF Generator</dc:Creator>
		<dc:Contributor>Brenda Gregory</dc:Contributor>
		<dc:Date>2011-04-27 15:42:32</dc:Date>
		<dc:Format>text/rdf</dc:Format>
		<dc:Language>en</dc:Language>
		<skos:editorialNote>Generated by testgen.php on Thu Jun 9 14:25:25 PDT 2011.</skos:editorialNote>
		<skos:historyNote>Revision 2: 1 previous definitions.</skos:historyNote>
		<skos:changeNote>See http://cognitiveatlas.org/id/trm_4c898bbab4fd4 for complete revision history.</skos:changeNote>
		<skos:scopeNote>http://www.w3.org/2004/02/skos/core#Concept</skos:scopeNote>
		<skos:Note>SKOS properties defined in http://www.w3.org/TR/skos-primer/#secrel</skos:Note>
		<skos:inScheme rdf:resource="http://cognitiveatlas.org/tasks/"/>
		<skos:definition>During the performance of an unrelated task, subjects simultaneously respond to auditory stimuli (tone or word discrimination, with or without distractors).   Also often co-coded with Tone Monitor/Discrimination.</skos:definition>
		<skos:prefLabel>Divided Auditory Attention</skos:prefLabel>
		<skos:altLabel></skos:altLabel>
		<skos:related rdf:resource="http://cognitiveatlas.org/id/trm_4a3fd79d0a252"/>
		<skos:related rdf:resource="http://cognitiveatlas.org/id/trm_4a3fd79d0a246"/>
		<skos:related rdf:resource="http://cognitiveatlas.org/id/trm_4a3fd79d09a10"/>
		<skos:related rdf:resource="http://cognitiveatlas.org/id/trm_4a3fd79d09713"/>
		<skos:example>executive function is measured by the contrast of response time and accuracy trials in the Divided Auditory Attention</skos:example>
		<skos:example>executive control is measured by the contrast of response time and accuracy trials in the Divided Auditory Attention</skos:example>
		<skos:example>auditory attention is measured by the contrast of response time and accuracy trials in the Divided Auditory Attention</skos:example>
		<skos:example>acoustic phonetic processing is measured by the contrast of response time and accuracy trials in the Divided Auditory Attention</skos:example>
</skos:Concept><skos:Concept rdf:about="http://cognitiveatlas.org/id/trm_4c898be57fcbc"> <dc:identifier>trm_4c898be57fcbc</dc:identifier>
		<dc:Title>Cognitive Atlas : Lexicon : Drawing</dc:Title>
		<dc:Description>RDF output for 'Drawing'</dc:Description>
		<dc:Type>InteractiveResource</dc:Type>
		<dc:Publisher>Cognitive Atlas</dc:Publisher>
		<dc:Creator>Cognitive Atlas RDF Generator</dc:Creator>
		<dc:Contributor>Brenda Gregory</dc:Contributor>
		<dc:Date>2011-04-27 15:42:01</dc:Date>
		<dc:Format>text/rdf</dc:Format>
		<dc:Language>en</dc:Language>
		<skos:editorialNote>Generated by testgen.php on Thu Jun 9 14:25:25 PDT 2011.</skos:editorialNote>
		<skos:historyNote>Revision 2: 1 previous definitions.</skos:historyNote>
		<skos:changeNote>See http://cognitiveatlas.org/id/trm_4c898be57fcbc for complete revision history.</skos:changeNote>
		<skos:scopeNote>http://www.w3.org/2004/02/skos/core#Concept</skos:scopeNote>
		<skos:Note>SKOS properties defined in http://www.w3.org/TR/skos-primer/#secrel</skos:Note>
		<skos:inScheme rdf:resource="http://cognitiveatlas.org/tasks/"/>
		<skos:definition>Subjects draw lines, circles, or drawings using a pen or stylus.</skos:definition>
		<skos:prefLabel>Drawing</skos:prefLabel>
		<skos:altLabel></skos:altLabel>
		<skos:related rdf:resource="http://cognitiveatlas.org/id/trm_4a3fd79d0a972"/>
		<skos:related rdf:resource="http://cognitiveatlas.org/id/trm_4a3fd79d0b4b5"/>
		<skos:example>motor control is measured by the contrast of overall similarity to intended picture trials in the Drawing</skos:example>
		<skos:example>visual perception is measured by the contrast of overall similarity to intended picture trials in the Drawing</skos:example>
		<cito:citesForInformation rdf:resource="http://cognitiveatlas.org/citation/id/cit_4de945dfc30cd"/>
		<cito:citesForInformation rdf:resource="http://cognitiveatlas.org/citation/id/cit_4de9461b6796c"/>
		<cito:citesForInformation rdf:resource="http://cognitiveatlas.org/citation/id/cit_4de94660f1003"/>
</skos:Concept><skos:Concept rdf:about="http://cognitiveatlas.org/id/trm_4c898c0786246"> <dc:identifier>trm_4c898c0786246</dc:identifier>
		<dc:Title>Cognitive Atlas : Lexicon : Eating/Drinking</dc:Title>
		<dc:Description>RDF output for 'Eating/Drinking'</dc:Description>
		<dc:Type>InteractiveResource</dc:Type>
		<dc:Publisher>Cognitive Atlas</dc:Publisher>
		<dc:Creator>Cognitive Atlas RDF Generator</dc:Creator>
		<dc:Contributor>Brenda Gregory</dc:Contributor>
		<dc:Date>2011-04-27 15:41:28</dc:Date>
		<dc:Format>text/rdf</dc:Format>
		<dc:Language>en</dc:Language>
		<skos:editorialNote>Generated by testgen.php on Thu Jun 9 14:25:25 PDT 2011.</skos:editorialNote>
		<skos:historyNote>Revision 2: 1 previous definitions.</skos:historyNote>
		<skos:changeNote>See http://cognitiveatlas.org/id/trm_4c898c0786246 for complete revision history.</skos:changeNote>
		<skos:scopeNote>http://www.w3.org/2004/02/skos/core#Concept</skos:scopeNote>
		<skos:Note>SKOS properties defined in http://www.w3.org/TR/skos-primer/#secrel</skos:Note>
		<skos:inScheme rdf:resource="http://cognitiveatlas.org/tasks/"/>
		<skos:definition>Subjects eat food (e.g., chocolate) or drink liquids (e.g., juice).</skos:definition>
		<skos:prefLabel>Eating/Drinking</skos:prefLabel>
		<skos:altLabel></skos:altLabel>
		<skos:related rdf:resource="http://cognitiveatlas.org/id/trm_4aae62e4ad209"/>
		<skos:related rdf:resource="http://cognitiveatlas.org/id/trm_4a3fd79d0b05e"/>
		<skos:example>cognitive control is measured by the contrast of amount consumed trials in the Eating/Drinking</skos:example>
		<skos:example>self monitoring is measured by the contrast of amount consumed trials in the Eating/Drinking</skos:example>
		<cito:citesForInformation rdf:resource="http://cognitiveatlas.org/citation/id/cit_4de95b9715bd7"/>
		<cito:citesForInformation rdf:resource="http://cognitiveatlas.org/citation/id/cit_4de95c52de732"/>
</skos:Concept><skos:Concept rdf:about="http://cognitiveatlas.org/id/trm_4c898c33ee5f8"> <dc:identifier>trm_4c898c33ee5f8</dc:identifier>
		<dc:Title>Cognitive Atlas : Lexicon : Encoding Task</dc:Title>
		<dc:Description>RDF output for 'Encoding Task'</dc:Description>
		<dc:Type>InteractiveResource</dc:Type>
		<dc:Publisher>Cognitive Atlas</dc:Publisher>
		<dc:Creator>Cognitive Atlas RDF Generator</dc:Creator>
		<dc:Contributor>Brenda Gregory</dc:Contributor>
		<dc:Date>2010-09-09 18:38:59</dc:Date>
		<dc:Format>text/rdf</dc:Format>
		<dc:Language>en</dc:Language>
		<skos:editorialNote>Generated by testgen.php on Thu Jun 9 14:25:25 PDT 2011.</skos:editorialNote>
		<skos:historyNote>No previous definition revisions.</skos:historyNote>
		<skos:changeNote>This is the first and only definition provided.</skos:changeNote>
		<skos:scopeNote>http://www.w3.org/2004/02/skos/core#Concept</skos:scopeNote>
		<skos:Note>SKOS properties defined in http://www.w3.org/TR/skos-primer/#secrel</skos:Note>
		<skos:inScheme rdf:resource="http://cognitiveatlas.org/tasks/"/>
		<skos:definition>Subjects view stimuli (words, pictures, letters) and are instructed to memorize them.</skos:definition>
		<skos:prefLabel>Encoding Task</skos:prefLabel>
		<skos:altLabel></skos:altLabel>
		<skos:related rdf:resource="http://cognitiveatlas.org/id/trm_4a3fd79d09707"/>
		<skos:related rdf:resource="http://cognitiveatlas.org/id/trm_4a3fd79d09a3d"/>
		<skos:related rdf:resource="http://cognitiveatlas.org/id/trm_4a3fd79d09a49"/>
		<skos:related rdf:resource="http://cognitiveatlas.org/id/trm_4a3fd79d0a15c"/>
		<skos:related rdf:resource="http://cognitiveatlas.org/id/trm_4a3fd79d0b8e5"/>
		<skos:related rdf:resource="http://cognitiveatlas.org/id/trm_4a3fd79d0b756"/>
		<skos:related rdf:resource="http://cognitiveatlas.org/id/trm_4a3fd79d0a7d4"/>
		<skos:related rdf:resource="http://cognitiveatlas.org/id/trm_4a3fd79d0ac87"/>
		<skos:related rdf:resource="http://cognitiveatlas.org/id/trm_4a3fd79d098a6"/>
		<skos:related rdf:resource="http://cognitiveatlas.org/id/trm_4a3fd79d0b8d9"/>
		<skos:example>acoustic encoding is measured by the contrast of # items remembered with encoding task - number remembered without trials in the Encoding Task</skos:example>
		<skos:example>auditory coding is measured by the contrast of # items remembered with encoding task - number remembered without trials in the Encoding Task</skos:example>
		<skos:example>auditory encoding is measured by the contrast of # items remembered with encoding task - number remembered without trials in the Encoding Task</skos:example>
		<skos:example>effortful processing is measured by the contrast of # items remembered with encoding task - number remembered without trials in the Encoding Task</skos:example>
		<skos:example>encoding is measured by the contrast of # items remembered with encoding task - number remembered without trials in the Encoding Task</skos:example>
		<skos:example>grammatical encoding is measured by the contrast of # items remembered with encoding task - number remembered without trials in the Encoding Task</skos:example>
		<skos:example>lexical encoding is measured by the contrast of # items remembered with encoding task - number remembered without trials in the Encoding Task</skos:example>
		<skos:example>phonological encoding is measured by the contrast of # items remembered with encoding task - number remembered without trials in the Encoding Task</skos:example>
		<skos:example>articulatory rehearsal is measured by the contrast of # items remembered with encoding task - number remembered without trials in the Encoding Task</skos:example>
		<skos:example>elaborative rehearsal is measured by the contrast of # items remembered with encoding task - number remembered without trials in the Encoding Task</skos:example>
		<cito:citesForInformation rdf:resource="http://cognitiveatlas.org/citation/id/cit_4de9676c85e39"/>
		<cito:citesForInformation rdf:resource="http://cognitiveatlas.org/citation/id/cit_4de96a66cba15"/>
</skos:Concept><skos:Concept rdf:about="http://cognitiveatlas.org/id/trm_4c898c8bf1b4f"> <dc:identifier>trm_4c898c8bf1b4f</dc:identifier>
		<dc:Title>Cognitive Atlas : Lexicon : Episodic Recall</dc:Title>
		<dc:Description>RDF output for 'Episodic Recall'</dc:Description>
		<dc:Type>InteractiveResource</dc:Type>
		<dc:Publisher>Cognitive Atlas</dc:Publisher>
		<dc:Creator>Cognitive Atlas RDF Generator</dc:Creator>
		<dc:Contributor>Brenda Gregory</dc:Contributor>
		<dc:Date>2011-04-27 15:40:36</dc:Date>
		<dc:Format>text/rdf</dc:Format>
		<dc:Language>en</dc:Language>
		<skos:editorialNote>Generated by testgen.php on Thu Jun 9 14:25:25 PDT 2011.</skos:editorialNote>
		<skos:historyNote>Revision 2: 1 previous definitions.</skos:historyNote>
		<skos:changeNote>See http://cognitiveatlas.org/id/trm_4c898c8bf1b4f for complete revision history.</skos:changeNote>
		<skos:scopeNote>http://www.w3.org/2004/02/skos/core#Concept</skos:scopeNote>
		<skos:Note>SKOS properties defined in http://www.w3.org/TR/skos-primer/#secrel</skos:Note>
		<skos:inScheme rdf:resource="http://cognitiveatlas.org/tasks/"/>
		<skos:definition>Subjects recall items from episodic memory (autobiographical history, long-term event memories).  This class is commonly used in generating a type of emotion linked to a specific memory.  This class does NOT include tasks which probe semantic memory (memory of facts or concepts) in which subjects are asked to recall stimuli that were memorized prior to scanning - those are coded as Cued Explicit Recognition.</skos:definition>
		<skos:prefLabel>Episodic Recall</skos:prefLabel>
		<skos:altLabel></skos:altLabel>
		<skos:related rdf:resource="http://cognitiveatlas.org/id/trm_4a3fd79d0a1f4"/>
		<skos:related rdf:resource="http://cognitiveatlas.org/id/trm_4a3fd79d09b1c"/>
		<skos:example>episodic memory is measured by the contrast of number of correct identifications trials in the Episodic Recall</skos:example>
		<skos:example>autobiographical recall is measured by the contrast of number of correct identifications trials in the Episodic Recall</skos:example>
		<cito:citesForInformation rdf:resource="http://cognitiveatlas.org/citation/id/cit_4de96b805dd7d"/>
		<cito:citesForInformation rdf:resource="http://cognitiveatlas.org/citation/id/cit_4de96cb32187e"/>
</skos:Concept><skos:Concept rdf:about="http://cognitiveatlas.org/id/trm_4c898cb4ada49"> <dc:identifier>trm_4c898cb4ada49</dc:identifier>
		<dc:Title>Cognitive Atlas : Lexicon : Face Monitor/Discrimination</dc:Title>
		<dc:Description>RDF output for 'Face Monitor/Discrimination'</dc:Description>
		<dc:Type>InteractiveResource</dc:Type>
		<dc:Publisher>Cognitive Atlas</dc:Publisher>
		<dc:Creator>Cognitive Atlas RDF Generator</dc:Creator>
		<dc:Contributor>Brenda Gregory</dc:Contributor>
		<dc:Date>2011-04-27 15:39:58</dc:Date>
		<dc:Format>text/rdf</dc:Format>
		<dc:Language>en</dc:Language>
		<skos:editorialNote>Generated by testgen.php on Thu Jun 9 14:25:25 PDT 2011.</skos:editorialNote>
		<skos:historyNote>Revision 2: 1 previous definitions.</skos:historyNote>
		<skos:changeNote>See http://cognitiveatlas.org/id/trm_4c898cb4ada49 for complete revision history.</skos:changeNote>
		<skos:scopeNote>http://www.w3.org/2004/02/skos/core#Concept</skos:scopeNote>
		<skos:Note>SKOS properties defined in http://www.w3.org/TR/skos-primer/#secrel</skos:Note>
		<skos:inScheme rdf:resource="http://cognitiveatlas.org/tasks/"/>
		<skos:definition>Subjects are presented with human faces and are instructed to view them passively or discriminate according to their order, gender, location, emotion, or appearance.  If the subjects view the faces passively, then the experiment is NOT co-coded with Passive Viewing.</skos:definition>
		<skos:prefLabel>Face Monitor/Discrimination</skos:prefLabel>
		<skos:altLabel></skos:altLabel>
		<cito:citesForInformation rdf:resource="http://cognitiveatlas.org/citation/id/cit_4ded0b038fa4f"/>
</skos:Concept><skos:Concept rdf:about="http://cognitiveatlas.org/id/trm_4c898da401420"> <dc:identifier>trm_4c898da401420</dc:identifier>
		<dc:Title>Cognitive Atlas : Lexicon : Film Viewing</dc:Title>
		<dc:Description>RDF output for 'Film Viewing'</dc:Description>
		<dc:Type>InteractiveResource</dc:Type>
		<dc:Publisher>Cognitive Atlas</dc:Publisher>
		<dc:Creator>Cognitive Atlas RDF Generator</dc:Creator>
		<dc:Contributor>Brenda Gregory</dc:Contributor>
		<dc:Date>2011-04-27 15:39:31</dc:Date>
		<dc:Format>text/rdf</dc:Format>
		<dc:Language>en</dc:Language>
		<skos:editorialNote>Generated by testgen.php on Thu Jun 9 14:25:25 PDT 2011.</skos:editorialNote>
		<skos:historyNote>Revision 2: 1 previous definitions.</skos:historyNote>
		<skos:changeNote>See http://cognitiveatlas.org/id/trm_4c898da401420 for complete revision history.</skos:changeNote>
		<skos:scopeNote>http://www.w3.org/2004/02/skos/core#Concept</skos:scopeNote>
		<skos:Note>SKOS properties defined in http://www.w3.org/TR/skos-primer/#secrel</skos:Note>
		<skos:inScheme rdf:resource="http://cognitiveatlas.org/tasks/"/>
		<skos:definition>Subjects view movie or film clips passively or are required to make a discrimination when the clip is over.</skos:definition>
		<skos:prefLabel>Film Viewing</skos:prefLabel>
		<skos:altLabel></skos:altLabel>
		<cito:citesForInformation rdf:resource="http://cognitiveatlas.org/citation/id/cit_4ded210380450"/>
		<cito:citesForInformation rdf:resource="http://cognitiveatlas.org/citation/id/cit_4ded21b26bd98"/>
		<cito:citesForInformation rdf:resource="http://cognitiveatlas.org/citation/id/cit_4ded21f250d0a"/>
</skos:Concept><skos:Concept rdf:about="http://cognitiveatlas.org/id/trm_4c898f079d05e"> <dc:identifier>trm_4c898f079d05e</dc:identifier>
		<dc:Title>Cognitive Atlas : Lexicon : Finger Tapping Task</dc:Title>
		<dc:Description>RDF output for 'Finger Tapping Task'</dc:Description>
		<dc:Type>InteractiveResource</dc:Type>
		<dc:Publisher>Cognitive Atlas</dc:Publisher>
		<dc:Creator>Cognitive Atlas RDF Generator</dc:Creator>
		<dc:Contributor>Brenda Gregory</dc:Contributor>
		<dc:Date>2011-04-27 15:39:02</dc:Date>
		<dc:Format>text/rdf</dc:Format>
		<dc:Language>en</dc:Language>
		<skos:editorialNote>Generated by testgen.php on Thu Jun 9 14:25:25 PDT 2011.</skos:editorialNote>
		<skos:historyNote>Revision 2: 1 previous definitions.</skos:historyNote>
		<skos:changeNote>See http://cognitiveatlas.org/id/trm_4c898f079d05e for complete revision history.</skos:changeNote>
		<skos:scopeNote>http://www.w3.org/2004/02/skos/core#Concept</skos:scopeNote>
		<skos:Note>SKOS properties defined in http://www.w3.org/TR/skos-primer/#secrel</skos:Note>
		<skos:inScheme rdf:resource="http://cognitiveatlas.org/tasks/"/>
		<skos:definition>Subjects tap their fingers according to a visual, auditory, or no cue.</skos:definition>
		<skos:prefLabel>Finger Tapping Task</skos:prefLabel>
		<skos:altLabel></skos:altLabel>
		<skos:related rdf:resource="http://cognitiveatlas.org/id/trm_4a3fd79d0a972"/>
		<skos:related rdf:resource="http://cognitiveatlas.org/id/trm_4a3fd79d0a972"/>
		<skos:related rdf:resource="http://cognitiveatlas.org/id/trm_4a3fd79d0afc3"/>
		<skos:related rdf:resource="http://cognitiveatlas.org/id/trm_4a3fd79d0a9a1"/>
		<skos:related rdf:resource="http://cognitiveatlas.org/id/trm_4a3fd79d0a9a1"/>
		<skos:example>motor control is measured by the contrast of % rhythm maintainance trials in the Finger Tapping Task</skos:example>
		<skos:example>motor control is measured by the contrast of tap speed trials in the Finger Tapping Task</skos:example>
		<skos:example>rhythm is measured by the contrast of % rhythm maintainance trials in the Finger Tapping Task</skos:example>
		<skos:example>motor planning is measured by the contrast of % rhythm maintainance trials in the Finger Tapping Task</skos:example>
		<skos:example>motor planning is measured by the contrast of tap speed trials in the Finger Tapping Task</skos:example>
		<cito:citesForInformation rdf:resource="http://cognitiveatlas.org/citation/id/cit_4ded24f51cbfe"/>
		<cito:citesForInformation rdf:resource="http://cognitiveatlas.org/citation/id/cit_4ded266c7ec7a"/>
		<cito:citesForInformation rdf:resource="http://cognitiveatlas.org/citation/id/cit_4ded2a5caaa84"/>
</skos:Concept><skos:Concept rdf:about="http://cognitiveatlas.org/id/trm_4c898f72228f3"> <dc:identifier>trm_4c898f72228f3</dc:identifier>
		<dc:Title>Cognitive Atlas : Lexicon : Fixation Task</dc:Title>
		<dc:Description>RDF output for 'Fixation Task'</dc:Description>
		<dc:Type>InteractiveResource</dc:Type>
		<dc:Publisher>Cognitive Atlas</dc:Publisher>
		<dc:Creator>Cognitive Atlas RDF Generator</dc:Creator>
		<dc:Contributor>Brenda Gregory</dc:Contributor>
		<dc:Date>2011-04-27 15:50:02</dc:Date>
		<dc:Format>text/rdf</dc:Format>
		<dc:Language>en</dc:Language>
		<skos:editorialNote>Generated by testgen.php on Thu Jun 9 14:25:25 PDT 2011.</skos:editorialNote>
		<skos:historyNote>Revision 2: 1 previous definitions.</skos:historyNote>
		<skos:changeNote>See http://cognitiveatlas.org/id/trm_4c898f72228f3 for complete revision history.</skos:changeNote>
		<skos:scopeNote>http://www.w3.org/2004/02/skos/core#Concept</skos:scopeNote>
		<skos:Note>SKOS properties defined in http://www.w3.org/TR/skos-primer/#secrel</skos:Note>
		<skos:inScheme rdf:resource="http://cognitiveatlas.org/tasks/"/>
		<skos:definition>Subjects fixate on a visual target.</skos:definition>
		<skos:prefLabel>Fixation Task</skos:prefLabel>
		<skos:altLabel></skos:altLabel>
		<skos:related rdf:resource="http://cognitiveatlas.org/id/trm_4a3fd79d0b5e3"/>
		<skos:related rdf:resource="http://cognitiveatlas.org/id/trm_4a3fd79d0a3d2"/>
		<skos:related rdf:resource="http://cognitiveatlas.org/id/trm_4a3fd79d0b46f"/>
		<skos:related rdf:resource="http://cognitiveatlas.org/id/trm_4a3fd79d0b5ef"/>
		<skos:related rdf:resource="http://cognitiveatlas.org/id/trm_4a3fd79d0a38d"/>
		<skos:example>attention span is measured by the contrast of fixation time below maximum degree of eye movement trials in the Fixation Task</skos:example>
		<skos:example>gaze is measured by the contrast of degree of eye movement trials in the Fixation Task</skos:example>
		<skos:example>visual attention is measured by the contrast of degree of eye movement trials in the Fixation Task</skos:example>
		<skos:example>attentional focusing is measured by the contrast of fixation time below maximum degree of eye movement trials in the Fixation Task</skos:example>
		<skos:example>focused attention is measured by the contrast of fixation time below maximum degree of eye movement trials in the Fixation Task</skos:example>
		<cito:citesForInformation rdf:resource="http://cognitiveatlas.org/citation/id/cit_4ded3987ad7d8"/>
		<cito:citesForInformation rdf:resource="http://cognitiveatlas.org/citation/id/cit_4ded39a505d17"/>
</skos:Concept><skos:Concept rdf:about="http://cognitiveatlas.org/id/trm_4c898f8f297ac"> <dc:identifier>trm_4c898f8f297ac</dc:identifier>
		<dc:Title>Cognitive Atlas : Lexicon : Flashing Checkerboard</dc:Title>
		<dc:Description>RDF output for 'Flashing Checkerboard'</dc:Description>
		<dc:Type>InteractiveResource</dc:Type>
		<dc:Publisher>Cognitive Atlas</dc:Publisher>
		<dc:Creator>Cognitive Atlas RDF Generator</dc:Creator>
		<dc:Contributor>Brenda Gregory</dc:Contributor>
		<dc:Date>2011-04-27 15:37:14</dc:Date>
		<dc:Format>text/rdf</dc:Format>
		<dc:Language>en</dc:Language>
		<skos:editorialNote>Generated by testgen.php on Thu Jun 9 14:25:25 PDT 2011.</skos:editorialNote>
		<skos:historyNote>Revision 2: 1 previous definitions.</skos:historyNote>
		<skos:changeNote>See http://cognitiveatlas.org/id/trm_4c898f8f297ac for complete revision history.</skos:changeNote>
		<skos:scopeNote>http://www.w3.org/2004/02/skos/core#Concept</skos:scopeNote>
		<skos:Note>SKOS properties defined in http://www.w3.org/TR/skos-primer/#secrel</skos:Note>
		<skos:inScheme rdf:resource="http://cognitiveatlas.org/tasks/"/>
		<skos:definition>Subjects view a flashing checkerboard.</skos:definition>
		<skos:prefLabel>Flashing Checkerboard</skos:prefLabel>
		<skos:altLabel></skos:altLabel>
		<cito:citesForInformation rdf:resource="http://cognitiveatlas.org/citation/id/cit_4ded3d4c05798"/>
		<cito:citesForInformation rdf:resource="http://cognitiveatlas.org/citation/id/cit_4ded3e2ad4374"/>
</skos:Concept><skos:Concept rdf:about="http://cognitiveatlas.org/id/trm_4c898fad429ed"> <dc:identifier>trm_4c898fad429ed</dc:identifier>
		<dc:Title>Cognitive Atlas : Lexicon : Flexion/Extension</dc:Title>
		<dc:Description>RDF output for 'Flexion/Extension'</dc:Description>
		<dc:Type>InteractiveResource</dc:Type>
		<dc:Publisher>Cognitive Atlas</dc:Publisher>
		<dc:Creator>Cognitive Atlas RDF Generator</dc:Creator>
		<dc:Contributor>Brenda Gregory</dc:Contributor>
		<dc:Date>2011-04-27 15:35:49</dc:Date>
		<dc:Format>text/rdf</dc:Format>
		<dc:Language>en</dc:Language>
		<skos:editorialNote>Generated by testgen.php on Thu Jun 9 14:25:25 PDT 2011.</skos:editorialNote>
		<skos:historyNote>Revision 2: 1 previous definitions.</skos:historyNote>
		<skos:changeNote>See http://cognitiveatlas.org/id/trm_4c898fad429ed for complete revision history.</skos:changeNote>
		<skos:scopeNote>http://www.w3.org/2004/02/skos/core#Concept</skos:scopeNote>
		<skos:Note>SKOS properties defined in http://www.w3.org/TR/skos-primer/#secrel</skos:Note>
		<skos:inScheme rdf:resource="http://cognitiveatlas.org/tasks/"/>
		<skos:definition>Subjects move (flex and extend) their hands, arms, legs, feet, lips, tongue, etc.</skos:definition>
		<skos:prefLabel>Flexion/Extension</skos:prefLabel>
		<skos:altLabel></skos:altLabel>
</skos:Concept><skos:Concept rdf:about="http://cognitiveatlas.org/id/trm_4c898fc6722f4"> <dc:identifier>trm_4c898fc6722f4</dc:identifier>
		<dc:Title>Cognitive Atlas : Lexicon : Free Word List Recall</dc:Title>
		<dc:Description>RDF output for 'Free Word List Recall'</dc:Description>
		<dc:Type>InteractiveResource</dc:Type>
		<dc:Publisher>Cognitive Atlas</dc:Publisher>
		<dc:Creator>Cognitive Atlas RDF Generator</dc:Creator>
		<dc:Contributor>Brenda Gregory</dc:Contributor>
		<dc:Date>2011-04-27 15:35:17</dc:Date>
		<dc:Format>text/rdf</dc:Format>
		<dc:Language>en</dc:Language>
		<skos:editorialNote>Generated by testgen.php on Thu Jun 9 14:25:25 PDT 2011.</skos:editorialNote>
		<skos:historyNote>Revision 2: 1 previous definitions.</skos:historyNote>
		<skos:changeNote>See http://cognitiveatlas.org/id/trm_4c898fc6722f4 for complete revision history.</skos:changeNote>
		<skos:scopeNote>http://www.w3.org/2004/02/skos/core#Concept</skos:scopeNote>
		<skos:Note>SKOS properties defined in http://www.w3.org/TR/skos-primer/#secrel</skos:Note>
		<skos:inScheme rdf:resource="http://cognitiveatlas.org/tasks/"/>
		<skos:definition>Subjects view a list of words and after a delay are asked to freely recall the words presented.</skos:definition>
		<skos:prefLabel>Free Word List Recall</skos:prefLabel>
		<skos:altLabel></skos:altLabel>
		<skos:related rdf:resource="http://cognitiveatlas.org/id/trm_4a3fd79d09cae"/>
		<skos:related rdf:resource="http://cognitiveatlas.org/id/trm_4a3fd79d0a1ae"/>
		<skos:related rdf:resource="http://cognitiveatlas.org/id/trm_4a3fd79d0b5a7"/>
		<skos:related rdf:resource="http://cognitiveatlas.org/id/trm_4a3fd79d0b5a7"/>
		<skos:example>chunking is measured by the contrast of category list trials in the Free Word List Recall</skos:example>
		<skos:example>emotional memory is measured by the contrast of emotion manipulation trials in the Free Word List Recall</skos:example>
		<skos:example>working memory is measured by the contrast of emotion manipulation trials in the Free Word List Recall</skos:example>
		<skos:example>working memory is measured by the contrast of category list trials in the Free Word List Recall</skos:example>
		<cito:citesForInformation rdf:resource="http://cognitiveatlas.org/citation/id/cit_4ded49d3ccb06"/>
		<cito:citesForInformation rdf:resource="http://cognitiveatlas.org/citation/id/cit_4ded4a820253d"/>
		<cito:citesForInformation rdf:resource="http://cognitiveatlas.org/citation/id/cit_4ded4cd6790d6"/>
</skos:Concept><skos:Concept rdf:about="http://cognitiveatlas.org/id/trm_4c898ff0bea97"> <dc:identifier>trm_4c898ff0bea97</dc:identifier>
		<dc:Title>Cognitive Atlas : Lexicon : Grasping Task</dc:Title>
		<dc:Description>RDF output for 'Grasping Task'</dc:Description>
		<dc:Type>InteractiveResource</dc:Type>
		<dc:Publisher>Cognitive Atlas</dc:Publisher>
		<dc:Creator>Cognitive Atlas RDF Generator</dc:Creator>
		<dc:Contributor>Brenda Gregory</dc:Contributor>
		<dc:Date>2011-04-27 15:34:50</dc:Date>
		<dc:Format>text/rdf</dc:Format>
		<dc:Language>en</dc:Language>
		<skos:editorialNote>Generated by testgen.php on Thu Jun 9 14:25:25 PDT 2011.</skos:editorialNote>
		<skos:historyNote>Revision 2: 1 previous definitions.</skos:historyNote>
		<skos:changeNote>See http://cognitiveatlas.org/id/trm_4c898ff0bea97 for complete revision history.</skos:changeNote>
		<skos:scopeNote>http://www.w3.org/2004/02/skos/core#Concept</skos:scopeNote>
		<skos:Note>SKOS properties defined in http://www.w3.org/TR/skos-primer/#secrel</skos:Note>
		<skos:inScheme rdf:resource="http://cognitiveatlas.org/tasks/"/>
		<skos:definition>Subjects grasped or gripped a presented stimulus with their hand or mimicked grasping one that was not physically presented (i.e., was imaginary or presented as a picture or video).</skos:definition>
		<skos:prefLabel>Grasping Task</skos:prefLabel>
		<skos:altLabel></skos:altLabel>
		<skos:related rdf:resource="http://cognitiveatlas.org/id/trm_4a3fd79d0a9a1"/>
		<skos:related rdf:resource="http://cognitiveatlas.org/id/trm_4a3fd79d0a972"/>
		<skos:example>motor planning is measured by the contrast of response time trials in the Grasping Task</skos:example>
		<skos:example>motor control is measured by the contrast of kinematics trials in the Grasping Task</skos:example>
		<cito:citesForInformation rdf:resource="http://cognitiveatlas.org/citation/id/cit_4ded4f12303ba"/>
		<cito:citesForInformation rdf:resource="http://cognitiveatlas.org/citation/id/cit_4ded50957217b"/>
</skos:Concept><skos:Concept rdf:about="http://cognitiveatlas.org/id/trm_4c899005b11d5"> <dc:identifier>trm_4c899005b11d5</dc:identifier>
		<dc:Title>Cognitive Atlas : Lexicon : Imagined Movement</dc:Title>
		<dc:Description>RDF output for 'Imagined Movement'</dc:Description>
		<dc:Type>InteractiveResource</dc:Type>
		<dc:Publisher>Cognitive Atlas</dc:Publisher>
		<dc:Creator>Cognitive Atlas RDF Generator</dc:Creator>
		<dc:Contributor>Brenda Gregory</dc:Contributor>
		<dc:Date>2011-04-27 15:34:21</dc:Date>
		<dc:Format>text/rdf</dc:Format>
		<dc:Language>en</dc:Language>
		<skos:editorialNote>Generated by testgen.php on Thu Jun 9 14:25:25 PDT 2011.</skos:editorialNote>
		<skos:historyNote>Revision 2: 1 previous definitions.</skos:historyNote>
		<skos:changeNote>See http://cognitiveatlas.org/id/trm_4c899005b11d5 for complete revision history.</skos:changeNote>
		<skos:scopeNote>http://www.w3.org/2004/02/skos/core#Concept</skos:scopeNote>
		<skos:Note>SKOS properties defined in http://www.w3.org/TR/skos-primer/#secrel</skos:Note>
		<skos:inScheme rdf:resource="http://cognitiveatlas.org/tasks/"/>
		<skos:definition>Subjects imagine performing some movement (e.g., finger tapping, reaching).</skos:definition>
		<skos:prefLabel>Imagined Movement</skos:prefLabel>
		<skos:altLabel></skos:altLabel>
		<skos:related rdf:resource="http://cognitiveatlas.org/id/trm_4a3fd79d09d4d"/>
		<skos:related rdf:resource="http://cognitiveatlas.org/id/trm_4a3fd79d0a504"/>
		<skos:related rdf:resource="http://cognitiveatlas.org/id/trm_4a3fd79d0a9a1"/>
		<skos:example>cognitive effort is measured by the contrast of real task effort minus imagined task effort trials in the Imagined Movement</skos:example>
		<skos:example>imageability is measured by the contrast of real task time minus imagined task time trials in the Imagined Movement</skos:example>
		<skos:example>motor planning is measured by the contrast of real task areas of activation minus imagined task areas of activation trials in the Imagined Movement</skos:example>
		<cito:citesForInformation rdf:resource="http://cognitiveatlas.org/citation/id/cit_4ded64ca43d85"/>
		<cito:citesForInformation rdf:resource="http://cognitiveatlas.org/citation/id/cit_4ded6591af1c4"/>
		<cito:citesForInformation rdf:resource="http://cognitiveatlas.org/citation/id/cit_4dee507055993"/>
</skos:Concept><skos:Concept rdf:about="http://cognitiveatlas.org/id/trm_4c89903149aeb"> <dc:identifier>trm_4c89903149aeb</dc:identifier>
		<dc:Title>Cognitive Atlas : Lexicon : Imagined Objects/Scenes</dc:Title>
		<dc:Description>RDF output for 'Imagined Objects/Scenes'</dc:Description>
		<dc:Type>InteractiveResource</dc:Type>
		<dc:Publisher>Cognitive Atlas</dc:Publisher>
		<dc:Creator>Cognitive Atlas RDF Generator</dc:Creator>
		<dc:Contributor>Brenda Gregory</dc:Contributor>
		<dc:Date>2011-04-27 14:07:59</dc:Date>
		<dc:Format>text/rdf</dc:Format>
		<dc:Language>en</dc:Language>
		<skos:editorialNote>Generated by testgen.php on Thu Jun 9 14:25:25 PDT 2011.</skos:editorialNote>
		<skos:historyNote>Revision 2: 1 previous definitions.</skos:historyNote>
		<skos:changeNote>See http://cognitiveatlas.org/id/trm_4c89903149aeb for complete revision history.</skos:changeNote>
		<skos:scopeNote>http://www.w3.org/2004/02/skos/core#Concept</skos:scopeNote>
		<skos:Note>SKOS properties defined in http://www.w3.org/TR/skos-primer/#secrel</skos:Note>
		<skos:inScheme rdf:resource="http://cognitiveatlas.org/tasks/"/>
		<skos:definition>Subject generate vivid images of objects, places, concepts, hypothetical events (not in their past), or the completion of tasks.</skos:definition>
		<skos:prefLabel>Imagined Objects/Scenes</skos:prefLabel>
		<skos:altLabel></skos:altLabel>
		<skos:related rdf:resource="http://cognitiveatlas.org/id/trm_4a3fd79d09d35"/>
		<skos:related rdf:resource="http://cognitiveatlas.org/id/trm_4a3fd79d0a908"/>
		<skos:example>cognitive development is measured by the contrast of physical representation of imagined object trials in the Imagined Objects/Scenes</skos:example>
		<skos:example>mental representation is measured by the contrast of real visual areas of activation minus imagined task areas of activation trials in the Imagined Objects/Scenes</skos:example>
		<cito:citesForInformation rdf:resource="http://cognitiveatlas.org/citation/id/cit_4dee531f3d1d2"/>
		<cito:citesForInformation rdf:resource="http://cognitiveatlas.org/citation/id/cit_4dee58e9e6249"/>
</skos:Concept><skos:Concept rdf:about="http://cognitiveatlas.org/id/trm_4c8990480ad0f"> <dc:identifier>trm_4c8990480ad0f</dc:identifier>
		<dc:Title>Cognitive Atlas : Lexicon : Isometric Force</dc:Title>
		<dc:Description>RDF output for 'Isometric Force'</dc:Description>
		<dc:Type>InteractiveResource</dc:Type>
		<dc:Publisher>Cognitive Atlas</dc:Publisher>
		<dc:Creator>Cognitive Atlas RDF Generator</dc:Creator>
		<dc:Contributor>Brenda Gregory</dc:Contributor>
		<dc:Date>2011-04-27 14:07:22</dc:Date>
		<dc:Format>text/rdf</dc:Format>
		<dc:Language>en</dc:Language>
		<skos:editorialNote>Generated by testgen.php on Thu Jun 9 14:25:25 PDT 2011.</skos:editorialNote>
		<skos:historyNote>Revision 2: 1 previous definitions.</skos:historyNote>
		<skos:changeNote>See http://cognitiveatlas.org/id/trm_4c8990480ad0f for complete revision history.</skos:changeNote>
		<skos:scopeNote>http://www.w3.org/2004/02/skos/core#Concept</skos:scopeNote>
		<skos:Note>SKOS properties defined in http://www.w3.org/TR/skos-primer/#secrel</skos:Note>
		<skos:inScheme rdf:resource="http://cognitiveatlas.org/tasks/"/>
		<skos:definition>Subjects use their hands or fingers to apply isometric force or complete a precision grip task.</skos:definition>
		<skos:prefLabel>Isometric Force</skos:prefLabel>
		<skos:altLabel></skos:altLabel>
		<skos:related rdf:resource="http://cognitiveatlas.org/id/trm_4a3fd79d0a972"/>
		<skos:related rdf:resource="http://cognitiveatlas.org/id/trm_4d7fc7c13b3c0"/>
		<skos:example>motor control is measured by the contrast of MVC minus baseline trials in the Isometric Force</skos:example>
		<skos:example>Self-Regulation is measured by the contrast of MVC minus baseline trials in the Isometric Force</skos:example>
		<cito:citesForInformation rdf:resource="http://cognitiveatlas.org/citation/id/cit_4df1170745145"/>
		<cito:citesForInformation rdf:resource="http://cognitiveatlas.org/citation/id/cit_4df118cd39510"/>
		<cito:citesForInformation rdf:resource="http://cognitiveatlas.org/citation/id/cit_4df118dbecd68"/>
</skos:Concept><skos:Concept rdf:about="http://cognitiveatlas.org/id/trm_4c8990810541d"> <dc:identifier>trm_4c8990810541d</dc:identifier>
		<dc:Title>Cognitive Atlas : Lexicon : Mental Rotation Task</dc:Title>
		<dc:Description>RDF output for 'Mental Rotation Task'</dc:Description>
		<dc:Type>InteractiveResource</dc:Type>
		<dc:Publisher>Cognitive Atlas</dc:Publisher>
		<dc:Creator>Cognitive Atlas RDF Generator</dc:Creator>
		<dc:Contributor>Brenda Gregory</dc:Contributor>
		<dc:Date>2011-04-27 14:06:49</dc:Date>
		<dc:Format>text/rdf</dc:Format>
		<dc:Language>en</dc:Language>
		<skos:editorialNote>Generated by testgen.php on Thu Jun 9 14:25:25 PDT 2011.</skos:editorialNote>
		<skos:historyNote>Revision 2: 1 previous definitions.</skos:historyNote>
		<skos:changeNote>See http://cognitiveatlas.org/id/trm_4c8990810541d for complete revision history.</skos:changeNote>
		<skos:scopeNote>http://www.w3.org/2004/02/skos/core#Concept</skos:scopeNote>
		<skos:Note>SKOS properties defined in http://www.w3.org/TR/skos-primer/#secrel</skos:Note>
		<skos:inScheme rdf:resource="http://cognitiveatlas.org/tasks/"/>
		<skos:definition>Subjects view rotated letters, numbers, or objects (2D or 3D) and indicate if they are in their normal or mirror orientation; includes variations, but all tasks include mental rotation of stimuli.</skos:definition>
		<skos:prefLabel>Mental Rotation Task</skos:prefLabel>
		<skos:altLabel></skos:altLabel>
</skos:Concept><skos:Concept rdf:about="http://cognitiveatlas.org/id/trm_4c89909cc1f33"> <dc:identifier>trm_4c89909cc1f33</dc:identifier>
		<dc:Title>Cognitive Atlas : Lexicon : Micturition Task</dc:Title>
		<dc:Description>RDF output for 'Micturition Task'</dc:Description>
		<dc:Type>InteractiveResource</dc:Type>
		<dc:Publisher>Cognitive Atlas</dc:Publisher>
		<dc:Creator>Cognitive Atlas RDF Generator</dc:Creator>
		<dc:Contributor>Brenda Gregory</dc:Contributor>
		<dc:Date>2011-04-27 14:02:26</dc:Date>
		<dc:Format>text/rdf</dc:Format>
		<dc:Language>en</dc:Language>
		<skos:editorialNote>Generated by testgen.php on Thu Jun 9 14:25:25 PDT 2011.</skos:editorialNote>
		<skos:historyNote>Revision 2: 1 previous definitions.</skos:historyNote>
		<skos:changeNote>See http://cognitiveatlas.org/id/trm_4c89909cc1f33 for complete revision history.</skos:changeNote>
		<skos:scopeNote>http://www.w3.org/2004/02/skos/core#Concept</skos:scopeNote>
		<skos:Note>SKOS properties defined in http://www.w3.org/TR/skos-primer/#secrel</skos:Note>
		<skos:inScheme rdf:resource="http://cognitiveatlas.org/tasks/"/>
		<skos:definition>Subjects voided urine.</skos:definition>
		<skos:prefLabel>Micturition Task</skos:prefLabel>
		<skos:altLabel></skos:altLabel>
</skos:Concept><skos:Concept rdf:about="http://cognitiveatlas.org/id/trm_4c8990b07a037"> <dc:identifier>trm_4c8990b07a037</dc:identifier>
		<dc:Title>Cognitive Atlas : Lexicon : Music Comprehension/Production</dc:Title>
		<dc:Description>RDF output for 'Music Comprehension/Production'</dc:Description>
		<dc:Type>InteractiveResource</dc:Type>
		<dc:Publisher>Cognitive Atlas</dc:Publisher>
		<dc:Creator>Cognitive Atlas RDF Generator</dc:Creator>
		<dc:Contributor>Brenda Gregory</dc:Contributor>
		<dc:Date>2011-04-27 14:01:56</dc:Date>
		<dc:Format>text/rdf</dc:Format>
		<dc:Language>en</dc:Language>
		<skos:editorialNote>Generated by testgen.php on Thu Jun 9 14:25:25 PDT 2011.</skos:editorialNote>
		<skos:historyNote>Revision 2: 1 previous definitions.</skos:historyNote>
		<skos:changeNote>See http://cognitiveatlas.org/id/trm_4c8990b07a037 for complete revision history.</skos:changeNote>
		<skos:scopeNote>http://www.w3.org/2004/02/skos/core#Concept</skos:scopeNote>
		<skos:Note>SKOS properties defined in http://www.w3.org/TR/skos-primer/#secrel</skos:Note>
		<skos:inScheme rdf:resource="http://cognitiveatlas.org/tasks/"/>
		<skos:definition>Subjects listen to music passively or are asked to sing overtly.</skos:definition>
		<skos:prefLabel>Music Comprehension/Production</skos:prefLabel>
		<skos:altLabel></skos:altLabel>
</skos:Concept><skos:Concept rdf:about="http://cognitiveatlas.org/id/trm_4c8990c87035d"> <dc:identifier>trm_4c8990c87035d</dc:identifier>
		<dc:Title>Cognitive Atlas : Lexicon : Naming (Covert)</dc:Title>
		<dc:Description>RDF output for 'Naming (Covert)'</dc:Description>
		<dc:Type>InteractiveResource</dc:Type>
		<dc:Publisher>Cognitive Atlas</dc:Publisher>
		<dc:Creator>Cognitive Atlas RDF Generator</dc:Creator>
		<dc:Contributor>Brenda Gregory</dc:Contributor>
		<dc:Date>2011-04-27 14:01:14</dc:Date>
		<dc:Format>text/rdf</dc:Format>
		<dc:Language>en</dc:Language>
		<skos:editorialNote>Generated by testgen.php on Thu Jun 9 14:25:25 PDT 2011.</skos:editorialNote>
		<skos:historyNote>Revision 2: 1 previous definitions.</skos:historyNote>
		<skos:changeNote>See http://cognitiveatlas.org/id/trm_4c8990c87035d for complete revision history.</skos:changeNote>
		<skos:scopeNote>http://www.w3.org/2004/02/skos/core#Concept</skos:scopeNote>
		<skos:Note>SKOS properties defined in http://www.w3.org/TR/skos-primer/#secrel</skos:Note>
		<skos:inScheme rdf:resource="http://cognitiveatlas.org/tasks/"/>
		<skos:definition>Subjects view objects (pictures, line drawings, etc.) and name them silently.</skos:definition>
		<skos:prefLabel>Naming (Covert)</skos:prefLabel>
		<skos:altLabel></skos:altLabel>
</skos:Concept><skos:Concept rdf:about="http://cognitiveatlas.org/id/trm_4c8990e187dc7"> <dc:identifier>trm_4c8990e187dc7</dc:identifier>
		<dc:Title>Cognitive Atlas : Lexicon : Naming (Overt)</dc:Title>
		<dc:Description>RDF output for 'Naming (Overt)'</dc:Description>
		<dc:Type>InteractiveResource</dc:Type>
		<dc:Publisher>Cognitive Atlas</dc:Publisher>
		<dc:Creator>Cognitive Atlas RDF Generator</dc:Creator>
		<dc:Contributor>Brenda Gregory</dc:Contributor>
		<dc:Date>2011-04-27 14:00:46</dc:Date>
		<dc:Format>text/rdf</dc:Format>
		<dc:Language>en</dc:Language>
		<skos:editorialNote>Generated by testgen.php on Thu Jun 9 14:25:25 PDT 2011.</skos:editorialNote>
		<skos:historyNote>Revision 2: 1 previous definitions.</skos:historyNote>
		<skos:changeNote>See http://cognitiveatlas.org/id/trm_4c8990e187dc7 for complete revision history.</skos:changeNote>
		<skos:scopeNote>http://www.w3.org/2004/02/skos/core#Concept</skos:scopeNote>
		<skos:Note>SKOS properties defined in http://www.w3.org/TR/skos-primer/#secrel</skos:Note>
		<skos:inScheme rdf:resource="http://cognitiveatlas.org/tasks/"/>
		<skos:definition>Subjects view objects (pictures, line drawings, etc.)  and name them aloud.</skos:definition>
		<skos:prefLabel>Naming (Overt)</skos:prefLabel>
		<skos:altLabel></skos:altLabel>
</skos:Concept><skos:Concept rdf:about="http://cognitiveatlas.org/id/trm_4c8990f59266f"> <dc:identifier>trm_4c8990f59266f</dc:identifier>
		<dc:Title>Cognitive Atlas : Lexicon : Non-Painful Electrical Stimulation</dc:Title>
		<dc:Description>RDF output for 'Non-Painful Electrical Stimulation'</dc:Description>
		<dc:Type>InteractiveResource</dc:Type>
		<dc:Publisher>Cognitive Atlas</dc:Publisher>
		<dc:Creator>Cognitive Atlas RDF Generator</dc:Creator>
		<dc:Contributor>Brenda Gregory</dc:Contributor>
		<dc:Date>2011-04-27 14:11:03</dc:Date>
		<dc:Format>text/rdf</dc:Format>
		<dc:Language>en</dc:Language>
		<skos:editorialNote>Generated by testgen.php on Thu Jun 9 14:25:25 PDT 2011.</skos:editorialNote>
		<skos:historyNote>Revision 2: 1 previous definitions.</skos:historyNote>
		<skos:changeNote>See http://cognitiveatlas.org/id/trm_4c8990f59266f for complete revision history.</skos:changeNote>
		<skos:scopeNote>http://www.w3.org/2004/02/skos/core#Concept</skos:scopeNote>
		<skos:Note>SKOS properties defined in http://www.w3.org/TR/skos-primer/#secrel</skos:Note>
		<skos:inScheme rdf:resource="http://cognitiveatlas.org/tasks/"/>
		<skos:definition>Subjects are electrically stimulated at a non-painful threshold.</skos:definition>
		<skos:prefLabel>Non-Painful Electrical Stimulation</skos:prefLabel>
		<skos:altLabel></skos:altLabel>
</skos:Concept><skos:Concept rdf:about="http://cognitiveatlas.org/id/trm_4c89910b7f8bc"> <dc:identifier>trm_4c89910b7f8bc</dc:identifier>
		<dc:Title>Cognitive Atlas : Lexicon : Non-Painful Thermal Stimulation</dc:Title>
		<dc:Description>RDF output for 'Non-Painful Thermal Stimulation'</dc:Description>
		<dc:Type>InteractiveResource</dc:Type>
		<dc:Publisher>Cognitive Atlas</dc:Publisher>
		<dc:Creator>Cognitive Atlas RDF Generator</dc:Creator>
		<dc:Contributor>Brenda Gregory</dc:Contributor>
		<dc:Date>2011-04-27 14:11:36</dc:Date>
		<dc:Format>text/rdf</dc:Format>
		<dc:Language>en</dc:Language>
		<skos:editorialNote>Generated by testgen.php on Thu Jun 9 14:25:25 PDT 2011.</skos:editorialNote>
		<skos:historyNote>Revision 2: 1 previous definitions.</skos:historyNote>
		<skos:changeNote>See http://cognitiveatlas.org/id/trm_4c89910b7f8bc for complete revision history.</skos:changeNote>
		<skos:scopeNote>http://www.w3.org/2004/02/skos/core#Concept</skos:scopeNote>
		<skos:Note>SKOS properties defined in http://www.w3.org/TR/skos-primer/#secrel</skos:Note>
		<skos:inScheme rdf:resource="http://cognitiveatlas.org/tasks/"/>
		<skos:definition>Subjects experience thermal stimulation (heat) at a non-painful threshold.</skos:definition>
		<skos:prefLabel>Non-Painful Thermal Stimulation</skos:prefLabel>
		<skos:altLabel></skos:altLabel>
</skos:Concept><skos:Concept rdf:about="http://cognitiveatlas.org/id/trm_4c89912c79030"> <dc:identifier>trm_4c89912c79030</dc:identifier>
		<dc:Title>Cognitive Atlas : Lexicon : Olfactory Monitor/Discrimination</dc:Title>
		<dc:Description>RDF output for 'Olfactory Monitor/Discrimination'</dc:Description>
		<dc:Type>InteractiveResource</dc:Type>
		<dc:Publisher>Cognitive Atlas</dc:Publisher>
		<dc:Creator>Cognitive Atlas RDF Generator</dc:Creator>
		<dc:Contributor>Brenda Gregory</dc:Contributor>
		<dc:Date>2011-04-27 14:10:26</dc:Date>
		<dc:Format>text/rdf</dc:Format>
		<dc:Language>en</dc:Language>
		<skos:editorialNote>Generated by testgen.php on Thu Jun 9 14:25:25 PDT 2011.</skos:editorialNote>
		<skos:historyNote>Revision 2: 1 previous definitions.</skos:historyNote>
		<skos:changeNote>See http://cognitiveatlas.org/id/trm_4c89912c79030 for complete revision history.</skos:changeNote>
		<skos:scopeNote>http://www.w3.org/2004/02/skos/core#Concept</skos:scopeNote>
		<skos:Note>SKOS properties defined in http://www.w3.org/TR/skos-primer/#secrel</skos:Note>
		<skos:inScheme rdf:resource="http://cognitiveatlas.org/tasks/"/>
		<skos:definition>Subjects are presented with odors and are instructed to smell them passively or to discriminate according to some feature (pleasant/unpleasant, strong/weak, same/different, etc.).</skos:definition>
		<skos:prefLabel>Olfactory Monitor/Discrimination</skos:prefLabel>
		<skos:altLabel></skos:altLabel>
</skos:Concept><skos:Concept rdf:about="http://cognitiveatlas.org/id/trm_4c89913f80802"> <dc:identifier>trm_4c89913f80802</dc:identifier>
		<dc:Title>Cognitive Atlas : Lexicon : Orthographic Discrimination</dc:Title>
		<dc:Description>RDF output for 'Orthographic Discrimination'</dc:Description>
		<dc:Type>InteractiveResource</dc:Type>
		<dc:Publisher>Cognitive Atlas</dc:Publisher>
		<dc:Creator>Cognitive Atlas RDF Generator</dc:Creator>
		<dc:Contributor>Brenda Gregory</dc:Contributor>
		<dc:Date>2011-04-27 14:09:45</dc:Date>
		<dc:Format>text/rdf</dc:Format>
		<dc:Language>en</dc:Language>
		<skos:editorialNote>Generated by testgen.php on Thu Jun 9 14:25:25 PDT 2011.</skos:editorialNote>
		<skos:historyNote>Revision 2: 1 previous definitions.</skos:historyNote>
		<skos:changeNote>See http://cognitiveatlas.org/id/trm_4c89913f80802 for complete revision history.</skos:changeNote>
		<skos:scopeNote>http://www.w3.org/2004/02/skos/core#Concept</skos:scopeNote>
		<skos:Note>SKOS properties defined in http://www.w3.org/TR/skos-primer/#secrel</skos:Note>
		<skos:inScheme rdf:resource="http://cognitiveatlas.org/tasks/"/>
		<skos:definition>Subjects view letters and discriminate according to some feature (uppercase/lowercase, alphabetic order, same/different spelling of words, vowel/consonant, font size, etc.).</skos:definition>
		<skos:prefLabel>Orthographic Discrimination</skos:prefLabel>
		<skos:altLabel></skos:altLabel>
</skos:Concept><skos:Concept rdf:about="http://cognitiveatlas.org/id/trm_4c8991c5beb0a"> <dc:identifier>trm_4c8991c5beb0a</dc:identifier>
		<dc:Title>Cognitive Atlas : Lexicon : Pain Monitor/Discrimination Task</dc:Title>
		<dc:Description>RDF output for 'Pain Monitor/Discrimination Task'</dc:Description>
		<dc:Type>InteractiveResource</dc:Type>
		<dc:Publisher>Cognitive Atlas</dc:Publisher>
		<dc:Creator>Cognitive Atlas RDF Generator</dc:Creator>
		<dc:Contributor>Brenda Gregory</dc:Contributor>
		<dc:Date>2011-04-27 14:09:14</dc:Date>
		<dc:Format>text/rdf</dc:Format>
		<dc:Language>en</dc:Language>
		<skos:editorialNote>Generated by testgen.php on Thu Jun 9 14:25:25 PDT 2011.</skos:editorialNote>
		<skos:historyNote>Revision 3: 2 previous definitions.</skos:historyNote>
		<skos:changeNote>See http://cognitiveatlas.org/id/trm_4c8991c5beb0a for complete revision history.</skos:changeNote>
		<skos:scopeNote>http://www.w3.org/2004/02/skos/core#Concept</skos:scopeNote>
		<skos:Note>SKOS properties defined in http://www.w3.org/TR/skos-primer/#secrel</skos:Note>
		<skos:inScheme rdf:resource="http://cognitiveatlas.org/tasks/"/>
		<skos:definition>Subjects experience thermal or electrical stimulation at a painful threshold.</skos:definition>
		<skos:prefLabel>Pain Monitor/Discrimination Task</skos:prefLabel>
		<skos:altLabel></skos:altLabel>
</skos:Concept><skos:Concept rdf:about="http://cognitiveatlas.org/id/trm_4c8991e6e8597"> <dc:identifier>trm_4c8991e6e8597</dc:identifier>
		<dc:Title>Cognitive Atlas : Lexicon : Paired Associate Recall</dc:Title>
		<dc:Description>RDF output for 'Paired Associate Recall'</dc:Description>
		<dc:Type>InteractiveResource</dc:Type>
		<dc:Publisher>Cognitive Atlas</dc:Publisher>
		<dc:Creator>Cognitive Atlas RDF Generator</dc:Creator>
		<dc:Contributor>Brenda Gregory</dc:Contributor>
		<dc:Date>2011-04-27 14:08:41</dc:Date>
		<dc:Format>text/rdf</dc:Format>
		<dc:Language>en</dc:Language>
		<skos:editorialNote>Generated by testgen.php on Thu Jun 9 14:25:25 PDT 2011.</skos:editorialNote>
		<skos:historyNote>Revision 2: 1 previous definitions.</skos:historyNote>
		<skos:changeNote>See http://cognitiveatlas.org/id/trm_4c8991e6e8597 for complete revision history.</skos:changeNote>
		<skos:scopeNote>http://www.w3.org/2004/02/skos/core#Concept</skos:scopeNote>
		<skos:Note>SKOS properties defined in http://www.w3.org/TR/skos-primer/#secrel</skos:Note>
		<skos:inScheme rdf:resource="http://cognitiveatlas.org/tasks/"/>
		<skos:definition>Subjects are shown paired stimuli prior to the task.  During the task, subjects are shown a single stimuli and are asked to recall the associated pair.  Stimuli may be words, faces, objects, etc.</skos:definition>
		<skos:prefLabel>Paired Associate Recall</skos:prefLabel>
		<skos:altLabel></skos:altLabel>
</skos:Concept><skos:Concept rdf:about="http://cognitiveatlas.org/id/trm_4c8991fadfe01"> <dc:identifier>trm_4c8991fadfe01</dc:identifier>
		<dc:Title>Cognitive Atlas : Lexicon : Passive Listening</dc:Title>
		<dc:Description>RDF output for 'Passive Listening'</dc:Description>
		<dc:Type>InteractiveResource</dc:Type>
		<dc:Publisher>Cognitive Atlas</dc:Publisher>
		<dc:Creator>Cognitive Atlas RDF Generator</dc:Creator>
		<dc:Contributor>Brenda Gregory</dc:Contributor>
		<dc:Date>2011-04-27 14:06:12</dc:Date>
		<dc:Format>text/rdf</dc:Format>
		<dc:Language>en</dc:Language>
		<skos:editorialNote>Generated by testgen.php on Thu Jun 9 14:25:25 PDT 2011.</skos:editorialNote>
		<skos:historyNote>Revision 2: 1 previous definitions.</skos:historyNote>
		<skos:changeNote>See http://cognitiveatlas.org/id/trm_4c8991fadfe01 for complete revision history.</skos:changeNote>
		<skos:scopeNote>http://www.w3.org/2004/02/skos/core#Concept</skos:scopeNote>
		<skos:Note>SKOS properties defined in http://www.w3.org/TR/skos-primer/#secrel</skos:Note>
		<skos:inScheme rdf:resource="http://cognitiveatlas.org/tasks/"/>
		<skos:definition>Subjects listen to various auditory stimuli and make no response.  Stimuli include speech (words, sentences), noise, tones, etc.  If the stimulus is tones, then the experiment is co-coded with Tone Monitor/Discrimination.</skos:definition>
		<skos:prefLabel>Passive Listening</skos:prefLabel>
		<skos:altLabel></skos:altLabel>
</skos:Concept><skos:Concept rdf:about="http://cognitiveatlas.org/id/trm_4c899211a965c"> <dc:identifier>trm_4c899211a965c</dc:identifier>
		<dc:Title>Cognitive Atlas : Lexicon : Passive Viewing</dc:Title>
		<dc:Description>RDF output for 'Passive Viewing'</dc:Description>
		<dc:Type>InteractiveResource</dc:Type>
		<dc:Publisher>Cognitive Atlas</dc:Publisher>
		<dc:Creator>Cognitive Atlas RDF Generator</dc:Creator>
		<dc:Contributor>Brenda Gregory</dc:Contributor>
		<dc:Date>2011-04-27 14:05:32</dc:Date>
		<dc:Format>text/rdf</dc:Format>
		<dc:Language>en</dc:Language>
		<skos:editorialNote>Generated by testgen.php on Thu Jun 9 14:25:25 PDT 2011.</skos:editorialNote>
		<skos:historyNote>Revision 2: 1 previous definitions.</skos:historyNote>
		<skos:changeNote>See http://cognitiveatlas.org/id/trm_4c899211a965c for complete revision history.</skos:changeNote>
		<skos:scopeNote>http://www.w3.org/2004/02/skos/core#Concept</skos:scopeNote>
		<skos:Note>SKOS properties defined in http://www.w3.org/TR/skos-primer/#secrel</skos:Note>
		<skos:inScheme rdf:resource="http://cognitiveatlas.org/tasks/"/>
		<skos:definition>Subjects view various visual stimuli and make no response.  Stimuli include houses, faces, objects, fractals, letter strings, line drawings, complex scenes, etc. If the presented stimuli were faces, the experiments are co-coded with Face Monitor/Discrimination.  But if the presented stimuli are words, the experiments are NOT coded as Passive Viewing but rather as Reading (Covert).</skos:definition>
		<skos:prefLabel>Passive Viewing</skos:prefLabel>
		<skos:altLabel></skos:altLabel>
</skos:Concept><skos:Concept rdf:about="http://cognitiveatlas.org/id/trm_4c89922cb6402"> <dc:identifier>trm_4c89922cb6402</dc:identifier>
		<dc:Title>Cognitive Atlas : Lexicon : Phonological Discrimination</dc:Title>
		<dc:Description>RDF output for 'Phonological Discrimination'</dc:Description>
		<dc:Type>InteractiveResource</dc:Type>
		<dc:Publisher>Cognitive Atlas</dc:Publisher>
		<dc:Creator>Cognitive Atlas RDF Generator</dc:Creator>
		<dc:Contributor>Brenda Gregory</dc:Contributor>
		<dc:Date>2011-04-27 14:04:53</dc:Date>
		<dc:Format>text/rdf</dc:Format>
		<dc:Language>en</dc:Language>
		<skos:editorialNote>Generated by testgen.php on Thu Jun 9 14:25:25 PDT 2011.</skos:editorialNote>
		<skos:historyNote>Revision 2: 1 previous definitions.</skos:historyNote>
		<skos:changeNote>See http://cognitiveatlas.org/id/trm_4c89922cb6402 for complete revision history.</skos:changeNote>
		<skos:scopeNote>http://www.w3.org/2004/02/skos/core#Concept</skos:scopeNote>
		<skos:Note>SKOS properties defined in http://www.w3.org/TR/skos-primer/#secrel</skos:Note>
		<skos:inScheme rdf:resource="http://cognitiveatlas.org/tasks/"/>
		<skos:definition>Subjects view or listen to phonemes, syllables, or words and discriminate according to some feature of their sounds (rhyming, number of syllables, homophones, etc.).</skos:definition>
		<skos:prefLabel>Phonological Discrimination</skos:prefLabel>
		<skos:altLabel></skos:altLabel>
</skos:Concept><skos:Concept rdf:about="http://cognitiveatlas.org/id/trm_4c89924414c69"> <dc:identifier>trm_4c89924414c69</dc:identifier>
		<dc:Title>Cognitive Atlas : Lexicon : Pitch Monitor/Discrimination</dc:Title>
		<dc:Description>RDF output for 'Pitch Monitor/Discrimination'</dc:Description>
		<dc:Type>InteractiveResource</dc:Type>
		<dc:Publisher>Cognitive Atlas</dc:Publisher>
		<dc:Creator>Cognitive Atlas RDF Generator</dc:Creator>
		<dc:Contributor>Brenda Gregory</dc:Contributor>
		<dc:Date>2011-04-27 14:04:13</dc:Date>
		<dc:Format>text/rdf</dc:Format>
		<dc:Language>en</dc:Language>
		<skos:editorialNote>Generated by testgen.php on Thu Jun 9 14:25:25 PDT 2011.</skos:editorialNote>
		<skos:historyNote>Revision 2: 1 previous definitions.</skos:historyNote>
		<skos:changeNote>See http://cognitiveatlas.org/id/trm_4c89924414c69 for complete revision history.</skos:changeNote>
		<skos:scopeNote>http://www.w3.org/2004/02/skos/core#Concept</skos:scopeNote>
		<skos:Note>SKOS properties defined in http://www.w3.org/TR/skos-primer/#secrel</skos:Note>
		<skos:inScheme rdf:resource="http://cognitiveatlas.org/tasks/"/>
		<skos:definition>Subjects are presented with various stimuli (human speech and non-speech vocalizations, animal vocalization, mechanical noise, etc.) and are instructed to listen to them passively (also co-coded with Passive Listening), or discriminate based on pitch (pleasant/unpleasant, same/different, duration, familiar/unfamiliar, male/female).</skos:definition>
		<skos:prefLabel>Pitch Monitor/Discrimination</skos:prefLabel>
		<skos:altLabel></skos:altLabel>
</skos:Concept><skos:Concept rdf:about="http://cognitiveatlas.org/id/trm_4c89926767870"> <dc:identifier>trm_4c89926767870</dc:identifier>
		<dc:Title>Cognitive Atlas : Lexicon : Pointing</dc:Title>
		<dc:Description>RDF output for 'Pointing'</dc:Description>
		<dc:Type>InteractiveResource</dc:Type>
		<dc:Publisher>Cognitive Atlas</dc:Publisher>
		<dc:Creator>Cognitive Atlas RDF Generator</dc:Creator>
		<dc:Contributor>Brenda Gregory</dc:Contributor>
		<dc:Date>2011-04-27 14:03:44</dc:Date>
		<dc:Format>text/rdf</dc:Format>
		<dc:Language>en</dc:Language>
		<skos:editorialNote>Generated by testgen.php on Thu Jun 9 14:25:25 PDT 2011.</skos:editorialNote>
		<skos:historyNote>Revision 2: 1 previous definitions.</skos:historyNote>
		<skos:changeNote>See http://cognitiveatlas.org/id/trm_4c89926767870 for complete revision history.</skos:changeNote>
		<skos:scopeNote>http://www.w3.org/2004/02/skos/core#Concept</skos:scopeNote>
		<skos:Note>SKOS properties defined in http://www.w3.org/TR/skos-primer/#secrel</skos:Note>
		<skos:inScheme rdf:resource="http://cognitiveatlas.org/tasks/"/>
		<skos:definition>Subjects look and point at a target (e.g., cursor with their arm, hand, finger, or shoulder.</skos:definition>
		<skos:prefLabel>Pointing</skos:prefLabel>
		<skos:altLabel></skos:altLabel>
</skos:Concept><skos:Concept rdf:about="http://cognitiveatlas.org/id/trm_4c8a82ba8a538"> <dc:identifier>trm_4c8a82ba8a538</dc:identifier>
		<dc:Title>Cognitive Atlas : Lexicon : Reading (Covert)</dc:Title>
		<dc:Description>RDF output for 'Reading (Covert)'</dc:Description>
		<dc:Type>InteractiveResource</dc:Type>
		<dc:Publisher>Cognitive Atlas</dc:Publisher>
		<dc:Creator>Cognitive Atlas RDF Generator</dc:Creator>
		<dc:Contributor>Brenda Gregory</dc:Contributor>
		<dc:Date>2011-04-27 14:03:08</dc:Date>
		<dc:Format>text/rdf</dc:Format>
		<dc:Language>en</dc:Language>
		<skos:editorialNote>Generated by testgen.php on Thu Jun 9 14:25:25 PDT 2011.</skos:editorialNote>
		<skos:historyNote>Revision 2: 1 previous definitions.</skos:historyNote>
		<skos:changeNote>See http://cognitiveatlas.org/id/trm_4c8a82ba8a538 for complete revision history.</skos:changeNote>
		<skos:scopeNote>http://www.w3.org/2004/02/skos/core#Concept</skos:scopeNote>
		<skos:Note>SKOS properties defined in http://www.w3.org/TR/skos-primer/#secrel</skos:Note>
		<skos:inScheme rdf:resource="http://cognitiveatlas.org/tasks/"/>
		<skos:definition>Subjects view words, pseudo-words,  Asian characters, phrases, or sentences and read them silently.</skos:definition>
		<skos:prefLabel>Reading (Covert)</skos:prefLabel>
		<skos:altLabel></skos:altLabel>
</skos:Concept><skos:Concept rdf:about="http://cognitiveatlas.org/id/trm_4c8a82eeaa58f"> <dc:identifier>trm_4c8a82eeaa58f</dc:identifier>
		<dc:Title>Cognitive Atlas : Lexicon : Reading (Overt)</dc:Title>
		<dc:Description>RDF output for 'Reading (Overt)'</dc:Description>
		<dc:Type>InteractiveResource</dc:Type>
		<dc:Publisher>Cognitive Atlas</dc:Publisher>
		<dc:Creator>Cognitive Atlas RDF Generator</dc:Creator>
		<dc:Contributor>Brenda Gregory</dc:Contributor>
		<dc:Date>2011-04-26 14:20:27</dc:Date>
		<dc:Format>text/rdf</dc:Format>
		<dc:Language>en</dc:Language>
		<skos:editorialNote>Generated by testgen.php on Thu Jun 9 14:25:25 PDT 2011.</skos:editorialNote>
		<skos:historyNote>Revision 2: 1 previous definitions.</skos:historyNote>
		<skos:changeNote>See http://cognitiveatlas.org/id/trm_4c8a82eeaa58f for complete revision history.</skos:changeNote>
		<skos:scopeNote>http://www.w3.org/2004/02/skos/core#Concept</skos:scopeNote>
		<skos:Note>SKOS properties defined in http://www.w3.org/TR/skos-primer/#secrel</skos:Note>
		<skos:inScheme rdf:resource="http://cognitiveatlas.org/tasks/"/>
		<skos:definition>Subjects view words, pseudo-words, Asian characters, phrases, or sentences and read them aloud.</skos:definition>
		<skos:prefLabel>Reading (Overt)</skos:prefLabel>
		<skos:altLabel></skos:altLabel>
</skos:Concept><skos:Concept rdf:about="http://cognitiveatlas.org/id/trm_4c8a830dec136"> <dc:identifier>trm_4c8a830dec136</dc:identifier>
		<dc:Title>Cognitive Atlas : Lexicon : Recitation/Repetition (Covert)</dc:Title>
		<dc:Description>RDF output for 'Recitation/Repetition (Covert)'</dc:Description>
		<dc:Type>InteractiveResource</dc:Type>
		<dc:Publisher>Cognitive Atlas</dc:Publisher>
		<dc:Creator>Cognitive Atlas RDF Generator</dc:Creator>
		<dc:Contributor>Brenda Gregory</dc:Contributor>
		<dc:Date>2011-04-26 14:20:07</dc:Date>
		<dc:Format>text/rdf</dc:Format>
		<dc:Language>en</dc:Language>
		<skos:editorialNote>Generated by testgen.php on Thu Jun 9 14:25:25 PDT 2011.</skos:editorialNote>
		<skos:historyNote>Revision 2: 1 previous definitions.</skos:historyNote>
		<skos:changeNote>See http://cognitiveatlas.org/id/trm_4c8a830dec136 for complete revision history.</skos:changeNote>
		<skos:scopeNote>http://www.w3.org/2004/02/skos/core#Concept</skos:scopeNote>
		<skos:Note>SKOS properties defined in http://www.w3.org/TR/skos-primer/#secrel</skos:Note>
		<skos:inScheme rdf:resource="http://cognitiveatlas.org/tasks/"/>
		<skos:definition>Subjects silently repeat or recite phonemes, words, or well-known text (nursery rhymes, Pledge of Allegiance, months of the year, etc.).</skos:definition>
		<skos:prefLabel>Recitation/Repetition (Covert)</skos:prefLabel>
		<skos:altLabel></skos:altLabel>
</skos:Concept><skos:Concept rdf:about="http://cognitiveatlas.org/id/trm_4c8a8329cb8ff"> <dc:identifier>trm_4c8a8329cb8ff</dc:identifier>
		<dc:Title>Cognitive Atlas : Lexicon : Recitation/Repetition (Overt)</dc:Title>
		<dc:Description>RDF output for 'Recitation/Repetition (Overt)'</dc:Description>
		<dc:Type>InteractiveResource</dc:Type>
		<dc:Publisher>Cognitive Atlas</dc:Publisher>
		<dc:Creator>Cognitive Atlas RDF Generator</dc:Creator>
		<dc:Contributor>Brenda Gregory</dc:Contributor>
		<dc:Date>2011-04-26 14:19:47</dc:Date>
		<dc:Format>text/rdf</dc:Format>
		<dc:Language>en</dc:Language>
		<skos:editorialNote>Generated by testgen.php on Thu Jun 9 14:25:25 PDT 2011.</skos:editorialNote>
		<skos:historyNote>Revision 2: 1 previous definitions.</skos:historyNote>
		<skos:changeNote>See http://cognitiveatlas.org/id/trm_4c8a8329cb8ff for complete revision history.</skos:changeNote>
		<skos:scopeNote>http://www.w3.org/2004/02/skos/core#Concept</skos:scopeNote>
		<skos:Note>SKOS properties defined in http://www.w3.org/TR/skos-primer/#secrel</skos:Note>
		<skos:inScheme rdf:resource="http://cognitiveatlas.org/tasks/"/>
		<skos:definition>Subjects repeat or recite phonemes, words, or well-known text (nursery rhymes, Pledge of Allegiance, months of the year, etc.) aloud.</skos:definition>
		<skos:prefLabel>Recitation/Repetition (Overt)</skos:prefLabel>
		<skos:altLabel></skos:altLabel>
</skos:Concept><skos:Concept rdf:about="http://cognitiveatlas.org/id/trm_4c8a834779883"> <dc:identifier>trm_4c8a834779883</dc:identifier>
		<dc:Title>Cognitive Atlas : Lexicon : Rest</dc:Title>
		<dc:Description>RDF output for 'Rest'</dc:Description>
		<dc:Type>InteractiveResource</dc:Type>
		<dc:Publisher>Cognitive Atlas</dc:Publisher>
		<dc:Creator>Cognitive Atlas RDF Generator</dc:Creator>
		<dc:Contributor>Brenda Gregory</dc:Contributor>
		<dc:Date>2011-04-26 14:19:25</dc:Date>
		<dc:Format>text/rdf</dc:Format>
		<dc:Language>en</dc:Language>
		<skos:editorialNote>Generated by testgen.php on Thu Jun 9 14:25:25 PDT 2011.</skos:editorialNote>
		<skos:historyNote>Revision 2: 1 previous definitions.</skos:historyNote>
		<skos:changeNote>See http://cognitiveatlas.org/id/trm_4c8a834779883 for complete revision history.</skos:changeNote>
		<skos:scopeNote>http://www.w3.org/2004/02/skos/core#Concept</skos:scopeNote>
		<skos:Note>SKOS properties defined in http://www.w3.org/TR/skos-primer/#secrel</skos:Note>
		<skos:inScheme rdf:resource="http://cognitiveatlas.org/tasks/"/>
		<skos:definition>Subjects rest passively with their eyes open or closed.</skos:definition>
		<skos:prefLabel>Rest</skos:prefLabel>
		<skos:altLabel></skos:altLabel>
</skos:Concept><skos:Concept rdf:about="http://cognitiveatlas.org/id/trm_4c8a8388de5ea"> <dc:identifier>trm_4c8a8388de5ea</dc:identifier>
		<dc:Title>Cognitive Atlas : Lexicon : Reward Task</dc:Title>
		<dc:Description>RDF output for 'Reward Task'</dc:Description>
		<dc:Type>InteractiveResource</dc:Type>
		<dc:Publisher>Cognitive Atlas</dc:Publisher>
		<dc:Creator>Cognitive Atlas RDF Generator</dc:Creator>
		<dc:Contributor>Brenda Gregory</dc:Contributor>
		<dc:Date>2011-04-26 14:19:10</dc:Date>
		<dc:Format>text/rdf</dc:Format>
		<dc:Language>en</dc:Language>
		<skos:editorialNote>Generated by testgen.php on Thu Jun 9 14:25:25 PDT 2011.</skos:editorialNote>
		<skos:historyNote>Revision 2: 1 previous definitions.</skos:historyNote>
		<skos:changeNote>See http://cognitiveatlas.org/id/trm_4c8a8388de5ea for complete revision history.</skos:changeNote>
		<skos:scopeNote>http://www.w3.org/2004/02/skos/core#Concept</skos:scopeNote>
		<skos:Note>SKOS properties defined in http://www.w3.org/TR/skos-primer/#secrel</skos:Note>
		<skos:inScheme rdf:resource="http://cognitiveatlas.org/tasks/"/>
		<skos:definition>Subjects perform a task in which correct performance is associated with reward, often monetary reward.</skos:definition>
		<skos:prefLabel>Reward Task</skos:prefLabel>
		<skos:altLabel></skos:altLabel>
</skos:Concept><skos:Concept rdf:about="http://cognitiveatlas.org/id/trm_4c8a83cac75f5"> <dc:identifier>trm_4c8a83cac75f5</dc:identifier>
		<dc:Title>Cognitive Atlas : Lexicon : Sequence Recall/Learning</dc:Title>
		<dc:Description>RDF output for 'Sequence Recall/Learning'</dc:Description>
		<dc:Type>InteractiveResource</dc:Type>
		<dc:Publisher>Cognitive Atlas</dc:Publisher>
		<dc:Creator>Cognitive Atlas RDF Generator</dc:Creator>
		<dc:Contributor>Brenda Gregory</dc:Contributor>
		<dc:Date>2011-04-26 14:18:50</dc:Date>
		<dc:Format>text/rdf</dc:Format>
		<dc:Language>en</dc:Language>
		<skos:editorialNote>Generated by testgen.php on Thu Jun 9 14:25:25 PDT 2011.</skos:editorialNote>
		<skos:historyNote>Revision 2: 1 previous definitions.</skos:historyNote>
		<skos:changeNote>See http://cognitiveatlas.org/id/trm_4c8a83cac75f5 for complete revision history.</skos:changeNote>
		<skos:scopeNote>http://www.w3.org/2004/02/skos/core#Concept</skos:scopeNote>
		<skos:Note>SKOS properties defined in http://www.w3.org/TR/skos-primer/#secrel</skos:Note>
		<skos:inScheme rdf:resource="http://cognitiveatlas.org/tasks/"/>
		<skos:definition>Subjects learn and/or perform a complex sequence of finger tapping, button pressing, pointing/clicking, or various other motor responses.</skos:definition>
		<skos:prefLabel>Sequence Recall/Learning</skos:prefLabel>
		<skos:altLabel></skos:altLabel>
</skos:Concept><skos:Concept rdf:about="http://cognitiveatlas.org/id/trm_4c8a83f27ac55"> <dc:identifier>trm_4c8a83f27ac55</dc:identifier>
		<dc:Title>Cognitive Atlas : Lexicon : Spatial/Location Discrimination</dc:Title>
		<dc:Description>RDF output for 'Spatial/Location Discrimination'</dc:Description>
		<dc:Type>InteractiveResource</dc:Type>
		<dc:Publisher>Cognitive Atlas</dc:Publisher>
		<dc:Creator>Cognitive Atlas RDF Generator</dc:Creator>
		<dc:Contributor>Brenda Gregory</dc:Contributor>
		<dc:Date>2011-04-26 14:18:31</dc:Date>
		<dc:Format>text/rdf</dc:Format>
		<dc:Language>en</dc:Language>
		<skos:editorialNote>Generated by testgen.php on Thu Jun 9 14:25:25 PDT 2011.</skos:editorialNote>
		<skos:historyNote>Revision 2: 1 previous definitions.</skos:historyNote>
		<skos:changeNote>See http://cognitiveatlas.org/id/trm_4c8a83f27ac55 for complete revision history.</skos:changeNote>
		<skos:scopeNote>http://www.w3.org/2004/02/skos/core#Concept</skos:scopeNote>
		<skos:Note>SKOS properties defined in http://www.w3.org/TR/skos-primer/#secrel</skos:Note>
		<skos:inScheme rdf:resource="http://cognitiveatlas.org/tasks/"/>
		<skos:definition>Subjects view shapes or other stimuli (letters, pictures, numbers, or arrows) and discriminate according to their location, orientation, or size.</skos:definition>
		<skos:prefLabel>Spatial/Location Discrimination</skos:prefLabel>
		<skos:altLabel></skos:altLabel>
</skos:Concept><skos:Concept rdf:about="http://cognitiveatlas.org/id/trm_4c8a840d6f969"> <dc:identifier>trm_4c8a840d6f969</dc:identifier>
		<dc:Title>Cognitive Atlas : Lexicon : Subjective Emotional Picture Discrimination</dc:Title>
		<dc:Description>RDF output for 'Subjective Emotional Picture Discrimination'</dc:Description>
		<dc:Type>InteractiveResource</dc:Type>
		<dc:Publisher>Cognitive Atlas</dc:Publisher>
		<dc:Creator>Cognitive Atlas RDF Generator</dc:Creator>
		<dc:Contributor>Brenda Gregory</dc:Contributor>
		<dc:Date>2011-04-26 14:18:08</dc:Date>
		<dc:Format>text/rdf</dc:Format>
		<dc:Language>en</dc:Language>
		<skos:editorialNote>Generated by testgen.php on Thu Jun 9 14:25:25 PDT 2011.</skos:editorialNote>
		<skos:historyNote>Revision 2: 1 previous definitions.</skos:historyNote>
		<skos:changeNote>See http://cognitiveatlas.org/id/trm_4c8a840d6f969 for complete revision history.</skos:changeNote>
		<skos:scopeNote>http://www.w3.org/2004/02/skos/core#Concept</skos:scopeNote>
		<skos:Note>SKOS properties defined in http://www.w3.org/TR/skos-primer/#secrel</skos:Note>
		<skos:inScheme rdf:resource="http://cognitiveatlas.org/tasks/"/>
		<skos:definition>Subjects view pictures and are instructed to respond to emotional pictures, to indicate which pictures are pleasant/unpleasant or funny/not funny, or rate the valence of emotional pictures.</skos:definition>
		<skos:prefLabel>Subjective Emotional Picture Discrimination</skos:prefLabel>
		<skos:altLabel></skos:altLabel>
</skos:Concept><skos:Concept rdf:about="http://cognitiveatlas.org/id/trm_4c8a842512a33"> <dc:identifier>trm_4c8a842512a33</dc:identifier>
		<dc:Title>Cognitive Atlas : Lexicon : Syntactic Discrimination</dc:Title>
		<dc:Description>RDF output for 'Syntactic Discrimination'</dc:Description>
		<dc:Type>InteractiveResource</dc:Type>
		<dc:Publisher>Cognitive Atlas</dc:Publisher>
		<dc:Creator>Cognitive Atlas RDF Generator</dc:Creator>
		<dc:Contributor>Brenda Gregory</dc:Contributor>
		<dc:Date>2011-04-26 14:17:49</dc:Date>
		<dc:Format>text/rdf</dc:Format>
		<dc:Language>en</dc:Language>
		<skos:editorialNote>Generated by testgen.php on Thu Jun 9 14:25:25 PDT 2011.</skos:editorialNote>
		<skos:historyNote>Revision 2: 1 previous definitions.</skos:historyNote>
		<skos:changeNote>See http://cognitiveatlas.org/id/trm_4c8a842512a33 for complete revision history.</skos:changeNote>
		<skos:scopeNote>http://www.w3.org/2004/02/skos/core#Concept</skos:scopeNote>
		<skos:Note>SKOS properties defined in http://www.w3.org/TR/skos-primer/#secrel</skos:Note>
		<skos:inScheme rdf:resource="http://cognitiveatlas.org/tasks/"/>
		<skos:definition>Subjects viewed grammatically correct and incorrect sentences and discriminate according to their grammar.  This class also includes morphosyntactic tasks such as gender discrimination of words.</skos:definition>
		<skos:prefLabel>Syntactic Discrimination</skos:prefLabel>
		<skos:altLabel></skos:altLabel>
</skos:Concept><skos:Concept rdf:about="http://cognitiveatlas.org/id/trm_4c8a843d8d352"> <dc:identifier>trm_4c8a843d8d352</dc:identifier>
		<dc:Title>Cognitive Atlas : Lexicon : Tactile Monitor/Discrimination</dc:Title>
		<dc:Description>RDF output for 'Tactile Monitor/Discrimination'</dc:Description>
		<dc:Type>InteractiveResource</dc:Type>
		<dc:Publisher>Cognitive Atlas</dc:Publisher>
		<dc:Creator>Cognitive Atlas RDF Generator</dc:Creator>
		<dc:Contributor>Brenda Gregory</dc:Contributor>
		<dc:Date>2011-04-26 14:17:27</dc:Date>
		<dc:Format>text/rdf</dc:Format>
		<dc:Language>en</dc:Language>
		<skos:editorialNote>Generated by testgen.php on Thu Jun 9 14:25:25 PDT 2011.</skos:editorialNote>
		<skos:historyNote>Revision 2: 1 previous definitions.</skos:historyNote>
		<skos:changeNote>See http://cognitiveatlas.org/id/trm_4c8a843d8d352 for complete revision history.</skos:changeNote>
		<skos:scopeNote>http://www.w3.org/2004/02/skos/core#Concept</skos:scopeNote>
		<skos:Note>SKOS properties defined in http://www.w3.org/TR/skos-primer/#secrel</skos:Note>
		<skos:inScheme rdf:resource="http://cognitiveatlas.org/tasks/"/>
		<skos:definition>Subjects experience tactile/somatosensory stimulation and are asked to attend passively or discriminate according to some feature (shape, texture, same/different, frequency of presentation,  etc.)  Also includes: subjects are presented with 3-dimensional objects and are asked to manipulate them in their hands and probe their features.</skos:definition>
		<skos:prefLabel>Tactile Monitor/Discrimination</skos:prefLabel>
		<skos:altLabel></skos:altLabel>
</skos:Concept><skos:Concept rdf:about="http://cognitiveatlas.org/id/trm_4c8a8467304e2"> <dc:identifier>trm_4c8a8467304e2</dc:identifier>
		<dc:Title>Cognitive Atlas : Lexicon : Theory of Mind Task</dc:Title>
		<dc:Description>RDF output for 'Theory of Mind Task'</dc:Description>
		<dc:Type>InteractiveResource</dc:Type>
		<dc:Publisher>Cognitive Atlas</dc:Publisher>
		<dc:Creator>Cognitive Atlas RDF Generator</dc:Creator>
		<dc:Contributor>Brenda Gregory</dc:Contributor>
		<dc:Date>2011-04-26 14:17:11</dc:Date>
		<dc:Format>text/rdf</dc:Format>
		<dc:Language>en</dc:Language>
		<skos:editorialNote>Generated by testgen.php on Thu Jun 9 14:25:25 PDT 2011.</skos:editorialNote>
		<skos:historyNote>Revision 2: 1 previous definitions.</skos:historyNote>
		<skos:changeNote>See http://cognitiveatlas.org/id/trm_4c8a8467304e2 for complete revision history.</skos:changeNote>
		<skos:scopeNote>http://www.w3.org/2004/02/skos/core#Concept</skos:scopeNote>
		<skos:Note>SKOS properties defined in http://www.w3.org/TR/skos-primer/#secrel</skos:Note>
		<skos:inScheme rdf:resource="http://cognitiveatlas.org/tasks/"/>
		<skos:definition>Subjects are asked to perform a task involving the understanding of another&#39;s personal beliefs and feelings or forming hypotheses regarding the mental states of others.</skos:definition>
		<skos:prefLabel>Theory of Mind Task</skos:prefLabel>
		<skos:altLabel></skos:altLabel>
</skos:Concept><skos:Concept rdf:about="http://cognitiveatlas.org/id/trm_4c8a84825c4e4"> <dc:identifier>trm_4c8a84825c4e4</dc:identifier>
		<dc:Title>Cognitive Atlas : Lexicon : Tone Monitor/Discrimination</dc:Title>
		<dc:Description>RDF output for 'Tone Monitor/Discrimination'</dc:Description>
		<dc:Type>InteractiveResource</dc:Type>
		<dc:Publisher>Cognitive Atlas</dc:Publisher>
		<dc:Creator>Cognitive Atlas RDF Generator</dc:Creator>
		<dc:Contributor>Brenda Gregory</dc:Contributor>
		<dc:Date>2011-04-26 14:16:53</dc:Date>
		<dc:Format>text/rdf</dc:Format>
		<dc:Language>en</dc:Language>
		<skos:editorialNote>Generated by testgen.php on Thu Jun 9 14:25:25 PDT 2011.</skos:editorialNote>
		<skos:historyNote>Revision 2: 1 previous definitions.</skos:historyNote>
		<skos:changeNote>See http://cognitiveatlas.org/id/trm_4c8a84825c4e4 for complete revision history.</skos:changeNote>
		<skos:scopeNote>http://www.w3.org/2004/02/skos/core#Concept</skos:scopeNote>
		<skos:Note>SKOS properties defined in http://www.w3.org/TR/skos-primer/#secrel</skos:Note>
		<skos:inScheme rdf:resource="http://cognitiveatlas.org/tasks/"/>
		<skos:definition>Subjects are presented with tones and are instructed to listen to them passively (also coded as Passive Listening) or discriminate according to their order, timing, pitch, frequency, or amplitude.</skos:definition>
		<skos:prefLabel>Tone Monitor/Discrimination</skos:prefLabel>
		<skos:altLabel></skos:altLabel>
</skos:Concept><skos:Concept rdf:about="http://cognitiveatlas.org/id/trm_4c8a8497df574"> <dc:identifier>trm_4c8a8497df574</dc:identifier>
		<dc:Title>Cognitive Atlas : Lexicon : Transcranial Magnetic Stimulation</dc:Title>
		<dc:Description>RDF output for 'Transcranial Magnetic Stimulation'</dc:Description>
		<dc:Type>InteractiveResource</dc:Type>
		<dc:Publisher>Cognitive Atlas</dc:Publisher>
		<dc:Creator>Cognitive Atlas RDF Generator</dc:Creator>
		<dc:Contributor>Brenda Gregory</dc:Contributor>
		<dc:Date>2011-04-26 14:16:36</dc:Date>
		<dc:Format>text/rdf</dc:Format>
		<dc:Language>en</dc:Language>
		<skos:editorialNote>Generated by testgen.php on Thu Jun 9 14:25:25 PDT 2011.</skos:editorialNote>
		<skos:historyNote>Revision 2: 1 previous definitions.</skos:historyNote>
		<skos:changeNote>See http://cognitiveatlas.org/id/trm_4c8a8497df574 for complete revision history.</skos:changeNote>
		<skos:scopeNote>http://www.w3.org/2004/02/skos/core#Concept</skos:scopeNote>
		<skos:Note>SKOS properties defined in http://www.w3.org/TR/skos-primer/#secrel</skos:Note>
		<skos:inScheme rdf:resource="http://cognitiveatlas.org/tasks/"/>
		<skos:definition>Subjects are stimulated with transcranial magnetic stimulation (TMS).</skos:definition>
		<skos:prefLabel>Transcranial Magnetic Stimulation</skos:prefLabel>
		<skos:altLabel></skos:altLabel>
</skos:Concept><skos:Concept rdf:about="http://cognitiveatlas.org/id/trm_4c8a84afdd863"> <dc:identifier>trm_4c8a84afdd863</dc:identifier>
		<dc:Title>Cognitive Atlas : Lexicon : Vibrotactile Monitor/Discrimination</dc:Title>
		<dc:Description>RDF output for 'Vibrotactile Monitor/Discrimination'</dc:Description>
		<dc:Type>InteractiveResource</dc:Type>
		<dc:Publisher>Cognitive Atlas</dc:Publisher>
		<dc:Creator>Cognitive Atlas RDF Generator</dc:Creator>
		<dc:Contributor>Brenda Gregory</dc:Contributor>
		<dc:Date>2011-04-26 14:16:12</dc:Date>
		<dc:Format>text/rdf</dc:Format>
		<dc:Language>en</dc:Language>
		<skos:editorialNote>Generated by testgen.php on Thu Jun 9 14:25:25 PDT 2011.</skos:editorialNote>
		<skos:historyNote>Revision 2: 1 previous definitions.</skos:historyNote>
		<skos:changeNote>See http://cognitiveatlas.org/id/trm_4c8a84afdd863 for complete revision history.</skos:changeNote>
		<skos:scopeNote>http://www.w3.org/2004/02/skos/core#Concept</skos:scopeNote>
		<skos:Note>SKOS properties defined in http://www.w3.org/TR/skos-primer/#secrel</skos:Note>
		<skos:inScheme rdf:resource="http://cognitiveatlas.org/tasks/"/>
		<skos:definition>Subjects experience vibrotactile stimulation to the hand, finger, arm, toe, or lip.</skos:definition>
		<skos:prefLabel>Vibrotactile Monitor/Discrimination</skos:prefLabel>
		<skos:altLabel></skos:altLabel>
</skos:Concept><skos:Concept rdf:about="http://cognitiveatlas.org/id/trm_4c8a84d4c4157"> <dc:identifier>trm_4c8a84d4c4157</dc:identifier>
		<dc:Title>Cognitive Atlas : Lexicon : Video Games</dc:Title>
		<dc:Description>RDF output for 'Video Games'</dc:Description>
		<dc:Type>InteractiveResource</dc:Type>
		<dc:Publisher>Cognitive Atlas</dc:Publisher>
		<dc:Creator>Cognitive Atlas RDF Generator</dc:Creator>
		<dc:Contributor>Brenda Gregory</dc:Contributor>
		<dc:Date>2011-04-26 14:15:53</dc:Date>
		<dc:Format>text/rdf</dc:Format>
		<dc:Language>en</dc:Language>
		<skos:editorialNote>Generated by testgen.php on Thu Jun 9 14:25:25 PDT 2011.</skos:editorialNote>
		<skos:historyNote>Revision 2: 1 previous definitions.</skos:historyNote>
		<skos:changeNote>See http://cognitiveatlas.org/id/trm_4c8a84d4c4157 for complete revision history.</skos:changeNote>
		<skos:scopeNote>http://www.w3.org/2004/02/skos/core#Concept</skos:scopeNote>
		<skos:Note>SKOS properties defined in http://www.w3.org/TR/skos-primer/#secrel</skos:Note>
		<skos:inScheme rdf:resource="http://cognitiveatlas.org/tasks/"/>
		<skos:definition>Subjects play video games.</skos:definition>
		<skos:prefLabel>Video Games</skos:prefLabel>
		<skos:altLabel></skos:altLabel>
</skos:Concept><skos:Concept rdf:about="http://cognitiveatlas.org/id/trm_4c8a84f20dde2"> <dc:identifier>trm_4c8a84f20dde2</dc:identifier>
		<dc:Title>Cognitive Atlas : Lexicon : Visual Distractor/Visual Attention</dc:Title>
		<dc:Description>RDF output for 'Visual Distractor/Visual Attention'</dc:Description>
		<dc:Type>InteractiveResource</dc:Type>
		<dc:Publisher>Cognitive Atlas</dc:Publisher>
		<dc:Creator>Cognitive Atlas RDF Generator</dc:Creator>
		<dc:Contributor>Brenda Gregory</dc:Contributor>
		<dc:Date>2011-04-26 14:14:54</dc:Date>
		<dc:Format>text/rdf</dc:Format>
		<dc:Language>en</dc:Language>
		<skos:editorialNote>Generated by testgen.php on Thu Jun 9 14:25:25 PDT 2011.</skos:editorialNote>
		<skos:historyNote>Revision 2: 1 previous definitions.</skos:historyNote>
		<skos:changeNote>See http://cognitiveatlas.org/id/trm_4c8a84f20dde2 for complete revision history.</skos:changeNote>
		<skos:scopeNote>http://www.w3.org/2004/02/skos/core#Concept</skos:scopeNote>
		<skos:Note>SKOS properties defined in http://www.w3.org/TR/skos-primer/#secrel</skos:Note>
		<skos:inScheme rdf:resource="http://cognitiveatlas.org/tasks/"/>
		<skos:definition>This category is a catch-all for visuoattention paradigms.  Examples include:  subjects press a button when a visual target (letters, bars, circles, asterisks, LEDs, etc) appears; subjects detect changes in luminance, shape, or color of visual stimuli; subjects fixate on a central stimuli while ignoring peripheral distractors.  Also includes cued, attention shift, and divided attention paradigms.</skos:definition>
		<skos:prefLabel>Visual Distractor/Visual Attention</skos:prefLabel>
		<skos:altLabel></skos:altLabel>
</skos:Concept><skos:Concept rdf:about="http://cognitiveatlas.org/id/trm_4c8a85534241d"> <dc:identifier>trm_4c8a85534241d</dc:identifier>
		<dc:Title>Cognitive Atlas : Lexicon : Visual Pursuit/Tracking</dc:Title>
		<dc:Description>RDF output for 'Visual Pursuit/Tracking'</dc:Description>
		<dc:Type>InteractiveResource</dc:Type>
		<dc:Publisher>Cognitive Atlas</dc:Publisher>
		<dc:Creator>Cognitive Atlas RDF Generator</dc:Creator>
		<dc:Contributor>Brenda Gregory</dc:Contributor>
		<dc:Date>2011-04-26 14:14:30</dc:Date>
		<dc:Format>text/rdf</dc:Format>
		<dc:Language>en</dc:Language>
		<skos:editorialNote>Generated by testgen.php on Thu Jun 9 14:25:25 PDT 2011.</skos:editorialNote>
		<skos:historyNote>Revision 2: 1 previous definitions.</skos:historyNote>
		<skos:changeNote>See http://cognitiveatlas.org/id/trm_4c8a85534241d for complete revision history.</skos:changeNote>
		<skos:scopeNote>http://www.w3.org/2004/02/skos/core#Concept</skos:scopeNote>
		<skos:Note>SKOS properties defined in http://www.w3.org/TR/skos-primer/#secrel</skos:Note>
		<skos:inScheme rdf:resource="http://cognitiveatlas.org/tasks/"/>
		<skos:definition>Subjects view a moving target(s) and track its movement across the screen.  Frequently, stimuli are moving dots.</skos:definition>
		<skos:prefLabel>Visual Pursuit/Tracking</skos:prefLabel>
		<skos:altLabel></skos:altLabel>
</skos:Concept><skos:Concept rdf:about="http://cognitiveatlas.org/id/trm_4c8a8575d1e55"> <dc:identifier>trm_4c8a8575d1e55</dc:identifier>
		<dc:Title>Cognitive Atlas : Lexicon : Whistling</dc:Title>
		<dc:Description>RDF output for 'Whistling'</dc:Description>
		<dc:Type>InteractiveResource</dc:Type>
		<dc:Publisher>Cognitive Atlas</dc:Publisher>
		<dc:Creator>Cognitive Atlas RDF Generator</dc:Creator>
		<dc:Contributor>Brenda Gregory</dc:Contributor>
		<dc:Date>2011-04-26 14:14:09</dc:Date>
		<dc:Format>text/rdf</dc:Format>
		<dc:Language>en</dc:Language>
		<skos:editorialNote>Generated by testgen.php on Thu Jun 9 14:25:25 PDT 2011.</skos:editorialNote>
		<skos:historyNote>Revision 2: 1 previous definitions.</skos:historyNote>
		<skos:changeNote>See http://cognitiveatlas.org/id/trm_4c8a8575d1e55 for complete revision history.</skos:changeNote>
		<skos:scopeNote>http://www.w3.org/2004/02/skos/core#Concept</skos:scopeNote>
		<skos:Note>SKOS properties defined in http://www.w3.org/TR/skos-primer/#secrel</skos:Note>
		<skos:inScheme rdf:resource="http://cognitiveatlas.org/tasks/"/>
		<skos:definition>Subjects whistle.</skos:definition>
		<skos:prefLabel>Whistling</skos:prefLabel>
		<skos:altLabel></skos:altLabel>
</skos:Concept><skos:Concept rdf:about="http://cognitiveatlas.org/id/trm_4c8a858da803d"> <dc:identifier>trm_4c8a858da803d</dc:identifier>
		<dc:Title>Cognitive Atlas : Lexicon : Word Stem Completion (Covert)</dc:Title>
		<dc:Description>RDF output for 'Word Stem Completion (Covert)'</dc:Description>
		<dc:Type>InteractiveResource</dc:Type>
		<dc:Publisher>Cognitive Atlas</dc:Publisher>
		<dc:Creator>Cognitive Atlas RDF Generator</dc:Creator>
		<dc:Contributor>Brenda Gregory</dc:Contributor>
		<dc:Date>2011-04-26 14:13:49</dc:Date>
		<dc:Format>text/rdf</dc:Format>
		<dc:Language>en</dc:Language>
		<skos:editorialNote>Generated by testgen.php on Thu Jun 9 14:25:25 PDT 2011.</skos:editorialNote>
		<skos:historyNote>Revision 2: 1 previous definitions.</skos:historyNote>
		<skos:changeNote>See http://cognitiveatlas.org/id/trm_4c8a858da803d for complete revision history.</skos:changeNote>
		<skos:scopeNote>http://www.w3.org/2004/02/skos/core#Concept</skos:scopeNote>
		<skos:Note>SKOS properties defined in http://www.w3.org/TR/skos-primer/#secrel</skos:Note>
		<skos:inScheme rdf:resource="http://cognitiveatlas.org/tasks/"/>
		<skos:definition>Subjects view word stems and silently generate a word that completes the stem.</skos:definition>
		<skos:prefLabel>Word Stem Completion (Covert)</skos:prefLabel>
		<skos:altLabel></skos:altLabel>
</skos:Concept><skos:Concept rdf:about="http://cognitiveatlas.org/id/trm_4c8a85a4564b2"> <dc:identifier>trm_4c8a85a4564b2</dc:identifier>
		<dc:Title>Cognitive Atlas : Lexicon : Word Stem Completion (Overt)</dc:Title>
		<dc:Description>RDF output for 'Word Stem Completion (Overt)'</dc:Description>
		<dc:Type>InteractiveResource</dc:Type>
		<dc:Publisher>Cognitive Atlas</dc:Publisher>
		<dc:Creator>Cognitive Atlas RDF Generator</dc:Creator>
		<dc:Contributor>Brenda Gregory</dc:Contributor>
		<dc:Date>2011-04-19 13:57:34</dc:Date>
		<dc:Format>text/rdf</dc:Format>
		<dc:Language>en</dc:Language>
		<skos:editorialNote>Generated by testgen.php on Thu Jun 9 14:25:25 PDT 2011.</skos:editorialNote>
		<skos:historyNote>Revision 2: 1 previous definitions.</skos:historyNote>
		<skos:changeNote>See http://cognitiveatlas.org/id/trm_4c8a85a4564b2 for complete revision history.</skos:changeNote>
		<skos:scopeNote>http://www.w3.org/2004/02/skos/core#Concept</skos:scopeNote>
		<skos:Note>SKOS properties defined in http://www.w3.org/TR/skos-primer/#secrel</skos:Note>
		<skos:inScheme rdf:resource="http://cognitiveatlas.org/tasks/"/>
		<skos:definition>Subjects view word stems and overtly generate a word that completes the stem.</skos:definition>
		<skos:prefLabel>Word Stem Completion (Overt)</skos:prefLabel>
		<skos:altLabel></skos:altLabel>
</skos:Concept><skos:Concept rdf:about="http://cognitiveatlas.org/id/trm_4c8a85c5c75eb"> <dc:identifier>trm_4c8a85c5c75eb</dc:identifier>
		<dc:Title>Cognitive Atlas : Lexicon : Writing Task</dc:Title>
		<dc:Description>RDF output for 'Writing Task'</dc:Description>
		<dc:Type>InteractiveResource</dc:Type>
		<dc:Publisher>Cognitive Atlas</dc:Publisher>
		<dc:Creator>Cognitive Atlas RDF Generator</dc:Creator>
		<dc:Contributor>Brenda Gregory</dc:Contributor>
		<dc:Date>2011-04-19 13:56:38</dc:Date>
		<dc:Format>text/rdf</dc:Format>
		<dc:Language>en</dc:Language>
		<skos:editorialNote>Generated by testgen.php on Thu Jun 9 14:25:25 PDT 2011.</skos:editorialNote>
		<skos:historyNote>Revision 2: 1 previous definitions.</skos:historyNote>
		<skos:changeNote>See http://cognitiveatlas.org/id/trm_4c8a85c5c75eb for complete revision history.</skos:changeNote>
		<skos:scopeNote>http://www.w3.org/2004/02/skos/core#Concept</skos:scopeNote>
		<skos:Note>SKOS properties defined in http://www.w3.org/TR/skos-primer/#secrel</skos:Note>
		<skos:inScheme rdf:resource="http://cognitiveatlas.org/tasks/"/>
		<skos:definition>Subjects write letters or words with a pen, stylus, or their finger.</skos:definition>
		<skos:prefLabel>Writing Task</skos:prefLabel>
		<skos:altLabel></skos:altLabel>
</skos:Concept><skos:Concept rdf:about="http://cognitiveatlas.org/id/trm_4cacee4a1d875"> <dc:identifier>trm_4cacee4a1d875</dc:identifier>
		<dc:Title>Cognitive Atlas : Lexicon : Mixed gambles task</dc:Title>
		<dc:Description>RDF output for 'Mixed gambles task'</dc:Description>
		<dc:Type>InteractiveResource</dc:Type>
		<dc:Publisher>Cognitive Atlas</dc:Publisher>
		<dc:Creator>Cognitive Atlas RDF Generator</dc:Creator>
		<dc:Contributor>Russ Poldrack</dc:Contributor>
		<dc:Date>2010-10-06 14:46:50</dc:Date>
		<dc:Format>text/rdf</dc:Format>
		<dc:Language>en</dc:Language>
		<skos:editorialNote>Generated by testgen.php on Thu Jun 9 14:25:25 PDT 2011.</skos:editorialNote>
		<skos:historyNote>No previous definition revisions.</skos:historyNote>
		<skos:changeNote>This is the first and only definition provided.</skos:changeNote>
		<skos:scopeNote>http://www.w3.org/2004/02/skos/core#Concept</skos:scopeNote>
		<skos:Note>SKOS properties defined in http://www.w3.org/TR/skos-primer/#secrel</skos:Note>
		<skos:inScheme rdf:resource="http://cognitiveatlas.org/tasks/"/>
		<skos:definition>Subjects are presented with gambles in which they have a 50% chance of gaining some amount of money and a 50% chance of losing some other amount of money.  The subject decides whether or not they would accept the gamble.  The amount of the potential gain and loss are varied across trials.  Gambles are not resolved during performance of the task; after the end of the task, some gambles are chosen at random and played for real money if they were accepted. </skos:definition>
		<skos:prefLabel>Mixed gambles task</skos:prefLabel>
		<skos:altLabel></skos:altLabel>
		<cito:citesForInformation rdf:resource="http://cognitiveatlas.org/citation/id/cit_4cacee5971d20"/>
</skos:Concept><skos:Concept rdf:about="http://cognitiveatlas.org/id/trm_4cacf22a22d80"> <dc:identifier>trm_4cacf22a22d80</dc:identifier>
		<dc:Title>Cognitive Atlas : Lexicon : Probabilistic classification task</dc:Title>
		<dc:Description>RDF output for 'Probabilistic classification task'</dc:Description>
		<dc:Type>InteractiveResource</dc:Type>
		<dc:Publisher>Cognitive Atlas</dc:Publisher>
		<dc:Creator>Cognitive Atlas RDF Generator</dc:Creator>
		<dc:Contributor>Russ Poldrack</dc:Contributor>
		<dc:Date>2010-10-06 15:03:22</dc:Date>
		<dc:Format>text/rdf</dc:Format>
		<dc:Language>en</dc:Language>
		<skos:editorialNote>Generated by testgen.php on Thu Jun 9 14:25:25 PDT 2011.</skos:editorialNote>
		<skos:historyNote>No previous definition revisions.</skos:historyNote>
		<skos:changeNote>This is the first and only definition provided.</skos:changeNote>
		<skos:scopeNote>http://www.w3.org/2004/02/skos/core#Concept</skos:scopeNote>
		<skos:Note>SKOS properties defined in http://www.w3.org/TR/skos-primer/#secrel</skos:Note>
		<skos:inScheme rdf:resource="http://cognitiveatlas.org/tasks/"/>
		<skos:definition>Subjects are presented with a set of stimuli and must classify those stimuli into one of two categories. In a common version known as the &#34;weather prediction task&#34; the stimuli are cards with geometric shapes on them and the outcomes are rainy versus sunny weather.  The feedback is probabilistic, and performance is measured by the proportion of statistically optimal responses.</skos:definition>
		<skos:prefLabel>Probabilistic classification task</skos:prefLabel>
		<skos:altLabel></skos:altLabel>
		<cito:citesForInformation rdf:resource="http://cognitiveatlas.org/citation/id/cit_4cacf245b81ba"/>
</skos:Concept><skos:Concept rdf:about="http://cognitiveatlas.org/id/trm_4cacf3fbc503b"> <dc:identifier>trm_4cacf3fbc503b</dc:identifier>
		<dc:Title>Cognitive Atlas : Lexicon : Conditional stop signal task</dc:Title>
		<dc:Description>RDF output for 'Conditional stop signal task'</dc:Description>
		<dc:Type>InteractiveResource</dc:Type>
		<dc:Publisher>Cognitive Atlas</dc:Publisher>
		<dc:Creator>Cognitive Atlas RDF Generator</dc:Creator>
		<dc:Contributor>Russ Poldrack</dc:Contributor>
		<dc:Date>2010-10-06 15:11:07</dc:Date>
		<dc:Format>text/rdf</dc:Format>
		<dc:Language>en</dc:Language>
		<skos:editorialNote>Generated by testgen.php on Thu Jun 9 14:25:25 PDT 2011.</skos:editorialNote>
		<skos:historyNote>No previous definition revisions.</skos:historyNote>
		<skos:changeNote>This is the first and only definition provided.</skos:changeNote>
		<skos:scopeNote>http://www.w3.org/2004/02/skos/core#Concept</skos:scopeNote>
		<skos:Note>SKOS properties defined in http://www.w3.org/TR/skos-primer/#secrel</skos:Note>
		<skos:inScheme rdf:resource="http://cognitiveatlas.org/tasks/"/>
		<skos:definition>A task in which an external stimulus signals the participant to interrupt an already-initiated motor response, but only for a subset of possible responses.  </skos:definition>
		<skos:prefLabel>Conditional stop signal task</skos:prefLabel>
		<skos:altLabel></skos:altLabel>
		<skos:related rdf:resource="http://cognitiveatlas.org/id/trm_4a3fd79d0a613"/>
		<skos:related rdf:resource="http://cognitiveatlas.org/id/trm_4a3fd79d0af66"/>
		<skos:example>inhibition is measured by the contrast of Stop-critical trial trials in the Conditional stop signal task</skos:example>
		<skos:example>response inhibition is measured by the contrast of Stop-critical trial trials in the Conditional stop signal task</skos:example>
		<cito:citesForInformation rdf:resource="http://cognitiveatlas.org/citation/id/cit_4cacf48576093"/>
		<cito:citesForInformation rdf:resource="http://cognitiveatlas.org/citation/id/cit_4de7becce685e"/>
		<cito:citesForInformation rdf:resource="http://cognitiveatlas.org/citation/id/cit_4cacf48576093"/>
		<cito:citesForInformation rdf:resource="http://cognitiveatlas.org/citation/id/cit_4de7bf28e2457"/>
</skos:Concept><skos:Concept rdf:about="http://cognitiveatlas.org/id/tsk_4a57abb94981d"> <dc:identifier>tsk_4a57abb94981d</dc:identifier>
		<dc:Title>Cognitive Atlas : Lexicon : Action imitation task</dc:Title>
		<dc:Description>RDF output for 'Action imitation task'</dc:Description>
		<dc:Type>InteractiveResource</dc:Type>
		<dc:Publisher>Cognitive Atlas</dc:Publisher>
		<dc:Creator>Cognitive Atlas RDF Generator</dc:Creator>
		<dc:Contributor>Antonia Hamilton</dc:Contributor>
		<dc:Date>2010-04-27 08:37:35</dc:Date>
		<dc:Format>text/rdf</dc:Format>
		<dc:Language>en</dc:Language>
		<skos:editorialNote>Generated by testgen.php on Thu Jun 9 14:25:25 PDT 2011.</skos:editorialNote>
		<skos:historyNote>Revision 2: 1 previous definitions.</skos:historyNote>
		<skos:changeNote>See http://cognitiveatlas.org/id/tsk_4a57abb94981d for complete revision history.</skos:changeNote>
		<skos:scopeNote>http://www.w3.org/2004/02/skos/core#Concept</skos:scopeNote>
		<skos:Note>SKOS properties defined in http://www.w3.org/TR/skos-primer/#secrel</skos:Note>
		<skos:inScheme rdf:resource="http://cognitiveatlas.org/tasks/"/>
		<skos:definition>A task in which a participant sees another person perform an action and later performs the same action him/herself.  Imitation can be immediate or delayed.  It can be instructed or elicited implicitly (without the participant&#39;s conscious awareness).  The actions imitated can be familar/meaningful actions or unfamilar/meaningless actions.</skos:definition>
		<skos:prefLabel>Action imitation task</skos:prefLabel>
		<skos:altLabel></skos:altLabel>
		<cito:citesForInformation rdf:resource="http://cognitiveatlas.org/citation/id/cit_4de538b33bb4f"/>
		<cito:citesForInformation rdf:resource="http://cognitiveatlas.org/citation/id/cit_4de539c965bec"/>
		<cito:citesForInformation rdf:resource="http://cognitiveatlas.org/citation/id/cit_4de539ea4f537"/>
</skos:Concept><skos:Concept rdf:about="http://cognitiveatlas.org/id/tsk_4a57abb949846"> <dc:identifier>tsk_4a57abb949846</dc:identifier>
		<dc:Title>Cognitive Atlas : Lexicon : Action observation task</dc:Title>
		<dc:Description>RDF output for 'Action observation task'</dc:Description>
		<dc:Type>InteractiveResource</dc:Type>
		<dc:Publisher>Cognitive Atlas</dc:Publisher>
		<dc:Creator>Cognitive Atlas RDF Generator</dc:Creator>
		<dc:Contributor>Carinna Torgerson</dc:Contributor>
		<dc:Date>2011-05-31 15:54:08</dc:Date>
		<dc:Format>text/rdf</dc:Format>
		<dc:Language>en</dc:Language>
		<skos:editorialNote>Generated by testgen.php on Thu Jun 9 14:25:25 PDT 2011.</skos:editorialNote>
		<skos:historyNote>Revision 4: 3 previous definitions.</skos:historyNote>
		<skos:changeNote>See http://cognitiveatlas.org/id/tsk_4a57abb949846 for complete revision history.</skos:changeNote>
		<skos:scopeNote>http://www.w3.org/2004/02/skos/core#Concept</skos:scopeNote>
		<skos:Note>SKOS properties defined in http://www.w3.org/TR/skos-primer/#secrel</skos:Note>
		<skos:inScheme rdf:resource="http://cognitiveatlas.org/tasks/"/>
		<skos:definition>Subjects view images of actions in order to learn the action themselves. </skos:definition>
		<skos:prefLabel>Action observation task</skos:prefLabel>
		<skos:altLabel></skos:altLabel>
		<cito:citesForInformation rdf:resource="http://cognitiveatlas.org/citation/id/cit_4de54d5ebe6b8"/>
		<cito:citesForInformation rdf:resource="http://cognitiveatlas.org/citation/id/cit_4de54f7dc7893"/>
		<cito:citesForInformation rdf:resource="http://cognitiveatlas.org/citation/id/cit_4de550d699f55"/>
</skos:Concept><skos:Concept rdf:about="http://cognitiveatlas.org/id/tsk_4a57abb949858"> <dc:identifier>tsk_4a57abb949858</dc:identifier>
		<dc:Title>Cognitive Atlas : Lexicon : Adult Attachment Interview</dc:Title>
		<dc:Description>RDF output for 'Adult Attachment Interview'</dc:Description>
		<dc:Type>InteractiveResource</dc:Type>
		<dc:Publisher>Cognitive Atlas</dc:Publisher>
		<dc:Creator>Cognitive Atlas RDF Generator</dc:Creator>
		<dc:Contributor>Brenda Gregory</dc:Contributor>
		<dc:Date>2011-04-29 15:55:14</dc:Date>
		<dc:Format>text/rdf</dc:Format>
		<dc:Language>en</dc:Language>
		<skos:editorialNote>Generated by testgen.php on Thu Jun 9 14:25:25 PDT 2011.</skos:editorialNote>
		<skos:historyNote>Revision 3: 2 previous definitions.</skos:historyNote>
		<skos:changeNote>See http://cognitiveatlas.org/id/tsk_4a57abb949858 for complete revision history.</skos:changeNote>
		<skos:scopeNote>http://www.w3.org/2004/02/skos/core#Concept</skos:scopeNote>
		<skos:Note>SKOS properties defined in http://www.w3.org/TR/skos-primer/#secrel</skos:Note>
		<skos:inScheme rdf:resource="http://cognitiveatlas.org/tasks/"/>
		<skos:definition>a procedure for assessing adults&#39; strategies for identifying, preventing, and protecting the self from perceived dangers, particularly dangers tied to intimate relationships.</skos:definition>
		<skos:prefLabel>Adult Attachment Interview</skos:prefLabel>
		<skos:altLabel></skos:altLabel>
		<cito:citesForInformation rdf:resource="http://cognitiveatlas.org/citation/id/cit_4de556688b4f4"/>
		<cito:citesForInformation rdf:resource="http://cognitiveatlas.org/citation/id/cit_4de55832c02cd"/>
		<cito:citesForInformation rdf:resource="http://cognitiveatlas.org/citation/id/cit_4de558973ecc8"/>
</skos:Concept><skos:Concept rdf:about="http://cognitiveatlas.org/id/tsk_4a57abb949869"> <dc:identifier>tsk_4a57abb949869</dc:identifier>
		<dc:Title>Cognitive Atlas : Lexicon : Antisaccade/prosaccade task</dc:Title>
		<dc:Description>RDF output for 'Antisaccade/prosaccade task'</dc:Description>
		<dc:Type>InteractiveResource</dc:Type>
		<dc:Publisher>Cognitive Atlas</dc:Publisher>
		<dc:Creator>Cognitive Atlas RDF Generator</dc:Creator>
		<dc:Contributor>Brenda Gregory</dc:Contributor>
		<dc:Date>2011-04-19 13:56:17</dc:Date>
		<dc:Format>text/rdf</dc:Format>
		<dc:Language>en</dc:Language>
		<skos:editorialNote>Generated by testgen.php on Thu Jun 9 14:25:25 PDT 2011.</skos:editorialNote>
		<skos:historyNote>Revision 3: 2 previous definitions.</skos:historyNote>
		<skos:changeNote>See http://cognitiveatlas.org/id/tsk_4a57abb949869 for complete revision history.</skos:changeNote>
		<skos:scopeNote>http://www.w3.org/2004/02/skos/core#Concept</skos:scopeNote>
		<skos:Note>SKOS properties defined in http://www.w3.org/TR/skos-primer/#secrel</skos:Note>
		<skos:inScheme rdf:resource="http://cognitiveatlas.org/tasks/"/>
		<skos:definition>Subjects view a target and are instructed to make a saccade away from the target (to the opposite visual field)/Subjects view a target and are instructed to make a saccade to its location.</skos:definition>
		<skos:prefLabel>Antisaccade/prosaccade task</skos:prefLabel>
		<skos:altLabel></skos:altLabel>
		<cito:citesForInformation rdf:resource="http://cognitiveatlas.org/citation/id/cit_4de55a73e5d36"/>
		<cito:citesForInformation rdf:resource="http://cognitiveatlas.org/citation/id/cit_4de55c07b5a3b"/>
</skos:Concept><skos:Concept rdf:about="http://cognitiveatlas.org/id/tsk_4a57abb949879"> <dc:identifier>tsk_4a57abb949879</dc:identifier>
		<dc:Title>Cognitive Atlas : Lexicon : attentional blink task</dc:Title>
		<dc:Description>RDF output for 'attentional blink task'</dc:Description>
		<dc:Type>InteractiveResource</dc:Type>
		<dc:Publisher>Cognitive Atlas</dc:Publisher>
		<dc:Creator>Cognitive Atlas RDF Generator</dc:Creator>
		<dc:Contributor>Carinna Torgerson</dc:Contributor>
		<dc:Date>2011-05-31 14:27:57</dc:Date>
		<dc:Format>text/rdf</dc:Format>
		<dc:Language>en</dc:Language>
		<skos:editorialNote>Generated by testgen.php on Thu Jun 9 14:25:25 PDT 2011.</skos:editorialNote>
		<skos:historyNote>Revision 2: 1 previous definitions.</skos:historyNote>
		<skos:changeNote>See http://cognitiveatlas.org/id/tsk_4a57abb949879 for complete revision history.</skos:changeNote>
		<skos:scopeNote>http://www.w3.org/2004/02/skos/core#Concept</skos:scopeNote>
		<skos:Note>SKOS properties defined in http://www.w3.org/TR/skos-primer/#secrel</skos:Note>
		<skos:inScheme rdf:resource="http://cognitiveatlas.org/tasks/"/>
		<skos:definition>attentional processing of a first stimulus interferes with and/or delays the allocation of attention to a second stimulus if the second is presented before the processing of the first has been completed.</skos:definition>
		<skos:prefLabel>attentional blink task</skos:prefLabel>
		<skos:altLabel></skos:altLabel>
		<skos:related rdf:resource="http://cognitiveatlas.org/id/trm_4a3fd79d0a61f"/>
		<skos:example>inhibition of return is measured by the contrast of magnitude of response to second stimulus trials in the attentional blink task</skos:example>
		<cito:citesForInformation rdf:resource="http://cognitiveatlas.org/citation/id/cit_4de55d7a4b8b5"/>
		<cito:citesForInformation rdf:resource="http://cognitiveatlas.org/citation/id/cit_4de560080b812"/>
		<cito:citesForInformation rdf:resource="http://cognitiveatlas.org/citation/id/cit_4de560e975f67"/>
</skos:Concept><skos:Concept rdf:about="http://cognitiveatlas.org/id/tsk_4a57abb949889"> <dc:identifier>tsk_4a57abb949889</dc:identifier>
		<dc:Title>Cognitive Atlas : Lexicon : audio-visual target-detection task</dc:Title>
		<dc:Description>RDF output for 'audio-visual target-detection task'</dc:Description>
		<dc:Type>InteractiveResource</dc:Type>
		<dc:Publisher>Cognitive Atlas</dc:Publisher>
		<dc:Creator>Cognitive Atlas RDF Generator</dc:Creator>
		<dc:Contributor>System Administrator</dc:Contributor>
		<dc:Date>2009-07-10 14:06:33</dc:Date>
		<dc:Format>text/rdf</dc:Format>
		<dc:Language>en</dc:Language>
		<skos:editorialNote>Generated by testgen.php on Thu Jun 9 14:25:25 PDT 2011.</skos:editorialNote>
		<skos:historyNote>No previous definition revisions.</skos:historyNote>
		<skos:changeNote>This is the first and only definition provided.</skos:changeNote>
		<skos:scopeNote>http://www.w3.org/2004/02/skos/core#Concept</skos:scopeNote>
		<skos:Note>SKOS properties defined in http://www.w3.org/TR/skos-primer/#secrel</skos:Note>
		<skos:inScheme rdf:resource="http://cognitiveatlas.org/tasks/"/>
		<skos:definition>No definition submitted yet</skos:definition>
		<skos:prefLabel>audio-visual target-detection task</skos:prefLabel>
		<skos:altLabel></skos:altLabel>
</skos:Concept><skos:Concept rdf:about="http://cognitiveatlas.org/id/tsk_4a57abb94989b"> <dc:identifier>tsk_4a57abb94989b</dc:identifier>
		<dc:Title>Cognitive Atlas : Lexicon : Backward digit span task</dc:Title>
		<dc:Description>RDF output for 'Backward digit span task'</dc:Description>
		<dc:Type>InteractiveResource</dc:Type>
		<dc:Publisher>Cognitive Atlas</dc:Publisher>
		<dc:Creator>Cognitive Atlas RDF Generator</dc:Creator>
		<dc:Contributor>Brenda Gregory</dc:Contributor>
		<dc:Date>2011-05-16 13:18:25</dc:Date>
		<dc:Format>text/rdf</dc:Format>
		<dc:Language>en</dc:Language>
		<skos:editorialNote>Generated by testgen.php on Thu Jun 9 14:25:25 PDT 2011.</skos:editorialNote>
		<skos:historyNote>Revision 3: 2 previous definitions.</skos:historyNote>
		<skos:changeNote>See http://cognitiveatlas.org/id/tsk_4a57abb94989b for complete revision history.</skos:changeNote>
		<skos:scopeNote>http://www.w3.org/2004/02/skos/core#Concept</skos:scopeNote>
		<skos:Note>SKOS properties defined in http://www.w3.org/TR/skos-primer/#secrel</skos:Note>
		<skos:inScheme rdf:resource="http://cognitiveatlas.org/tasks/"/>
		<skos:definition>a test used to measure working memory, attention, concentration, and mental control.  In a typical test of memory span, a list of random numbers or letters is read out loud or presented on a computer screen at the rate of one per second. The test begins with two to three numbers, increasing until the person commits errors. At the end of a sequence, the person being tested is asked to recall the items in reverse of the presented order.</skos:definition>
		<skos:prefLabel>Backward digit span task</skos:prefLabel>
		<skos:altLabel></skos:altLabel>
		<skos:related rdf:resource="http://cognitiveatlas.org/id/tsk_4a57abb949f12"/>
		<skos:related rdf:resource="http://cognitiveatlas.org/id/tsk_4a57abb949a0d"/>
		<skos:related rdf:resource="http://cognitiveatlas.org/id/tsk_4a57abb949a85"/>
		<skos:example>Backward digit span task is related to Wechsler Adult Intelligence Scale - Revised</skos:example>
		<skos:example>Backward digit span task is descended from Digit span task</skos:example>
		<skos:example>Backward digit span task is an exact synonym of Forward digit span task</skos:example>
		<cito:citesForInformation rdf:resource="http://cognitiveatlas.org/citation/id/cit_4de575709967d"/>
</skos:Concept><skos:Concept rdf:about="http://cognitiveatlas.org/id/tsk_4a57abb9498ab"> <dc:identifier>tsk_4a57abb9498ab</dc:identifier>
		<dc:Title>Cognitive Atlas : Lexicon : Behavioral Rating Inventory of Executive Function</dc:Title>
		<dc:Description>RDF output for 'Behavioral Rating Inventory of Executive Function'</dc:Description>
		<dc:Type>InteractiveResource</dc:Type>
		<dc:Publisher>Cognitive Atlas</dc:Publisher>
		<dc:Creator>Cognitive Atlas RDF Generator</dc:Creator>
		<dc:Contributor>Brenda Gregory</dc:Contributor>
		<dc:Date>2011-04-28 17:22:32</dc:Date>
		<dc:Format>text/rdf</dc:Format>
		<dc:Language>en</dc:Language>
		<skos:editorialNote>Generated by testgen.php on Thu Jun 9 14:25:25 PDT 2011.</skos:editorialNote>
		<skos:historyNote>Revision 5: 4 previous definitions.</skos:historyNote>
		<skos:changeNote>See http://cognitiveatlas.org/id/tsk_4a57abb9498ab for complete revision history.</skos:changeNote>
		<skos:scopeNote>http://www.w3.org/2004/02/skos/core#Concept</skos:scopeNote>
		<skos:Note>SKOS properties defined in http://www.w3.org/TR/skos-primer/#secrel</skos:Note>
		<skos:inScheme rdf:resource="http://cognitiveatlas.org/tasks/"/>
		<skos:definition>used for evaluating and planning treatment strategies for a wide spectrum of developmental and acquired neurological conditions, including learning disabilities, low birth weight, ADHD, Tourette&#39;s disorder, Traumatic Brain Injury, and Autism; consists of 8 non-overlapping clinical scales that form two broader indexes: Behavior Regulation (three scales) and Metacognition (five scales). A Global Executive Composite score is also produced; completed by parents and teachers, is suitable for children as young as 5 years old.</skos:definition>
		<skos:prefLabel>Behavioral Rating Inventory of Executive Function</skos:prefLabel>
		<skos:altLabel></skos:altLabel>
		<skos:related rdf:resource="http://cognitiveatlas.org/id/trm_4a3fd79d0a252"/>
		<skos:related rdf:resource="http://cognitiveatlas.org/id/trm_4a3fd79d0a252"/>
		<skos:example>executive function is measured by the contrast of Negativity Scale trials in the Behavioral Rating Inventory of Executive Function</skos:example>
		<skos:example>executive function is measured by the contrast of Inconsistency Scale trials in the Behavioral Rating Inventory of Executive Function</skos:example>
		<cito:citesForInformation rdf:resource="http://cognitiveatlas.org/citation/id/cit_4de57dbb23ab8"/>
		<cito:citesForInformation rdf:resource="http://cognitiveatlas.org/citation/id/cit_4de5816f70873"/>
		<cito:citesForInformation rdf:resource="http://cognitiveatlas.org/citation/id/cit_4de581a4dcac0"/>
</skos:Concept><skos:Concept rdf:about="http://cognitiveatlas.org/id/tsk_4a57abb9498bc"> <dc:identifier>tsk_4a57abb9498bc</dc:identifier>
		<dc:Title>Cognitive Atlas : Lexicon : Benton Facial Recognition Test</dc:Title>
		<dc:Description>RDF output for 'Benton Facial Recognition Test'</dc:Description>
		<dc:Type>InteractiveResource</dc:Type>
		<dc:Publisher>Cognitive Atlas</dc:Publisher>
		<dc:Creator>Cognitive Atlas RDF Generator</dc:Creator>
		<dc:Contributor>Brenda Gregory</dc:Contributor>
		<dc:Date>2010-04-29 08:07:35</dc:Date>
		<dc:Format>text/rdf</dc:Format>
		<dc:Language>en</dc:Language>
		<skos:editorialNote>Generated by testgen.php on Thu Jun 9 14:25:25 PDT 2011.</skos:editorialNote>
		<skos:historyNote>Revision 2: 1 previous definitions.</skos:historyNote>
		<skos:changeNote>See http://cognitiveatlas.org/id/tsk_4a57abb9498bc for complete revision history.</skos:changeNote>
		<skos:scopeNote>http://www.w3.org/2004/02/skos/core#Concept</skos:scopeNote>
		<skos:Note>SKOS properties defined in http://www.w3.org/TR/skos-primer/#secrel</skos:Note>
		<skos:inScheme rdf:resource="http://cognitiveatlas.org/tasks/"/>
		<skos:definition>A tool used to assess deficits in facial recognition.</skos:definition>
		<skos:prefLabel>Benton Facial Recognition Test</skos:prefLabel>
		<skos:altLabel></skos:altLabel>
		<cito:citesForInformation rdf:resource="http://cognitiveatlas.org/citation/id/cit_4de5835057136"/>
		<cito:citesForInformation rdf:resource="http://cognitiveatlas.org/citation/id/cit_4de5851834e44"/>
</skos:Concept><skos:Concept rdf:about="http://cognitiveatlas.org/id/tsk_4a57abb9498ce"> <dc:identifier>tsk_4a57abb9498ce</dc:identifier>
		<dc:Title>Cognitive Atlas : Lexicon : Birmingham Object Recognition Battery</dc:Title>
		<dc:Description>RDF output for 'Birmingham Object Recognition Battery'</dc:Description>
		<dc:Type>InteractiveResource</dc:Type>
		<dc:Publisher>Cognitive Atlas</dc:Publisher>
		<dc:Creator>Cognitive Atlas RDF Generator</dc:Creator>
		<dc:Contributor>Brenda Gregory</dc:Contributor>
		<dc:Date>2011-04-19 13:54:34</dc:Date>
		<dc:Format>text/rdf</dc:Format>
		<dc:Language>en</dc:Language>
		<skos:editorialNote>Generated by testgen.php on Thu Jun 9 14:25:25 PDT 2011.</skos:editorialNote>
		<skos:historyNote>Revision 3: 2 previous definitions.</skos:historyNote>
		<skos:changeNote>See http://cognitiveatlas.org/id/tsk_4a57abb9498ce for complete revision history.</skos:changeNote>
		<skos:scopeNote>http://www.w3.org/2004/02/skos/core#Concept</skos:scopeNote>
		<skos:Note>SKOS properties defined in http://www.w3.org/TR/skos-primer/#secrel</skos:Note>
		<skos:inScheme rdf:resource="http://cognitiveatlas.org/tasks/"/>
		<skos:definition>a set of standardized procedures for assessing neuropsychological disorders of visual object recognition which includes tests to assess low-level aspects of visual perception (using same-different matching of basic perceptual features, such as orientation, length, position and object size), intermediate visual processes (e.g., matching objects different in viewpoint), access to stored perceptual knowledge about objects (object decision), access to semantic knowledge (function and associative matches) and access to names from object (picture naming).</skos:definition>
		<skos:prefLabel>Birmingham Object Recognition Battery</skos:prefLabel>
		<skos:altLabel></skos:altLabel>
		<skos:related rdf:resource="http://cognitiveatlas.org/id/trm_4a3fd79d0a533"/>
		<skos:related rdf:resource="http://cognitiveatlas.org/id/trm_4a3fd79d0b4b5"/>
		<skos:related rdf:resource="http://cognitiveatlas.org/id/trm_4a3fd79d0b4b5"/>
		<skos:related rdf:resource="http://cognitiveatlas.org/id/trm_4a3fd79d0b4a9"/>
		<skos:related rdf:resource="http://cognitiveatlas.org/id/trm_4a3fd79d0a398"/>
		<skos:related rdf:resource="http://cognitiveatlas.org/id/trm_4a3fd79d0a398"/>
		<skos:related rdf:resource="http://cognitiveatlas.org/id/trm_4a3fd79d0a398"/>
		<skos:related rdf:resource="http://cognitiveatlas.org/id/trm_4a3fd79d0a398"/>
		<skos:related rdf:resource="http://cognitiveatlas.org/id/trm_4a3fd79d0a398"/>
		<skos:related rdf:resource="http://cognitiveatlas.org/id/trm_4a3fd79d0a398"/>
		<skos:related rdf:resource="http://cognitiveatlas.org/id/trm_4a3fd79d0a398"/>
		<skos:example>implicit memory is measured by the contrast of object decision trials in the Birmingham Object Recognition Battery</skos:example>
		<skos:example>visual perception is measured by the contrast of copying test trials in the Birmingham Object Recognition Battery</skos:example>
		<skos:example>visual perception is measured by the contrast of overlapping figures test trials in the Birmingham Object Recognition Battery</skos:example>
		<skos:example>visual object recognition is measured by the contrast of picture naming trials in the Birmingham Object Recognition Battery</skos:example>
		<skos:example>form perception is measured by the contrast of size match trials in the Birmingham Object Recognition Battery</skos:example>
		<skos:example>form perception is measured by the contrast of length match trials in the Birmingham Object Recognition Battery</skos:example>
		<skos:example>form perception is measured by the contrast of orientation match trials in the Birmingham Object Recognition Battery</skos:example>
		<skos:example>form perception is measured by the contrast of position gap match trials in the Birmingham Object Recognition Battery</skos:example>
		<skos:example>form perception is measured by the contrast of overlapping figures test trials in the Birmingham Object Recognition Battery</skos:example>
		<skos:example>form perception is measured by the contrast of minimal feature match trials in the Birmingham Object Recognition Battery</skos:example>
		<skos:example>form perception is measured by the contrast of foreshortened match trials in the Birmingham Object Recognition Battery</skos:example>
		<cito:citesForInformation rdf:resource="http://cognitiveatlas.org/citation/id/cit_4de672a871c2b"/>
		<cito:citesForInformation rdf:resource="http://cognitiveatlas.org/citation/id/cit_4de67a6a537ec"/>
</skos:Concept><skos:Concept rdf:about="http://cognitiveatlas.org/id/tsk_4a57abb9498df"> <dc:identifier>tsk_4a57abb9498df</dc:identifier>
		<dc:Title>Cognitive Atlas : Lexicon : Block Tapping Test</dc:Title>
		<dc:Description>RDF output for 'Block Tapping Test'</dc:Description>
		<dc:Type>InteractiveResource</dc:Type>
		<dc:Publisher>Cognitive Atlas</dc:Publisher>
		<dc:Creator>Cognitive Atlas RDF Generator</dc:Creator>
		<dc:Contributor>Carinna Torgerson</dc:Contributor>
		<dc:Date>2011-06-01 11:43:29</dc:Date>
		<dc:Format>text/rdf</dc:Format>
		<dc:Language>en</dc:Language>
		<skos:editorialNote>Generated by testgen.php on Thu Jun 9 14:25:25 PDT 2011.</skos:editorialNote>
		<skos:historyNote>Revision 5: 4 previous definitions.</skos:historyNote>
		<skos:changeNote>See http://cognitiveatlas.org/id/tsk_4a57abb9498df for complete revision history.</skos:changeNote>
		<skos:scopeNote>http://www.w3.org/2004/02/skos/core#Concept</skos:scopeNote>
		<skos:Note>SKOS properties defined in http://www.w3.org/TR/skos-primer/#secrel</skos:Note>
		<skos:inScheme rdf:resource="http://cognitiveatlas.org/tasks/"/>
		<skos:definition>tool used for assessment of visual short-term memory and implicit visual-spatial learning. An examiner taps a series of blocks and the subject must repeat in the correct sequential order. If the sequence is correct, the examiner adds another tap to the next sequence.</skos:definition>
		<skos:prefLabel>Block Tapping Test</skos:prefLabel>
		<skos:altLabel></skos:altLabel>
		<skos:related rdf:resource="http://cognitiveatlas.org/id/trm_4a3fd79d0b4d8"/>
		<skos:related rdf:resource="http://cognitiveatlas.org/id/trm_4da881dace79c"/>
		<skos:example>Block Tapping Test is descended from Corsi Blocks</skos:example>
		<skos:example>visual working memory is measured by the contrast of percent correct (number of correct sequences/number of total sequences) trials in the Block Tapping Test</skos:example>
		<cito:citesForInformation rdf:resource="http://cognitiveatlas.org/citation/id/cit_4de68558af17d"/>
		<cito:citesForInformation rdf:resource="http://cognitiveatlas.org/citation/id/cit_4de688a847c71"/>
		<cito:citesForInformation rdf:resource="http://cognitiveatlas.org/citation/id/cit_4de688f69b2cc"/>
</skos:Concept><skos:Concept rdf:about="http://cognitiveatlas.org/id/tsk_4a57abb9498ef"> <dc:identifier>tsk_4a57abb9498ef</dc:identifier>
		<dc:Title>Cognitive Atlas : Lexicon : Boston Naming Test</dc:Title>
		<dc:Description>RDF output for 'Boston Naming Test'</dc:Description>
		<dc:Type>InteractiveResource</dc:Type>
		<dc:Publisher>Cognitive Atlas</dc:Publisher>
		<dc:Creator>Cognitive Atlas RDF Generator</dc:Creator>
		<dc:Contributor>Brenda Gregory</dc:Contributor>
		<dc:Date>2011-04-28 12:19:45</dc:Date>
		<dc:Format>text/rdf</dc:Format>
		<dc:Language>en</dc:Language>
		<skos:editorialNote>Generated by testgen.php on Thu Jun 9 14:25:25 PDT 2011.</skos:editorialNote>
		<skos:historyNote>Revision 3: 2 previous definitions.</skos:historyNote>
		<skos:changeNote>See http://cognitiveatlas.org/id/tsk_4a57abb9498ef for complete revision history.</skos:changeNote>
		<skos:scopeNote>http://www.w3.org/2004/02/skos/core#Concept</skos:scopeNote>
		<skos:Note>SKOS properties defined in http://www.w3.org/TR/skos-primer/#secrel</skos:Note>
		<skos:inScheme rdf:resource="http://cognitiveatlas.org/tasks/"/>
		<skos:definition>assesses the ability to name pictures of objects through spontaneous responses and need for various types of cueing, inferences can be drawn regarding language facility and possible localization of cerebral damage.</skos:definition>
		<skos:prefLabel>Boston Naming Test</skos:prefLabel>
		<skos:altLabel></skos:altLabel>
		<skos:related rdf:resource="http://cognitiveatlas.org/id/trm_4a3fd79d0a7e0"/>
		<skos:related rdf:resource="http://cognitiveatlas.org/id/trm_4a3fd79d0b80f"/>
		<skos:example>lexical retrieval is measured by the contrast of percent correct (number of correct responses/number of total pictures) trials in the Boston Naming Test</skos:example>
		<skos:example>lexical access is measured by the contrast of percent correct (number of correct responses/number of total pictures) trials in the Boston Naming Test</skos:example>
		<cito:citesForInformation rdf:resource="http://cognitiveatlas.org/citation/id/cit_4de68d6f15aa1"/>
		<cito:citesForInformation rdf:resource="http://cognitiveatlas.org/citation/id/cit_4de68dd700a49"/>
		<cito:citesForInformation rdf:resource="http://cognitiveatlas.org/citation/id/cit_4de68e47e2dd6"/>
</skos:Concept><skos:Concept rdf:about="http://cognitiveatlas.org/id/tsk_4a57abb949900"> <dc:identifier>tsk_4a57abb949900</dc:identifier>
		<dc:Title>Cognitive Atlas : Lexicon : California Verbal Learning Test-II</dc:Title>
		<dc:Description>RDF output for 'California Verbal Learning Test-II'</dc:Description>
		<dc:Type>InteractiveResource</dc:Type>
		<dc:Publisher>Cognitive Atlas</dc:Publisher>
		<dc:Creator>Cognitive Atlas RDF Generator</dc:Creator>
		<dc:Contributor>Brenda Gregory</dc:Contributor>
		<dc:Date>2011-05-18 14:05:42</dc:Date>
		<dc:Format>text/rdf</dc:Format>
		<dc:Language>en</dc:Language>
		<skos:editorialNote>Generated by testgen.php on Thu Jun 9 14:25:25 PDT 2011.</skos:editorialNote>
		<skos:historyNote>Revision 3: 2 previous definitions.</skos:historyNote>
		<skos:changeNote>See http://cognitiveatlas.org/id/tsk_4a57abb949900 for complete revision history.</skos:changeNote>
		<skos:scopeNote>http://www.w3.org/2004/02/skos/core#Concept</skos:scopeNote>
		<skos:Note>SKOS properties defined in http://www.w3.org/TR/skos-primer/#secrel</skos:Note>
		<skos:inScheme rdf:resource="http://cognitiveatlas.org/tasks/"/>
		<skos:definition>A comprehensive and detailed assessment of verbal learning and memory available for older adolescents and adults. In addition to recall and recognition scores, it measures encoding strategies, learning rates, error types, and other process data.</skos:definition>
		<skos:prefLabel>California Verbal Learning Test-II</skos:prefLabel>
		<skos:altLabel></skos:altLabel>
		<skos:related rdf:resource="http://cognitiveatlas.org/id/trm_4a3fd79d09cae"/>
		<skos:related rdf:resource="http://cognitiveatlas.org/id/trm_4a3fd79d09cae"/>
		<skos:related rdf:resource="http://cognitiveatlas.org/id/trm_4a3fd79d0ba01"/>
		<skos:related rdf:resource="http://cognitiveatlas.org/id/trm_4a3fd79d0ba01"/>
		<skos:related rdf:resource="http://cognitiveatlas.org/id/trm_4a3fd79d0ba01"/>
		<skos:related rdf:resource="http://cognitiveatlas.org/id/trm_4a3fd79d0ba01"/>
		<skos:related rdf:resource="http://cognitiveatlas.org/id/trm_4a3fd79d0afab"/>
		<skos:related rdf:resource="http://cognitiveatlas.org/id/trm_4a3fd79d0ba6c"/>
		<skos:example>chunking is measured by the contrast of immediate recall trials in the California Verbal Learning Test-II</skos:example>
		<skos:example>chunking is measured by the contrast of long recall trials in the California Verbal Learning Test-II</skos:example>
		<skos:example>memory retrieval is measured by the contrast of immediate recall trials in the California Verbal Learning Test-II</skos:example>
		<skos:example>memory retrieval is measured by the contrast of interference trials in the California Verbal Learning Test-II</skos:example>
		<skos:example>memory retrieval is measured by the contrast of long recall trials in the California Verbal Learning Test-II</skos:example>
		<skos:example>memory retrieval is measured by the contrast of recognition trial trials in the California Verbal Learning Test-II</skos:example>
		<skos:example>retroactive interference is measured by the contrast of interference trials in the California Verbal Learning Test-II</skos:example>
		<skos:example>working memory retrieval is measured by the contrast of immediate recall trials in the California Verbal Learning Test-II</skos:example>
		<cito:citesForInformation rdf:resource="http://cognitiveatlas.org/citation/id/cit_4de69e5b88fc9"/>
		<cito:citesForInformation rdf:resource="http://cognitiveatlas.org/citation/id/cit_4de69f3e615d3"/>
</skos:Concept><skos:Concept rdf:about="http://cognitiveatlas.org/id/tsk_4a57abb949912"> <dc:identifier>tsk_4a57abb949912</dc:identifier>
		<dc:Title>Cognitive Atlas : Lexicon : Cambridge Face Memory Test</dc:Title>
		<dc:Description>RDF output for 'Cambridge Face Memory Test'</dc:Description>
		<dc:Type>InteractiveResource</dc:Type>
		<dc:Publisher>Cognitive Atlas</dc:Publisher>
		<dc:Creator>Cognitive Atlas RDF Generator</dc:Creator>
		<dc:Contributor>Carinna Torgerson</dc:Contributor>
		<dc:Date>2011-06-01 14:13:24</dc:Date>
		<dc:Format>text/rdf</dc:Format>
		<dc:Language>en</dc:Language>
		<skos:editorialNote>Generated by testgen.php on Thu Jun 9 14:25:25 PDT 2011.</skos:editorialNote>
		<skos:historyNote>Revision 2: 1 previous definitions.</skos:historyNote>
		<skos:changeNote>See http://cognitiveatlas.org/id/tsk_4a57abb949912 for complete revision history.</skos:changeNote>
		<skos:scopeNote>http://www.w3.org/2004/02/skos/core#Concept</skos:scopeNote>
		<skos:Note>SKOS properties defined in http://www.w3.org/TR/skos-primer/#secrel</skos:Note>
		<skos:inScheme rdf:resource="http://cognitiveatlas.org/tasks/"/>
		<skos:definition>a test with high reliability and validity that assesses the ability to learn and then recognize six new faces.</skos:definition>
		<skos:prefLabel>Cambridge Face Memory Test</skos:prefLabel>
		<skos:altLabel></skos:altLabel>
		<skos:related rdf:resource="http://cognitiveatlas.org/id/trm_4a3fd79d0a30c"/>
		<skos:related rdf:resource="http://cognitiveatlas.org/id/trm_4a3fd79d0a30c"/>
		<skos:related rdf:resource="http://cognitiveatlas.org/id/trm_4a3fd79d0a30c"/>
		<skos:example>face recognition is measured by the contrast of same images trials in the Cambridge Face Memory Test</skos:example>
		<skos:example>face recognition is measured by the contrast of novel images trials in the Cambridge Face Memory Test</skos:example>
		<skos:example>face recognition is measured by the contrast of novel images with noise trials in the Cambridge Face Memory Test</skos:example>
		<cito:citesForInformation rdf:resource="http://cognitiveatlas.org/citation/id/cit_4de6ae747d7df"/>
		<cito:citesForInformation rdf:resource="http://cognitiveatlas.org/citation/id/cit_4de6ae8530714"/>
		<cito:citesForInformation rdf:resource="http://cognitiveatlas.org/citation/id/cit_4de6aec3e8c37"/>
</skos:Concept><skos:Concept rdf:about="http://cognitiveatlas.org/id/tsk_4a57abb949923"> <dc:identifier>tsk_4a57abb949923</dc:identifier>
		<dc:Title>Cognitive Atlas : Lexicon : category fluency test</dc:Title>
		<dc:Description>RDF output for 'category fluency test'</dc:Description>
		<dc:Type>InteractiveResource</dc:Type>
		<dc:Publisher>Cognitive Atlas</dc:Publisher>
		<dc:Creator>Cognitive Atlas RDF Generator</dc:Creator>
		<dc:Contributor>Brenda Gregory</dc:Contributor>
		<dc:Date>2011-04-19 13:52:08</dc:Date>
		<dc:Format>text/rdf</dc:Format>
		<dc:Language>en</dc:Language>
		<skos:editorialNote>Generated by testgen.php on Thu Jun 9 14:25:25 PDT 2011.</skos:editorialNote>
		<skos:historyNote>Revision 3: 2 previous definitions.</skos:historyNote>
		<skos:changeNote>See http://cognitiveatlas.org/id/tsk_4a57abb949923 for complete revision history.</skos:changeNote>
		<skos:scopeNote>http://www.w3.org/2004/02/skos/core#Concept</skos:scopeNote>
		<skos:Note>SKOS properties defined in http://www.w3.org/TR/skos-primer/#secrel</skos:Note>
		<skos:inScheme rdf:resource="http://cognitiveatlas.org/tasks/"/>
		<skos:definition>a psychological test in which participants have to say as many words as possible from a category in a given time (usually 60 seconds), this category can be semantic, such as animals or fruits, or phonemic, such as words that begin with letter p.</skos:definition>
		<skos:prefLabel>category fluency test</skos:prefLabel>
		<skos:altLabel></skos:altLabel>
		<skos:related rdf:resource="http://cognitiveatlas.org/id/trm_4a3fd79d0b077"/>
		<skos:related rdf:resource="http://cognitiveatlas.org/id/trm_4a3fd79d0b083"/>
		<skos:related rdf:resource="http://cognitiveatlas.org/id/trm_4a3fd79d0b87a"/>
		<skos:example>semantic knowledge is measured by the contrast of total correct responses for all categories trials in the category fluency test</skos:example>
		<skos:example>semantic memory is measured by the contrast of total correct responses for all categories trials in the category fluency test</skos:example>
		<skos:example>semantic processing is measured by the contrast of total correct responses for all categories trials in the category fluency test</skos:example>
		<cito:citesForInformation rdf:resource="http://cognitiveatlas.org/citation/id/cit_4de6b8980e553"/>
		<cito:citesForInformation rdf:resource="http://cognitiveatlas.org/citation/id/cit_4de6b8cfaa710"/>
		<cito:citesForInformation rdf:resource="http://cognitiveatlas.org/citation/id/cit_4de6b9186135d"/>
</skos:Concept><skos:Concept rdf:about="http://cognitiveatlas.org/id/tsk_4a57abb949934"> <dc:identifier>tsk_4a57abb949934</dc:identifier>
		<dc:Title>Cognitive Atlas : Lexicon : choice reaction time task</dc:Title>
		<dc:Description>RDF output for 'choice reaction time task'</dc:Description>
		<dc:Type>InteractiveResource</dc:Type>
		<dc:Publisher>Cognitive Atlas</dc:Publisher>
		<dc:Creator>Cognitive Atlas RDF Generator</dc:Creator>
		<dc:Contributor>Natalie Picchetti</dc:Contributor>
		<dc:Date>2011-04-15 12:04:24</dc:Date>
		<dc:Format>text/rdf</dc:Format>
		<dc:Language>en</dc:Language>
		<skos:editorialNote>Generated by testgen.php on Thu Jun 9 14:25:25 PDT 2011.</skos:editorialNote>
		<skos:historyNote>Revision 3: 2 previous definitions.</skos:historyNote>
		<skos:changeNote>See http://cognitiveatlas.org/id/tsk_4a57abb949934 for complete revision history.</skos:changeNote>
		<skos:scopeNote>http://www.w3.org/2004/02/skos/core#Concept</skos:scopeNote>
		<skos:Note>SKOS properties defined in http://www.w3.org/TR/skos-primer/#secrel</skos:Note>
		<skos:inScheme rdf:resource="http://cognitiveatlas.org/tasks/"/>
		<skos:definition>Choice reaction time tasks require distinct responses for each possible class of stimulus. For example, the subject might be asked to press one button if a red light appears and a different button if a yellow light appears.</skos:definition>
		<skos:prefLabel>choice reaction time task</skos:prefLabel>
		<skos:altLabel></skos:altLabel>
		<skos:related rdf:resource="http://cognitiveatlas.org/id/trm_4a3fd79d0af71"/>
		<skos:related rdf:resource="http://cognitiveatlas.org/id/trm_4a3fd79d0af66"/>
		<skos:related rdf:resource="http://cognitiveatlas.org/id/trm_4a3fd79d0b61f"/>
		<skos:related rdf:resource="http://cognitiveatlas.org/id/trm_4a3fd79d0b61f"/>
		<skos:related rdf:resource="http://cognitiveatlas.org/id/trm_4a3fd79d0b61f"/>
		<skos:related rdf:resource="http://cognitiveatlas.org/id/trm_4a3fd79d0b61f"/>
		<skos:related rdf:resource="http://cognitiveatlas.org/id/trm_4a3fd79d09c8c"/>
		<skos:related rdf:resource="http://cognitiveatlas.org/id/trm_4a3fd79d09c8c"/>
		<skos:related rdf:resource="http://cognitiveatlas.org/id/trm_4a3fd79d09c8c"/>
		<skos:related rdf:resource="http://cognitiveatlas.org/id/trm_4a3fd79d09c8c"/>
		<skos:example>response selection is measured by the contrast of stimulus trials in the choice reaction time task</skos:example>
		<skos:example>response inhibition is measured by the contrast of non-stimulus trials in the choice reaction time task</skos:example>
		<skos:example>decision is measured by the contrast of stimulus trials in the choice reaction time task</skos:example>
		<skos:example>decision is measured by the contrast of non-stimulus trials in the choice reaction time task</skos:example>
		<skos:example>decision is measured by the contrast of right hand trials in the choice reaction time task</skos:example>
		<skos:example>decision is measured by the contrast of left hand trials in the choice reaction time task</skos:example>
		<skos:example>choice is measured by the contrast of stimulus trials in the choice reaction time task</skos:example>
		<skos:example>choice is measured by the contrast of non-stimulus trials in the choice reaction time task</skos:example>
		<skos:example>choice is measured by the contrast of right hand trials in the choice reaction time task</skos:example>
		<skos:example>choice is measured by the contrast of left hand trials in the choice reaction time task</skos:example>
		<cito:citesForInformation rdf:resource="http://cognitiveatlas.org/citation/id/cit_4de6be81bb92a"/>
		<cito:citesForInformation rdf:resource="http://cognitiveatlas.org/citation/id/cit_4de6c044a5928"/>
		<cito:citesForInformation rdf:resource="http://cognitiveatlas.org/citation/id/cit_4de6c0f7c1bec"/>
</skos:Concept><skos:Concept rdf:about="http://cognitiveatlas.org/id/tsk_4a57abb9499a8"> <dc:identifier>tsk_4a57abb9499a8</dc:identifier>
		<dc:Title>Cognitive Atlas : Lexicon : Clinical Evaluation of Language Fundamentals-3</dc:Title>
		<dc:Description>RDF output for 'Clinical Evaluation of Language Fundamentals-3'</dc:Description>
		<dc:Type>InteractiveResource</dc:Type>
		<dc:Publisher>Cognitive Atlas</dc:Publisher>
		<dc:Creator>Cognitive Atlas RDF Generator</dc:Creator>
		<dc:Contributor>Brenda Gregory</dc:Contributor>
		<dc:Date>2011-05-10 15:00:36</dc:Date>
		<dc:Format>text/rdf</dc:Format>
		<dc:Language>en</dc:Language>
		<skos:editorialNote>Generated by testgen.php on Thu Jun 9 14:25:25 PDT 2011.</skos:editorialNote>
		<skos:historyNote>Revision 3: 2 previous definitions.</skos:historyNote>
		<skos:changeNote>See http://cognitiveatlas.org/id/tsk_4a57abb9499a8 for complete revision history.</skos:changeNote>
		<skos:scopeNote>http://www.w3.org/2004/02/skos/core#Concept</skos:scopeNote>
		<skos:Note>SKOS properties defined in http://www.w3.org/TR/skos-primer/#secrel</skos:Note>
		<skos:inScheme rdf:resource="http://cognitiveatlas.org/tasks/"/>
		<skos:definition>3rd edition of an assessment used to evaluate the nature and extent of language difficulties in school children and adolescents.</skos:definition>
		<skos:prefLabel>Clinical Evaluation of Language Fundamentals-3</skos:prefLabel>
		<skos:altLabel></skos:altLabel>
		<skos:related rdf:resource="http://cognitiveatlas.org/id/trm_4a3fd79d0b340"/>
		<skos:related rdf:resource="http://cognitiveatlas.org/id/trm_4a3fd79d0b340"/>
		<skos:related rdf:resource="http://cognitiveatlas.org/id/trm_4a3fd79d0b340"/>
		<skos:related rdf:resource="http://cognitiveatlas.org/id/trm_4a3fd79d0a775"/>
		<skos:related rdf:resource="http://cognitiveatlas.org/id/trm_4a3fd79d0a775"/>
		<skos:related rdf:resource="http://cognitiveatlas.org/id/trm_4a3fd79d0a7f8"/>
		<skos:related rdf:resource="http://cognitiveatlas.org/id/trm_4a3fd79d0a7f8"/>
		<skos:related rdf:resource="http://cognitiveatlas.org/id/trm_4a3fd79d0a7f8"/>
		<skos:related rdf:resource="http://cognitiveatlas.org/id/trm_4a3fd79d0a7f8"/>
		<skos:related rdf:resource="http://cognitiveatlas.org/id/trm_4a3fd79d0a7f8"/>
		<skos:related rdf:resource="http://cognitiveatlas.org/id/trm_4a3fd79d0b06b"/>
		<skos:related rdf:resource="http://cognitiveatlas.org/id/trm_4a3fd79d0b892"/>
		<skos:related rdf:resource="http://cognitiveatlas.org/id/trm_4a3fd79d0b892"/>
		<skos:related rdf:resource="http://cognitiveatlas.org/id/trm_4a3fd79d0b56b"/>
		<skos:related rdf:resource="http://cognitiveatlas.org/id/trm_4a3fd79d0b1f7"/>
		<skos:example>syntactic parsing is measured by the contrast of formulating sentences subtest trials in the Clinical Evaluation of Language Fundamentals-3</skos:example>
		<skos:example>syntactic parsing is measured by the contrast of sentence structure subtest trials in the Clinical Evaluation of Language Fundamentals-3</skos:example>
		<skos:example>syntactic parsing is measured by the contrast of sentence assembly subtest trials in the Clinical Evaluation of Language Fundamentals-3</skos:example>
		<skos:example>language comprehension is measured by the contrast of concepts and directions subtest trials in the Clinical Evaluation of Language Fundamentals-3</skos:example>
		<skos:example>language comprehension is measured by the contrast of semantic relationships subtest trials in the Clinical Evaluation of Language Fundamentals-3</skos:example>
		<skos:example>linguistic competence is measured by the contrast of formulating sentences subtest trials in the Clinical Evaluation of Language Fundamentals-3</skos:example>
		<skos:example>linguistic competence is measured by the contrast of sentence structure subtest trials in the Clinical Evaluation of Language Fundamentals-3</skos:example>
		<skos:example>linguistic competence is measured by the contrast of word classes subtest trials in the Clinical Evaluation of Language Fundamentals-3</skos:example>
		<skos:example>linguistic competence is measured by the contrast of word structure subtest trials in the Clinical Evaluation of Language Fundamentals-3</skos:example>
		<skos:example>linguistic competence is measured by the contrast of sentence assembly subtest trials in the Clinical Evaluation of Language Fundamentals-3</skos:example>
		<skos:example>semantic category is measured by the contrast of semantic relationships subtest trials in the Clinical Evaluation of Language Fundamentals-3</skos:example>
		<skos:example>sentence comprehension is measured by the contrast of sentence structure subtest trials in the Clinical Evaluation of Language Fundamentals-3</skos:example>
		<skos:example>sentence comprehension is measured by the contrast of sentence assembly subtest trials in the Clinical Evaluation of Language Fundamentals-3</skos:example>
		<skos:example>word order is measured by the contrast of sentence structure subtest trials in the Clinical Evaluation of Language Fundamentals-3</skos:example>
		<skos:example>speech perception is measured by the contrast of concepts and directions subtest trials in the Clinical Evaluation of Language Fundamentals-3</skos:example>
		<cito:citesForInformation rdf:resource="http://cognitiveatlas.org/citation/id/cit_4de6d36356597"/>
		<cito:citesForInformation rdf:resource="http://cognitiveatlas.org/citation/id/cit_4de6d481e3982"/>
</skos:Concept><skos:Concept rdf:about="http://cognitiveatlas.org/id/tsk_4a57abb9499b8"> <dc:identifier>tsk_4a57abb9499b8</dc:identifier>
		<dc:Title>Cognitive Atlas : Lexicon : color-discrimination task</dc:Title>
		<dc:Description>RDF output for 'color-discrimination task'</dc:Description>
		<dc:Type>InteractiveResource</dc:Type>
		<dc:Publisher>Cognitive Atlas</dc:Publisher>
		<dc:Creator>Cognitive Atlas RDF Generator</dc:Creator>
		<dc:Contributor>Natalie Picchetti</dc:Contributor>
		<dc:Date>2011-03-15 09:24:36</dc:Date>
		<dc:Format>text/rdf</dc:Format>
		<dc:Language>en</dc:Language>
		<skos:editorialNote>Generated by testgen.php on Thu Jun 9 14:25:25 PDT 2011.</skos:editorialNote>
		<skos:historyNote>Revision 2: 1 previous definitions.</skos:historyNote>
		<skos:changeNote>See http://cognitiveatlas.org/id/tsk_4a57abb9499b8 for complete revision history.</skos:changeNote>
		<skos:scopeNote>http://www.w3.org/2004/02/skos/core#Concept</skos:scopeNote>
		<skos:Note>SKOS properties defined in http://www.w3.org/TR/skos-primer/#secrel</skos:Note>
		<skos:inScheme rdf:resource="http://cognitiveatlas.org/tasks/"/>
		<skos:definition>is a behavioral task where a subject is to make specific responses when presented with particular colors.  The responses to the various colors are then evaluated to see if the subject was able to discern between different colors.    </skos:definition>
		<skos:prefLabel>color-discrimination task</skos:prefLabel>
		<skos:altLabel></skos:altLabel>
		<skos:related rdf:resource="http://cognitiveatlas.org/id/trm_4a3fd79d09d93"/>
		<skos:example>color perception is measured by the contrast of accuracy trials in the color-discrimination task</skos:example>
		<cito:citesForInformation rdf:resource="http://cognitiveatlas.org/citation/id/cit_4de7b6b2401d2"/>
		<cito:citesForInformation rdf:resource="http://cognitiveatlas.org/citation/id/cit_4de7b9f69e8ed"/>
</skos:Concept><skos:Concept rdf:about="http://cognitiveatlas.org/id/tsk_4a57abb9499c7"> <dc:identifier>tsk_4a57abb9499c7</dc:identifier>
		<dc:Title>Cognitive Atlas : Lexicon : continuous recognition paradigm</dc:Title>
		<dc:Description>RDF output for 'continuous recognition paradigm'</dc:Description>
		<dc:Type>InteractiveResource</dc:Type>
		<dc:Publisher>Cognitive Atlas</dc:Publisher>
		<dc:Creator>Cognitive Atlas RDF Generator</dc:Creator>
		<dc:Contributor>Brenda Gregory</dc:Contributor>
		<dc:Date>2011-04-19 12:06:22</dc:Date>
		<dc:Format>text/rdf</dc:Format>
		<dc:Language>en</dc:Language>
		<skos:editorialNote>Generated by testgen.php on Thu Jun 9 14:25:25 PDT 2011.</skos:editorialNote>
		<skos:historyNote>Revision 3: 2 previous definitions.</skos:historyNote>
		<skos:changeNote>See http://cognitiveatlas.org/id/tsk_4a57abb9499c7 for complete revision history.</skos:changeNote>
		<skos:scopeNote>http://www.w3.org/2004/02/skos/core#Concept</skos:scopeNote>
		<skos:Note>SKOS properties defined in http://www.w3.org/TR/skos-primer/#secrel</skos:Note>
		<skos:inScheme rdf:resource="http://cognitiveatlas.org/tasks/"/>
		<skos:definition>In the continuous recognition paradigm, study and test phases are not separate entities, but rather, items are continuously presented and the participant is instructed to respond to an item as &#34;old&#34; if it has been seen before (generally presented a second time) in this continual stream of item presentation. Items that were correctly called &#34;old&#34; are the subsequently remembered trials, and items that were &#34;missed&#34; (not called old upon second presentation) make up the subsequently forgotten trials. </skos:definition>
		<skos:prefLabel>continuous recognition paradigm</skos:prefLabel>
		<skos:altLabel></skos:altLabel>
		<skos:related rdf:resource="http://cognitiveatlas.org/id/trm_4a3fd79d0b58f"/>
		<skos:related rdf:resource="http://cognitiveatlas.org/id/trm_4a3fd79d0a323"/>
		<skos:related rdf:resource="http://cognitiveatlas.org/id/trm_4a3fd79d0b908"/>
		<skos:related rdf:resource="http://cognitiveatlas.org/id/trm_4c898b29660b0"/>
		<skos:example>word recognition is measured by the contrast of number of correct identifications trials in the continuous recognition paradigm</skos:example>
		<skos:example>false memory is measured by the contrast of number of false positives trials in the continuous recognition paradigm</skos:example>
		<skos:example>forgetting is measured by the contrast of number of false negatives (missed words) trials in the continuous recognition paradigm</skos:example>
		<skos:example>Cued Explicit Recognition is related to continuous recognition paradigm</skos:example>
		<cito:citesForInformation rdf:resource="http://cognitiveatlas.org/citation/id/cit_4de7c4d6b3c33"/>
		<cito:citesForInformation rdf:resource="http://cognitiveatlas.org/citation/id/cit_4de7c838e4fbd"/>
</skos:Concept><skos:Concept rdf:about="http://cognitiveatlas.org/id/tsk_4a57abb9499d5"> <dc:identifier>tsk_4a57abb9499d5</dc:identifier>
		<dc:Title>Cognitive Atlas : Lexicon : Cups task</dc:Title>
		<dc:Description>RDF output for 'Cups task'</dc:Description>
		<dc:Type>InteractiveResource</dc:Type>
		<dc:Publisher>Cognitive Atlas</dc:Publisher>
		<dc:Creator>Cognitive Atlas RDF Generator</dc:Creator>
		<dc:Contributor>Carinna Torgerson</dc:Contributor>
		<dc:Date>2011-06-02 11:36:09</dc:Date>
		<dc:Format>text/rdf</dc:Format>
		<dc:Language>en</dc:Language>
		<skos:editorialNote>Generated by testgen.php on Thu Jun 9 14:25:25 PDT 2011.</skos:editorialNote>
		<skos:historyNote>Revision 5: 4 previous definitions.</skos:historyNote>
		<skos:changeNote>See http://cognitiveatlas.org/id/tsk_4a57abb9499d5 for complete revision history.</skos:changeNote>
		<skos:scopeNote>http://www.w3.org/2004/02/skos/core#Concept</skos:scopeNote>
		<skos:Note>SKOS properties defined in http://www.w3.org/TR/skos-primer/#secrel</skos:Note>
		<skos:inScheme rdf:resource="http://cognitiveatlas.org/tasks/"/>
		<skos:definition>a task in which subjects are presented with a number of overturned cups. In some cases only one cup contains a reward, while in other studies the cups contain various levels of rewards (usually different amounts of money).</skos:definition>
		<skos:prefLabel>Cups task</skos:prefLabel>
		<skos:altLabel></skos:altLabel>
		<skos:related rdf:resource="http://cognitiveatlas.org/id/trm_4a3fd79d0b64e"/>
		<skos:related rdf:resource="http://cognitiveatlas.org/id/trm_4a3fd79d0afcf"/>
		<skos:related rdf:resource="http://cognitiveatlas.org/id/trm_4b6525253c63f"/>
		<skos:example>risk seeking is measured by the contrast of number or value of rewards times probability of reward trials in the Cups task</skos:example>
		<skos:example>risk is measured by the contrast of probability of highest reward trials in the Cups task</skos:example>
		<skos:example>reward is measured by the contrast of money earned trials in the Cups task</skos:example>
		<cito:citesForInformation rdf:resource="http://cognitiveatlas.org/citation/id/cit_4dac930abcaca"/>
		<cito:citesForInformation rdf:resource="http://cognitiveatlas.org/citation/id/cit_4d559a46899b6"/>
		<cito:citesForInformation rdf:resource="http://cognitiveatlas.org/citation/id/cit_4de7d6f5ea564"/>
</skos:Concept><skos:Concept rdf:about="http://cognitiveatlas.org/id/tsk_4a57abb9499e3"> <dc:identifier>tsk_4a57abb9499e3</dc:identifier>
		<dc:Title>Cognitive Atlas : Lexicon : delayed match to sample task</dc:Title>
		<dc:Description>RDF output for 'delayed match to sample task'</dc:Description>
		<dc:Type>InteractiveResource</dc:Type>
		<dc:Publisher>Cognitive Atlas</dc:Publisher>
		<dc:Creator>Cognitive Atlas RDF Generator</dc:Creator>
		<dc:Contributor>Brenda Gregory</dc:Contributor>
		<dc:Date>2011-04-19 12:09:20</dc:Date>
		<dc:Format>text/rdf</dc:Format>
		<dc:Language>en</dc:Language>
		<skos:editorialNote>Generated by testgen.php on Thu Jun 9 14:25:25 PDT 2011.</skos:editorialNote>
		<skos:historyNote>Revision 3: 2 previous definitions.</skos:historyNote>
		<skos:changeNote>See http://cognitiveatlas.org/id/tsk_4a57abb9499e3 for complete revision history.</skos:changeNote>
		<skos:scopeNote>http://www.w3.org/2004/02/skos/core#Concept</skos:scopeNote>
		<skos:Note>SKOS properties defined in http://www.w3.org/TR/skos-primer/#secrel</skos:Note>
		<skos:inScheme rdf:resource="http://cognitiveatlas.org/tasks/"/>
		<skos:definition>Subjects view an item(s). After a brief delay a probe item is presented and subjects are asked to recall if the probe item was presented before the delay (during encoding). Stimuli can be words, pictures, or abstract patterns. </skos:definition>
		<skos:prefLabel>delayed match to sample task</skos:prefLabel>
		<skos:altLabel></skos:altLabel>
		<skos:related rdf:resource="http://cognitiveatlas.org/id/trm_4a3fd79d0ba0d"/>
		<skos:related rdf:resource="http://cognitiveatlas.org/id/trm_4a3fd79d0a431"/>
		<skos:related rdf:resource="http://cognitiveatlas.org/id/trm_4a3fd79d0b92c"/>
		<skos:related rdf:resource="http://cognitiveatlas.org/id/trm_4a3fd79d0ba6c"/>
		<skos:related rdf:resource="http://cognitiveatlas.org/id/trm_4a3fd79d0b5a7"/>
		<skos:related rdf:resource="http://cognitiveatlas.org/id/tsk_4a57abb949e0c"/>
		<skos:example>delayed match to sample task is a broader synonym of Sternberg delayed recognition task</skos:example>
		<skos:example>active maintenance is measured by the contrast of reaction time to correct stimuli trials in the delayed match to sample task</skos:example>
		<skos:example>goal maintenance is measured by the contrast of reaction time to correct stimuli trials in the delayed match to sample task</skos:example>
		<skos:example>memory decay is measured by the contrast of reaction time to correct stimuli trials in the delayed match to sample task</skos:example>
		<skos:example>working memory retrieval is measured by the contrast of reaction time to correct stimuli trials in the delayed match to sample task</skos:example>
		<skos:example>working memory is measured by the contrast of reaction time to correct stimuli trials in the delayed match to sample task</skos:example>
		<cito:citesForInformation rdf:resource="http://cognitiveatlas.org/citation/id/cit_4de90c3072da3"/>
		<cito:citesForInformation rdf:resource="http://cognitiveatlas.org/citation/id/cit_4de90e59e864b"/>
</skos:Concept><skos:Concept rdf:about="http://cognitiveatlas.org/id/tsk_4a57abb9499f1"> <dc:identifier>tsk_4a57abb9499f1</dc:identifier>
		<dc:Title>Cognitive Atlas : Lexicon : delayed nonmatch to sample task</dc:Title>
		<dc:Description>RDF output for 'delayed nonmatch to sample task'</dc:Description>
		<dc:Type>InteractiveResource</dc:Type>
		<dc:Publisher>Cognitive Atlas</dc:Publisher>
		<dc:Creator>Cognitive Atlas RDF Generator</dc:Creator>
		<dc:Contributor>Agatha Lenartowicz</dc:Contributor>
		<dc:Date>2009-07-10 14:06:33</dc:Date>
		<dc:Format>text/rdf</dc:Format>
		<dc:Language>en</dc:Language>
		<skos:editorialNote>Generated by testgen.php on Thu Jun 9 14:25:25 PDT 2011.</skos:editorialNote>
		<skos:historyNote>No previous definition revisions.</skos:historyNote>
		<skos:changeNote>This is the first and only definition provided.</skos:changeNote>
		<skos:scopeNote>http://www.w3.org/2004/02/skos/core#Concept</skos:scopeNote>
		<skos:Note>SKOS properties defined in http://www.w3.org/TR/skos-primer/#secrel</skos:Note>
		<skos:inScheme rdf:resource="http://cognitiveatlas.org/tasks/"/>
		<skos:definition>A task in which an target is presented and then removed from view. This target must be maintained in working memory for a delay, after which it is presented with non-target(s). The participant&#39;s task is to identify the non-target.</skos:definition>
		<skos:prefLabel>delayed nonmatch to sample task</skos:prefLabel>
		<skos:altLabel></skos:altLabel>
		<skos:related rdf:resource="http://cognitiveatlas.org/id/trm_4a3fd79d0b5a7"/>
		<skos:related rdf:resource="http://cognitiveatlas.org/id/trm_4a3fd79d0b5a7"/>
		<skos:related rdf:resource="http://cognitiveatlas.org/id/trm_4a3fd79d0b92c"/>
		<skos:related rdf:resource="http://cognitiveatlas.org/id/trm_4a3fd79d0b5a7"/>
		<skos:example>working memory is measured by the contrast of delay trials in the delayed nonmatch to sample task</skos:example>
		<skos:example>working memory is measured by the contrast of delay minus no delay trials in the delayed nonmatch to sample task</skos:example>
		<skos:example>memory decay is measured by the contrast of delay minus no delay trials in the delayed nonmatch to sample task</skos:example>
		<skos:example>working memory is measured by the contrast of delay minus no delay trials in the delayed nonmatch to sample task</skos:example>
		<cito:citesForInformation rdf:resource="http://cognitiveatlas.org/citation/id/cit_4de91383320ad"/>
		<cito:citesForInformation rdf:resource="http://cognitiveatlas.org/citation/id/cit_4de913bd78e06"/>
</skos:Concept><skos:Concept rdf:about="http://cognitiveatlas.org/id/tsk_4a57abb9499ff"> <dc:identifier>tsk_4a57abb9499ff</dc:identifier>
		<dc:Title>Cognitive Atlas : Lexicon : delayed recall test</dc:Title>
		<dc:Description>RDF output for 'delayed recall test'</dc:Description>
		<dc:Type>InteractiveResource</dc:Type>
		<dc:Publisher>Cognitive Atlas</dc:Publisher>
		<dc:Creator>Cognitive Atlas RDF Generator</dc:Creator>
		<dc:Contributor>Agatha Lenartowicz</dc:Contributor>
		<dc:Date>2009-07-10 14:06:33</dc:Date>
		<dc:Format>text/rdf</dc:Format>
		<dc:Language>en</dc:Language>
		<skos:editorialNote>Generated by testgen.php on Thu Jun 9 14:25:25 PDT 2011.</skos:editorialNote>
		<skos:historyNote>No previous definition revisions.</skos:historyNote>
		<skos:changeNote>This is the first and only definition provided.</skos:changeNote>
		<skos:scopeNote>http://www.w3.org/2004/02/skos/core#Concept</skos:scopeNote>
		<skos:Note>SKOS properties defined in http://www.w3.org/TR/skos-primer/#secrel</skos:Note>
		<skos:inScheme rdf:resource="http://cognitiveatlas.org/tasks/"/>
		<skos:definition>A task in which participants are given information to remember (list of words or paragraph) and which they are asked to reproduce after some span of time.</skos:definition>
		<skos:prefLabel>delayed recall test</skos:prefLabel>
		<skos:altLabel></skos:altLabel>
		<skos:related rdf:resource="http://cognitiveatlas.org/id/trm_4a3fd79d0ba01"/>
		<skos:example>memory retrieval is measured by the contrast of d&#39; trials in the delayed recall test</skos:example>
		<cito:citesForInformation rdf:resource="http://cognitiveatlas.org/citation/id/cit_4de916aca4c94"/>
		<cito:citesForInformation rdf:resource="http://cognitiveatlas.org/citation/id/cit_4de9177761ed9"/>
</skos:Concept><skos:Concept rdf:about="http://cognitiveatlas.org/id/tsk_4a57abb949a0d"> <dc:identifier>tsk_4a57abb949a0d</dc:identifier>
		<dc:Title>Cognitive Atlas : Lexicon : Digit span task</dc:Title>
		<dc:Description>RDF output for 'Digit span task'</dc:Description>
		<dc:Type>InteractiveResource</dc:Type>
		<dc:Publisher>Cognitive Atlas</dc:Publisher>
		<dc:Creator>Cognitive Atlas RDF Generator</dc:Creator>
		<dc:Contributor>Agatha Lenartowicz</dc:Contributor>
		<dc:Date>2009-07-10 14:06:33</dc:Date>
		<dc:Format>text/rdf</dc:Format>
		<dc:Language>en</dc:Language>
		<skos:editorialNote>Generated by testgen.php on Thu Jun 9 14:25:25 PDT 2011.</skos:editorialNote>
		<skos:historyNote>No previous definition revisions.</skos:historyNote>
		<skos:changeNote>This is the first and only definition provided.</skos:changeNote>
		<skos:scopeNote>http://www.w3.org/2004/02/skos/core#Concept</skos:scopeNote>
		<skos:Note>SKOS properties defined in http://www.w3.org/TR/skos-primer/#secrel</skos:Note>
		<skos:inScheme rdf:resource="http://cognitiveatlas.org/tasks/"/>
		<skos:definition>A task in which participants are presented with sequentially presented digits and are then asked to recall the items. The number of digits that can be correctly recalled provides an estimate of working memory capacity.</skos:definition>
		<skos:prefLabel>Digit span task</skos:prefLabel>
		<skos:altLabel></skos:altLabel>
		<skos:related rdf:resource="http://cognitiveatlas.org/id/trm_4a3fd79d0a252"/>
		<skos:related rdf:resource="http://cognitiveatlas.org/id/trm_4a3fd79d0ac9e"/>
		<skos:related rdf:resource="http://cognitiveatlas.org/id/tsk_4a57abb94989b"/>
		<skos:related rdf:resource="http://cognitiveatlas.org/id/tsk_4a57abb949a85"/>
		<skos:related rdf:resource="http://cognitiveatlas.org/id/trm_4a3fd79d0b5a7"/>
		<skos:related rdf:resource="http://cognitiveatlas.org/id/trm_4a3fd79d0b5a7"/>
		<skos:example>executive function is measured by the contrast of backward trials in the Digit span task</skos:example>
		<skos:example>phonological working memory is measured by the contrast of forward trials in the Digit span task</skos:example>
		<skos:example>Backward digit span task is descended from Digit span task</skos:example>
		<skos:example>Forward digit span task is descended from Digit span task</skos:example>
		<skos:example>working memory is measured by the contrast of forward trials in the Digit span task</skos:example>
		<skos:example>working memory is measured by the contrast of backward trials in the Digit span task</skos:example>
		<cito:citesForInformation rdf:resource="http://cognitiveatlas.org/citation/id/cit_4de923c052e03"/>
		<cito:citesForInformation rdf:resource="http://cognitiveatlas.org/citation/id/cit_4de9247400a43"/>
		<cito:citesForInformation rdf:resource="http://cognitiveatlas.org/citation/id/cit_4de925a401795"/>
</skos:Concept><skos:Concept rdf:about="http://cognitiveatlas.org/id/tsk_4a57abb949a25"> <dc:identifier>tsk_4a57abb949a25</dc:identifier>
		<dc:Title>Cognitive Atlas : Lexicon : Digit/Symbol Coding test</dc:Title>
		<dc:Description>RDF output for 'Digit/Symbol Coding test'</dc:Description>
		<dc:Type>InteractiveResource</dc:Type>
		<dc:Publisher>Cognitive Atlas</dc:Publisher>
		<dc:Creator>Cognitive Atlas RDF Generator</dc:Creator>
		<dc:Contributor>Natalie Picchetti</dc:Contributor>
		<dc:Date>2011-04-19 13:20:28</dc:Date>
		<dc:Format>text/rdf</dc:Format>
		<dc:Language>en</dc:Language>
		<skos:editorialNote>Generated by testgen.php on Thu Jun 9 14:25:25 PDT 2011.</skos:editorialNote>
		<skos:historyNote>Revision 3: 2 previous definitions.</skos:historyNote>
		<skos:changeNote>See http://cognitiveatlas.org/id/tsk_4a57abb949a25 for complete revision history.</skos:changeNote>
		<skos:scopeNote>http://www.w3.org/2004/02/skos/core#Concept</skos:scopeNote>
		<skos:Note>SKOS properties defined in http://www.w3.org/TR/skos-primer/#secrel</skos:Note>
		<skos:inScheme rdf:resource="http://cognitiveatlas.org/tasks/"/>
		<skos:definition>a neuropsychological test sensitive to brain damage, dementia, age and depression; consists of (e.g. nine) digit-symbol pairs (e.g. 1/-,2/┴ ... 7/Λ,8/X,9/=) followed by a list of digits. Under each digit the subject should write down the corresponding symbol as fast as possible. The number of correct symbols within the allowed time (e.g. 90 or 120 sec) is measured.</skos:definition>
		<skos:prefLabel>Digit/Symbol Coding test</skos:prefLabel>
		<skos:altLabel></skos:altLabel>
		<skos:related rdf:resource="http://cognitiveatlas.org/id/trm_4a3fd79d0a972"/>
		<skos:related rdf:resource="http://cognitiveatlas.org/id/trm_4a3fd79d0b5a7"/>
		<skos:related rdf:resource="http://cognitiveatlas.org/id/trm_4a3fd79d0b8c1"/>
		<skos:related rdf:resource="http://cognitiveatlas.org/id/trm_4a3fd79d0b8c1"/>
		<skos:related rdf:resource="http://cognitiveatlas.org/id/trm_4a3fd79d0ba01"/>
		<skos:related rdf:resource="http://cognitiveatlas.org/id/tsk_4a57abb949f12"/>
		<skos:example>Digit/Symbol Coding test is descended from Wechsler Adult Intelligence Scale - Revised</skos:example>
		<skos:example>motor control is measured by the contrast of digit/symbol coding - symbol copy trials in the Digit/Symbol Coding test</skos:example>
		<skos:example>working memory is measured by the contrast of immediate memory copy trials in the Digit/Symbol Coding test</skos:example>
		<skos:example>active retrieval is measured by the contrast of immediate memory copy trials in the Digit/Symbol Coding test</skos:example>
		<skos:example>active retrieval is measured by the contrast of general memory copy trials in the Digit/Symbol Coding test</skos:example>
		<skos:example>memory retrieval is measured by the contrast of general memory copy trials in the Digit/Symbol Coding test</skos:example>
		<cito:citesForInformation rdf:resource="http://cognitiveatlas.org/citation/id/cit_4de927e5da6b5"/>
		<cito:citesForInformation rdf:resource="http://cognitiveatlas.org/citation/id/cit_4de92a7fb8ecc"/>
</skos:Concept><skos:Concept rdf:about="http://cognitiveatlas.org/id/tsk_4a57abb949a33"> <dc:identifier>tsk_4a57abb949a33</dc:identifier>
		<dc:Title>Cognitive Atlas : Lexicon : Doors and People Test</dc:Title>
		<dc:Description>RDF output for 'Doors and People Test'</dc:Description>
		<dc:Type>InteractiveResource</dc:Type>
		<dc:Publisher>Cognitive Atlas</dc:Publisher>
		<dc:Creator>Cognitive Atlas RDF Generator</dc:Creator>
		<dc:Contributor>Brenda Gregory</dc:Contributor>
		<dc:Date>2011-05-16 13:29:43</dc:Date>
		<dc:Format>text/rdf</dc:Format>
		<dc:Language>en</dc:Language>
		<skos:editorialNote>Generated by testgen.php on Thu Jun 9 14:25:25 PDT 2011.</skos:editorialNote>
		<skos:historyNote>Revision 3: 2 previous definitions.</skos:historyNote>
		<skos:changeNote>See http://cognitiveatlas.org/id/tsk_4a57abb949a33 for complete revision history.</skos:changeNote>
		<skos:scopeNote>http://www.w3.org/2004/02/skos/core#Concept</skos:scopeNote>
		<skos:Note>SKOS properties defined in http://www.w3.org/TR/skos-primer/#secrel</skos:Note>
		<skos:inScheme rdf:resource="http://cognitiveatlas.org/tasks/"/>
		<skos:definition>Doors and People is a test of long-term memory. It yields a single age-scaled overall score which can be ‘unpacked’ to give separate measures of visual and verbal memory, recall and recognition, and forgetting.</skos:definition>
		<skos:prefLabel>Doors and People Test</skos:prefLabel>
		<skos:altLabel></skos:altLabel>
		<skos:related rdf:resource="http://cognitiveatlas.org/id/trm_4a3fd79d0b0f7"/>
		<skos:related rdf:resource="http://cognitiveatlas.org/id/trm_4a3fd79d0b0f7"/>
		<skos:related rdf:resource="http://cognitiveatlas.org/id/trm_4a3fd79d0b0f7"/>
		<skos:related rdf:resource="http://cognitiveatlas.org/id/trm_4a3fd79d0b0f7"/>
		<skos:related rdf:resource="http://cognitiveatlas.org/id/trm_4a3fd79d0a4f9"/>
		<skos:related rdf:resource="http://cognitiveatlas.org/id/trm_4a3fd79d0a4f9"/>
		<skos:related rdf:resource="http://cognitiveatlas.org/id/trm_4a3fd79d0b95b"/>
		<skos:related rdf:resource="http://cognitiveatlas.org/id/trm_4a3fd79d0b95b"/>
		<skos:related rdf:resource="http://cognitiveatlas.org/id/trm_4a3fd79d0b95b"/>
		<skos:related rdf:resource="http://cognitiveatlas.org/id/trm_4a3fd79d0b95b"/>
		<skos:example>short term memory is measured by the contrast of verbal recall (people test) trials in the Doors and People Test</skos:example>
		<skos:example>short term memory is measured by the contrast of visual recognition (doors test) trials in the Doors and People Test</skos:example>
		<skos:example>short term memory is measured by the contrast of visual recall (shapes test) trials in the Doors and People Test</skos:example>
		<skos:example>short term memory is measured by the contrast of verbal recognition (names test) trials in the Doors and People Test</skos:example>
		<skos:example>iconic memory is measured by the contrast of visual recognition (doors test) trials in the Doors and People Test</skos:example>
		<skos:example>iconic memory is measured by the contrast of visual recall (shapes test) trials in the Doors and People Test</skos:example>
		<skos:example>recall is measured by the contrast of verbal recall (people test) trials in the Doors and People Test</skos:example>
		<skos:example>recall is measured by the contrast of visual recognition (doors test) trials in the Doors and People Test</skos:example>
		<skos:example>recall is measured by the contrast of visual recall (shapes test) trials in the Doors and People Test</skos:example>
		<skos:example>recall is measured by the contrast of verbal recognition (names test) trials in the Doors and People Test</skos:example>
		<cito:citesForInformation rdf:resource="http://cognitiveatlas.org/citation/id/cit_4de93edaee646"/>
		<cito:citesForInformation rdf:resource="http://cognitiveatlas.org/citation/id/cit_4de93eebd4580"/>
</skos:Concept><skos:Concept rdf:about="http://cognitiveatlas.org/id/tsk_4a57abb949a41"> <dc:identifier>tsk_4a57abb949a41</dc:identifier>
		<dc:Title>Cognitive Atlas : Lexicon : Edinburgh Handedness Inventory</dc:Title>
		<dc:Description>RDF output for 'Edinburgh Handedness Inventory'</dc:Description>
		<dc:Type>InteractiveResource</dc:Type>
		<dc:Publisher>Cognitive Atlas</dc:Publisher>
		<dc:Creator>Cognitive Atlas RDF Generator</dc:Creator>
		<dc:Contributor>Carinna Torgerson</dc:Contributor>
		<dc:Date>2011-06-03 15:37:06</dc:Date>
		<dc:Format>text/rdf</dc:Format>
		<dc:Language>en</dc:Language>
		<skos:editorialNote>Generated by testgen.php on Thu Jun 9 14:25:25 PDT 2011.</skos:editorialNote>
		<skos:historyNote>Revision 4: 3 previous definitions.</skos:historyNote>
		<skos:changeNote>See http://cognitiveatlas.org/id/tsk_4a57abb949a41 for complete revision history.</skos:changeNote>
		<skos:scopeNote>http://www.w3.org/2004/02/skos/core#Concept</skos:scopeNote>
		<skos:Note>SKOS properties defined in http://www.w3.org/TR/skos-primer/#secrel</skos:Note>
		<skos:inScheme rdf:resource="http://cognitiveatlas.org/tasks/"/>
		<skos:definition>a measurement scale used to assess the dominance of a person&#39;s right or left hand in everyday activities. It consists of a questionnaire with 10 activities listed (writing, drawing, throwing, using scissors, using a toothbrush, using a knife without a fork, using a spoon, the upper hand when using a broom, striking a match, and opening the lid of a box). Participants must indicate which hand they would use, and the strength of this preference (strong, less strong, indifferent).</skos:definition>
		<skos:prefLabel>Edinburgh Handedness Inventory</skos:prefLabel>
		<skos:altLabel></skos:altLabel>
		<skos:related rdf:resource="http://cognitiveatlas.org/id/trm_4a3fd79d0a972"/>
		<skos:example>motor control is measured by the contrast of sum of strength scores x sum of items per hand trials in the Edinburgh Handedness Inventory</skos:example>
		<cito:citesForInformation rdf:resource="http://cognitiveatlas.org/citation/id/cit_4de960c6f2de9"/>
		<cito:citesForInformation rdf:resource="http://cognitiveatlas.org/citation/id/cit_4de960eae240d"/>
		<cito:citesForInformation rdf:resource="http://cognitiveatlas.org/citation/id/cit_4de964cc5ca4e"/>
</skos:Concept><skos:Concept rdf:about="http://cognitiveatlas.org/id/tsk_4a57abb949a4f"> <dc:identifier>tsk_4a57abb949a4f</dc:identifier>
		<dc:Title>Cognitive Atlas : Lexicon : Eriksen flanker task</dc:Title>
		<dc:Description>RDF output for 'Eriksen flanker task'</dc:Description>
		<dc:Type>InteractiveResource</dc:Type>
		<dc:Publisher>Cognitive Atlas</dc:Publisher>
		<dc:Creator>Cognitive Atlas RDF Generator</dc:Creator>
		<dc:Contributor>Agatha Lenartowicz</dc:Contributor>
		<dc:Date>2009-07-10 14:06:33</dc:Date>
		<dc:Format>text/rdf</dc:Format>
		<dc:Language>en</dc:Language>
		<skos:editorialNote>Generated by testgen.php on Thu Jun 9 14:25:25 PDT 2011.</skos:editorialNote>
		<skos:historyNote>No previous definition revisions.</skos:historyNote>
		<skos:changeNote>This is the first and only definition provided.</skos:changeNote>
		<skos:scopeNote>http://www.w3.org/2004/02/skos/core#Concept</skos:scopeNote>
		<skos:Note>SKOS properties defined in http://www.w3.org/TR/skos-primer/#secrel</skos:Note>
		<skos:inScheme rdf:resource="http://cognitiveatlas.org/tasks/"/>
		<skos:definition>A task in which participants view stimuli (typically arrows) presented one at a time and to which they must make a simple lexical response. These stimuli are surrounded by either distracting or facilitating items. Distracting items are typically associated with an opposite response (&#34;incongruent&#34; = pointing in opposite direction to target stimulus), whereas facilitating items are typically associated with the same response as the target stimulus (&#34;congruent&#34; = pointing in the same direction as the target stimulus).</skos:definition>
		<skos:prefLabel>Eriksen flanker task</skos:prefLabel>
		<skos:altLabel></skos:altLabel>
		<skos:related rdf:resource="http://cognitiveatlas.org/id/trm_4a3fd79d0a613"/>
		<skos:related rdf:resource="http://cognitiveatlas.org/id/trm_4a3fd79d0a252"/>
		<skos:example>inhibition is measured by the contrast of incongruent response time - congruent response time trials in the Eriksen flanker task</skos:example>
		<skos:example>executive function is measured by the contrast of incongruent response time - congruent response time trials in the Eriksen flanker task</skos:example>
		<cito:citesForInformation rdf:resource="http://cognitiveatlas.org/citation/id/cit_4decff805f5d3"/>
		<cito:citesForInformation rdf:resource="http://cognitiveatlas.org/citation/id/cit_4ded00170b7f2"/>
		<cito:citesForInformation rdf:resource="http://cognitiveatlas.org/citation/id/cit_4ded002c8ae1c"/>
</skos:Concept><skos:Concept rdf:about="http://cognitiveatlas.org/id/tsk_4a57abb949a5d"> <dc:identifier>tsk_4a57abb949a5d</dc:identifier>
		<dc:Title>Cognitive Atlas : Lexicon : Extradimensional shift task</dc:Title>
		<dc:Description>RDF output for 'Extradimensional shift task'</dc:Description>
		<dc:Type>InteractiveResource</dc:Type>
		<dc:Publisher>Cognitive Atlas</dc:Publisher>
		<dc:Creator>Cognitive Atlas RDF Generator</dc:Creator>
		<dc:Contributor>Agatha Lenartowicz</dc:Contributor>
		<dc:Date>2009-07-10 14:06:33</dc:Date>
		<dc:Format>text/rdf</dc:Format>
		<dc:Language>en</dc:Language>
		<skos:editorialNote>Generated by testgen.php on Thu Jun 9 14:25:25 PDT 2011.</skos:editorialNote>
		<skos:historyNote>No previous definition revisions.</skos:historyNote>
		<skos:changeNote>This is the first and only definition provided.</skos:changeNote>
		<skos:scopeNote>http://www.w3.org/2004/02/skos/core#Concept</skos:scopeNote>
		<skos:Note>SKOS properties defined in http://www.w3.org/TR/skos-primer/#secrel</skos:Note>
		<skos:inScheme rdf:resource="http://cognitiveatlas.org/tasks/"/>
		<skos:definition>A task in which multiple (typically two) stimuli are presented simultaneously and the subject must select the stimulus that matches the currently relevant rule. The relevant rule alternates or &#34;shifts&#34; among multiple (typically two) rules. The rule represents the relevant task &#34;dimension&#34;. The stimulus-response mappings are unique and constant within each possible rule dimension.</skos:definition>
		<skos:prefLabel>Extradimensional shift task</skos:prefLabel>
		<skos:altLabel></skos:altLabel>
		<skos:related rdf:resource="http://cognitiveatlas.org/id/trm_4a3fd79d0ab65"/>
		<skos:related rdf:resource="http://cognitiveatlas.org/id/trm_4a3fd79d0b5fb"/>
		<skos:related rdf:resource="http://cognitiveatlas.org/id/tsk_4a57abb949ad7"/>
		<skos:related rdf:resource="http://cognitiveatlas.org/id/trm_4a3fd79d0b5fb"/>
		<skos:related rdf:resource="http://cognitiveatlas.org/id/trm_4a3fd79d0ab65"/>
		<skos:example>pattern recognition is measured by the contrast of average number of trials per pattern change trials in the Extradimensional shift task</skos:example>
		<skos:example>attention shifting is measured by the contrast of average number of trials per pattern change trials in the Extradimensional shift task</skos:example>
		<skos:example>Intradimensional shift task is related to Extradimensional shift task</skos:example>
		<skos:example>attention shifting is measured by the contrast of accuracy of subject minus average accuracy of controls trials in the Extradimensional shift task</skos:example>
		<skos:example>pattern recognition is measured by the contrast of accuracy of subject minus average accuracy of controls trials in the Extradimensional shift task</skos:example>
		<cito:citesForInformation rdf:resource="http://cognitiveatlas.org/citation/id/cit_4ded02531ead1"/>
		<cito:citesForInformation rdf:resource="http://cognitiveatlas.org/citation/id/cit_4ded02d39297e"/>
		<cito:citesForInformation rdf:resource="http://cognitiveatlas.org/citation/id/cit_4ded0357be770"/>
</skos:Concept><skos:Concept rdf:about="http://cognitiveatlas.org/id/tsk_4a57abb949a6a"> <dc:identifier>tsk_4a57abb949a6a</dc:identifier>
		<dc:Title>Cognitive Atlas : Lexicon : face n-back task</dc:Title>
		<dc:Description>RDF output for 'face n-back task'</dc:Description>
		<dc:Type>InteractiveResource</dc:Type>
		<dc:Publisher>Cognitive Atlas</dc:Publisher>
		<dc:Creator>Cognitive Atlas RDF Generator</dc:Creator>
		<dc:Contributor>Carinna Torgerson</dc:Contributor>
		<dc:Date>2011-06-06 10:39:51</dc:Date>
		<dc:Format>text/rdf</dc:Format>
		<dc:Language>en</dc:Language>
		<skos:editorialNote>Generated by testgen.php on Thu Jun 9 14:25:25 PDT 2011.</skos:editorialNote>
		<skos:historyNote>Revision 3: 2 previous definitions.</skos:historyNote>
		<skos:changeNote>See http://cognitiveatlas.org/id/tsk_4a57abb949a6a for complete revision history.</skos:changeNote>
		<skos:scopeNote>http://www.w3.org/2004/02/skos/core#Concept</skos:scopeNote>
		<skos:Note>SKOS properties defined in http://www.w3.org/TR/skos-primer/#secrel</skos:Note>
		<skos:inScheme rdf:resource="http://cognitiveatlas.org/tasks/"/>
		<skos:definition>Task in which face stimuli are presented one at a time in a continuous stream, and the objective is to detect when the current face matches the face presented n previously (1,2, or 3 faces before).</skos:definition>
		<skos:prefLabel>face n-back task</skos:prefLabel>
		<skos:altLabel></skos:altLabel>
		<skos:related rdf:resource="http://cognitiveatlas.org/id/trm_4a3fd79d0b65a"/>
		<skos:related rdf:resource="http://cognitiveatlas.org/id/trm_4a3fd79d0a30c"/>
		<skos:related rdf:resource="http://cognitiveatlas.org/id/trm_4a3fd79d0a300"/>
		<skos:related rdf:resource="http://cognitiveatlas.org/id/trm_4a3fd79d0b08f"/>
		<skos:related rdf:resource="http://cognitiveatlas.org/id/trm_4a3fd79d0b4d8"/>
		<skos:related rdf:resource="http://cognitiveatlas.org/id/trm_4a3fd79d0b4d8"/>
		<skos:related rdf:resource="http://cognitiveatlas.org/id/trm_4a3fd79d0b5a7"/>
		<skos:related rdf:resource="http://cognitiveatlas.org/id/trm_4a3fd79d0b5a7"/>
		<skos:related rdf:resource="http://cognitiveatlas.org/id/trm_4a3fd79d0ba6c"/>
		<skos:related rdf:resource="http://cognitiveatlas.org/id/trm_4a3fd79d0ba6c"/>
		<skos:related rdf:resource="http://cognitiveatlas.org/id/tsk_4a57abb949bcd"/>
		<skos:related rdf:resource="http://cognitiveatlas.org/id/tsk_4a57abb949df1"/>
		<skos:related rdf:resource="http://cognitiveatlas.org/id/tsk_4a57abb949b1c"/>
		<skos:example>face n-back task is descended from n-back task</skos:example>
		<skos:example>face n-back task is related to spatial n-back task</skos:example>
		<skos:example>face n-back task is related to letter n-back task</skos:example>
		<skos:example>emotion perception is measured by the contrast of emotion detection trials in the face n-back task</skos:example>
		<skos:example>face recognition is measured by the contrast of identity detection trials in the face n-back task</skos:example>
		<skos:example>face perception is measured by the contrast of identity detection trials in the face n-back task</skos:example>
		<skos:example>semantic working memory is measured by the contrast of emotion detection trials in the face n-back task</skos:example>
		<skos:example>visual working memory is measured by the contrast of emotion detection trials in the face n-back task</skos:example>
		<skos:example>visual working memory is measured by the contrast of identity detection trials in the face n-back task</skos:example>
		<skos:example>working memory is measured by the contrast of emotion detection trials in the face n-back task</skos:example>
		<skos:example>working memory is measured by the contrast of identity detection trials in the face n-back task</skos:example>
		<skos:example>working memory retrieval is measured by the contrast of emotion detection trials in the face n-back task</skos:example>
		<skos:example>working memory retrieval is measured by the contrast of identity detection trials in the face n-back task</skos:example>
		<cito:citesForInformation rdf:resource="http://cognitiveatlas.org/citation/id/cit_4ded0c34d377f"/>
		<cito:citesForInformation rdf:resource="http://cognitiveatlas.org/citation/id/cit_4ded116d8ddff"/>
		<cito:citesForInformation rdf:resource="http://cognitiveatlas.org/citation/id/cit_4ded12df97519"/>
</skos:Concept><skos:Concept rdf:about="http://cognitiveatlas.org/id/tsk_4a57abb949a78"> <dc:identifier>tsk_4a57abb949a78</dc:identifier>
		<dc:Title>Cognitive Atlas : Lexicon : Fagerstrom Test for Nicotine Dependence</dc:Title>
		<dc:Description>RDF output for 'Fagerstrom Test for Nicotine Dependence'</dc:Description>
		<dc:Type>InteractiveResource</dc:Type>
		<dc:Publisher>Cognitive Atlas</dc:Publisher>
		<dc:Creator>Cognitive Atlas RDF Generator</dc:Creator>
		<dc:Contributor>Brenda Gregory</dc:Contributor>
		<dc:Date>2011-04-28 17:27:56</dc:Date>
		<dc:Format>text/rdf</dc:Format>
		<dc:Language>en</dc:Language>
		<skos:editorialNote>Generated by testgen.php on Thu Jun 9 14:25:25 PDT 2011.</skos:editorialNote>
		<skos:historyNote>Revision 3: 2 previous definitions.</skos:historyNote>
		<skos:changeNote>See http://cognitiveatlas.org/id/tsk_4a57abb949a78 for complete revision history.</skos:changeNote>
		<skos:scopeNote>http://www.w3.org/2004/02/skos/core#Concept</skos:scopeNote>
		<skos:Note>SKOS properties defined in http://www.w3.org/TR/skos-primer/#secrel</skos:Note>
		<skos:inScheme rdf:resource="http://cognitiveatlas.org/tasks/"/>
		<skos:definition>a standard instrument for assessing the intensity of physical addiction to nicotine.</skos:definition>
		<skos:prefLabel>Fagerstrom Test for Nicotine Dependence</skos:prefLabel>
		<skos:altLabel></skos:altLabel>
		<cito:citesForInformation rdf:resource="http://cognitiveatlas.org/citation/id/cit_4ded1500b344e"/>
		<cito:citesForInformation rdf:resource="http://cognitiveatlas.org/citation/id/cit_4ded1e256fbe7"/>
		<cito:citesForInformation rdf:resource="http://cognitiveatlas.org/citation/id/cit_4ded1ed9369d8"/>
		<cito:citesForInformation rdf:resource="http://cognitiveatlas.org/citation/id/cit_4ded1f253ee49"/>
</skos:Concept><skos:Concept rdf:about="http://cognitiveatlas.org/id/tsk_4a57abb949a85"> <dc:identifier>tsk_4a57abb949a85</dc:identifier>
		<dc:Title>Cognitive Atlas : Lexicon : Forward digit span task</dc:Title>
		<dc:Description>RDF output for 'Forward digit span task'</dc:Description>
		<dc:Type>InteractiveResource</dc:Type>
		<dc:Publisher>Cognitive Atlas</dc:Publisher>
		<dc:Creator>Cognitive Atlas RDF Generator</dc:Creator>
		<dc:Contributor>Brenda Gregory</dc:Contributor>
		<dc:Date>2010-03-25 15:52:06</dc:Date>
		<dc:Format>text/rdf</dc:Format>
		<dc:Language>en</dc:Language>
		<skos:editorialNote>Generated by testgen.php on Thu Jun 9 14:25:25 PDT 2011.</skos:editorialNote>
		<skos:historyNote>Revision 2: 1 previous definitions.</skos:historyNote>
		<skos:changeNote>See http://cognitiveatlas.org/id/tsk_4a57abb949a85 for complete revision history.</skos:changeNote>
		<skos:scopeNote>http://www.w3.org/2004/02/skos/core#Concept</skos:scopeNote>
		<skos:Note>SKOS properties defined in http://www.w3.org/TR/skos-primer/#secrel</skos:Note>
		<skos:inScheme rdf:resource="http://cognitiveatlas.org/tasks/"/>
		<skos:definition>A method of short-term memory measurement in which a person listens to someone say a series of single-digit numbers and must repeat them back in the same order they were given.</skos:definition>
		<skos:prefLabel>Forward digit span task</skos:prefLabel>
		<skos:altLabel></skos:altLabel>
		<skos:related rdf:resource="http://cognitiveatlas.org/id/tsk_4a57abb94989b"/>
		<skos:related rdf:resource="http://cognitiveatlas.org/id/trm_4a3fd79d0ac9e"/>
		<skos:related rdf:resource="http://cognitiveatlas.org/id/trm_4a3fd79d0b5a7"/>
		<skos:related rdf:resource="http://cognitiveatlas.org/id/tsk_4a57abb949a0d"/>
		<skos:example>Forward digit span task is descended from Digit span task</skos:example>
		<skos:example>Backward digit span task is an exact synonym of Forward digit span task</skos:example>
		<skos:example>phonological working memory is measured by the contrast of length of longest correct sequence trials in the Forward digit span task</skos:example>
		<skos:example>working memory is measured by the contrast of length of longest correct sequence trials in the Forward digit span task</skos:example>
		<cito:citesForInformation rdf:resource="http://cognitiveatlas.org/citation/id/cit_4de575709967d"/>
</skos:Concept><skos:Concept rdf:about="http://cognitiveatlas.org/id/tsk_4a57abb949a93"> <dc:identifier>tsk_4a57abb949a93</dc:identifier>
		<dc:Title>Cognitive Atlas : Lexicon : Go/no-go task</dc:Title>
		<dc:Description>RDF output for 'Go/no-go task'</dc:Description>
		<dc:Type>InteractiveResource</dc:Type>
		<dc:Publisher>Cognitive Atlas</dc:Publisher>
		<dc:Creator>Cognitive Atlas RDF Generator</dc:Creator>
		<dc:Contributor>Agatha Lenartowicz</dc:Contributor>
		<dc:Date>2009-07-10 14:06:33</dc:Date>
		<dc:Format>text/rdf</dc:Format>
		<dc:Language>en</dc:Language>
		<skos:editorialNote>Generated by testgen.php on Thu Jun 9 14:25:25 PDT 2011.</skos:editorialNote>
		<skos:historyNote>No previous definition revisions.</skos:historyNote>
		<skos:changeNote>This is the first and only definition provided.</skos:changeNote>
		<skos:scopeNote>http://www.w3.org/2004/02/skos/core#Concept</skos:scopeNote>
		<skos:Note>SKOS properties defined in http://www.w3.org/TR/skos-primer/#secrel</skos:Note>
		<skos:inScheme rdf:resource="http://cognitiveatlas.org/tasks/"/>
		<skos:definition>A task in which stimuli are presented in a continuous stream and participants perform a binary decision on each stimulus. One of the outcomes requires participants to make a motor response (go), whereas the other requires participants to withhold a response (no-go). Accuracy and reaction time are measured for each event. Go events typically occur with higher frequency than no-go events. </skos:definition>
		<skos:prefLabel>Go/no-go task</skos:prefLabel>
		<skos:altLabel></skos:altLabel>
		<skos:related rdf:resource="http://cognitiveatlas.org/id/trm_4a3fd79d0af66"/>
		<skos:related rdf:resource="http://cognitiveatlas.org/id/trm_4b7c270940f9d"/>
		<skos:related rdf:resource="http://cognitiveatlas.org/id/trm_4a3fd79d0a613"/>
		<skos:example>response inhibition is measured by the contrast of Stop trial trials in the Go/no-go task</skos:example>
		<skos:example>behavioral inhibition (cognitive) is measured by the contrast of stop minus go trials in the Go/no-go task</skos:example>
		<skos:example>inhibition is measured by the contrast of Stop trial trials in the Go/no-go task</skos:example>
		<cito:citesForInformation rdf:resource="http://cognitiveatlas.org/citation/id/cit_4ded4d890aeb6"/>
		<cito:citesForInformation rdf:resource="http://cognitiveatlas.org/citation/id/cit_4ded4db7342f2"/>
		<cito:citesForInformation rdf:resource="http://cognitiveatlas.org/citation/id/cit_4ded4defe2990"/>
</skos:Concept><skos:Concept rdf:about="http://cognitiveatlas.org/id/tsk_4a57abb949aa1"> <dc:identifier>tsk_4a57abb949aa1</dc:identifier>
		<dc:Title>Cognitive Atlas : Lexicon : Gray Oral Reading Test - 4</dc:Title>
		<dc:Description>RDF output for 'Gray Oral Reading Test - 4'</dc:Description>
		<dc:Type>InteractiveResource</dc:Type>
		<dc:Publisher>Cognitive Atlas</dc:Publisher>
		<dc:Creator>Cognitive Atlas RDF Generator</dc:Creator>
		<dc:Contributor>Brenda Gregory</dc:Contributor>
		<dc:Date>2011-05-16 11:23:19</dc:Date>
		<dc:Format>text/rdf</dc:Format>
		<dc:Language>en</dc:Language>
		<skos:editorialNote>Generated by testgen.php on Thu Jun 9 14:25:25 PDT 2011.</skos:editorialNote>
		<skos:historyNote>Revision 4: 3 previous definitions.</skos:historyNote>
		<skos:changeNote>See http://cognitiveatlas.org/id/tsk_4a57abb949aa1 for complete revision history.</skos:changeNote>
		<skos:scopeNote>http://www.w3.org/2004/02/skos/core#Concept</skos:scopeNote>
		<skos:Note>SKOS properties defined in http://www.w3.org/TR/skos-primer/#secrel</skos:Note>
		<skos:inScheme rdf:resource="http://cognitiveatlas.org/tasks/"/>
		<skos:definition>measures growth in oral reading and aids in the diagnosis of oral reading difficulties. Five scores provide information on oral reading skills in terms of: Rate, accuracy, fluency, comprehension, overall reading ability, and comprehension. The test consists of two parallel forms, each containing 14 developmentally sequenced reading passages with five comprehension questions following each passage.</skos:definition>
		<skos:prefLabel>Gray Oral Reading Test - 4</skos:prefLabel>
		<skos:altLabel></skos:altLabel>
		<skos:related rdf:resource="http://cognitiveatlas.org/id/trm_4a3fd79d0aeb6"/>
		<skos:related rdf:resource="http://cognitiveatlas.org/id/trm_4a3fd79d09bbf"/>
		<skos:related rdf:resource="http://cognitiveatlas.org/id/trm_4a3fd79d0a775"/>
		<skos:example>reading is measured by the contrast of sum of rate, accuracy, fluency, and comprehension scaled scores trials in the Gray Oral Reading Test - 4</skos:example>
		<skos:example>binocular vision is measured by the contrast of sum of rate, accuracy, fluency, and comprehension scaled scores trials in the Gray Oral Reading Test - 4</skos:example>
		<skos:example>language comprehension is measured by the contrast of sum of rate, accuracy, fluency, and comprehension scaled scores trials in the Gray Oral Reading Test - 4</skos:example>
		<cito:citesForInformation rdf:resource="http://cognitiveatlas.org/citation/id/cit_4ded57332dc2d"/>
		<cito:citesForInformation rdf:resource="http://cognitiveatlas.org/citation/id/cit_4ded57b5106eb"/>
</skos:Concept><skos:Concept rdf:about="http://cognitiveatlas.org/id/tsk_4a57abb949aae"> <dc:identifier>tsk_4a57abb949aae</dc:identifier>
		<dc:Title>Cognitive Atlas : Lexicon : Hooper Visual Organization Test</dc:Title>
		<dc:Description>RDF output for 'Hooper Visual Organization Test'</dc:Description>
		<dc:Type>InteractiveResource</dc:Type>
		<dc:Publisher>Cognitive Atlas</dc:Publisher>
		<dc:Creator>Cognitive Atlas RDF Generator</dc:Creator>
		<dc:Contributor>Naomi Kenner</dc:Contributor>
		<dc:Date>2009-07-10 14:06:33</dc:Date>
		<dc:Format>text/rdf</dc:Format>
		<dc:Language>en</dc:Language>
		<skos:editorialNote>Generated by testgen.php on Thu Jun 9 14:25:25 PDT 2011.</skos:editorialNote>
		<skos:historyNote>No previous definition revisions.</skos:historyNote>
		<skos:changeNote>This is the first and only definition provided.</skos:changeNote>
		<skos:scopeNote>http://www.w3.org/2004/02/skos/core#Concept</skos:scopeNote>
		<skos:Note>SKOS properties defined in http://www.w3.org/TR/skos-primer/#secrel</skos:Note>
		<skos:inScheme rdf:resource="http://cognitiveatlas.org/tasks/"/>
		<skos:definition>a neuropsychological test of visual spatial ability that presents participants with a line drawing of a common object that has been broken into fragments, and asks participants to name what the object would be if reassembled.</skos:definition>
		<skos:prefLabel>Hooper Visual Organization Test</skos:prefLabel>
		<skos:altLabel></skos:altLabel>
		<skos:related rdf:resource="http://cognitiveatlas.org/id/trm_4b82c75498408"/>
		<skos:related rdf:resource="http://cognitiveatlas.org/id/trm_4a3fd79d0aaa4"/>
		<skos:related rdf:resource="http://cognitiveatlas.org/id/trm_4a3fd79d0b4a9"/>
		<skos:related rdf:resource="http://cognitiveatlas.org/id/trm_4a3fd79d0b9ad"/>
		<skos:example>Central Coherence is measured by the contrast of accuracy trials in the Hooper Visual Organization Test</skos:example>
		<skos:example>object perception is measured by the contrast of accuracy trials in the Hooper Visual Organization Test</skos:example>
		<skos:example>visual object recognition is measured by the contrast of accuracy trials in the Hooper Visual Organization Test</skos:example>
		<skos:example>feature detection is measured by the contrast of accuracy trials in the Hooper Visual Organization Test</skos:example>
		<cito:citesForInformation rdf:resource="http://cognitiveatlas.org/citation/id/cit_4ded5aa586b91"/>
		<cito:citesForInformation rdf:resource="http://cognitiveatlas.org/citation/id/cit_4ded60908fe9f"/>
</skos:Concept><skos:Concept rdf:about="http://cognitiveatlas.org/id/tsk_4a57abb949abc"> <dc:identifier>tsk_4a57abb949abc</dc:identifier>
		<dc:Title>Cognitive Atlas : Lexicon : immediate recall test</dc:Title>
		<dc:Description>RDF output for 'immediate recall test'</dc:Description>
		<dc:Type>InteractiveResource</dc:Type>
		<dc:Publisher>Cognitive Atlas</dc:Publisher>
		<dc:Creator>Cognitive Atlas RDF Generator</dc:Creator>
		<dc:Contributor>Natalie Picchetti</dc:Contributor>
		<dc:Date>2011-03-04 12:55:55</dc:Date>
		<dc:Format>text/rdf</dc:Format>
		<dc:Language>en</dc:Language>
		<skos:editorialNote>Generated by testgen.php on Thu Jun 9 14:25:25 PDT 2011.</skos:editorialNote>
		<skos:historyNote>Revision 2: 1 previous definitions.</skos:historyNote>
		<skos:changeNote>See http://cognitiveatlas.org/id/tsk_4a57abb949abc for complete revision history.</skos:changeNote>
		<skos:scopeNote>http://www.w3.org/2004/02/skos/core#Concept</skos:scopeNote>
		<skos:Note>SKOS properties defined in http://www.w3.org/TR/skos-primer/#secrel</skos:Note>
		<skos:inScheme rdf:resource="http://cognitiveatlas.org/tasks/"/>
		<skos:definition>involves presenting a subject with material that is to be memorized.  Once the material is removed the subject is to immediately demonstrate everything that they remember from the material.

</skos:definition>
		<skos:prefLabel>immediate recall test</skos:prefLabel>
		<skos:altLabel></skos:altLabel>
		<skos:related rdf:resource="http://cognitiveatlas.org/id/trm_4a3fd79d0b5a7"/>
		<skos:related rdf:resource="http://cognitiveatlas.org/id/trm_4a3fd79d0ba6c"/>
		<skos:related rdf:resource="http://cognitiveatlas.org/id/trm_4a3fd79d0a04f"/>
		<skos:related rdf:resource="http://cognitiveatlas.org/id/trm_4da63357e4999"/>
		<skos:example>immediate recall test is descended from Wechsler Memory Scale (revised)</skos:example>
		<skos:example>working memory is measured by the contrast of number or percentage of words remembered trials in the immediate recall test</skos:example>
		<skos:example>working memory retrieval is measured by the contrast of number or percentage of words remembered trials in the immediate recall test</skos:example>
		<skos:example>declarative memory is measured by the contrast of number or percentage of words remembered trials in the immediate recall test</skos:example>
		<cito:citesForInformation rdf:resource="http://cognitiveatlas.org/citation/id/cit_4dee5e76d4914"/>
		<cito:citesForInformation rdf:resource="http://cognitiveatlas.org/citation/id/cit_4dee5f971af95"/>
		<cito:citesForInformation rdf:resource="http://cognitiveatlas.org/citation/id/cit_4dee6011c4cdc"/>
</skos:Concept><skos:Concept rdf:about="http://cognitiveatlas.org/id/tsk_4a57abb949aca"> <dc:identifier>tsk_4a57abb949aca</dc:identifier>
		<dc:Title>Cognitive Atlas : Lexicon : International Affective Picture System</dc:Title>
		<dc:Description>RDF output for 'International Affective Picture System'</dc:Description>
		<dc:Type>InteractiveResource</dc:Type>
		<dc:Publisher>Cognitive Atlas</dc:Publisher>
		<dc:Creator>Cognitive Atlas RDF Generator</dc:Creator>
		<dc:Contributor>Brenda Gregory</dc:Contributor>
		<dc:Date>2011-05-10 14:46:45</dc:Date>
		<dc:Format>text/rdf</dc:Format>
		<dc:Language>en</dc:Language>
		<skos:editorialNote>Generated by testgen.php on Thu Jun 9 14:25:25 PDT 2011.</skos:editorialNote>
		<skos:historyNote>Revision 3: 2 previous definitions.</skos:historyNote>
		<skos:changeNote>See http://cognitiveatlas.org/id/tsk_4a57abb949aca for complete revision history.</skos:changeNote>
		<skos:scopeNote>http://www.w3.org/2004/02/skos/core#Concept</skos:scopeNote>
		<skos:Note>SKOS properties defined in http://www.w3.org/TR/skos-primer/#secrel</skos:Note>
		<skos:inScheme rdf:resource="http://cognitiveatlas.org/tasks/"/>
		<skos:definition>a database of photographs used in emotion research.</skos:definition>
		<skos:prefLabel>International Affective Picture System</skos:prefLabel>
		<skos:altLabel></skos:altLabel>
		<skos:related rdf:resource="http://cognitiveatlas.org/id/trm_4a3fd79d0b65a"/>
		<skos:example>emotion perception is measured by the contrast of arousal in response to picture minus baseline arousal trials in the International Affective Picture System</skos:example>
		<cito:citesForInformation rdf:resource="http://cognitiveatlas.org/citation/id/cit_4dee84ea9e443"/>
		<cito:citesForInformation rdf:resource="http://cognitiveatlas.org/citation/id/cit_4deeb0ea55189"/>
		<cito:citesForInformation rdf:resource="http://cognitiveatlas.org/citation/id/cit_4deeb25602cb2"/>
</skos:Concept><skos:Concept rdf:about="http://cognitiveatlas.org/id/tsk_4a57abb949ad7"> <dc:identifier>tsk_4a57abb949ad7</dc:identifier>
		<dc:Title>Cognitive Atlas : Lexicon : Intradimensional shift task</dc:Title>
		<dc:Description>RDF output for 'Intradimensional shift task'</dc:Description>
		<dc:Type>InteractiveResource</dc:Type>
		<dc:Publisher>Cognitive Atlas</dc:Publisher>
		<dc:Creator>Cognitive Atlas RDF Generator</dc:Creator>
		<dc:Contributor>Agatha Lenartowicz</dc:Contributor>
		<dc:Date>2009-07-10 14:06:33</dc:Date>
		<dc:Format>text/rdf</dc:Format>
		<dc:Language>en</dc:Language>
		<skos:editorialNote>Generated by testgen.php on Thu Jun 9 14:25:25 PDT 2011.</skos:editorialNote>
		<skos:historyNote>No previous definition revisions.</skos:historyNote>
		<skos:changeNote>This is the first and only definition provided.</skos:changeNote>
		<skos:scopeNote>http://www.w3.org/2004/02/skos/core#Concept</skos:scopeNote>
		<skos:Note>SKOS properties defined in http://www.w3.org/TR/skos-primer/#secrel</skos:Note>
		<skos:inScheme rdf:resource="http://cognitiveatlas.org/tasks/"/>
		<skos:definition>A task in which multiple (typically two) stimuli are presented simultaneously and the subject must select the stimulus that matches the currently relevant rule. The rule represents the relevant task &#34;dimension&#34;. The stimulus-response mappings within this dimension alternate or &#34;shift&#34; among multiple (typically two) alternatives. </skos:definition>
		<skos:prefLabel>Intradimensional shift task</skos:prefLabel>
		<skos:altLabel></skos:altLabel>
		<skos:related rdf:resource="http://cognitiveatlas.org/id/trm_4a3fd79d0ab65"/>
		<skos:related rdf:resource="http://cognitiveatlas.org/id/trm_4a3fd79d0b5fb"/>
		<skos:related rdf:resource="http://cognitiveatlas.org/id/tsk_4a57abb949a5d"/>
		<skos:related rdf:resource="http://cognitiveatlas.org/id/tsk_4a57abb949f21"/>
		<skos:example>Intradimensional shift task is related to Extradimensional shift task</skos:example>
		<skos:example>Intradimensional shift task is a broader synonym of Wisconsin Card Sorting test</skos:example>
		<skos:example>pattern recognition is measured by the contrast of accuracy of subject minus average accuracy of controls trials in the Intradimensional shift task</skos:example>
		<skos:example>attention shifting is measured by the contrast of accuracy of subject minus average accuracy of controls trials in the Intradimensional shift task</skos:example>
		<cito:citesForInformation rdf:resource="http://cognitiveatlas.org/citation/id/cit_4ded02531ead1"/>
		<cito:citesForInformation rdf:resource="http://cognitiveatlas.org/citation/id/cit_4df107788dc80"/>
		<cito:citesForInformation rdf:resource="http://cognitiveatlas.org/citation/id/cit_4df1081c042e8"/>
</skos:Concept><skos:Concept rdf:about="http://cognitiveatlas.org/id/tsk_4a57abb949ae5"> <dc:identifier>tsk_4a57abb949ae5</dc:identifier>
		<dc:Title>Cognitive Atlas : Lexicon : Iowa Gambling Task</dc:Title>
		<dc:Description>RDF output for 'Iowa Gambling Task'</dc:Description>
		<dc:Type>InteractiveResource</dc:Type>
		<dc:Publisher>Cognitive Atlas</dc:Publisher>
		<dc:Creator>Cognitive Atlas RDF Generator</dc:Creator>
		<dc:Contributor>Tom Schonberg</dc:Contributor>
		<dc:Date>2011-02-11 12:25:41</dc:Date>
		<dc:Format>text/rdf</dc:Format>
		<dc:Language>en</dc:Language>
		<skos:editorialNote>Generated by testgen.php on Thu Jun 9 14:25:25 PDT 2011.</skos:editorialNote>
		<skos:historyNote>Revision 3: 2 previous definitions.</skos:historyNote>
		<skos:changeNote>See http://cognitiveatlas.org/id/tsk_4a57abb949ae5 for complete revision history.</skos:changeNote>
		<skos:scopeNote>http://www.w3.org/2004/02/skos/core#Concept</skos:scopeNote>
		<skos:Note>SKOS properties defined in http://www.w3.org/TR/skos-primer/#secrel</skos:Note>
		<skos:inScheme rdf:resource="http://cognitiveatlas.org/tasks/"/>
		<skos:definition>a widely used experiment in the areas of cognition &amp; emotion that was originally developed to assist in detecting decision-making impairment in patients with prefrontal cortex damage; a computerized experiment that is carried out in real time and resembles real-world contingencies. The task allows participants to select cards from four decks displayed on-screen. Participants are instructed that the selection of each card will result in winning or losing money. The objective is to attempt to win as much money as possible. (from http://iowagamblingtask.com/)

On each trial, participants select a card from one of four decks; two ‘bad’ decks offer a higher reward on most trials but also higher possible loss and lower overall expected value, whereas two ‘good’ decks offer a lower reward on most trials but lower possible loss and higher expected value. Participants learn the nature of the decks through trial-and- error. In some versions of the task, the probabilities are not stationary.</skos:definition>
		<skos:prefLabel>Iowa Gambling Task</skos:prefLabel>
		<skos:altLabel></skos:altLabel>
		<skos:related rdf:resource="http://cognitiveatlas.org/id/trm_4d54b2cc0f943"/>
		<skos:related rdf:resource="http://cognitiveatlas.org/id/trm_4a3fd79d0b64e"/>
		<skos:related rdf:resource="http://cognitiveatlas.org/id/trm_4d55a2bbcfdff"/>
		<skos:example>Iowa Gambling Task is a narrower synonym of Choice task between risky and non-risky options</skos:example>
		<skos:example>Cambridge Gambling Task is related to Iowa Gambling Task</skos:example>
		<skos:example>risk seeking is measured by the contrast of accuracy of subject minus average accuracy of controls trials in the Iowa Gambling Task</skos:example>
		<cito:citesForInformation rdf:resource="http://cognitiveatlas.org/citation/id/cit_4d559af0468e0"/>
		<cito:citesForInformation rdf:resource="http://cognitiveatlas.org/citation/id/cit_4d559b7391b2f"/>
		<cito:citesForInformation rdf:resource="http://cognitiveatlas.org/citation/id/cit_4df10ba550665"/>
</skos:Concept><skos:Concept rdf:about="http://cognitiveatlas.org/id/tsk_4a57abb949af3"> <dc:identifier>tsk_4a57abb949af3</dc:identifier>
		<dc:Title>Cognitive Atlas : Lexicon : Ishihara plates for color blindness</dc:Title>
		<dc:Description>RDF output for 'Ishihara plates for color blindness'</dc:Description>
		<dc:Type>InteractiveResource</dc:Type>
		<dc:Publisher>Cognitive Atlas</dc:Publisher>
		<dc:Creator>Cognitive Atlas RDF Generator</dc:Creator>
		<dc:Contributor>Brenda Gregory</dc:Contributor>
		<dc:Date>2011-04-28 16:07:09</dc:Date>
		<dc:Format>text/rdf</dc:Format>
		<dc:Language>en</dc:Language>
		<skos:editorialNote>Generated by testgen.php on Thu Jun 9 14:25:25 PDT 2011.</skos:editorialNote>
		<skos:historyNote>Revision 3: 2 previous definitions.</skos:historyNote>
		<skos:changeNote>See http://cognitiveatlas.org/id/tsk_4a57abb949af3 for complete revision history.</skos:changeNote>
		<skos:scopeNote>http://www.w3.org/2004/02/skos/core#Concept</skos:scopeNote>
		<skos:Note>SKOS properties defined in http://www.w3.org/TR/skos-primer/#secrel</skos:Note>
		<skos:inScheme rdf:resource="http://cognitiveatlas.org/tasks/"/>
		<skos:definition>a test for red-green color deficiencies that consists of a number of colored plates, called Ishihara plates, each of which contain a circle of dots appearing randomized in color and size. Within the pattern are dots which form a number visible to those with normal color vision and invisible, or difficult to see, for those with a red-green color vision defect.</skos:definition>
		<skos:prefLabel>Ishihara plates for color blindness</skos:prefLabel>
		<skos:altLabel></skos:altLabel>
		<skos:related rdf:resource="http://cognitiveatlas.org/id/trm_4a3fd79d09d93"/>
		<skos:example>color perception is measured by the contrast of number of plates read correctly by controls with normal color vision minus number of plates read correctly by subject trials in the Ishihara plates for color blindness</skos:example>
		<cito:citesForInformation rdf:resource="http://cognitiveatlas.org/citation/id/cit_4df114bf31698"/>
		<cito:citesForInformation rdf:resource="http://cognitiveatlas.org/citation/id/cit_4df11508648d7"/>
</skos:Concept><skos:Concept rdf:about="http://cognitiveatlas.org/id/tsk_4a57abb949b00"> <dc:identifier>tsk_4a57abb949b00</dc:identifier>
		<dc:Title>Cognitive Atlas : Lexicon : Kanizsa figures</dc:Title>
		<dc:Description>RDF output for 'Kanizsa figures'</dc:Description>
		<dc:Type>InteractiveResource</dc:Type>
		<dc:Publisher>Cognitive Atlas</dc:Publisher>
		<dc:Creator>Cognitive Atlas RDF Generator</dc:Creator>
		<dc:Contributor>Brenda Gregory</dc:Contributor>
		<dc:Date>2011-05-16 15:44:40</dc:Date>
		<dc:Format>text/rdf</dc:Format>
		<dc:Language>en</dc:Language>
		<skos:editorialNote>Generated by testgen.php on Thu Jun 9 14:25:25 PDT 2011.</skos:editorialNote>
		<skos:historyNote>Revision 3: 2 previous definitions.</skos:historyNote>
		<skos:changeNote>See http://cognitiveatlas.org/id/tsk_4a57abb949b00 for complete revision history.</skos:changeNote>
		<skos:scopeNote>http://www.w3.org/2004/02/skos/core#Concept</skos:scopeNote>
		<skos:Note>SKOS properties defined in http://www.w3.org/TR/skos-primer/#secrel</skos:Note>
		<skos:inScheme rdf:resource="http://cognitiveatlas.org/tasks/"/>
		<skos:definition>An ambiguous figure in which the illusory contour of a square (or triangle) appears in the middle of four (or three) truncated solid squares (or circles). It is an illustration of the perceptual ability to make sense of an incomplete figure by creating a &#39;whole&#39; image from the separate elements (Gestalt organization).</skos:definition>
		<skos:prefLabel>Kanizsa figures</skos:prefLabel>
		<skos:altLabel></skos:altLabel>
		<skos:related rdf:resource="http://cognitiveatlas.org/id/trm_4a3fd79d0b1a6"/>
		<skos:related rdf:resource="http://cognitiveatlas.org/id/trm_4a3fd79d0ab88"/>
		<skos:related rdf:resource="http://cognitiveatlas.org/id/trm_4a3fd79d0b9c5"/>
		<skos:related rdf:resource="http://cognitiveatlas.org/id/trm_4a3fd79d0b9c5"/>
		<skos:example>spatial ability is measured by the contrast of accuracy of participant minus average accuracy of controls trials in the Kanizsa figures</skos:example>
		<skos:example>perceptual binding is measured by the contrast of reaction time to figures minus reaction time to Kanizsa figures trials in the Kanizsa figures</skos:example>
		<skos:example>figure ground relations is measured by the contrast of reaction time to figures minus reaction time to Kanizsa figures trials in the Kanizsa figures</skos:example>
		<skos:example>figure ground relations is measured by the contrast of accuracy of participant minus average accuracy of controls trials in the Kanizsa figures</skos:example>
		<cito:citesForInformation rdf:resource="http://cognitiveatlas.org/citation/id/cit_4df12ffac3c10"/>
		<cito:citesForInformation rdf:resource="http://cognitiveatlas.org/citation/id/cit_4df1318cdbaf1"/>
		<cito:citesForInformation rdf:resource="http://cognitiveatlas.org/citation/id/cit_4df131e0b8a48"/>
		<cito:citesForInformation rdf:resource="http://cognitiveatlas.org/citation/id/cit_4df132ea6863d"/>
</skos:Concept><skos:Concept rdf:about="http://cognitiveatlas.org/id/tsk_4a57abb949b0e"> <dc:identifier>tsk_4a57abb949b0e</dc:identifier>
		<dc:Title>Cognitive Atlas : Lexicon : letter fluency test </dc:Title>
		<dc:Description>RDF output for 'letter fluency test '</dc:Description>
		<dc:Type>InteractiveResource</dc:Type>
		<dc:Publisher>Cognitive Atlas</dc:Publisher>
		<dc:Creator>Cognitive Atlas RDF Generator</dc:Creator>
		<dc:Contributor>Natalie Picchetti</dc:Contributor>
		<dc:Date>2011-04-18 11:42:37</dc:Date>
		<dc:Format>text/rdf</dc:Format>
		<dc:Language>en</dc:Language>
		<skos:editorialNote>Generated by testgen.php on Thu Jun 9 14:25:25 PDT 2011.</skos:editorialNote>
		<skos:historyNote>Revision 3: 2 previous definitions.</skos:historyNote>
		<skos:changeNote>See http://cognitiveatlas.org/id/tsk_4a57abb949b0e for complete revision history.</skos:changeNote>
		<skos:scopeNote>http://www.w3.org/2004/02/skos/core#Concept</skos:scopeNote>
		<skos:Note>SKOS properties defined in http://www.w3.org/TR/skos-primer/#secrel</skos:Note>
		<skos:inScheme rdf:resource="http://cognitiveatlas.org/tasks/"/>
		<skos:definition>is a test that requires generation of words cued with a specific letter and depends on phonemic abilities.
</skos:definition>
		<skos:prefLabel>letter fluency test </skos:prefLabel>
		<skos:altLabel></skos:altLabel>
		<cito:citesForInformation rdf:resource="http://cognitiveatlas.org/citation/id/cit_4dac85c619a65"/>
</skos:Concept><skos:Concept rdf:about="http://cognitiveatlas.org/id/tsk_4a57abb949b1c"> <dc:identifier>tsk_4a57abb949b1c</dc:identifier>
		<dc:Title>Cognitive Atlas : Lexicon : letter n-back task</dc:Title>
		<dc:Description>RDF output for 'letter n-back task'</dc:Description>
		<dc:Type>InteractiveResource</dc:Type>
		<dc:Publisher>Cognitive Atlas</dc:Publisher>
		<dc:Creator>Cognitive Atlas RDF Generator</dc:Creator>
		<dc:Contributor>Agatha Lenartowicz</dc:Contributor>
		<dc:Date>2009-07-10 14:06:33</dc:Date>
		<dc:Format>text/rdf</dc:Format>
		<dc:Language>en</dc:Language>
		<skos:editorialNote>Generated by testgen.php on Thu Jun 9 14:25:25 PDT 2011.</skos:editorialNote>
		<skos:historyNote>No previous definition revisions.</skos:historyNote>
		<skos:changeNote>This is the first and only definition provided.</skos:changeNote>
		<skos:scopeNote>http://www.w3.org/2004/02/skos/core#Concept</skos:scopeNote>
		<skos:Note>SKOS properties defined in http://www.w3.org/TR/skos-primer/#secrel</skos:Note>
		<skos:inScheme rdf:resource="http://cognitiveatlas.org/tasks/"/>
		<skos:definition>A task in which participants view a continuous stream of letter stimuli. The object of the task is to identify letter repetitions that occur n-trials preceding to the current stimulus.</skos:definition>
		<skos:prefLabel>letter n-back task</skos:prefLabel>
		<skos:altLabel></skos:altLabel>
		<skos:related rdf:resource="http://cognitiveatlas.org/id/tsk_4a57abb949a6a"/>
		<skos:related rdf:resource="http://cognitiveatlas.org/id/tsk_4a57abb949bcd"/>
		<skos:example>letter n-back task is descended from n-back task</skos:example>
		<skos:example>face n-back task is related to letter n-back task</skos:example>
</skos:Concept><skos:Concept rdf:about="http://cognitiveatlas.org/id/tsk_4a57abb949b2b"> <dc:identifier>tsk_4a57abb949b2b</dc:identifier>
		<dc:Title>Cognitive Atlas : Lexicon : Letter naming task</dc:Title>
		<dc:Description>RDF output for 'Letter naming task'</dc:Description>
		<dc:Type>InteractiveResource</dc:Type>
		<dc:Publisher>Cognitive Atlas</dc:Publisher>
		<dc:Creator>Cognitive Atlas RDF Generator</dc:Creator>
		<dc:Contributor>System Administrator</dc:Contributor>
		<dc:Date>2009-07-10 14:06:33</dc:Date>
		<dc:Format>text/rdf</dc:Format>
		<dc:Language>en</dc:Language>
		<skos:editorialNote>Generated by testgen.php on Thu Jun 9 14:25:25 PDT 2011.</skos:editorialNote>
		<skos:historyNote>No previous definition revisions.</skos:historyNote>
		<skos:changeNote>This is the first and only definition provided.</skos:changeNote>
		<skos:scopeNote>http://www.w3.org/2004/02/skos/core#Concept</skos:scopeNote>
		<skos:Note>SKOS properties defined in http://www.w3.org/TR/skos-primer/#secrel</skos:Note>
		<skos:inScheme rdf:resource="http://cognitiveatlas.org/tasks/"/>
		<skos:definition>No definition submitted yet</skos:definition>
		<skos:prefLabel>Letter naming task</skos:prefLabel>
		<skos:altLabel></skos:altLabel>
</skos:Concept><skos:Concept rdf:about="http://cognitiveatlas.org/id/tsk_4a57abb949b38"> <dc:identifier>tsk_4a57abb949b38</dc:identifier>
		<dc:Title>Cognitive Atlas : Lexicon : Lexical decision task</dc:Title>
		<dc:Description>RDF output for 'Lexical decision task'</dc:Description>
		<dc:Type>InteractiveResource</dc:Type>
		<dc:Publisher>Cognitive Atlas</dc:Publisher>
		<dc:Creator>Cognitive Atlas RDF Generator</dc:Creator>
		<dc:Contributor>Brenda Gregory</dc:Contributor>
		<dc:Date>2011-05-16 15:53:08</dc:Date>
		<dc:Format>text/rdf</dc:Format>
		<dc:Language>en</dc:Language>
		<skos:editorialNote>Generated by testgen.php on Thu Jun 9 14:25:25 PDT 2011.</skos:editorialNote>
		<skos:historyNote>Revision 3: 2 previous definitions.</skos:historyNote>
		<skos:changeNote>See http://cognitiveatlas.org/id/tsk_4a57abb949b38 for complete revision history.</skos:changeNote>
		<skos:scopeNote>http://www.w3.org/2004/02/skos/core#Concept</skos:scopeNote>
		<skos:Note>SKOS properties defined in http://www.w3.org/TR/skos-primer/#secrel</skos:Note>
		<skos:inScheme rdf:resource="http://cognitiveatlas.org/tasks/"/>
		<skos:definition>a procedure used in many psychology and psycholinguistics experiments; the basic procedure involves measuring how quickly people classify stimuli as words or nonwords.  Subjects are presented, either visually or auditorily, with a mixture of words and pseudowords (nonsense strings that respect the phonotactic rules of a language, like trud in English). Their task is to indicate, usually with a button-press, whether the presented stimulus is a word or not.</skos:definition>
		<skos:prefLabel>Lexical decision task</skos:prefLabel>
		<skos:altLabel></skos:altLabel>
</skos:Concept><skos:Concept rdf:about="http://cognitiveatlas.org/id/tsk_4a57abb949b46"> <dc:identifier>tsk_4a57abb949b46</dc:identifier>
		<dc:Title>Cognitive Atlas : Lexicon : matching pennies game </dc:Title>
		<dc:Description>RDF output for 'matching pennies game '</dc:Description>
		<dc:Type>InteractiveResource</dc:Type>
		<dc:Publisher>Cognitive Atlas</dc:Publisher>
		<dc:Creator>Cognitive Atlas RDF Generator</dc:Creator>
		<dc:Contributor>Brenda Gregory</dc:Contributor>
		<dc:Date>2011-05-18 14:03:40</dc:Date>
		<dc:Format>text/rdf</dc:Format>
		<dc:Language>en</dc:Language>
		<skos:editorialNote>Generated by testgen.php on Thu Jun 9 14:25:25 PDT 2011.</skos:editorialNote>
		<skos:historyNote>Revision 3: 2 previous definitions.</skos:historyNote>
		<skos:changeNote>See http://cognitiveatlas.org/id/tsk_4a57abb949b46 for complete revision history.</skos:changeNote>
		<skos:scopeNote>http://www.w3.org/2004/02/skos/core#Concept</skos:scopeNote>
		<skos:Note>SKOS properties defined in http://www.w3.org/TR/skos-primer/#secrel</skos:Note>
		<skos:inScheme rdf:resource="http://cognitiveatlas.org/tasks/"/>
		<skos:definition>The game is played between two players, Player A and Player B. Each player has a penny and must secretly turn the penny to heads or tails. The players then reveal their choices simultaneously. If the pennies match (both heads or both tails), Player A receives one dollar from Player B (+1 for A, -1 for B). If the pennies do not match (one heads and one tails), Player B receives one dollar from Player A (-1 for A, +1 for B). This is an example of a zero-sum game, where one player&#39;s gain is exactly equal to the other player&#39;s loss.</skos:definition>
		<skos:prefLabel>matching pennies game </skos:prefLabel>
		<skos:altLabel></skos:altLabel>
</skos:Concept><skos:Concept rdf:about="http://cognitiveatlas.org/id/tsk_4a57abb949b54"> <dc:identifier>tsk_4a57abb949b54</dc:identifier>
		<dc:Title>Cognitive Atlas : Lexicon : Maudsley Obsessive Compulsive Inventory</dc:Title>
		<dc:Description>RDF output for 'Maudsley Obsessive Compulsive Inventory'</dc:Description>
		<dc:Type>InteractiveResource</dc:Type>
		<dc:Publisher>Cognitive Atlas</dc:Publisher>
		<dc:Creator>Cognitive Atlas RDF Generator</dc:Creator>
		<dc:Contributor>Brenda Gregory</dc:Contributor>
		<dc:Date>2011-04-28 16:09:27</dc:Date>
		<dc:Format>text/rdf</dc:Format>
		<dc:Language>en</dc:Language>
		<skos:editorialNote>Generated by testgen.php on Thu Jun 9 14:25:25 PDT 2011.</skos:editorialNote>
		<skos:historyNote>Revision 3: 2 previous definitions.</skos:historyNote>
		<skos:changeNote>See http://cognitiveatlas.org/id/tsk_4a57abb949b54 for complete revision history.</skos:changeNote>
		<skos:scopeNote>http://www.w3.org/2004/02/skos/core#Concept</skos:scopeNote>
		<skos:Note>SKOS properties defined in http://www.w3.org/TR/skos-primer/#secrel</skos:Note>
		<skos:inScheme rdf:resource="http://cognitiveatlas.org/tasks/"/>
		<skos:definition>assess obsessive-compulsive symptoms in the areas of contamination fears and washing behaviors, checking, and worries using 30 dichotomously scored (true/false) items. </skos:definition>
		<skos:prefLabel>Maudsley Obsessive Compulsive Inventory</skos:prefLabel>
		<skos:altLabel></skos:altLabel>
</skos:Concept><skos:Concept rdf:about="http://cognitiveatlas.org/id/tsk_4a57abb949bb1"> <dc:identifier>tsk_4a57abb949bb1</dc:identifier>
		<dc:Title>Cognitive Atlas : Lexicon : Mini Mental State Examination</dc:Title>
		<dc:Description>RDF output for 'Mini Mental State Examination'</dc:Description>
		<dc:Type>InteractiveResource</dc:Type>
		<dc:Publisher>Cognitive Atlas</dc:Publisher>
		<dc:Creator>Cognitive Atlas RDF Generator</dc:Creator>
		<dc:Contributor>Tom Schonberg</dc:Contributor>
		<dc:Date>2010-03-11 08:36:33</dc:Date>
		<dc:Format>text/rdf</dc:Format>
		<dc:Language>en</dc:Language>
		<skos:editorialNote>Generated by testgen.php on Thu Jun 9 14:25:25 PDT 2011.</skos:editorialNote>
		<skos:historyNote>Revision 2: 1 previous definitions.</skos:historyNote>
		<skos:changeNote>See http://cognitiveatlas.org/id/tsk_4a57abb949bb1 for complete revision history.</skos:changeNote>
		<skos:scopeNote>http://www.w3.org/2004/02/skos/core#Concept</skos:scopeNote>
		<skos:Note>SKOS properties defined in http://www.w3.org/TR/skos-primer/#secrel</skos:Note>
		<skos:inScheme rdf:resource="http://cognitiveatlas.org/tasks/"/>
		<skos:definition>The mini-mental state examination (MMSE) or Folstein test is a brief 30-point questionnaire test that is used to screen for cognitive impairment. It is commonly used in medicine to screen for dementia. It is also used to estimate the severity of cognitive impairment at a given point in time and to follow the course of cognitive changes in an individual over time, thus making it an effective way to document an individual&#39;s response to treatment.</skos:definition>
		<skos:prefLabel>Mini Mental State Examination</skos:prefLabel>
		<skos:altLabel></skos:altLabel>
</skos:Concept><skos:Concept rdf:about="http://cognitiveatlas.org/id/tsk_4a57abb949bbf"> <dc:identifier>tsk_4a57abb949bbf</dc:identifier>
		<dc:Title>Cognitive Atlas : Lexicon : motor sequencing task</dc:Title>
		<dc:Description>RDF output for 'motor sequencing task'</dc:Description>
		<dc:Type>InteractiveResource</dc:Type>
		<dc:Publisher>Cognitive Atlas</dc:Publisher>
		<dc:Creator>Cognitive Atlas RDF Generator</dc:Creator>
		<dc:Contributor>System Administrator</dc:Contributor>
		<dc:Date>2009-07-10 14:06:33</dc:Date>
		<dc:Format>text/rdf</dc:Format>
		<dc:Language>en</dc:Language>
		<skos:editorialNote>Generated by testgen.php on Thu Jun 9 14:25:25 PDT 2011.</skos:editorialNote>
		<skos:historyNote>No previous definition revisions.</skos:historyNote>
		<skos:changeNote>This is the first and only definition provided.</skos:changeNote>
		<skos:scopeNote>http://www.w3.org/2004/02/skos/core#Concept</skos:scopeNote>
		<skos:Note>SKOS properties defined in http://www.w3.org/TR/skos-primer/#secrel</skos:Note>
		<skos:inScheme rdf:resource="http://cognitiveatlas.org/tasks/"/>
		<skos:definition>No definition submitted yet</skos:definition>
		<skos:prefLabel>motor sequencing task</skos:prefLabel>
		<skos:altLabel></skos:altLabel>
</skos:Concept><skos:Concept rdf:about="http://cognitiveatlas.org/id/tsk_4a57abb949bcd"> <dc:identifier>tsk_4a57abb949bcd</dc:identifier>
		<dc:Title>Cognitive Atlas : Lexicon : n-back task</dc:Title>
		<dc:Description>RDF output for 'n-back task'</dc:Description>
		<dc:Type>InteractiveResource</dc:Type>
		<dc:Publisher>Cognitive Atlas</dc:Publisher>
		<dc:Creator>Cognitive Atlas RDF Generator</dc:Creator>
		<dc:Contributor>Agatha Lenartowicz</dc:Contributor>
		<dc:Date>2009-07-10 14:06:33</dc:Date>
		<dc:Format>text/rdf</dc:Format>
		<dc:Language>en</dc:Language>
		<skos:editorialNote>Generated by testgen.php on Thu Jun 9 14:25:25 PDT 2011.</skos:editorialNote>
		<skos:historyNote>No previous definition revisions.</skos:historyNote>
		<skos:changeNote>This is the first and only definition provided.</skos:changeNote>
		<skos:scopeNote>http://www.w3.org/2004/02/skos/core#Concept</skos:scopeNote>
		<skos:Note>SKOS properties defined in http://www.w3.org/TR/skos-primer/#secrel</skos:Note>
		<skos:inScheme rdf:resource="http://cognitiveatlas.org/tasks/"/>
		<skos:definition>A task in which items (e.g., letters) are presented one at a time and participants must identify each item that repeats relative to the item that occurred &#34;n&#34; items before its onset.</skos:definition>
		<skos:prefLabel>n-back task</skos:prefLabel>
		<skos:altLabel></skos:altLabel>
		<skos:related rdf:resource="http://cognitiveatlas.org/id/trm_4a3fd79d0b5a7"/>
		<skos:related rdf:resource="http://cognitiveatlas.org/id/trm_4a3fd79d0b5a7"/>
		<skos:related rdf:resource="http://cognitiveatlas.org/id/trm_4a3fd79d0b5a7"/>
		<skos:related rdf:resource="http://cognitiveatlas.org/id/trm_4a3fd79d0b5a7"/>
		<skos:related rdf:resource="http://cognitiveatlas.org/id/tsk_4a57abb949b1c"/>
		<skos:related rdf:resource="http://cognitiveatlas.org/id/tsk_4a57abb949a6a"/>
		<skos:related rdf:resource="http://cognitiveatlas.org/id/trm_4b4a537644d76"/>
		<skos:example>n-back task is descended from Continuous Performance Task</skos:example>
		<skos:example>working memory is measured by the contrast of 1-back trials in the n-back task</skos:example>
		<skos:example>working memory is measured by the contrast of 2-back trials in the n-back task</skos:example>
		<skos:example>working memory is measured by the contrast of 3-back trials in the n-back task</skos:example>
		<skos:example>working memory is measured by the contrast of 3-back minus 1-back trials in the n-back task</skos:example>
		<skos:example>letter n-back task is descended from n-back task</skos:example>
		<skos:example>face n-back task is descended from n-back task</skos:example>
		<cito:citesForInformation rdf:resource="http://cognitiveatlas.org/citation/id/cit_4b4a52cc53998"/>
</skos:Concept><skos:Concept rdf:about="http://cognitiveatlas.org/id/tsk_4a57abb949bdb"> <dc:identifier>tsk_4a57abb949bdb</dc:identifier>
		<dc:Title>Cognitive Atlas : Lexicon : nine-hole peg test</dc:Title>
		<dc:Description>RDF output for 'nine-hole peg test'</dc:Description>
		<dc:Type>InteractiveResource</dc:Type>
		<dc:Publisher>Cognitive Atlas</dc:Publisher>
		<dc:Creator>Cognitive Atlas RDF Generator</dc:Creator>
		<dc:Contributor>Brenda Gregory</dc:Contributor>
		<dc:Date>2011-05-03 13:58:07</dc:Date>
		<dc:Format>text/rdf</dc:Format>
		<dc:Language>en</dc:Language>
		<skos:editorialNote>Generated by testgen.php on Thu Jun 9 14:25:25 PDT 2011.</skos:editorialNote>
		<skos:historyNote>Revision 3: 2 previous definitions.</skos:historyNote>
		<skos:changeNote>See http://cognitiveatlas.org/id/tsk_4a57abb949bdb for complete revision history.</skos:changeNote>
		<skos:scopeNote>http://www.w3.org/2004/02/skos/core#Concept</skos:scopeNote>
		<skos:Note>SKOS properties defined in http://www.w3.org/TR/skos-primer/#secrel</skos:Note>
		<skos:inScheme rdf:resource="http://cognitiveatlas.org/tasks/"/>
		<skos:definition>a timed test of fine motor coordination; the test involves the subject placing 9 dowels in 9 holes. Subjects are scored on the amount of time it takes to place and remove all 9 pegs.</skos:definition>
		<skos:prefLabel>nine-hole peg test</skos:prefLabel>
		<skos:altLabel></skos:altLabel>
</skos:Concept><skos:Concept rdf:about="http://cognitiveatlas.org/id/tsk_4a57abb949be9"> <dc:identifier>tsk_4a57abb949be9</dc:identifier>
		<dc:Title>Cognitive Atlas : Lexicon : object-discrimination task</dc:Title>
		<dc:Description>RDF output for 'object-discrimination task'</dc:Description>
		<dc:Type>InteractiveResource</dc:Type>
		<dc:Publisher>Cognitive Atlas</dc:Publisher>
		<dc:Creator>Cognitive Atlas RDF Generator</dc:Creator>
		<dc:Contributor>System Administrator</dc:Contributor>
		<dc:Date>2009-07-10 14:06:33</dc:Date>
		<dc:Format>text/rdf</dc:Format>
		<dc:Language>en</dc:Language>
		<skos:editorialNote>Generated by testgen.php on Thu Jun 9 14:25:25 PDT 2011.</skos:editorialNote>
		<skos:historyNote>No previous definition revisions.</skos:historyNote>
		<skos:changeNote>This is the first and only definition provided.</skos:changeNote>
		<skos:scopeNote>http://www.w3.org/2004/02/skos/core#Concept</skos:scopeNote>
		<skos:Note>SKOS properties defined in http://www.w3.org/TR/skos-primer/#secrel</skos:Note>
		<skos:inScheme rdf:resource="http://cognitiveatlas.org/tasks/"/>
		<skos:definition>No definition submitted yet</skos:definition>
		<skos:prefLabel>object-discrimination task</skos:prefLabel>
		<skos:altLabel></skos:altLabel>
</skos:Concept><skos:Concept rdf:about="http://cognitiveatlas.org/id/tsk_4a57abb949bf6"> <dc:identifier>tsk_4a57abb949bf6</dc:identifier>
		<dc:Title>Cognitive Atlas : Lexicon : oddball task</dc:Title>
		<dc:Description>RDF output for 'oddball task'</dc:Description>
		<dc:Type>InteractiveResource</dc:Type>
		<dc:Publisher>Cognitive Atlas</dc:Publisher>
		<dc:Creator>Cognitive Atlas RDF Generator</dc:Creator>
		<dc:Contributor>Agatha Lenartowicz</dc:Contributor>
		<dc:Date>2009-07-10 14:06:33</dc:Date>
		<dc:Format>text/rdf</dc:Format>
		<dc:Language>en</dc:Language>
		<skos:editorialNote>Generated by testgen.php on Thu Jun 9 14:25:25 PDT 2011.</skos:editorialNote>
		<skos:historyNote>No previous definition revisions.</skos:historyNote>
		<skos:changeNote>This is the first and only definition provided.</skos:changeNote>
		<skos:scopeNote>http://www.w3.org/2004/02/skos/core#Concept</skos:scopeNote>
		<skos:Note>SKOS properties defined in http://www.w3.org/TR/skos-primer/#secrel</skos:Note>
		<skos:inScheme rdf:resource="http://cognitiveatlas.org/tasks/"/>
		<skos:definition>A task in which stimuli are presented in a continuous stream and participants must detect the presence of an oddball stimulus. The oddball is a stimulus that occurs infrequently relative to all other stimuli, and has distinct characteristics (e.g., a different tone among auditory stimuli).</skos:definition>
		<skos:prefLabel>oddball task</skos:prefLabel>
		<skos:altLabel></skos:altLabel>
</skos:Concept><skos:Concept rdf:about="http://cognitiveatlas.org/id/tsk_4a57abb949c04"> <dc:identifier>tsk_4a57abb949c04</dc:identifier>
		<dc:Title>Cognitive Atlas : Lexicon : Pantomime Task</dc:Title>
		<dc:Description>RDF output for 'Pantomime Task'</dc:Description>
		<dc:Type>InteractiveResource</dc:Type>
		<dc:Publisher>Cognitive Atlas</dc:Publisher>
		<dc:Creator>Cognitive Atlas RDF Generator</dc:Creator>
		<dc:Contributor>Natalie Picchetti</dc:Contributor>
		<dc:Date>2011-02-28 12:42:09</dc:Date>
		<dc:Format>text/rdf</dc:Format>
		<dc:Language>en</dc:Language>
		<skos:editorialNote>Generated by testgen.php on Thu Jun 9 14:25:25 PDT 2011.</skos:editorialNote>
		<skos:historyNote>Revision 2: 1 previous definitions.</skos:historyNote>
		<skos:changeNote>See http://cognitiveatlas.org/id/tsk_4a57abb949c04 for complete revision history.</skos:changeNote>
		<skos:scopeNote>http://www.w3.org/2004/02/skos/core#Concept</skos:scopeNote>
		<skos:Note>SKOS properties defined in http://www.w3.org/TR/skos-primer/#secrel</skos:Note>
		<skos:inScheme rdf:resource="http://cognitiveatlas.org/tasks/"/>
		<skos:definition>is when a subject is asked to explain an emotion or how an object is used by only gesturing with their hands and not using speech.  </skos:definition>
		<skos:prefLabel>Pantomime Task</skos:prefLabel>
		<skos:altLabel></skos:altLabel>
</skos:Concept><skos:Concept rdf:about="http://cognitiveatlas.org/id/tsk_4a57abb949ce9"> <dc:identifier>tsk_4a57abb949ce9</dc:identifier>
		<dc:Title>Cognitive Atlas : Lexicon : Parrott Scale</dc:Title>
		<dc:Description>RDF output for 'Parrott Scale'</dc:Description>
		<dc:Type>InteractiveResource</dc:Type>
		<dc:Publisher>Cognitive Atlas</dc:Publisher>
		<dc:Creator>Cognitive Atlas RDF Generator</dc:Creator>
		<dc:Contributor>System Administrator</dc:Contributor>
		<dc:Date>2009-07-10 14:06:33</dc:Date>
		<dc:Format>text/rdf</dc:Format>
		<dc:Language>en</dc:Language>
		<skos:editorialNote>Generated by testgen.php on Thu Jun 9 14:25:25 PDT 2011.</skos:editorialNote>
		<skos:historyNote>No previous definition revisions.</skos:historyNote>
		<skos:changeNote>This is the first and only definition provided.</skos:changeNote>
		<skos:scopeNote>http://www.w3.org/2004/02/skos/core#Concept</skos:scopeNote>
		<skos:Note>SKOS properties defined in http://www.w3.org/TR/skos-primer/#secrel</skos:Note>
		<skos:inScheme rdf:resource="http://cognitiveatlas.org/tasks/"/>
		<skos:definition>No definition submitted yet</skos:definition>
		<skos:prefLabel>Parrott Scale</skos:prefLabel>
		<skos:altLabel></skos:altLabel>
</skos:Concept><skos:Concept rdf:about="http://cognitiveatlas.org/id/tsk_4a57abb949cfb"> <dc:identifier>tsk_4a57abb949cfb</dc:identifier>
		<dc:Title>Cognitive Atlas : Lexicon : picture naming task</dc:Title>
		<dc:Description>RDF output for 'picture naming task'</dc:Description>
		<dc:Type>InteractiveResource</dc:Type>
		<dc:Publisher>Cognitive Atlas</dc:Publisher>
		<dc:Creator>Cognitive Atlas RDF Generator</dc:Creator>
		<dc:Contributor>System Administrator</dc:Contributor>
		<dc:Date>2009-07-10 14:06:33</dc:Date>
		<dc:Format>text/rdf</dc:Format>
		<dc:Language>en</dc:Language>
		<skos:editorialNote>Generated by testgen.php on Thu Jun 9 14:25:25 PDT 2011.</skos:editorialNote>
		<skos:historyNote>No previous definition revisions.</skos:historyNote>
		<skos:changeNote>This is the first and only definition provided.</skos:changeNote>
		<skos:scopeNote>http://www.w3.org/2004/02/skos/core#Concept</skos:scopeNote>
		<skos:Note>SKOS properties defined in http://www.w3.org/TR/skos-primer/#secrel</skos:Note>
		<skos:inScheme rdf:resource="http://cognitiveatlas.org/tasks/"/>
		<skos:definition>No definition submitted yet</skos:definition>
		<skos:prefLabel>picture naming task</skos:prefLabel>
		<skos:altLabel></skos:altLabel>
</skos:Concept><skos:Concept rdf:about="http://cognitiveatlas.org/id/tsk_4a57abb949d09"> <dc:identifier>tsk_4a57abb949d09</dc:identifier>
		<dc:Title>Cognitive Atlas : Lexicon : Positive and Negative Affect Scale</dc:Title>
		<dc:Description>RDF output for 'Positive and Negative Affect Scale'</dc:Description>
		<dc:Type>InteractiveResource</dc:Type>
		<dc:Publisher>Cognitive Atlas</dc:Publisher>
		<dc:Creator>Cognitive Atlas RDF Generator</dc:Creator>
		<dc:Contributor>Agatha Lenartowicz</dc:Contributor>
		<dc:Date>2009-07-10 14:06:33</dc:Date>
		<dc:Format>text/rdf</dc:Format>
		<dc:Language>en</dc:Language>
		<skos:editorialNote>Generated by testgen.php on Thu Jun 9 14:25:25 PDT 2011.</skos:editorialNote>
		<skos:historyNote>No previous definition revisions.</skos:historyNote>
		<skos:changeNote>This is the first and only definition provided.</skos:changeNote>
		<skos:scopeNote>http://www.w3.org/2004/02/skos/core#Concept</skos:scopeNote>
		<skos:Note>SKOS properties defined in http://www.w3.org/TR/skos-primer/#secrel</skos:Note>
		<skos:inScheme rdf:resource="http://cognitiveatlas.org/tasks/"/>
		<skos:definition>A psychometric scale to measure positive and negative affects in individuals, and both as states and traits.</skos:definition>
		<skos:prefLabel>Positive and Negative Affect Scale</skos:prefLabel>
		<skos:altLabel></skos:altLabel>
</skos:Concept><skos:Concept rdf:about="http://cognitiveatlas.org/id/tsk_4a57abb949d17"> <dc:identifier>tsk_4a57abb949d17</dc:identifier>
		<dc:Title>Cognitive Atlas : Lexicon : Posner cueing task</dc:Title>
		<dc:Description>RDF output for 'Posner cueing task'</dc:Description>
		<dc:Type>InteractiveResource</dc:Type>
		<dc:Publisher>Cognitive Atlas</dc:Publisher>
		<dc:Creator>Cognitive Atlas RDF Generator</dc:Creator>
		<dc:Contributor>Brenda Gregory</dc:Contributor>
		<dc:Date>2011-04-19 12:09:45</dc:Date>
		<dc:Format>text/rdf</dc:Format>
		<dc:Language>en</dc:Language>
		<skos:editorialNote>Generated by testgen.php on Thu Jun 9 14:25:25 PDT 2011.</skos:editorialNote>
		<skos:historyNote>Revision 3: 2 previous definitions.</skos:historyNote>
		<skos:changeNote>See http://cognitiveatlas.org/id/tsk_4a57abb949d17 for complete revision history.</skos:changeNote>
		<skos:scopeNote>http://www.w3.org/2004/02/skos/core#Concept</skos:scopeNote>
		<skos:Note>SKOS properties defined in http://www.w3.org/TR/skos-primer/#secrel</skos:Note>
		<skos:inScheme rdf:resource="http://cognitiveatlas.org/tasks/"/>
		<skos:definition>Subjects view two stimuli (boxes, letters, etc.) and are cued by an arrow to attend to one of the stimuli.  Subjects then discriminate and respond (e.g., press a button when one of the boxes is filled with a diagonal cross, or press the left button for an &#34;X&#34; and the right button for an &#34;O&#34;). </skos:definition>
		<skos:prefLabel>Posner cueing task</skos:prefLabel>
		<skos:altLabel></skos:altLabel>
</skos:Concept><skos:Concept rdf:about="http://cognitiveatlas.org/id/tsk_4a57abb949d25"> <dc:identifier>tsk_4a57abb949d25</dc:identifier>
		<dc:Title>Cognitive Atlas : Lexicon : Pseudoword naming task</dc:Title>
		<dc:Description>RDF output for 'Pseudoword naming task'</dc:Description>
		<dc:Type>InteractiveResource</dc:Type>
		<dc:Publisher>Cognitive Atlas</dc:Publisher>
		<dc:Creator>Cognitive Atlas RDF Generator</dc:Creator>
		<dc:Contributor>System Administrator</dc:Contributor>
		<dc:Date>2009-07-10 14:06:33</dc:Date>
		<dc:Format>text/rdf</dc:Format>
		<dc:Language>en</dc:Language>
		<skos:editorialNote>Generated by testgen.php on Thu Jun 9 14:25:25 PDT 2011.</skos:editorialNote>
		<skos:historyNote>No previous definition revisions.</skos:historyNote>
		<skos:changeNote>This is the first and only definition provided.</skos:changeNote>
		<skos:scopeNote>http://www.w3.org/2004/02/skos/core#Concept</skos:scopeNote>
		<skos:Note>SKOS properties defined in http://www.w3.org/TR/skos-primer/#secrel</skos:Note>
		<skos:inScheme rdf:resource="http://cognitiveatlas.org/tasks/"/>
		<skos:definition>No definition submitted yet</skos:definition>
		<skos:prefLabel>Pseudoword naming task</skos:prefLabel>
		<skos:altLabel></skos:altLabel>
</skos:Concept><skos:Concept rdf:about="http://cognitiveatlas.org/id/tsk_4a57abb949d32"> <dc:identifier>tsk_4a57abb949d32</dc:identifier>
		<dc:Title>Cognitive Atlas : Lexicon : pyramids and palm trees task</dc:Title>
		<dc:Description>RDF output for 'pyramids and palm trees task'</dc:Description>
		<dc:Type>InteractiveResource</dc:Type>
		<dc:Publisher>Cognitive Atlas</dc:Publisher>
		<dc:Creator>Cognitive Atlas RDF Generator</dc:Creator>
		<dc:Contributor>Brenda Gregory</dc:Contributor>
		<dc:Date>2011-04-29 11:03:26</dc:Date>
		<dc:Format>text/rdf</dc:Format>
		<dc:Language>en</dc:Language>
		<skos:editorialNote>Generated by testgen.php on Thu Jun 9 14:25:25 PDT 2011.</skos:editorialNote>
		<skos:historyNote>Revision 3: 2 previous definitions.</skos:historyNote>
		<skos:changeNote>See http://cognitiveatlas.org/id/tsk_4a57abb949d32 for complete revision history.</skos:changeNote>
		<skos:scopeNote>http://www.w3.org/2004/02/skos/core#Concept</skos:scopeNote>
		<skos:Note>SKOS properties defined in http://www.w3.org/TR/skos-primer/#secrel</skos:Note>
		<skos:inScheme rdf:resource="http://cognitiveatlas.org/tasks/"/>
		<skos:definition>a semantic memory test that measures the capacity to access detailed semantic information about words and pictures, necessary for the identification of the analogies, which link conceptually two perceptually, and functionally distinct entities.</skos:definition>
		<skos:prefLabel>pyramids and palm trees task</skos:prefLabel>
		<skos:altLabel></skos:altLabel>
		<cito:citesForInformation rdf:resource="http://cognitiveatlas.org/citation/id/cit_4dbaf245b2a5f"/>
</skos:Concept><skos:Concept rdf:about="http://cognitiveatlas.org/id/tsk_4a57abb949d40"> <dc:identifier>tsk_4a57abb949d40</dc:identifier>
		<dc:Title>Cognitive Atlas : Lexicon : recognition memory test</dc:Title>
		<dc:Description>RDF output for 'recognition memory test'</dc:Description>
		<dc:Type>InteractiveResource</dc:Type>
		<dc:Publisher>Cognitive Atlas</dc:Publisher>
		<dc:Creator>Cognitive Atlas RDF Generator</dc:Creator>
		<dc:Contributor>Dan Dillon</dc:Contributor>
		<dc:Date>2010-04-21 11:00:13</dc:Date>
		<dc:Format>text/rdf</dc:Format>
		<dc:Language>en</dc:Language>
		<skos:editorialNote>Generated by testgen.php on Thu Jun 9 14:25:25 PDT 2011.</skos:editorialNote>
		<skos:historyNote>Revision 2: 1 previous definitions.</skos:historyNote>
		<skos:changeNote>See http://cognitiveatlas.org/id/tsk_4a57abb949d40 for complete revision history.</skos:changeNote>
		<skos:scopeNote>http://www.w3.org/2004/02/skos/core#Concept</skos:scopeNote>
		<skos:Note>SKOS properties defined in http://www.w3.org/TR/skos-primer/#secrel</skos:Note>
		<skos:inScheme rdf:resource="http://cognitiveatlas.org/tasks/"/>
		<skos:definition>In a recognition memory test, a participant is presented with some or all of a set of &#34;old&#34; stimuli that were encoded earlier, as well as several &#34;new&#34; stimuli that were not previously presented. The participant&#39;s task is to indicate whether each stimulus is old or new. Responses in recognition memory tests are commonly sorted into four classes: Hits (&#34;old&#34; response to an old stimulus), Misses (&#34;new&#34; response to an old stimulus), False Alarms (&#34;old&#34; response to a new stimulus), and Correct Rejections (&#34;new&#34; response to a new stimulus). By comparing the percentage of responses that fall into each of these classes, the experimenter can assess both a participant&#39;s ability to discriminate between old and new stimuli, and his or her tendency to provide a particular response regardless of the type of stimulus presented. In many recognition memory tests, each old/new judgment is followed by a prompt asking participants to indicate either how confident they are in that old/new judgment, or what type of subjective experience was elicited by the stimulus being judged (e.g., was the old/new judgment accompanied by a vivid recollection of the encoding experience). This additional information can be used to generate and test more precise hypotheses about how recognition memory decisions are made.</skos:definition>
		<skos:prefLabel>recognition memory test</skos:prefLabel>
		<skos:altLabel></skos:altLabel>
</skos:Concept><skos:Concept rdf:about="http://cognitiveatlas.org/id/tsk_4a57abb949d4e"> <dc:identifier>tsk_4a57abb949d4e</dc:identifier>
		<dc:Title>Cognitive Atlas : Lexicon : reversal learning task</dc:Title>
		<dc:Description>RDF output for 'reversal learning task'</dc:Description>
		<dc:Type>InteractiveResource</dc:Type>
		<dc:Publisher>Cognitive Atlas</dc:Publisher>
		<dc:Creator>Cognitive Atlas RDF Generator</dc:Creator>
		<dc:Contributor>System Administrator</dc:Contributor>
		<dc:Date>2009-07-10 14:06:33</dc:Date>
		<dc:Format>text/rdf</dc:Format>
		<dc:Language>en</dc:Language>
		<skos:editorialNote>Generated by testgen.php on Thu Jun 9 14:25:25 PDT 2011.</skos:editorialNote>
		<skos:historyNote>No previous definition revisions.</skos:historyNote>
		<skos:changeNote>This is the first and only definition provided.</skos:changeNote>
		<skos:scopeNote>http://www.w3.org/2004/02/skos/core#Concept</skos:scopeNote>
		<skos:Note>SKOS properties defined in http://www.w3.org/TR/skos-primer/#secrel</skos:Note>
		<skos:inScheme rdf:resource="http://cognitiveatlas.org/tasks/"/>
		<skos:definition>No definition submitted yet</skos:definition>
		<skos:prefLabel>reversal learning task</skos:prefLabel>
		<skos:altLabel></skos:altLabel>
</skos:Concept><skos:Concept rdf:about="http://cognitiveatlas.org/id/tsk_4a57abb949d5b"> <dc:identifier>tsk_4a57abb949d5b</dc:identifier>
		<dc:Title>Cognitive Atlas : Lexicon : Risky Gains task</dc:Title>
		<dc:Description>RDF output for 'Risky Gains task'</dc:Description>
		<dc:Type>InteractiveResource</dc:Type>
		<dc:Publisher>Cognitive Atlas</dc:Publisher>
		<dc:Creator>Cognitive Atlas RDF Generator</dc:Creator>
		<dc:Contributor>Brenda Gregory</dc:Contributor>
		<dc:Date>2011-04-19 12:05:46</dc:Date>
		<dc:Format>text/rdf</dc:Format>
		<dc:Language>en</dc:Language>
		<skos:editorialNote>Generated by testgen.php on Thu Jun 9 14:25:25 PDT 2011.</skos:editorialNote>
		<skos:historyNote>Revision 3: 2 previous definitions.</skos:historyNote>
		<skos:changeNote>See http://cognitiveatlas.org/id/tsk_4a57abb949d5b for complete revision history.</skos:changeNote>
		<skos:scopeNote>http://www.w3.org/2004/02/skos/core#Concept</skos:scopeNote>
		<skos:Note>SKOS properties defined in http://www.w3.org/TR/skos-primer/#secrel</skos:Note>
		<skos:inScheme rdf:resource="http://cognitiveatlas.org/tasks/"/>
		<skos:definition>Subjects are presented with a sequence of three numbers in ascending order (20, 40, and 80).  Each number is displayed onscreen for one second and, if the subject presses a button while that number is displayed, he/she receives that number of points along with immediate positive visual and auditory feedback.  When a 40 or 80 appears, however, there is a chance that it will appear in an alternate color, along with immediate negative feedback signaling a loss of 40 or 80 points, respectively.  When this occurs, the trial ends immediately (i.e. the subject may not make a response). </skos:definition>
		<skos:prefLabel>Risky Gains task</skos:prefLabel>
		<skos:altLabel></skos:altLabel>
		<cito:citesForInformation rdf:resource="http://cognitiveatlas.org/citation/id/cit_4d55937f7d27c"/>
</skos:Concept><skos:Concept rdf:about="http://cognitiveatlas.org/id/tsk_4a57abb949d69"> <dc:identifier>tsk_4a57abb949d69</dc:identifier>
		<dc:Title>Cognitive Atlas : Lexicon : Salthouse and Babcock Listening Span task </dc:Title>
		<dc:Description>RDF output for 'Salthouse and Babcock Listening Span task '</dc:Description>
		<dc:Type>InteractiveResource</dc:Type>
		<dc:Publisher>Cognitive Atlas</dc:Publisher>
		<dc:Creator>Cognitive Atlas RDF Generator</dc:Creator>
		<dc:Contributor>System Administrator</dc:Contributor>
		<dc:Date>2009-07-10 14:06:33</dc:Date>
		<dc:Format>text/rdf</dc:Format>
		<dc:Language>en</dc:Language>
		<skos:editorialNote>Generated by testgen.php on Thu Jun 9 14:25:25 PDT 2011.</skos:editorialNote>
		<skos:historyNote>No previous definition revisions.</skos:historyNote>
		<skos:changeNote>This is the first and only definition provided.</skos:changeNote>
		<skos:scopeNote>http://www.w3.org/2004/02/skos/core#Concept</skos:scopeNote>
		<skos:Note>SKOS properties defined in http://www.w3.org/TR/skos-primer/#secrel</skos:Note>
		<skos:inScheme rdf:resource="http://cognitiveatlas.org/tasks/"/>
		<skos:definition>No definition submitted yet</skos:definition>
		<skos:prefLabel>Salthouse and Babcock Listening Span task </skos:prefLabel>
		<skos:altLabel></skos:altLabel>
		<skos:related rdf:resource="http://cognitiveatlas.org/id/trm_4c40d1d16071e"/>
		<skos:example>listening span task is a broader synonym of Salthouse and Babcock Listening Span task </skos:example>
</skos:Concept><skos:Concept rdf:about="http://cognitiveatlas.org/id/tsk_4a57abb949d76"> <dc:identifier>tsk_4a57abb949d76</dc:identifier>
		<dc:Title>Cognitive Atlas : Lexicon : selective attention task</dc:Title>
		<dc:Description>RDF output for 'selective attention task'</dc:Description>
		<dc:Type>InteractiveResource</dc:Type>
		<dc:Publisher>Cognitive Atlas</dc:Publisher>
		<dc:Creator>Cognitive Atlas RDF Generator</dc:Creator>
		<dc:Contributor>Natalie Picchetti</dc:Contributor>
		<dc:Date>2011-05-18 15:32:32</dc:Date>
		<dc:Format>text/rdf</dc:Format>
		<dc:Language>en</dc:Language>
		<skos:editorialNote>Generated by testgen.php on Thu Jun 9 14:25:25 PDT 2011.</skos:editorialNote>
		<skos:historyNote>Revision 5: 4 previous definitions.</skos:historyNote>
		<skos:changeNote>See http://cognitiveatlas.org/id/tsk_4a57abb949d76 for complete revision history.</skos:changeNote>
		<skos:scopeNote>http://www.w3.org/2004/02/skos/core#Concept</skos:scopeNote>
		<skos:Note>SKOS properties defined in http://www.w3.org/TR/skos-primer/#secrel</skos:Note>
		<skos:inScheme rdf:resource="http://cognitiveatlas.org/tasks/"/>
		<skos:definition>involves a participant to attend to a specific stimuli in the presence of competing stimuli.</skos:definition>
		<skos:prefLabel>selective attention task</skos:prefLabel>
		<skos:altLabel></skos:altLabel>
</skos:Concept><skos:Concept rdf:about="http://cognitiveatlas.org/id/tsk_4a57abb949d84"> <dc:identifier>tsk_4a57abb949d84</dc:identifier>
		<dc:Title>Cognitive Atlas : Lexicon : semantic anomaly judgement task</dc:Title>
		<dc:Description>RDF output for 'semantic anomaly judgement task'</dc:Description>
		<dc:Type>InteractiveResource</dc:Type>
		<dc:Publisher>Cognitive Atlas</dc:Publisher>
		<dc:Creator>Cognitive Atlas RDF Generator</dc:Creator>
		<dc:Contributor>System Administrator</dc:Contributor>
		<dc:Date>2009-07-10 14:06:33</dc:Date>
		<dc:Format>text/rdf</dc:Format>
		<dc:Language>en</dc:Language>
		<skos:editorialNote>Generated by testgen.php on Thu Jun 9 14:25:25 PDT 2011.</skos:editorialNote>
		<skos:historyNote>No previous definition revisions.</skos:historyNote>
		<skos:changeNote>This is the first and only definition provided.</skos:changeNote>
		<skos:scopeNote>http://www.w3.org/2004/02/skos/core#Concept</skos:scopeNote>
		<skos:Note>SKOS properties defined in http://www.w3.org/TR/skos-primer/#secrel</skos:Note>
		<skos:inScheme rdf:resource="http://cognitiveatlas.org/tasks/"/>
		<skos:definition>No definition submitted yet</skos:definition>
		<skos:prefLabel>semantic anomaly judgement task</skos:prefLabel>
		<skos:altLabel></skos:altLabel>
</skos:Concept><skos:Concept rdf:about="http://cognitiveatlas.org/id/tsk_4a57abb949d92"> <dc:identifier>tsk_4a57abb949d92</dc:identifier>
		<dc:Title>Cognitive Atlas : Lexicon : semantic association task</dc:Title>
		<dc:Description>RDF output for 'semantic association task'</dc:Description>
		<dc:Type>InteractiveResource</dc:Type>
		<dc:Publisher>Cognitive Atlas</dc:Publisher>
		<dc:Creator>Cognitive Atlas RDF Generator</dc:Creator>
		<dc:Contributor>System Administrator</dc:Contributor>
		<dc:Date>2009-07-10 14:06:33</dc:Date>
		<dc:Format>text/rdf</dc:Format>
		<dc:Language>en</dc:Language>
		<skos:editorialNote>Generated by testgen.php on Thu Jun 9 14:25:25 PDT 2011.</skos:editorialNote>
		<skos:historyNote>No previous definition revisions.</skos:historyNote>
		<skos:changeNote>This is the first and only definition provided.</skos:changeNote>
		<skos:scopeNote>http://www.w3.org/2004/02/skos/core#Concept</skos:scopeNote>
		<skos:Note>SKOS properties defined in http://www.w3.org/TR/skos-primer/#secrel</skos:Note>
		<skos:inScheme rdf:resource="http://cognitiveatlas.org/tasks/"/>
		<skos:definition>No definition submitted yet</skos:definition>
		<skos:prefLabel>semantic association task</skos:prefLabel>
		<skos:altLabel></skos:altLabel>
</skos:Concept><skos:Concept rdf:about="http://cognitiveatlas.org/id/tsk_4a57abb949d9f"> <dc:identifier>tsk_4a57abb949d9f</dc:identifier>
		<dc:Title>Cognitive Atlas : Lexicon : sentence completion test</dc:Title>
		<dc:Description>RDF output for 'sentence completion test'</dc:Description>
		<dc:Type>InteractiveResource</dc:Type>
		<dc:Publisher>Cognitive Atlas</dc:Publisher>
		<dc:Creator>Cognitive Atlas RDF Generator</dc:Creator>
		<dc:Contributor>Brenda Gregory</dc:Contributor>
		<dc:Date>2011-05-11 16:21:27</dc:Date>
		<dc:Format>text/rdf</dc:Format>
		<dc:Language>en</dc:Language>
		<skos:editorialNote>Generated by testgen.php on Thu Jun 9 14:25:25 PDT 2011.</skos:editorialNote>
		<skos:historyNote>Revision 3: 2 previous definitions.</skos:historyNote>
		<skos:changeNote>See http://cognitiveatlas.org/id/tsk_4a57abb949d9f for complete revision history.</skos:changeNote>
		<skos:scopeNote>http://www.w3.org/2004/02/skos/core#Concept</skos:scopeNote>
		<skos:Note>SKOS properties defined in http://www.w3.org/TR/skos-primer/#secrel</skos:Note>
		<skos:inScheme rdf:resource="http://cognitiveatlas.org/tasks/"/>
		<skos:definition>a test that provides respondents with beginnings of sentences, referred to as “stems,” and respondents then complete the sentences in ways that are meaningful to them. The responses are believed to provide indications of attitudes, beliefs, motivations, or other mental states.</skos:definition>
		<skos:prefLabel>sentence completion test</skos:prefLabel>
		<skos:altLabel></skos:altLabel>
</skos:Concept><skos:Concept rdf:about="http://cognitiveatlas.org/id/tsk_4a57abb949dad"> <dc:identifier>tsk_4a57abb949dad</dc:identifier>
		<dc:Title>Cognitive Atlas : Lexicon : Set-shifting task</dc:Title>
		<dc:Description>RDF output for 'Set-shifting task'</dc:Description>
		<dc:Type>InteractiveResource</dc:Type>
		<dc:Publisher>Cognitive Atlas</dc:Publisher>
		<dc:Creator>Cognitive Atlas RDF Generator</dc:Creator>
		<dc:Contributor>Agatha Lenartowicz</dc:Contributor>
		<dc:Date>2009-07-30 17:14:34</dc:Date>
		<dc:Format>text/rdf</dc:Format>
		<dc:Language>en</dc:Language>
		<skos:editorialNote>Generated by testgen.php on Thu Jun 9 14:25:25 PDT 2011.</skos:editorialNote>
		<skos:historyNote>No previous definition revisions.</skos:historyNote>
		<skos:changeNote>This is the first and only definition provided.</skos:changeNote>
		<skos:scopeNote>http://www.w3.org/2004/02/skos/core#Concept</skos:scopeNote>
		<skos:Note>SKOS properties defined in http://www.w3.org/TR/skos-primer/#secrel</skos:Note>
		<skos:inScheme rdf:resource="http://cognitiveatlas.org/tasks/"/>
		<skos:definition>A task in which participants alternate between two or more judgments typically regarding the same set of stimuli. Accuracy and reaction time are measured for each judgment.</skos:definition>
		<skos:prefLabel>Set-shifting task</skos:prefLabel>
		<skos:altLabel></skos:altLabel>
</skos:Concept><skos:Concept rdf:about="http://cognitiveatlas.org/id/tsk_4a57abb949dbb"> <dc:identifier>tsk_4a57abb949dbb</dc:identifier>
		<dc:Title>Cognitive Atlas : Lexicon : Simon task</dc:Title>
		<dc:Description>RDF output for 'Simon task'</dc:Description>
		<dc:Type>InteractiveResource</dc:Type>
		<dc:Publisher>Cognitive Atlas</dc:Publisher>
		<dc:Creator>Cognitive Atlas RDF Generator</dc:Creator>
		<dc:Contributor>Brenda Gregory</dc:Contributor>
		<dc:Date>2011-04-19 12:07:28</dc:Date>
		<dc:Format>text/rdf</dc:Format>
		<dc:Language>en</dc:Language>
		<skos:editorialNote>Generated by testgen.php on Thu Jun 9 14:25:25 PDT 2011.</skos:editorialNote>
		<skos:historyNote>Revision 3: 2 previous definitions.</skos:historyNote>
		<skos:changeNote>See http://cognitiveatlas.org/id/tsk_4a57abb949dbb for complete revision history.</skos:changeNote>
		<skos:scopeNote>http://www.w3.org/2004/02/skos/core#Concept</skos:scopeNote>
		<skos:Note>SKOS properties defined in http://www.w3.org/TR/skos-primer/#secrel</skos:Note>
		<skos:inScheme rdf:resource="http://cognitiveatlas.org/tasks/"/>
		<skos:definition>Subjects view arrows presented in the right or left visual field that were pointing to the left or right.  Subjects respond via button press as to the direction of the arrow.  In incongruent stimuli, left-pointing arrows are seen on the right side, and vice versa. </skos:definition>
		<skos:prefLabel>Simon task</skos:prefLabel>
		<skos:altLabel></skos:altLabel>
</skos:Concept><skos:Concept rdf:about="http://cognitiveatlas.org/id/tsk_4a57abb949dc8"> <dc:identifier>tsk_4a57abb949dc8</dc:identifier>
		<dc:Title>Cognitive Atlas : Lexicon : simple reaction time task</dc:Title>
		<dc:Description>RDF output for 'simple reaction time task'</dc:Description>
		<dc:Type>InteractiveResource</dc:Type>
		<dc:Publisher>Cognitive Atlas</dc:Publisher>
		<dc:Creator>Cognitive Atlas RDF Generator</dc:Creator>
		<dc:Contributor>Brenda Gregory</dc:Contributor>
		<dc:Date>2011-04-29 16:14:21</dc:Date>
		<dc:Format>text/rdf</dc:Format>
		<dc:Language>en</dc:Language>
		<skos:editorialNote>Generated by testgen.php on Thu Jun 9 14:25:25 PDT 2011.</skos:editorialNote>
		<skos:historyNote>Revision 3: 2 previous definitions.</skos:historyNote>
		<skos:changeNote>See http://cognitiveatlas.org/id/tsk_4a57abb949dc8 for complete revision history.</skos:changeNote>
		<skos:scopeNote>http://www.w3.org/2004/02/skos/core#Concept</skos:scopeNote>
		<skos:Note>SKOS properties defined in http://www.w3.org/TR/skos-primer/#secrel</skos:Note>
		<skos:inScheme rdf:resource="http://cognitiveatlas.org/tasks/"/>
		<skos:definition>task that assesses the ability of the subject to respond to an external cue and retrieve a reward.</skos:definition>
		<skos:prefLabel>simple reaction time task</skos:prefLabel>
		<skos:altLabel></skos:altLabel>
</skos:Concept><skos:Concept rdf:about="http://cognitiveatlas.org/id/tsk_4a57abb949dd6"> <dc:identifier>tsk_4a57abb949dd6</dc:identifier>
		<dc:Title>Cognitive Atlas : Lexicon : source memory test</dc:Title>
		<dc:Description>RDF output for 'source memory test'</dc:Description>
		<dc:Type>InteractiveResource</dc:Type>
		<dc:Publisher>Cognitive Atlas</dc:Publisher>
		<dc:Creator>Cognitive Atlas RDF Generator</dc:Creator>
		<dc:Contributor>System Administrator</dc:Contributor>
		<dc:Date>2009-07-10 14:06:33</dc:Date>
		<dc:Format>text/rdf</dc:Format>
		<dc:Language>en</dc:Language>
		<skos:editorialNote>Generated by testgen.php on Thu Jun 9 14:25:25 PDT 2011.</skos:editorialNote>
		<skos:historyNote>No previous definition revisions.</skos:historyNote>
		<skos:changeNote>This is the first and only definition provided.</skos:changeNote>
		<skos:scopeNote>http://www.w3.org/2004/02/skos/core#Concept</skos:scopeNote>
		<skos:Note>SKOS properties defined in http://www.w3.org/TR/skos-primer/#secrel</skos:Note>
		<skos:inScheme rdf:resource="http://cognitiveatlas.org/tasks/"/>
		<skos:definition>No definition submitted yet</skos:definition>
		<skos:prefLabel>source memory test</skos:prefLabel>
		<skos:altLabel></skos:altLabel>
</skos:Concept><skos:Concept rdf:about="http://cognitiveatlas.org/id/tsk_4a57abb949de3"> <dc:identifier>tsk_4a57abb949de3</dc:identifier>
		<dc:Title>Cognitive Atlas : Lexicon : Span/Supra-Span Test</dc:Title>
		<dc:Description>RDF output for 'Span/Supra-Span Test'</dc:Description>
		<dc:Type>InteractiveResource</dc:Type>
		<dc:Publisher>Cognitive Atlas</dc:Publisher>
		<dc:Creator>Cognitive Atlas RDF Generator</dc:Creator>
		<dc:Contributor>System Administrator</dc:Contributor>
		<dc:Date>2009-07-10 14:06:33</dc:Date>
		<dc:Format>text/rdf</dc:Format>
		<dc:Language>en</dc:Language>
		<skos:editorialNote>Generated by testgen.php on Thu Jun 9 14:25:25 PDT 2011.</skos:editorialNote>
		<skos:historyNote>No previous definition revisions.</skos:historyNote>
		<skos:changeNote>This is the first and only definition provided.</skos:changeNote>
		<skos:scopeNote>http://www.w3.org/2004/02/skos/core#Concept</skos:scopeNote>
		<skos:Note>SKOS properties defined in http://www.w3.org/TR/skos-primer/#secrel</skos:Note>
		<skos:inScheme rdf:resource="http://cognitiveatlas.org/tasks/"/>
		<skos:definition>No definition submitted yet</skos:definition>
		<skos:prefLabel>Span/Supra-Span Test</skos:prefLabel>
		<skos:altLabel></skos:altLabel>
</skos:Concept><skos:Concept rdf:about="http://cognitiveatlas.org/id/tsk_4a57abb949df1"> <dc:identifier>tsk_4a57abb949df1</dc:identifier>
		<dc:Title>Cognitive Atlas : Lexicon : spatial n-back task</dc:Title>
		<dc:Description>RDF output for 'spatial n-back task'</dc:Description>
		<dc:Type>InteractiveResource</dc:Type>
		<dc:Publisher>Cognitive Atlas</dc:Publisher>
		<dc:Creator>Cognitive Atlas RDF Generator</dc:Creator>
		<dc:Contributor>System Administrator</dc:Contributor>
		<dc:Date>2009-07-10 14:06:33</dc:Date>
		<dc:Format>text/rdf</dc:Format>
		<dc:Language>en</dc:Language>
		<skos:editorialNote>Generated by testgen.php on Thu Jun 9 14:25:25 PDT 2011.</skos:editorialNote>
		<skos:historyNote>No previous definition revisions.</skos:historyNote>
		<skos:changeNote>This is the first and only definition provided.</skos:changeNote>
		<skos:scopeNote>http://www.w3.org/2004/02/skos/core#Concept</skos:scopeNote>
		<skos:Note>SKOS properties defined in http://www.w3.org/TR/skos-primer/#secrel</skos:Note>
		<skos:inScheme rdf:resource="http://cognitiveatlas.org/tasks/"/>
		<skos:definition>No definition submitted yet</skos:definition>
		<skos:prefLabel>spatial n-back task</skos:prefLabel>
		<skos:altLabel></skos:altLabel>
		<skos:related rdf:resource="http://cognitiveatlas.org/id/tsk_4a57abb949a6a"/>
		<skos:example>face n-back task is related to spatial n-back task</skos:example>
</skos:Concept><skos:Concept rdf:about="http://cognitiveatlas.org/id/tsk_4a57abb949dfe"> <dc:identifier>tsk_4a57abb949dfe</dc:identifier>
		<dc:Title>Cognitive Atlas : Lexicon : Spielberger's State-Trait Anxiety Questionnaire</dc:Title>
		<dc:Description>RDF output for 'Spielberger's State-Trait Anxiety Questionnaire'</dc:Description>
		<dc:Type>InteractiveResource</dc:Type>
		<dc:Publisher>Cognitive Atlas</dc:Publisher>
		<dc:Creator>Cognitive Atlas RDF Generator</dc:Creator>
		<dc:Contributor>Brenda Gregory</dc:Contributor>
		<dc:Date>2011-04-28 16:17:36</dc:Date>
		<dc:Format>text/rdf</dc:Format>
		<dc:Language>en</dc:Language>
		<skos:editorialNote>Generated by testgen.php on Thu Jun 9 14:25:25 PDT 2011.</skos:editorialNote>
		<skos:historyNote>Revision 4: 3 previous definitions.</skos:historyNote>
		<skos:changeNote>See http://cognitiveatlas.org/id/tsk_4a57abb949dfe for complete revision history.</skos:changeNote>
		<skos:scopeNote>http://www.w3.org/2004/02/skos/core#Concept</skos:scopeNote>
		<skos:Note>SKOS properties defined in http://www.w3.org/TR/skos-primer/#secrel</skos:Note>
		<skos:inScheme rdf:resource="http://cognitiveatlas.org/tasks/"/>
		<skos:definition>instrument used to measure trait (chronic) anxiety, a general propensity to be anxious, and state (temporary) anxiety, a temporary state varying in intensity, in adults.</skos:definition>
		<skos:prefLabel>Spielberger's State-Trait Anxiety Questionnaire</skos:prefLabel>
		<skos:altLabel></skos:altLabel>
</skos:Concept><skos:Concept rdf:about="http://cognitiveatlas.org/id/tsk_4a57abb949e0c"> <dc:identifier>tsk_4a57abb949e0c</dc:identifier>
		<dc:Title>Cognitive Atlas : Lexicon : Sternberg delayed recognition task</dc:Title>
		<dc:Description>RDF output for 'Sternberg delayed recognition task'</dc:Description>
		<dc:Type>InteractiveResource</dc:Type>
		<dc:Publisher>Cognitive Atlas</dc:Publisher>
		<dc:Creator>Cognitive Atlas RDF Generator</dc:Creator>
		<dc:Contributor>Brenda Gregory</dc:Contributor>
		<dc:Date>2011-04-19 12:10:46</dc:Date>
		<dc:Format>text/rdf</dc:Format>
		<dc:Language>en</dc:Language>
		<skos:editorialNote>Generated by testgen.php on Thu Jun 9 14:25:25 PDT 2011.</skos:editorialNote>
		<skos:historyNote>Revision 3: 2 previous definitions.</skos:historyNote>
		<skos:changeNote>See http://cognitiveatlas.org/id/tsk_4a57abb949e0c for complete revision history.</skos:changeNote>
		<skos:scopeNote>http://www.w3.org/2004/02/skos/core#Concept</skos:scopeNote>
		<skos:Note>SKOS properties defined in http://www.w3.org/TR/skos-primer/#secrel</skos:Note>
		<skos:inScheme rdf:resource="http://cognitiveatlas.org/tasks/"/>
		<skos:definition>Subjects view a string of letters.  After a delay, a probe letter is presented and subjects indicate if the presented letter was in the previously viewed group. </skos:definition>
		<skos:prefLabel>Sternberg delayed recognition task</skos:prefLabel>
		<skos:altLabel></skos:altLabel>
		<skos:related rdf:resource="http://cognitiveatlas.org/id/tsk_4a57abb9499e3"/>
		<skos:example>delayed match to sample task is a broader synonym of Sternberg delayed recognition task</skos:example>
</skos:Concept><skos:Concept rdf:about="http://cognitiveatlas.org/id/tsk_4a57abb949e1a"> <dc:identifier>tsk_4a57abb949e1a</dc:identifier>
		<dc:Title>Cognitive Atlas : Lexicon : stop signal task</dc:Title>
		<dc:Description>RDF output for 'stop signal task'</dc:Description>
		<dc:Type>InteractiveResource</dc:Type>
		<dc:Publisher>Cognitive Atlas</dc:Publisher>
		<dc:Creator>Cognitive Atlas RDF Generator</dc:Creator>
		<dc:Contributor>Russ Poldrack</dc:Contributor>
		<dc:Date>2010-01-06 06:56:52</dc:Date>
		<dc:Format>text/rdf</dc:Format>
		<dc:Language>en</dc:Language>
		<skos:editorialNote>Generated by testgen.php on Thu Jun 9 14:25:25 PDT 2011.</skos:editorialNote>
		<skos:historyNote>Revision 2: 1 previous definitions.</skos:historyNote>
		<skos:changeNote>See http://cognitiveatlas.org/id/tsk_4a57abb949e1a for complete revision history.</skos:changeNote>
		<skos:scopeNote>http://www.w3.org/2004/02/skos/core#Concept</skos:scopeNote>
		<skos:Note>SKOS properties defined in http://www.w3.org/TR/skos-primer/#secrel</skos:Note>
		<skos:inScheme rdf:resource="http://cognitiveatlas.org/tasks/"/>
		<skos:definition>A task in which an external stimulus signals the participant to interrupt an already-initiated motor response.</skos:definition>
		<skos:prefLabel>stop signal task</skos:prefLabel>
		<skos:altLabel></skos:altLabel>
		<skos:related rdf:resource="http://cognitiveatlas.org/id/trm_4a3fd79d0af66"/>
		<skos:related rdf:resource="http://cognitiveatlas.org/id/trm_4da4b203ad5ae"/>
		<skos:example>response inhibition is measured by the contrast of Stop Signal Reaction Time trials in the stop signal task</skos:example>
		<skos:example>selective stop signal task is descended from stop signal task</skos:example>
		<cito:citesForInformation rdf:resource="http://cognitiveatlas.org/citation/id/cit_4b44a76c5485b"/>
		<cito:citesForInformation rdf:resource="http://cognitiveatlas.org/citation/id/cit_4c6b6036b8b88"/>
</skos:Concept><skos:Concept rdf:about="http://cognitiveatlas.org/id/tsk_4a57abb949e27"> <dc:identifier>tsk_4a57abb949e27</dc:identifier>
		<dc:Title>Cognitive Atlas : Lexicon : Stroop task</dc:Title>
		<dc:Description>RDF output for 'Stroop task'</dc:Description>
		<dc:Type>InteractiveResource</dc:Type>
		<dc:Publisher>Cognitive Atlas</dc:Publisher>
		<dc:Creator>Cognitive Atlas RDF Generator</dc:Creator>
		<dc:Contributor>Brenda Gregory</dc:Contributor>
		<dc:Date>2011-04-19 12:10:14</dc:Date>
		<dc:Format>text/rdf</dc:Format>
		<dc:Language>en</dc:Language>
		<skos:editorialNote>Generated by testgen.php on Thu Jun 9 14:25:25 PDT 2011.</skos:editorialNote>
		<skos:historyNote>Revision 4: 3 previous definitions.</skos:historyNote>
		<skos:changeNote>See http://cognitiveatlas.org/id/tsk_4a57abb949e27 for complete revision history.</skos:changeNote>
		<skos:scopeNote>http://www.w3.org/2004/02/skos/core#Concept</skos:scopeNote>
		<skos:Note>SKOS properties defined in http://www.w3.org/TR/skos-primer/#secrel</skos:Note>
		<skos:inScheme rdf:resource="http://cognitiveatlas.org/tasks/"/>
		<skos:definition>measures selective attention, cognitive flexibility and processing speed, and it is used as a tool in the evaluation of executive functions. (from Wikipedia)

Subjects view color names presented in various ink colors and are instructed to name the color of the ink.  In incongruent stimuli, color names and ink colors are non-matching.  Also includes variations such as the Counting Stroop and Emotional Stroop. </skos:definition>
		<skos:prefLabel>Stroop task</skos:prefLabel>
		<skos:altLabel></skos:altLabel>
		<skos:related rdf:resource="http://cognitiveatlas.org/id/trm_4dadbfd771a54"/>
		<skos:related rdf:resource="http://cognitiveatlas.org/id/trm_4b843655d5d75"/>
		<skos:related rdf:resource="http://cognitiveatlas.org/id/trm_4b1968619b00b"/>
		<skos:related rdf:resource="http://cognitiveatlas.org/id/trm_4b1968619b00b"/>
		<skos:example>Picture-word Stroop task is descended from Stroop task</skos:example>
		<skos:example>Chimeric Animal Stroop Task is descended from Stroop task</skos:example>
		<skos:example>Color-word Stroop Task is descended from Stroop task</skos:example>
		<skos:example>Color-word Stroop Task is a narrower synonym of Stroop task</skos:example>
</skos:Concept><skos:Concept rdf:about="http://cognitiveatlas.org/id/tsk_4a57abb949e35"> <dc:identifier>tsk_4a57abb949e35</dc:identifier>
		<dc:Title>Cognitive Atlas : Lexicon : Structured Clinical Interview for Diagnostic and Statistical Manual of Mental Disorders (DSM-IV) Axis I Disorder</dc:Title>
		<dc:Description>RDF output for 'Structured Clinical Interview for Diagnostic and Statistical Manual of Mental Disorders (DSM-IV) Axis I Disorder'</dc:Description>
		<dc:Type>InteractiveResource</dc:Type>
		<dc:Publisher>Cognitive Atlas</dc:Publisher>
		<dc:Creator>Cognitive Atlas RDF Generator</dc:Creator>
		<dc:Contributor>Brenda Gregory</dc:Contributor>
		<dc:Date>2011-05-11 16:17:39</dc:Date>
		<dc:Format>text/rdf</dc:Format>
		<dc:Language>en</dc:Language>
		<skos:editorialNote>Generated by testgen.php on Thu Jun 9 14:25:25 PDT 2011.</skos:editorialNote>
		<skos:historyNote>Revision 3: 2 previous definitions.</skos:historyNote>
		<skos:changeNote>See http://cognitiveatlas.org/id/tsk_4a57abb949e35 for complete revision history.</skos:changeNote>
		<skos:scopeNote>http://www.w3.org/2004/02/skos/core#Concept</skos:scopeNote>
		<skos:Note>SKOS properties defined in http://www.w3.org/TR/skos-primer/#secrel</skos:Note>
		<skos:inScheme rdf:resource="http://cognitiveatlas.org/tasks/"/>
		<skos:definition>a diagnostic exam used to determine DSM-IV Axis I disorders (major mental disorders).</skos:definition>
		<skos:prefLabel>Structured Clinical Interview for Diagnostic and Statistical Manual of Mental Disorders (DSM-IV) Axis I Disorder</skos:prefLabel>
		<skos:altLabel></skos:altLabel>
</skos:Concept><skos:Concept rdf:about="http://cognitiveatlas.org/id/tsk_4a57abb949e44"> <dc:identifier>tsk_4a57abb949e44</dc:identifier>
		<dc:Title>Cognitive Atlas : Lexicon : symbol-digit substitution</dc:Title>
		<dc:Description>RDF output for 'symbol-digit substitution'</dc:Description>
		<dc:Type>InteractiveResource</dc:Type>
		<dc:Publisher>Cognitive Atlas</dc:Publisher>
		<dc:Creator>Cognitive Atlas RDF Generator</dc:Creator>
		<dc:Contributor>Natalie Picchetti</dc:Contributor>
		<dc:Date>2011-04-07 11:03:43</dc:Date>
		<dc:Format>text/rdf</dc:Format>
		<dc:Language>en</dc:Language>
		<skos:editorialNote>Generated by testgen.php on Thu Jun 9 14:25:25 PDT 2011.</skos:editorialNote>
		<skos:historyNote>Revision 3: 2 previous definitions.</skos:historyNote>
		<skos:changeNote>See http://cognitiveatlas.org/id/tsk_4a57abb949e44 for complete revision history.</skos:changeNote>
		<skos:scopeNote>http://www.w3.org/2004/02/skos/core#Concept</skos:scopeNote>
		<skos:Note>SKOS properties defined in http://www.w3.org/TR/skos-primer/#secrel</skos:Note>
		<skos:inScheme rdf:resource="http://cognitiveatlas.org/tasks/"/>
		<skos:definition>DSST is a neuropsychological test sensitive to brain damage, dementia, age and depression. It isn’t sensitive to the location of brain-damage (except for damage comprising part of the visual field). It consists of (e.g. nine) digit-symbol pairs (e.g. 1/-,2/┴ ... 7/Λ,8/X,9/=) followed by a list of digits. Under each digit the subject should write down the corresponding symbol as fast as possible. The number of correct symbols within the allowed time (e.g. 90 or 120 sec) is measured.
</skos:definition>
		<skos:prefLabel>symbol-digit substitution</skos:prefLabel>
		<skos:altLabel></skos:altLabel>
</skos:Concept><skos:Concept rdf:about="http://cognitiveatlas.org/id/tsk_4a57abb949e5b"> <dc:identifier>tsk_4a57abb949e5b</dc:identifier>
		<dc:Title>Cognitive Atlas : Lexicon : Symptom Checklist-90-Revised </dc:Title>
		<dc:Description>RDF output for 'Symptom Checklist-90-Revised '</dc:Description>
		<dc:Type>InteractiveResource</dc:Type>
		<dc:Publisher>Cognitive Atlas</dc:Publisher>
		<dc:Creator>Cognitive Atlas RDF Generator</dc:Creator>
		<dc:Contributor>Brenda Gregory</dc:Contributor>
		<dc:Date>2011-05-18 14:02:21</dc:Date>
		<dc:Format>text/rdf</dc:Format>
		<dc:Language>en</dc:Language>
		<skos:editorialNote>Generated by testgen.php on Thu Jun 9 14:25:25 PDT 2011.</skos:editorialNote>
		<skos:historyNote>Revision 3: 2 previous definitions.</skos:historyNote>
		<skos:changeNote>See http://cognitiveatlas.org/id/tsk_4a57abb949e5b for complete revision history.</skos:changeNote>
		<skos:scopeNote>http://www.w3.org/2004/02/skos/core#Concept</skos:scopeNote>
		<skos:Note>SKOS properties defined in http://www.w3.org/TR/skos-primer/#secrel</skos:Note>
		<skos:inScheme rdf:resource="http://cognitiveatlas.org/tasks/"/>
		<skos:definition>a relatively brief self-report psychometric instrument designed to evaluate a broad range of psychological problems and symptoms of psychopathology. It is also useful in measuring the progress and outcome of psychiatric and psychological treatments or for research purposes.</skos:definition>
		<skos:prefLabel>Symptom Checklist-90-Revised </skos:prefLabel>
		<skos:altLabel></skos:altLabel>
</skos:Concept><skos:Concept rdf:about="http://cognitiveatlas.org/id/tsk_4a57abb949e7c"> <dc:identifier>tsk_4a57abb949e7c</dc:identifier>
		<dc:Title>Cognitive Atlas : Lexicon : syntactic acceptability judgement task</dc:Title>
		<dc:Description>RDF output for 'syntactic acceptability judgement task'</dc:Description>
		<dc:Type>InteractiveResource</dc:Type>
		<dc:Publisher>Cognitive Atlas</dc:Publisher>
		<dc:Creator>Cognitive Atlas RDF Generator</dc:Creator>
		<dc:Contributor>System Administrator</dc:Contributor>
		<dc:Date>2009-07-10 14:06:33</dc:Date>
		<dc:Format>text/rdf</dc:Format>
		<dc:Language>en</dc:Language>
		<skos:editorialNote>Generated by testgen.php on Thu Jun 9 14:25:25 PDT 2011.</skos:editorialNote>
		<skos:historyNote>No previous definition revisions.</skos:historyNote>
		<skos:changeNote>This is the first and only definition provided.</skos:changeNote>
		<skos:scopeNote>http://www.w3.org/2004/02/skos/core#Concept</skos:scopeNote>
		<skos:Note>SKOS properties defined in http://www.w3.org/TR/skos-primer/#secrel</skos:Note>
		<skos:inScheme rdf:resource="http://cognitiveatlas.org/tasks/"/>
		<skos:definition>No definition submitted yet</skos:definition>
		<skos:prefLabel>syntactic acceptability judgement task</skos:prefLabel>
		<skos:altLabel></skos:altLabel>
</skos:Concept><skos:Concept rdf:about="http://cognitiveatlas.org/id/tsk_4a57abb949e8a"> <dc:identifier>tsk_4a57abb949e8a</dc:identifier>
		<dc:Title>Cognitive Atlas : Lexicon : task-switching </dc:Title>
		<dc:Description>RDF output for 'task-switching '</dc:Description>
		<dc:Type>InteractiveResource</dc:Type>
		<dc:Publisher>Cognitive Atlas</dc:Publisher>
		<dc:Creator>Cognitive Atlas RDF Generator</dc:Creator>
		<dc:Contributor>Agatha Lenartowicz</dc:Contributor>
		<dc:Date>2009-07-10 14:06:33</dc:Date>
		<dc:Format>text/rdf</dc:Format>
		<dc:Language>en</dc:Language>
		<skos:editorialNote>Generated by testgen.php on Thu Jun 9 14:25:25 PDT 2011.</skos:editorialNote>
		<skos:historyNote>No previous definition revisions.</skos:historyNote>
		<skos:changeNote>This is the first and only definition provided.</skos:changeNote>
		<skos:scopeNote>http://www.w3.org/2004/02/skos/core#Concept</skos:scopeNote>
		<skos:Note>SKOS properties defined in http://www.w3.org/TR/skos-primer/#secrel</skos:Note>
		<skos:inScheme rdf:resource="http://cognitiveatlas.org/tasks/"/>
		<skos:definition>A task in which participants alternate between two or more judgments typically regarding the same set of stimuli. Accuracy and reaction time are measured for each judgment.</skos:definition>
		<skos:prefLabel>task-switching </skos:prefLabel>
		<skos:altLabel></skos:altLabel>
</skos:Concept><skos:Concept rdf:about="http://cognitiveatlas.org/id/tsk_4a57abb949e98"> <dc:identifier>tsk_4a57abb949e98</dc:identifier>
		<dc:Title>Cognitive Atlas : Lexicon : Temporal discounting task</dc:Title>
		<dc:Description>RDF output for 'Temporal discounting task'</dc:Description>
		<dc:Type>InteractiveResource</dc:Type>
		<dc:Publisher>Cognitive Atlas</dc:Publisher>
		<dc:Creator>Cognitive Atlas RDF Generator</dc:Creator>
		<dc:Contributor>Natalie Picchetti</dc:Contributor>
		<dc:Date>2011-05-20 14:51:31</dc:Date>
		<dc:Format>text/rdf</dc:Format>
		<dc:Language>en</dc:Language>
		<skos:editorialNote>Generated by testgen.php on Thu Jun 9 14:25:25 PDT 2011.</skos:editorialNote>
		<skos:historyNote>Revision 2: 1 previous definitions.</skos:historyNote>
		<skos:changeNote>See http://cognitiveatlas.org/id/tsk_4a57abb949e98 for complete revision history.</skos:changeNote>
		<skos:scopeNote>http://www.w3.org/2004/02/skos/core#Concept</skos:scopeNote>
		<skos:Note>SKOS properties defined in http://www.w3.org/TR/skos-primer/#secrel</skos:Note>
		<skos:inScheme rdf:resource="http://cognitiveatlas.org/tasks/"/>
		<skos:definition>refers to the tendency of people to discount rewards as they approach a temporal horizon in the future or the past (i.e., become so distant in time that they cease to be valuable or to have additive effects). To put it another way, it is a tendency to give greater value to rewards as they move away from their temporal horizons and towards the &#34;now&#34;. For instance, a nicotine deprived smoker may highly value a cigarette available any time in the next 6 hours but assign little or no value to a cigarette available in 6 months.</skos:definition>
		<skos:prefLabel>Temporal discounting task</skos:prefLabel>
		<skos:altLabel></skos:altLabel>
</skos:Concept><skos:Concept rdf:about="http://cognitiveatlas.org/id/tsk_4a57abb949ea5"> <dc:identifier>tsk_4a57abb949ea5</dc:identifier>
		<dc:Title>Cognitive Atlas : Lexicon : Test of Word Reading Efficiency</dc:Title>
		<dc:Description>RDF output for 'Test of Word Reading Efficiency'</dc:Description>
		<dc:Type>InteractiveResource</dc:Type>
		<dc:Publisher>Cognitive Atlas</dc:Publisher>
		<dc:Creator>Cognitive Atlas RDF Generator</dc:Creator>
		<dc:Contributor>Brenda Gregory</dc:Contributor>
		<dc:Date>2011-04-28 17:27:36</dc:Date>
		<dc:Format>text/rdf</dc:Format>
		<dc:Language>en</dc:Language>
		<skos:editorialNote>Generated by testgen.php on Thu Jun 9 14:25:25 PDT 2011.</skos:editorialNote>
		<skos:historyNote>Revision 3: 2 previous definitions.</skos:historyNote>
		<skos:changeNote>See http://cognitiveatlas.org/id/tsk_4a57abb949ea5 for complete revision history.</skos:changeNote>
		<skos:scopeNote>http://www.w3.org/2004/02/skos/core#Concept</skos:scopeNote>
		<skos:Note>SKOS properties defined in http://www.w3.org/TR/skos-primer/#secrel</skos:Note>
		<skos:inScheme rdf:resource="http://cognitiveatlas.org/tasks/"/>
		<skos:definition>a nationally normed measure of word reading accuracy and fluency that provides an efficient means of monitoring the growth of two kinds of word reading skills that are critical in the development of overall reading ability: the ability to accurately recognize familiar words as whole units or “sight words” and the ability to “sound out” words quickly. </skos:definition>
		<skos:prefLabel>Test of Word Reading Efficiency</skos:prefLabel>
		<skos:altLabel></skos:altLabel>
</skos:Concept><skos:Concept rdf:about="http://cognitiveatlas.org/id/tsk_4a57abb949eb3"> <dc:identifier>tsk_4a57abb949eb3</dc:identifier>
		<dc:Title>Cognitive Atlas : Lexicon : Tobacco Craving Questionnaire</dc:Title>
		<dc:Description>RDF output for 'Tobacco Craving Questionnaire'</dc:Description>
		<dc:Type>InteractiveResource</dc:Type>
		<dc:Publisher>Cognitive Atlas</dc:Publisher>
		<dc:Creator>Cognitive Atlas RDF Generator</dc:Creator>
		<dc:Contributor>Natalie Picchetti</dc:Contributor>
		<dc:Date>2011-04-11 15:21:30</dc:Date>
		<dc:Format>text/rdf</dc:Format>
		<dc:Language>en</dc:Language>
		<skos:editorialNote>Generated by testgen.php on Thu Jun 9 14:25:25 PDT 2011.</skos:editorialNote>
		<skos:historyNote>Revision 3: 2 previous definitions.</skos:historyNote>
		<skos:changeNote>See http://cognitiveatlas.org/id/tsk_4a57abb949eb3 for complete revision history.</skos:changeNote>
		<skos:scopeNote>http://www.w3.org/2004/02/skos/core#Concept</skos:scopeNote>
		<skos:Note>SKOS properties defined in http://www.w3.org/TR/skos-primer/#secrel</skos:Note>
		<skos:inScheme rdf:resource="http://cognitiveatlas.org/tasks/"/>
		<skos:definition>a multidimensional questionnaire to assess tobacco craving.  It consists of a 47-item TCQ and other forms assessing demographics, tobacco and other drug use history, quit attempts, and current mood.  It represents four specific constructs that characterize craving for tobacco: (a) Emotionality, or smoking in anticipation of relief from withdrawal symptoms or negative mood, (b) expectancy, or anticipation of positive outcomes from smoking, (c) compulsivity, or an inability to control tobacco use, and (d) purposefulness, or intention and planning to smoke for positive outcomes.  It is an instrument for assessing tobacco craving in individuals not attempting to reduce or quit smoking.
</skos:definition>
		<skos:prefLabel>Tobacco Craving Questionnaire</skos:prefLabel>
		<skos:altLabel></skos:altLabel>
		<cito:citesForInformation rdf:resource="http://cognitiveatlas.org/citation/id/cit_4da37ea20ce3d"/>
</skos:Concept><skos:Concept rdf:about="http://cognitiveatlas.org/id/tsk_4a57abb949ec0"> <dc:identifier>tsk_4a57abb949ec0</dc:identifier>
		<dc:Title>Cognitive Atlas : Lexicon : Trail Making Test A and B</dc:Title>
		<dc:Description>RDF output for 'Trail Making Test A and B'</dc:Description>
		<dc:Type>InteractiveResource</dc:Type>
		<dc:Publisher>Cognitive Atlas</dc:Publisher>
		<dc:Creator>Cognitive Atlas RDF Generator</dc:Creator>
		<dc:Contributor>Agatha Lenartowicz</dc:Contributor>
		<dc:Date>2009-07-10 14:06:33</dc:Date>
		<dc:Format>text/rdf</dc:Format>
		<dc:Language>en</dc:Language>
		<skos:editorialNote>Generated by testgen.php on Thu Jun 9 14:25:25 PDT 2011.</skos:editorialNote>
		<skos:historyNote>No previous definition revisions.</skos:historyNote>
		<skos:changeNote>This is the first and only definition provided.</skos:changeNote>
		<skos:scopeNote>http://www.w3.org/2004/02/skos/core#Concept</skos:scopeNote>
		<skos:Note>SKOS properties defined in http://www.w3.org/TR/skos-primer/#secrel</skos:Note>
		<skos:inScheme rdf:resource="http://cognitiveatlas.org/tasks/"/>
		<skos:definition>A neuropsychological test in which participants must connect-the-dots (traverse between items) according to some specified order. In Test A these items are numbers (1,2,3 etc.) and the order is determined by increasing magnitude. In Test B these items are both numbers and letters (1,2,3, A,B,C etc.) and the order is determined by a combination of increasing numbers AND letters (e.g., 1 A 2 B 3 C..) requiring participants to alternate between letters and numbers.</skos:definition>
		<skos:prefLabel>Trail Making Test A and B</skos:prefLabel>
		<skos:altLabel></skos:altLabel>
</skos:Concept><skos:Concept rdf:about="http://cognitiveatlas.org/id/tsk_4a57abb949ece"> <dc:identifier>tsk_4a57abb949ece</dc:identifier>
		<dc:Title>Cognitive Atlas : Lexicon : Unified Parkinson's Disease Rating Scale</dc:Title>
		<dc:Description>RDF output for 'Unified Parkinson's Disease Rating Scale'</dc:Description>
		<dc:Type>InteractiveResource</dc:Type>
		<dc:Publisher>Cognitive Atlas</dc:Publisher>
		<dc:Creator>Cognitive Atlas RDF Generator</dc:Creator>
		<dc:Contributor>Brenda Gregory</dc:Contributor>
		<dc:Date>2011-05-16 11:26:33</dc:Date>
		<dc:Format>text/rdf</dc:Format>
		<dc:Language>en</dc:Language>
		<skos:editorialNote>Generated by testgen.php on Thu Jun 9 14:25:25 PDT 2011.</skos:editorialNote>
		<skos:historyNote>Revision 3: 2 previous definitions.</skos:historyNote>
		<skos:changeNote>See http://cognitiveatlas.org/id/tsk_4a57abb949ece for complete revision history.</skos:changeNote>
		<skos:scopeNote>http://www.w3.org/2004/02/skos/core#Concept</skos:scopeNote>
		<skos:Note>SKOS properties defined in http://www.w3.org/TR/skos-primer/#secrel</skos:Note>
		<skos:inScheme rdf:resource="http://cognitiveatlas.org/tasks/"/>
		<skos:definition>a rating scale used to follow the longitudinal course of Parkinson&#39;s disease, made up of the following sections: (1)evaluation of Mentation, behavior, and mood, (2)self evaluation of the activities of daily life (ADLs), (3)clinician-scored motor evaluation, (4)Hoehn and Yahr stating of severity of Parkinson disease, (5)Schwab and England ADL scale; these are evaluated by interview and clinical observation.</skos:definition>
		<skos:prefLabel>Unified Parkinson's Disease Rating Scale</skos:prefLabel>
		<skos:altLabel></skos:altLabel>
</skos:Concept><skos:Concept rdf:about="http://cognitiveatlas.org/id/tsk_4a57abb949edb"> <dc:identifier>tsk_4a57abb949edb</dc:identifier>
		<dc:Title>Cognitive Atlas : Lexicon : visual alignment task </dc:Title>
		<dc:Description>RDF output for 'visual alignment task '</dc:Description>
		<dc:Type>InteractiveResource</dc:Type>
		<dc:Publisher>Cognitive Atlas</dc:Publisher>
		<dc:Creator>Cognitive Atlas RDF Generator</dc:Creator>
		<dc:Contributor>System Administrator</dc:Contributor>
		<dc:Date>2009-07-10 14:06:33</dc:Date>
		<dc:Format>text/rdf</dc:Format>
		<dc:Language>en</dc:Language>
		<skos:editorialNote>Generated by testgen.php on Thu Jun 9 14:25:25 PDT 2011.</skos:editorialNote>
		<skos:historyNote>No previous definition revisions.</skos:historyNote>
		<skos:changeNote>This is the first and only definition provided.</skos:changeNote>
		<skos:scopeNote>http://www.w3.org/2004/02/skos/core#Concept</skos:scopeNote>
		<skos:Note>SKOS properties defined in http://www.w3.org/TR/skos-primer/#secrel</skos:Note>
		<skos:inScheme rdf:resource="http://cognitiveatlas.org/tasks/"/>
		<skos:definition>No definition submitted yet</skos:definition>
		<skos:prefLabel>visual alignment task </skos:prefLabel>
		<skos:altLabel></skos:altLabel>
</skos:Concept><skos:Concept rdf:about="http://cognitiveatlas.org/id/tsk_4a57abb949ee9"> <dc:identifier>tsk_4a57abb949ee9</dc:identifier>
		<dc:Title>Cognitive Atlas : Lexicon : visuospatial cueing task</dc:Title>
		<dc:Description>RDF output for 'visuospatial cueing task'</dc:Description>
		<dc:Type>InteractiveResource</dc:Type>
		<dc:Publisher>Cognitive Atlas</dc:Publisher>
		<dc:Creator>Cognitive Atlas RDF Generator</dc:Creator>
		<dc:Contributor>System Administrator</dc:Contributor>
		<dc:Date>2009-07-10 14:06:33</dc:Date>
		<dc:Format>text/rdf</dc:Format>
		<dc:Language>en</dc:Language>
		<skos:editorialNote>Generated by testgen.php on Thu Jun 9 14:25:25 PDT 2011.</skos:editorialNote>
		<skos:historyNote>No previous definition revisions.</skos:historyNote>
		<skos:changeNote>This is the first and only definition provided.</skos:changeNote>
		<skos:scopeNote>http://www.w3.org/2004/02/skos/core#Concept</skos:scopeNote>
		<skos:Note>SKOS properties defined in http://www.w3.org/TR/skos-primer/#secrel</skos:Note>
		<skos:inScheme rdf:resource="http://cognitiveatlas.org/tasks/"/>
		<skos:definition>No definition submitted yet</skos:definition>
		<skos:prefLabel>visuospatial cueing task</skos:prefLabel>
		<skos:altLabel></skos:altLabel>
</skos:Concept><skos:Concept rdf:about="http://cognitiveatlas.org/id/tsk_4a57abb949ef7"> <dc:identifier>tsk_4a57abb949ef7</dc:identifier>
		<dc:Title>Cognitive Atlas : Lexicon : Warrington's Face/Word Recognition Test</dc:Title>
		<dc:Description>RDF output for 'Warrington's Face/Word Recognition Test'</dc:Description>
		<dc:Type>InteractiveResource</dc:Type>
		<dc:Publisher>Cognitive Atlas</dc:Publisher>
		<dc:Creator>Cognitive Atlas RDF Generator</dc:Creator>
		<dc:Contributor>System Administrator</dc:Contributor>
		<dc:Date>2009-07-10 14:06:33</dc:Date>
		<dc:Format>text/rdf</dc:Format>
		<dc:Language>en</dc:Language>
		<skos:editorialNote>Generated by testgen.php on Thu Jun 9 14:25:25 PDT 2011.</skos:editorialNote>
		<skos:historyNote>No previous definition revisions.</skos:historyNote>
		<skos:changeNote>This is the first and only definition provided.</skos:changeNote>
		<skos:scopeNote>http://www.w3.org/2004/02/skos/core#Concept</skos:scopeNote>
		<skos:Note>SKOS properties defined in http://www.w3.org/TR/skos-primer/#secrel</skos:Note>
		<skos:inScheme rdf:resource="http://cognitiveatlas.org/tasks/"/>
		<skos:definition>No definition submitted yet</skos:definition>
		<skos:prefLabel>Warrington's Face/Word Recognition Test</skos:prefLabel>
		<skos:altLabel></skos:altLabel>
</skos:Concept><skos:Concept rdf:about="http://cognitiveatlas.org/id/tsk_4a57abb949f04"> <dc:identifier>tsk_4a57abb949f04</dc:identifier>
		<dc:Title>Cognitive Atlas : Lexicon : Wechsler Adult Intelligence Scale-Revised</dc:Title>
		<dc:Description>RDF output for 'Wechsler Adult Intelligence Scale-Revised'</dc:Description>
		<dc:Type>InteractiveResource</dc:Type>
		<dc:Publisher>Cognitive Atlas</dc:Publisher>
		<dc:Creator>Cognitive Atlas RDF Generator</dc:Creator>
		<dc:Contributor>Brenda Gregory</dc:Contributor>
		<dc:Date>2011-05-16 10:54:51</dc:Date>
		<dc:Format>text/rdf</dc:Format>
		<dc:Language>en</dc:Language>
		<skos:editorialNote>Generated by testgen.php on Thu Jun 9 14:25:25 PDT 2011.</skos:editorialNote>
		<skos:historyNote>Revision 3: 2 previous definitions.</skos:historyNote>
		<skos:changeNote>See http://cognitiveatlas.org/id/tsk_4a57abb949f04 for complete revision history.</skos:changeNote>
		<skos:scopeNote>http://www.w3.org/2004/02/skos/core#Concept</skos:scopeNote>
		<skos:Note>SKOS properties defined in http://www.w3.org/TR/skos-primer/#secrel</skos:Note>
		<skos:inScheme rdf:resource="http://cognitiveatlas.org/tasks/"/>
		<skos:definition>a general test of intelligence, which Wechsler defined as, &#34;... the global capacity of the individual to act purposefully, to think rationally, and to deal effectively with his environment.&#34; In keeping with this definition of intelligence as an aggregate of mental aptitudes or abilities, the WAIS-R consists of 11 subtests divided into two parts, verbal and performance.</skos:definition>
		<skos:prefLabel>Wechsler Adult Intelligence Scale-Revised</skos:prefLabel>
		<skos:altLabel></skos:altLabel>
</skos:Concept><skos:Concept rdf:about="http://cognitiveatlas.org/id/tsk_4a57abb949f12"> <dc:identifier>tsk_4a57abb949f12</dc:identifier>
		<dc:Title>Cognitive Atlas : Lexicon : Wechsler Adult Intelligence Scale - Revised</dc:Title>
		<dc:Description>RDF output for 'Wechsler Adult Intelligence Scale - Revised'</dc:Description>
		<dc:Type>InteractiveResource</dc:Type>
		<dc:Publisher>Cognitive Atlas</dc:Publisher>
		<dc:Creator>Cognitive Atlas RDF Generator</dc:Creator>
		<dc:Contributor>Brenda Gregory</dc:Contributor>
		<dc:Date>2011-04-29 11:00:03</dc:Date>
		<dc:Format>text/rdf</dc:Format>
		<dc:Language>en</dc:Language>
		<skos:editorialNote>Generated by testgen.php on Thu Jun 9 14:25:25 PDT 2011.</skos:editorialNote>
		<skos:historyNote>Revision 3: 2 previous definitions.</skos:historyNote>
		<skos:changeNote>See http://cognitiveatlas.org/id/tsk_4a57abb949f12 for complete revision history.</skos:changeNote>
		<skos:scopeNote>http://www.w3.org/2004/02/skos/core#Concept</skos:scopeNote>
		<skos:Note>SKOS properties defined in http://www.w3.org/TR/skos-primer/#secrel</skos:Note>
		<skos:inScheme rdf:resource="http://cognitiveatlas.org/tasks/"/>
		<skos:definition>used with adults ages 16 to 90 and measures cognitive ability using a core battery of 10 unique subtests that focus on four specific domains of intelligence: verbal comprehension, perceptual reasoning, working memory, and processing speed. </skos:definition>
		<skos:prefLabel>Wechsler Adult Intelligence Scale - Revised</skos:prefLabel>
		<skos:altLabel></skos:altLabel>
		<skos:related rdf:resource="http://cognitiveatlas.org/id/tsk_4a57abb94989b"/>
		<skos:related rdf:resource="http://cognitiveatlas.org/id/trm_4b7497a289534"/>
		<skos:related rdf:resource="http://cognitiveatlas.org/id/tsk_4a57abb949a25"/>
		<skos:example>Backward digit span task is related to Wechsler Adult Intelligence Scale - Revised</skos:example>
		<skos:example>Block Design Test is descended from Wechsler Adult Intelligence Scale - Revised</skos:example>
		<skos:example>Digit/Symbol Coding test is descended from Wechsler Adult Intelligence Scale - Revised</skos:example>
</skos:Concept><skos:Concept rdf:about="http://cognitiveatlas.org/id/tsk_4a57abb949f21"> <dc:identifier>tsk_4a57abb949f21</dc:identifier>
		<dc:Title>Cognitive Atlas : Lexicon : Wisconsin Card Sorting test</dc:Title>
		<dc:Description>RDF output for 'Wisconsin Card Sorting test'</dc:Description>
		<dc:Type>InteractiveResource</dc:Type>
		<dc:Publisher>Cognitive Atlas</dc:Publisher>
		<dc:Creator>Cognitive Atlas RDF Generator</dc:Creator>
		<dc:Contributor>Russ Poldrack</dc:Contributor>
		<dc:Date>2010-02-17 07:05:44</dc:Date>
		<dc:Format>text/rdf</dc:Format>
		<dc:Language>en</dc:Language>
		<skos:editorialNote>Generated by testgen.php on Thu Jun 9 14:25:25 PDT 2011.</skos:editorialNote>
		<skos:historyNote>Revision 3: 2 previous definitions.</skos:historyNote>
		<skos:changeNote>See http://cognitiveatlas.org/id/tsk_4a57abb949f21 for complete revision history.</skos:changeNote>
		<skos:scopeNote>http://www.w3.org/2004/02/skos/core#Concept</skos:scopeNote>
		<skos:Note>SKOS properties defined in http://www.w3.org/TR/skos-primer/#secrel</skos:Note>
		<skos:inScheme rdf:resource="http://cognitiveatlas.org/tasks/"/>
		<skos:definition>The participant is presented with stimulus cards with shapes on them.  The cards differ in color of the shapes, number of the shapes, and the form of the shapes. The participant is asked to sort these cards into two piles. The participant is not told what stimulus dimension to use in order to sort the cards, but the administrator tells the participant if a particular match is correct. During the test, the sorting rules are changed and the participant must discover the new sorting rule in order to be successful. </skos:definition>
		<skos:prefLabel>Wisconsin Card Sorting test</skos:prefLabel>
		<skos:altLabel></skos:altLabel>
		<skos:related rdf:resource="http://cognitiveatlas.org/id/trm_4a3fd79d0b613"/>
		<skos:related rdf:resource="http://cognitiveatlas.org/id/trm_4a3fd79d0b5a7"/>
		<skos:related rdf:resource="http://cognitiveatlas.org/id/tsk_4a57abb949ad7"/>
		<skos:example>task switching is measured by the contrast of Perseverative errors trials in the Wisconsin Card Sorting test</skos:example>
		<skos:example>working memory is measured by the contrast of Failure to maintain set trials in the Wisconsin Card Sorting test</skos:example>
		<skos:example>Intradimensional shift task is a broader synonym of Wisconsin Card Sorting test</skos:example>
</skos:Concept><skos:Concept rdf:about="http://cognitiveatlas.org/id/tsk_4a57abb949f2f"> <dc:identifier>tsk_4a57abb949f2f</dc:identifier>
		<dc:Title>Cognitive Atlas : Lexicon : word attack</dc:Title>
		<dc:Description>RDF output for 'word attack'</dc:Description>
		<dc:Type>InteractiveResource</dc:Type>
		<dc:Publisher>Cognitive Atlas</dc:Publisher>
		<dc:Creator>Cognitive Atlas RDF Generator</dc:Creator>
		<dc:Contributor>System Administrator</dc:Contributor>
		<dc:Date>2009-07-10 14:06:33</dc:Date>
		<dc:Format>text/rdf</dc:Format>
		<dc:Language>en</dc:Language>
		<skos:editorialNote>Generated by testgen.php on Thu Jun 9 14:25:25 PDT 2011.</skos:editorialNote>
		<skos:historyNote>No previous definition revisions.</skos:historyNote>
		<skos:changeNote>This is the first and only definition provided.</skos:changeNote>
		<skos:scopeNote>http://www.w3.org/2004/02/skos/core#Concept</skos:scopeNote>
		<skos:Note>SKOS properties defined in http://www.w3.org/TR/skos-primer/#secrel</skos:Note>
		<skos:inScheme rdf:resource="http://cognitiveatlas.org/tasks/"/>
		<skos:definition>No definition submitted yet</skos:definition>
		<skos:prefLabel>word attack</skos:prefLabel>
		<skos:altLabel></skos:altLabel>
</skos:Concept><skos:Concept rdf:about="http://cognitiveatlas.org/id/tsk_4a57abb949f3d"> <dc:identifier>tsk_4a57abb949f3d</dc:identifier>
		<dc:Title>Cognitive Atlas : Lexicon : Word generation task</dc:Title>
		<dc:Description>RDF output for 'Word generation task'</dc:Description>
		<dc:Type>InteractiveResource</dc:Type>
		<dc:Publisher>Cognitive Atlas</dc:Publisher>
		<dc:Creator>Cognitive Atlas RDF Generator</dc:Creator>
		<dc:Contributor>Brenda Gregory</dc:Contributor>
		<dc:Date>2011-04-19 12:06:57</dc:Date>
		<dc:Format>text/rdf</dc:Format>
		<dc:Language>en</dc:Language>
		<skos:editorialNote>Generated by testgen.php on Thu Jun 9 14:25:25 PDT 2011.</skos:editorialNote>
		<skos:historyNote>Revision 3: 2 previous definitions.</skos:historyNote>
		<skos:changeNote>See http://cognitiveatlas.org/id/tsk_4a57abb949f3d for complete revision history.</skos:changeNote>
		<skos:scopeNote>http://www.w3.org/2004/02/skos/core#Concept</skos:scopeNote>
		<skos:Note>SKOS properties defined in http://www.w3.org/TR/skos-primer/#secrel</skos:Note>
		<skos:inScheme rdf:resource="http://cognitiveatlas.org/tasks/"/>
		<skos:definition>Covert: Semantic: subjects listen to or view nouns and silently generate an associated verb, or subjects view a category and silently generate as many exemplars as possible; Orthographic: subjects listen to or view a letter and silently generate as many words as possible that start with that letter; Phonologic: subjects listen to or view a word and silently generate words that rhyme. 

Overt: semantic: subjects listen to or view nouns and overtly generate an associated verb, or subjects view a category and overtly generate as many exemplars as possible; Orthographic: subjects listen to or view a letter and overtly generate as many words as possible that start with that letter; Phonologic: subjects listen to or view a word and overtly generate words that rhyme.</skos:definition>
		<skos:prefLabel>Word generation task</skos:prefLabel>
		<skos:altLabel></skos:altLabel>
</skos:Concept><skos:Concept rdf:about="http://cognitiveatlas.org/id/tsk_4a57abb949f4a"> <dc:identifier>tsk_4a57abb949f4a</dc:identifier>
		<dc:Title>Cognitive Atlas : Lexicon : word identification</dc:Title>
		<dc:Description>RDF output for 'word identification'</dc:Description>
		<dc:Type>InteractiveResource</dc:Type>
		<dc:Publisher>Cognitive Atlas</dc:Publisher>
		<dc:Creator>Cognitive Atlas RDF Generator</dc:Creator>
		<dc:Contributor>Natalie Picchetti</dc:Contributor>
		<dc:Date>2011-04-15 12:01:55</dc:Date>
		<dc:Format>text/rdf</dc:Format>
		<dc:Language>en</dc:Language>
		<skos:editorialNote>Generated by testgen.php on Thu Jun 9 14:25:25 PDT 2011.</skos:editorialNote>
		<skos:historyNote>Revision 3: 2 previous definitions.</skos:historyNote>
		<skos:changeNote>See http://cognitiveatlas.org/id/tsk_4a57abb949f4a for complete revision history.</skos:changeNote>
		<skos:scopeNote>http://www.w3.org/2004/02/skos/core#Concept</skos:scopeNote>
		<skos:Note>SKOS properties defined in http://www.w3.org/TR/skos-primer/#secrel</skos:Note>
		<skos:inScheme rdf:resource="http://cognitiveatlas.org/tasks/"/>
		<skos:definition>is the process of determining the pronunciation and some degree of meaning of an unknown word. Note: Word- identification skills commonly taught are phonic analysis, structural analysis, context clues, configuration clues, dictionary skills, and sometimes picture clues.
</skos:definition>
		<skos:prefLabel>word identification</skos:prefLabel>
		<skos:altLabel></skos:altLabel>
</skos:Concept><skos:Concept rdf:about="http://cognitiveatlas.org/id/trm_4d54b2cc0f943"> <dc:identifier>trm_4d54b2cc0f943</dc:identifier>
		<dc:Title>Cognitive Atlas : Lexicon : Cambridge Gambling Task</dc:Title>
		<dc:Description>RDF output for 'Cambridge Gambling Task'</dc:Description>
		<dc:Type>InteractiveResource</dc:Type>
		<dc:Publisher>Cognitive Atlas</dc:Publisher>
		<dc:Creator>Cognitive Atlas RDF Generator</dc:Creator>
		<dc:Contributor>Tom Schonberg</dc:Contributor>
		<dc:Date>2011-02-10 19:53:48</dc:Date>
		<dc:Format>text/rdf</dc:Format>
		<dc:Language>en</dc:Language>
		<skos:editorialNote>Generated by testgen.php on Thu Jun 9 14:25:25 PDT 2011.</skos:editorialNote>
		<skos:historyNote>No previous definition revisions.</skos:historyNote>
		<skos:changeNote>This is the first and only definition provided.</skos:changeNote>
		<skos:scopeNote>http://www.w3.org/2004/02/skos/core#Concept</skos:scopeNote>
		<skos:Note>SKOS properties defined in http://www.w3.org/TR/skos-primer/#secrel</skos:Note>
		<skos:inScheme rdf:resource="http://cognitiveatlas.org/tasks/"/>
		<skos:definition>A behavioral task intended to measure risky decision making by subjects.
A token is hidden under one of six boxes that are each one of two colors.Different trials
have different ratios between box colors(3:3,4:2,5:1).On each trial,participants choose a
color on which to bet.The color with the higher probability (more boxes) is associated with
lower potential gains and lower potential losses of points than is the color with lower
probability. </skos:definition>
		<skos:prefLabel>Cambridge Gambling Task</skos:prefLabel>
		<skos:altLabel></skos:altLabel>
		<skos:related rdf:resource="http://cognitiveatlas.org/id/trm_4a3fd79d0b64e"/>
		<skos:related rdf:resource="http://cognitiveatlas.org/id/trm_4b6525253c63f"/>
		<skos:related rdf:resource="http://cognitiveatlas.org/id/trm_4d55a2bbcfdff"/>
		<skos:related rdf:resource="http://cognitiveatlas.org/id/tsk_4a57abb949ae5"/>
		<skos:example>Cambridge Gambling Task is a narrower synonym of Choice task between risky and non-risky options</skos:example>
		<skos:example>Cambridge Gambling Task is related to Iowa Gambling Task</skos:example>
		<skos:example>risk seeking is measured by the contrast of correct answers times probability of each color trials in the Cambridge Gambling Task</skos:example>
		<skos:example>reward is measured by the contrast of ratio trials in the Cambridge Gambling Task</skos:example>
		<cito:citesForInformation rdf:resource="http://cognitiveatlas.org/citation/id/cit_4d54b48147b06"/>
		<cito:citesForInformation rdf:resource="http://cognitiveatlas.org/citation/id/cit_4de6b6e412117"/>
		<cito:citesForInformation rdf:resource="http://cognitiveatlas.org/citation/id/cit_4de6b72e283ad"/>
</skos:Concept><skos:Concept rdf:about="http://cognitiveatlas.org/id/trm_4d54b61a14a14"> <dc:identifier>trm_4d54b61a14a14</dc:identifier>
		<dc:Title>Cognitive Atlas : Lexicon : Probabilistic gambling task</dc:Title>
		<dc:Description>RDF output for 'Probabilistic gambling task'</dc:Description>
		<dc:Type>InteractiveResource</dc:Type>
		<dc:Publisher>Cognitive Atlas</dc:Publisher>
		<dc:Creator>Cognitive Atlas RDF Generator</dc:Creator>
		<dc:Contributor>Tom Schonberg</dc:Contributor>
		<dc:Date>2011-02-11 13:02:24</dc:Date>
		<dc:Format>text/rdf</dc:Format>
		<dc:Language>en</dc:Language>
		<skos:editorialNote>Generated by testgen.php on Thu Jun 9 14:25:25 PDT 2011.</skos:editorialNote>
		<skos:historyNote>Revision 2: 1 previous definitions.</skos:historyNote>
		<skos:changeNote>See http://cognitiveatlas.org/id/trm_4d54b61a14a14 for complete revision history.</skos:changeNote>
		<skos:scopeNote>http://www.w3.org/2004/02/skos/core#Concept</skos:scopeNote>
		<skos:Note>SKOS properties defined in http://www.w3.org/TR/skos-primer/#secrel</skos:Note>
		<skos:inScheme rdf:resource="http://cognitiveatlas.org/tasks/"/>
		<skos:definition>Two cards are drawn without replacement from a deck containing cards numbered from one to ten (one of each). After the first card is presented, participants bet whether the next card will be higher or lower than the first card. Thus there is maximal risk when the first card is five or six, zero risk when it is ten or one. 

In later version of the task participants bet on whether the second card will be higher or lower before seeing the first card.</skos:definition>
		<skos:prefLabel>Probabilistic gambling task</skos:prefLabel>
		<skos:altLabel></skos:altLabel>
		<cito:citesForInformation rdf:resource="http://cognitiveatlas.org/citation/id/cit_4d54b62d050c7"/>
		<cito:citesForInformation rdf:resource="http://cognitiveatlas.org/citation/id/cit_4d54b63f0dcd8"/>
		<cito:citesForInformation rdf:resource="http://cognitiveatlas.org/citation/id/cit_4d54b673a9469"/>
</skos:Concept><skos:Concept rdf:about="http://cognitiveatlas.org/id/trm_4d54b8361e93e"> <dc:identifier>trm_4d54b8361e93e</dc:identifier>
		<dc:Title>Cognitive Atlas : Lexicon : Behavioral Investment allocation strategy (BIAS)</dc:Title>
		<dc:Description>RDF output for 'Behavioral Investment allocation strategy (BIAS)'</dc:Description>
		<dc:Type>InteractiveResource</dc:Type>
		<dc:Publisher>Cognitive Atlas</dc:Publisher>
		<dc:Creator>Cognitive Atlas RDF Generator</dc:Creator>
		<dc:Contributor>Tom Schonberg</dc:Contributor>
		<dc:Date>2011-02-10 20:16:54</dc:Date>
		<dc:Format>text/rdf</dc:Format>
		<dc:Language>en</dc:Language>
		<skos:editorialNote>Generated by testgen.php on Thu Jun 9 14:25:25 PDT 2011.</skos:editorialNote>
		<skos:historyNote>No previous definition revisions.</skos:historyNote>
		<skos:changeNote>This is the first and only definition provided.</skos:changeNote>
		<skos:scopeNote>http://www.w3.org/2004/02/skos/core#Concept</skos:scopeNote>
		<skos:Note>SKOS properties defined in http://www.w3.org/TR/skos-primer/#secrel</skos:Note>
		<skos:inScheme rdf:resource="http://cognitiveatlas.org/tasks/"/>
		<skos:definition>On each trial, participants choose between two stocks (gain/loss gambles, one stochastically dominating the other) and one bond (a sure gain of $1). They must learn through trial-and-error the characteristics of the stocks, which change over blocks of trials. Feedback on payoffs of the forgone options is presented on each trial. </skos:definition>
		<skos:prefLabel>Behavioral Investment allocation strategy (BIAS)</skos:prefLabel>
		<skos:altLabel></skos:altLabel>
		<skos:related rdf:resource="http://cognitiveatlas.org/id/trm_4d55a2bbcfdff"/>
		<skos:example>Behavioral Investment allocation strategy (BIAS) is a narrower synonym of Choice task between risky and non-risky options</skos:example>
		<cito:citesForInformation rdf:resource="http://cognitiveatlas.org/citation/id/cit_4d54b861dc450"/>
		<cito:citesForInformation rdf:resource="http://cognitiveatlas.org/citation/id/cit_4de57c44b29d6"/>
</skos:Concept><skos:Concept rdf:about="http://cognitiveatlas.org/id/trm_4d55997cd3edb"> <dc:identifier>trm_4d55997cd3edb</dc:identifier>
		<dc:Title>Cognitive Atlas : Lexicon : Non-choice task to study expected value and uncertainty</dc:Title>
		<dc:Description>RDF output for 'Non-choice task to study expected value and uncertainty'</dc:Description>
		<dc:Type>InteractiveResource</dc:Type>
		<dc:Publisher>Cognitive Atlas</dc:Publisher>
		<dc:Creator>Cognitive Atlas RDF Generator</dc:Creator>
		<dc:Contributor>Tom Schonberg</dc:Contributor>
		<dc:Date>2011-02-11 12:18:04</dc:Date>
		<dc:Format>text/rdf</dc:Format>
		<dc:Language>en</dc:Language>
		<skos:editorialNote>Generated by testgen.php on Thu Jun 9 14:25:25 PDT 2011.</skos:editorialNote>
		<skos:historyNote>No previous definition revisions.</skos:historyNote>
		<skos:changeNote>This is the first and only definition provided.</skos:changeNote>
		<skos:scopeNote>http://www.w3.org/2004/02/skos/core#Concept</skos:scopeNote>
		<skos:Note>SKOS properties defined in http://www.w3.org/TR/skos-primer/#secrel</skos:Note>
		<skos:inScheme rdf:resource="http://cognitiveatlas.org/tasks/"/>
		<skos:definition>Each of 12 stimuli (circles of different colors, numbers and sizes) is associated with a different reward magnitude and probability. These include all combinations of (100 and 200) point rewards with (0, 0.25, 0.5, 0.75 and 1) probabilities, plus 300 and 400 rewards with 0.5 probability. Participants are first trained to learn the probabilities and outcomes associated with each stimulus. Next, on each trial, a stimulus appears in one of four quadrants of the screen, and participants indicate which quadrant using a button press</skos:definition>
		<skos:prefLabel>Non-choice task to study expected value and uncertainty</skos:prefLabel>
		<skos:altLabel></skos:altLabel>
		<cito:citesForInformation rdf:resource="http://cognitiveatlas.org/citation/id/cit_4d55999f3f7c9"/>
</skos:Concept><skos:Concept rdf:about="http://cognitiveatlas.org/id/trm_4d5599f8ed1bf"> <dc:identifier>trm_4d5599f8ed1bf</dc:identifier>
		<dc:Title>Cognitive Atlas : Lexicon : The Cups Task</dc:Title>
		<dc:Description>RDF output for 'The Cups Task'</dc:Description>
		<dc:Type>InteractiveResource</dc:Type>
		<dc:Publisher>Cognitive Atlas</dc:Publisher>
		<dc:Creator>Cognitive Atlas RDF Generator</dc:Creator>
		<dc:Contributor>Tom Schonberg</dc:Contributor>
		<dc:Date>2011-02-11 12:20:08</dc:Date>
		<dc:Format>text/rdf</dc:Format>
		<dc:Language>en</dc:Language>
		<skos:editorialNote>Generated by testgen.php on Thu Jun 9 14:25:25 PDT 2011.</skos:editorialNote>
		<skos:historyNote>No previous definition revisions.</skos:historyNote>
		<skos:changeNote>This is the first and only definition provided.</skos:changeNote>
		<skos:scopeNote>http://www.w3.org/2004/02/skos/core#Concept</skos:scopeNote>
		<skos:Note>SKOS properties defined in http://www.w3.org/TR/skos-primer/#secrel</skos:Note>
		<skos:inScheme rdf:resource="http://cognitiveatlas.org/tasks/"/>
		<skos:definition>On each trial, participants choose between a risky and safe option. Each trial involves either gains or losses. The options are presented as a choice of cups. The risky option involves two to five cups, one containing a gain (loss) of $2, $3 or $5, and the others containing $0. If the latter option is selected, the payoff from one cup is selected at random. The safe cup offers a sure gain (loss) $1.</skos:definition>
		<skos:prefLabel>The Cups Task</skos:prefLabel>
		<skos:altLabel></skos:altLabel>
		<cito:citesForInformation rdf:resource="http://cognitiveatlas.org/citation/id/cit_4d559a46899b6"/>
		<cito:citesForInformation rdf:resource="http://cognitiveatlas.org/citation/id/cit_4d559a784a767"/>
</skos:Concept><skos:Concept rdf:about="http://cognitiveatlas.org/id/trm_4d559bcd67c18"> <dc:identifier>trm_4d559bcd67c18</dc:identifier>
		<dc:Title>Cognitive Atlas : Lexicon : Balloon Analogue Risk Task (BART)</dc:Title>
		<dc:Description>RDF output for 'Balloon Analogue Risk Task (BART)'</dc:Description>
		<dc:Type>InteractiveResource</dc:Type>
		<dc:Publisher>Cognitive Atlas</dc:Publisher>
		<dc:Creator>Cognitive Atlas RDF Generator</dc:Creator>
		<dc:Contributor>Tom Schonberg</dc:Contributor>
		<dc:Date>2011-02-11 12:27:57</dc:Date>
		<dc:Format>text/rdf</dc:Format>
		<dc:Language>en</dc:Language>
		<skos:editorialNote>Generated by testgen.php on Thu Jun 9 14:25:25 PDT 2011.</skos:editorialNote>
		<skos:historyNote>No previous definition revisions.</skos:historyNote>
		<skos:changeNote>This is the first and only definition provided.</skos:changeNote>
		<skos:scopeNote>http://www.w3.org/2004/02/skos/core#Concept</skos:scopeNote>
		<skos:Note>SKOS properties defined in http://www.w3.org/TR/skos-primer/#secrel</skos:Note>
		<skos:inScheme rdf:resource="http://cognitiveatlas.org/tasks/"/>
		<skos:definition>On each trial, participants pump a simulated balloon without knowing when it will explode. Each pump increases the potential reward to be gained but also the probability of explosion, whichwipesoutallpotentialgains for that trial. Inmoststudies,balloonexplosionprobabilities are drawn from a uniform distribution, and participants must learn explosion probabilities through trial-and-error.</skos:definition>
		<skos:prefLabel>Balloon Analogue Risk Task (BART)</skos:prefLabel>
		<skos:altLabel></skos:altLabel>
		<skos:related rdf:resource="http://cognitiveatlas.org/id/trm_4a3fd79d0b64e"/>
		<skos:example>risk seeking is measured by the contrast of negative feedback trials in the Balloon Analogue Risk Task (BART)</skos:example>
		<cito:citesForInformation rdf:resource="http://cognitiveatlas.org/citation/id/cit_4d559c4dec264"/>
		<cito:citesForInformation rdf:resource="http://cognitiveatlas.org/citation/id/cit_4d559c87f3173"/>
		<cito:citesForInformation rdf:resource="http://cognitiveatlas.org/citation/id/cit_4d559cff860c8"/>
		<cito:citesForInformation rdf:resource="http://cognitiveatlas.org/citation/id/cit_4de57915b0eac"/>
</skos:Concept><skos:Concept rdf:about="http://cognitiveatlas.org/id/trm_4d559d2703bae"> <dc:identifier>trm_4d559d2703bae</dc:identifier>
		<dc:Title>Cognitive Atlas : Lexicon : Devils Task</dc:Title>
		<dc:Description>RDF output for 'Devils Task'</dc:Description>
		<dc:Type>InteractiveResource</dc:Type>
		<dc:Publisher>Cognitive Atlas</dc:Publisher>
		<dc:Creator>Cognitive Atlas RDF Generator</dc:Creator>
		<dc:Contributor>Tom Schonberg</dc:Contributor>
		<dc:Date>2011-02-11 12:33:43</dc:Date>
		<dc:Format>text/rdf</dc:Format>
		<dc:Language>en</dc:Language>
		<skos:editorialNote>Generated by testgen.php on Thu Jun 9 14:25:25 PDT 2011.</skos:editorialNote>
		<skos:historyNote>No previous definition revisions.</skos:historyNote>
		<skos:changeNote>This is the first and only definition provided.</skos:changeNote>
		<skos:scopeNote>http://www.w3.org/2004/02/skos/core#Concept</skos:scopeNote>
		<skos:Note>SKOS properties defined in http://www.w3.org/TR/skos-primer/#secrel</skos:Note>
		<skos:inScheme rdf:resource="http://cognitiveatlas.org/tasks/"/>
		<skos:definition>This task is a forerunner to the BART: on each trial, participants decide howmany of seven treasure chests to open. They are informed that six boxes contain a prize and one box contains a ‘devil’ that will cause themto lose all their potential gains on that trial. Similar to the BART, participants make sequential choices and, after opening each chest, decide whether to continue to the next chest or cash in their earnings to that point.</skos:definition>
		<skos:prefLabel>Devils Task</skos:prefLabel>
		<skos:altLabel></skos:altLabel>
		<skos:related rdf:resource="http://cognitiveatlas.org/id/trm_4a3fd79d0b64e"/>
		<skos:example>risk seeking is measured by the contrast of negative feedback trials in the Devils Task</skos:example>
		<cito:citesForInformation rdf:resource="http://cognitiveatlas.org/citation/id/cit_4d559d7572d80"/>
		<cito:citesForInformation rdf:resource="http://cognitiveatlas.org/citation/id/cit_4d559e9ca6aaf"/>
</skos:Concept><skos:Concept rdf:about="http://cognitiveatlas.org/id/trm_4d55a2bbcfdff"> <dc:identifier>trm_4d55a2bbcfdff</dc:identifier>
		<dc:Title>Cognitive Atlas : Lexicon : Choice task between risky and non-risky options</dc:Title>
		<dc:Description>RDF output for 'Choice task between risky and non-risky options'</dc:Description>
		<dc:Type>InteractiveResource</dc:Type>
		<dc:Publisher>Cognitive Atlas</dc:Publisher>
		<dc:Creator>Cognitive Atlas RDF Generator</dc:Creator>
		<dc:Contributor>Carinna Torgerson</dc:Contributor>
		<dc:Date>2011-06-01 16:02:57</dc:Date>
		<dc:Format>text/rdf</dc:Format>
		<dc:Language>en</dc:Language>
		<skos:editorialNote>Generated by testgen.php on Thu Jun 9 14:25:25 PDT 2011.</skos:editorialNote>
		<skos:historyNote>Revision 3: 2 previous definitions.</skos:historyNote>
		<skos:changeNote>See http://cognitiveatlas.org/id/trm_4d55a2bbcfdff for complete revision history.</skos:changeNote>
		<skos:scopeNote>http://www.w3.org/2004/02/skos/core#Concept</skos:scopeNote>
		<skos:Note>SKOS properties defined in http://www.w3.org/TR/skos-primer/#secrel</skos:Note>
		<skos:inScheme rdf:resource="http://cognitiveatlas.org/tasks/"/>
		<skos:definition>a choice made between two or more options when one of those options has some probability >0 of producing either a reinforcing or an aversive consequence</skos:definition>
		<skos:prefLabel>Choice task between risky and non-risky options</skos:prefLabel>
		<skos:altLabel></skos:altLabel>
		<skos:related rdf:resource="http://cognitiveatlas.org/id/trm_4d54b8361e93e"/>
		<skos:related rdf:resource="http://cognitiveatlas.org/id/trm_4a3fd79d0b64e"/>
		<skos:related rdf:resource="http://cognitiveatlas.org/id/trm_4d54b2cc0f943"/>
		<skos:related rdf:resource="http://cognitiveatlas.org/id/tsk_4a57abb949ae5"/>
		<skos:example>Behavioral Investment allocation strategy (BIAS) is a narrower synonym of Choice task between risky and non-risky options</skos:example>
		<skos:example>risk seeking is measured by the contrast of risky option trials in the Choice task between risky and non-risky options</skos:example>
		<skos:example>Cambridge Gambling Task is a narrower synonym of Choice task between risky and non-risky options</skos:example>
		<skos:example>Iowa Gambling Task is a narrower synonym of Choice task between risky and non-risky options</skos:example>
		<cito:citesForInformation rdf:resource="http://cognitiveatlas.org/citation/id/cit_4d55a32988c87"/>
		<cito:citesForInformation rdf:resource="http://cognitiveatlas.org/citation/id/cit_4d55a34cc2ddc"/>
</skos:Concept><skos:Concept rdf:about="http://cognitiveatlas.org/id/trm_4d8a48e403c78"> <dc:identifier>trm_4d8a48e403c78</dc:identifier>
		<dc:Title>Cognitive Atlas : Lexicon : Inductive reasoning aptitude</dc:Title>
		<dc:Description>RDF output for 'Inductive reasoning aptitude'</dc:Description>
		<dc:Type>InteractiveResource</dc:Type>
		<dc:Publisher>Cognitive Atlas</dc:Publisher>
		<dc:Creator>Cognitive Atlas RDF Generator</dc:Creator>
		<dc:Contributor>Natalie Picchetti</dc:Contributor>
		<dc:Date>2011-04-01 12:54:26</dc:Date>
		<dc:Format>text/rdf</dc:Format>
		<dc:Language>en</dc:Language>
		<skos:editorialNote>Generated by testgen.php on Thu Jun 9 14:25:25 PDT 2011.</skos:editorialNote>
		<skos:historyNote>Revision 2: 1 previous definitions.</skos:historyNote>
		<skos:changeNote>See http://cognitiveatlas.org/id/trm_4d8a48e403c78 for complete revision history.</skos:changeNote>
		<skos:scopeNote>http://www.w3.org/2004/02/skos/core#Concept</skos:scopeNote>
		<skos:Note>SKOS properties defined in http://www.w3.org/TR/skos-primer/#secrel</skos:Note>
		<skos:inScheme rdf:resource="http://cognitiveatlas.org/tasks/"/>
		<skos:definition>is a measurable aptitude for how well a person can identify a pattern within a large amount of data. 


</skos:definition>
		<skos:prefLabel>Inductive reasoning aptitude</skos:prefLabel>
		<skos:altLabel></skos:altLabel>
		<skos:related rdf:resource="http://cognitiveatlas.org/id/trm_4a3fd79d0a590"/>
		<skos:example>inductive reasoning is measured by the contrast of accuracy of participant minus average accuracy of controls trials in the Inductive reasoning aptitude</skos:example>
		<cito:citesForInformation rdf:resource="http://cognitiveatlas.org/citation/id/cit_4dee65850762a"/>
		<cito:citesForInformation rdf:resource="http://cognitiveatlas.org/citation/id/cit_4dee7f7b59573"/>
		<cito:citesForInformation rdf:resource="http://cognitiveatlas.org/citation/id/cit_4dee7ffa55ee8"/>
</skos:Concept><skos:Concept rdf:about="http://cognitiveatlas.org/id/trm_4d949c5b0e380"> <dc:identifier>trm_4d949c5b0e380</dc:identifier>
		<dc:Title>Cognitive Atlas : Lexicon : Rhyme verification task</dc:Title>
		<dc:Description>RDF output for 'Rhyme verification task'</dc:Description>
		<dc:Type>InteractiveResource</dc:Type>
		<dc:Publisher>Cognitive Atlas</dc:Publisher>
		<dc:Creator>Cognitive Atlas RDF Generator</dc:Creator>
		<dc:Contributor>Russ Poldrack</dc:Contributor>
		<dc:Date>2011-03-31 08:23:07</dc:Date>
		<dc:Format>text/rdf</dc:Format>
		<dc:Language>en</dc:Language>
		<skos:editorialNote>Generated by testgen.php on Thu Jun 9 14:25:25 PDT 2011.</skos:editorialNote>
		<skos:historyNote>No previous definition revisions.</skos:historyNote>
		<skos:changeNote>This is the first and only definition provided.</skos:changeNote>
		<skos:scopeNote>http://www.w3.org/2004/02/skos/core#Concept</skos:scopeNote>
		<skos:Note>SKOS properties defined in http://www.w3.org/TR/skos-primer/#secrel</skos:Note>
		<skos:inScheme rdf:resource="http://cognitiveatlas.org/tasks/"/>
		<skos:definition>Stimuli are presented in pairs (either words or pseudowords) and the subject is asked to judge whether the pair of stimuli rhyme with one another.</skos:definition>
		<skos:prefLabel>Rhyme verification task</skos:prefLabel>
		<skos:altLabel></skos:altLabel>
</skos:Concept><skos:Concept rdf:about="http://cognitiveatlas.org/id/trm_4da4b203ad5ae"> <dc:identifier>trm_4da4b203ad5ae</dc:identifier>
		<dc:Title>Cognitive Atlas : Lexicon : selective stop signal task</dc:Title>
		<dc:Description>RDF output for 'selective stop signal task'</dc:Description>
		<dc:Type>InteractiveResource</dc:Type>
		<dc:Publisher>Cognitive Atlas</dc:Publisher>
		<dc:Creator>Cognitive Atlas RDF Generator</dc:Creator>
		<dc:Contributor>Russ Poldrack</dc:Contributor>
		<dc:Date>2011-04-12 13:11:47</dc:Date>
		<dc:Format>text/rdf</dc:Format>
		<dc:Language>en</dc:Language>
		<skos:editorialNote>Generated by testgen.php on Thu Jun 9 14:25:25 PDT 2011.</skos:editorialNote>
		<skos:historyNote>No previous definition revisions.</skos:historyNote>
		<skos:changeNote>This is the first and only definition provided.</skos:changeNote>
		<skos:scopeNote>http://www.w3.org/2004/02/skos/core#Concept</skos:scopeNote>
		<skos:Note>SKOS properties defined in http://www.w3.org/TR/skos-primer/#secrel</skos:Note>
		<skos:inScheme rdf:resource="http://cognitiveatlas.org/tasks/"/>
		<skos:definition>A version of the stop signal task where inhibition is contingent upon both the presence of the stop signal and the particular stimulus.  </skos:definition>
		<skos:prefLabel>selective stop signal task</skos:prefLabel>
		<skos:altLabel></skos:altLabel>
		<skos:related rdf:resource="http://cognitiveatlas.org/id/tsk_4a57abb949e1a"/>
		<skos:example>selective stop signal task is descended from stop signal task</skos:example>
</skos:Concept><skos:Concept rdf:about="http://cognitiveatlas.org/id/trm_4da6304c9aa23"> <dc:identifier>trm_4da6304c9aa23</dc:identifier>
		<dc:Title>Cognitive Atlas : Lexicon : attention networks test</dc:Title>
		<dc:Description>RDF output for 'attention networks test'</dc:Description>
		<dc:Type>InteractiveResource</dc:Type>
		<dc:Publisher>Cognitive Atlas</dc:Publisher>
		<dc:Creator>Cognitive Atlas RDF Generator</dc:Creator>
		<dc:Contributor>Natalie Picchetti</dc:Contributor>
		<dc:Date>2011-04-13 16:22:52</dc:Date>
		<dc:Format>text/rdf</dc:Format>
		<dc:Language>en</dc:Language>
		<skos:editorialNote>Generated by testgen.php on Thu Jun 9 14:25:25 PDT 2011.</skos:editorialNote>
		<skos:historyNote>No previous definition revisions.</skos:historyNote>
		<skos:changeNote>This is the first and only definition provided.</skos:changeNote>
		<skos:scopeNote>http://www.w3.org/2004/02/skos/core#Concept</skos:scopeNote>
		<skos:Note>SKOS properties defined in http://www.w3.org/TR/skos-primer/#secrel</skos:Note>
		<skos:inScheme rdf:resource="http://cognitiveatlas.org/tasks/"/>
		<skos:definition>No definition submitted yet.</skos:definition>
		<skos:prefLabel>attention networks test</skos:prefLabel>
		<skos:altLabel></skos:altLabel>
</skos:Concept><skos:Concept rdf:about="http://cognitiveatlas.org/id/trm_4da630c52c011"> <dc:identifier>trm_4da630c52c011</dc:identifier>
		<dc:Title>Cognitive Atlas : Lexicon : delayed discounting task</dc:Title>
		<dc:Description>RDF output for 'delayed discounting task'</dc:Description>
		<dc:Type>InteractiveResource</dc:Type>
		<dc:Publisher>Cognitive Atlas</dc:Publisher>
		<dc:Creator>Cognitive Atlas RDF Generator</dc:Creator>
		<dc:Contributor>John Clithero</dc:Contributor>
		<dc:Date>2011-05-23 14:09:43</dc:Date>
		<dc:Format>text/rdf</dc:Format>
		<dc:Language>en</dc:Language>
		<skos:editorialNote>Generated by testgen.php on Thu Jun 9 14:25:25 PDT 2011.</skos:editorialNote>
		<skos:historyNote>Revision 2: 1 previous definitions.</skos:historyNote>
		<skos:changeNote>See http://cognitiveatlas.org/id/trm_4da630c52c011 for complete revision history.</skos:changeNote>
		<skos:scopeNote>http://www.w3.org/2004/02/skos/core#Concept</skos:scopeNote>
		<skos:Note>SKOS properties defined in http://www.w3.org/TR/skos-primer/#secrel</skos:Note>
		<skos:inScheme rdf:resource="http://cognitiveatlas.org/tasks/"/>
		<skos:definition>A task for identifying preferences over tradeoffs between costs and benefits occurring at different times.</skos:definition>
		<skos:prefLabel>delayed discounting task</skos:prefLabel>
		<skos:altLabel></skos:altLabel>
		<cito:citesForInformation rdf:resource="http://cognitiveatlas.org/citation/id/cit_4ddacd3d36e2d"/>
		<cito:citesForInformation rdf:resource="http://cognitiveatlas.org/citation/id/cit_4ddacd4fca66f"/>
		<cito:citesForInformation rdf:resource="http://cognitiveatlas.org/citation/id/cit_4ddacd68cee59"/>
</skos:Concept><skos:Concept rdf:about="http://cognitiveatlas.org/id/trm_4da63146f12d7"> <dc:identifier>trm_4da63146f12d7</dc:identifier>
		<dc:Title>Cognitive Atlas : Lexicon : remember/know task</dc:Title>
		<dc:Description>RDF output for 'remember/know task'</dc:Description>
		<dc:Type>InteractiveResource</dc:Type>
		<dc:Publisher>Cognitive Atlas</dc:Publisher>
		<dc:Creator>Cognitive Atlas RDF Generator</dc:Creator>
		<dc:Contributor>Natalie Picchetti</dc:Contributor>
		<dc:Date>2011-04-13 16:27:02</dc:Date>
		<dc:Format>text/rdf</dc:Format>
		<dc:Language>en</dc:Language>
		<skos:editorialNote>Generated by testgen.php on Thu Jun 9 14:25:25 PDT 2011.</skos:editorialNote>
		<skos:historyNote>No previous definition revisions.</skos:historyNote>
		<skos:changeNote>This is the first and only definition provided.</skos:changeNote>
		<skos:scopeNote>http://www.w3.org/2004/02/skos/core#Concept</skos:scopeNote>
		<skos:Note>SKOS properties defined in http://www.w3.org/TR/skos-primer/#secrel</skos:Note>
		<skos:inScheme rdf:resource="http://cognitiveatlas.org/tasks/"/>
		<skos:definition>No definition submitted yet.</skos:definition>
		<skos:prefLabel>remember/know task</skos:prefLabel>
		<skos:altLabel></skos:altLabel>
</skos:Concept><skos:Concept rdf:about="http://cognitiveatlas.org/id/trm_4da6318f7381b"> <dc:identifier>trm_4da6318f7381b</dc:identifier>
		<dc:Title>Cognitive Atlas : Lexicon : probabilistic reversal learning</dc:Title>
		<dc:Description>RDF output for 'probabilistic reversal learning'</dc:Description>
		<dc:Type>InteractiveResource</dc:Type>
		<dc:Publisher>Cognitive Atlas</dc:Publisher>
		<dc:Creator>Cognitive Atlas RDF Generator</dc:Creator>
		<dc:Contributor>Natalie Picchetti</dc:Contributor>
		<dc:Date>2011-04-13 16:28:15</dc:Date>
		<dc:Format>text/rdf</dc:Format>
		<dc:Language>en</dc:Language>
		<skos:editorialNote>Generated by testgen.php on Thu Jun 9 14:25:25 PDT 2011.</skos:editorialNote>
		<skos:historyNote>No previous definition revisions.</skos:historyNote>
		<skos:changeNote>This is the first and only definition provided.</skos:changeNote>
		<skos:scopeNote>http://www.w3.org/2004/02/skos/core#Concept</skos:scopeNote>
		<skos:Note>SKOS properties defined in http://www.w3.org/TR/skos-primer/#secrel</skos:Note>
		<skos:inScheme rdf:resource="http://cognitiveatlas.org/tasks/"/>
		<skos:definition>No definition submitted yet.</skos:definition>
		<skos:prefLabel>probabilistic reversal learning</skos:prefLabel>
		<skos:altLabel></skos:altLabel>
</skos:Concept><skos:Concept rdf:about="http://cognitiveatlas.org/id/trm_4da631be60291"> <dc:identifier>trm_4da631be60291</dc:identifier>
		<dc:Title>Cognitive Atlas : Lexicon : Counting Stroop Task</dc:Title>
		<dc:Description>RDF output for 'Counting Stroop Task'</dc:Description>
		<dc:Type>InteractiveResource</dc:Type>
		<dc:Publisher>Cognitive Atlas</dc:Publisher>
		<dc:Creator>Cognitive Atlas RDF Generator</dc:Creator>
		<dc:Contributor>Natalie Picchetti</dc:Contributor>
		<dc:Date>2011-04-13 16:29:02</dc:Date>
		<dc:Format>text/rdf</dc:Format>
		<dc:Language>en</dc:Language>
		<skos:editorialNote>Generated by testgen.php on Thu Jun 9 14:25:25 PDT 2011.</skos:editorialNote>
		<skos:historyNote>No previous definition revisions.</skos:historyNote>
		<skos:changeNote>This is the first and only definition provided.</skos:changeNote>
		<skos:scopeNote>http://www.w3.org/2004/02/skos/core#Concept</skos:scopeNote>
		<skos:Note>SKOS properties defined in http://www.w3.org/TR/skos-primer/#secrel</skos:Note>
		<skos:inScheme rdf:resource="http://cognitiveatlas.org/tasks/"/>
		<skos:definition>No definition submitted yet. </skos:definition>
		<skos:prefLabel>Counting Stroop Task</skos:prefLabel>
		<skos:altLabel></skos:altLabel>
</skos:Concept><skos:Concept rdf:about="http://cognitiveatlas.org/id/trm_4da6327154fd4"> <dc:identifier>trm_4da6327154fd4</dc:identifier>
		<dc:Title>Cognitive Atlas : Lexicon : scene recognition task</dc:Title>
		<dc:Description>RDF output for 'scene recognition task'</dc:Description>
		<dc:Type>InteractiveResource</dc:Type>
		<dc:Publisher>Cognitive Atlas</dc:Publisher>
		<dc:Creator>Cognitive Atlas RDF Generator</dc:Creator>
		<dc:Contributor>Natalie Picchetti</dc:Contributor>
		<dc:Date>2011-04-13 16:32:01</dc:Date>
		<dc:Format>text/rdf</dc:Format>
		<dc:Language>en</dc:Language>
		<skos:editorialNote>Generated by testgen.php on Thu Jun 9 14:25:25 PDT 2011.</skos:editorialNote>
		<skos:historyNote>No previous definition revisions.</skos:historyNote>
		<skos:changeNote>This is the first and only definition provided.</skos:changeNote>
		<skos:scopeNote>http://www.w3.org/2004/02/skos/core#Concept</skos:scopeNote>
		<skos:Note>SKOS properties defined in http://www.w3.org/TR/skos-primer/#secrel</skos:Note>
		<skos:inScheme rdf:resource="http://cognitiveatlas.org/tasks/"/>
		<skos:definition>No definition submitted yet.</skos:definition>
		<skos:prefLabel>scene recognition task</skos:prefLabel>
		<skos:altLabel></skos:altLabel>
</skos:Concept><skos:Concept rdf:about="http://cognitiveatlas.org/id/trm_4da632d09c89f"> <dc:identifier>trm_4da632d09c89f</dc:identifier>
		<dc:Title>Cognitive Atlas : Lexicon : set shifting task</dc:Title>
		<dc:Description>RDF output for 'set shifting task'</dc:Description>
		<dc:Type>InteractiveResource</dc:Type>
		<dc:Publisher>Cognitive Atlas</dc:Publisher>
		<dc:Creator>Cognitive Atlas RDF Generator</dc:Creator>
		<dc:Contributor>Natalie Picchetti</dc:Contributor>
		<dc:Date>2011-04-13 16:33:36</dc:Date>
		<dc:Format>text/rdf</dc:Format>
		<dc:Language>en</dc:Language>
		<skos:editorialNote>Generated by testgen.php on Thu Jun 9 14:25:25 PDT 2011.</skos:editorialNote>
		<skos:historyNote>No previous definition revisions.</skos:historyNote>
		<skos:changeNote>This is the first and only definition provided.</skos:changeNote>
		<skos:scopeNote>http://www.w3.org/2004/02/skos/core#Concept</skos:scopeNote>
		<skos:Note>SKOS properties defined in http://www.w3.org/TR/skos-primer/#secrel</skos:Note>
		<skos:inScheme rdf:resource="http://cognitiveatlas.org/tasks/"/>
		<skos:definition>No definition submitted yet.</skos:definition>
		<skos:prefLabel>set shifting task</skos:prefLabel>
		<skos:altLabel></skos:altLabel>
</skos:Concept><skos:Concept rdf:about="http://cognitiveatlas.org/id/trm_4da632fa57098"> <dc:identifier>trm_4da632fa57098</dc:identifier>
		<dc:Title>Cognitive Atlas : Lexicon : task switching paradigm</dc:Title>
		<dc:Description>RDF output for 'task switching paradigm'</dc:Description>
		<dc:Type>InteractiveResource</dc:Type>
		<dc:Publisher>Cognitive Atlas</dc:Publisher>
		<dc:Creator>Cognitive Atlas RDF Generator</dc:Creator>
		<dc:Contributor>Natalie Picchetti</dc:Contributor>
		<dc:Date>2011-04-13 16:34:18</dc:Date>
		<dc:Format>text/rdf</dc:Format>
		<dc:Language>en</dc:Language>
		<skos:editorialNote>Generated by testgen.php on Thu Jun 9 14:25:25 PDT 2011.</skos:editorialNote>
		<skos:historyNote>No previous definition revisions.</skos:historyNote>
		<skos:changeNote>This is the first and only definition provided.</skos:changeNote>
		<skos:scopeNote>http://www.w3.org/2004/02/skos/core#Concept</skos:scopeNote>
		<skos:Note>SKOS properties defined in http://www.w3.org/TR/skos-primer/#secrel</skos:Note>
		<skos:inScheme rdf:resource="http://cognitiveatlas.org/tasks/"/>
		<skos:definition>No definition submitted yet.</skos:definition>
		<skos:prefLabel>task switching paradigm</skos:prefLabel>
		<skos:altLabel></skos:altLabel>
</skos:Concept><skos:Concept rdf:about="http://cognitiveatlas.org/id/trm_4da6331cdeeb5"> <dc:identifier>trm_4da6331cdeeb5</dc:identifier>
		<dc:Title>Cognitive Atlas : Lexicon : California Verbal Learning Test</dc:Title>
		<dc:Description>RDF output for 'California Verbal Learning Test'</dc:Description>
		<dc:Type>InteractiveResource</dc:Type>
		<dc:Publisher>Cognitive Atlas</dc:Publisher>
		<dc:Creator>Cognitive Atlas RDF Generator</dc:Creator>
		<dc:Contributor>Natalie Picchetti</dc:Contributor>
		<dc:Date>2011-04-13 16:34:52</dc:Date>
		<dc:Format>text/rdf</dc:Format>
		<dc:Language>en</dc:Language>
		<skos:editorialNote>Generated by testgen.php on Thu Jun 9 14:25:25 PDT 2011.</skos:editorialNote>
		<skos:historyNote>No previous definition revisions.</skos:historyNote>
		<skos:changeNote>This is the first and only definition provided.</skos:changeNote>
		<skos:scopeNote>http://www.w3.org/2004/02/skos/core#Concept</skos:scopeNote>
		<skos:Note>SKOS properties defined in http://www.w3.org/TR/skos-primer/#secrel</skos:Note>
		<skos:inScheme rdf:resource="http://cognitiveatlas.org/tasks/"/>
		<skos:definition>No definition submitted yet.</skos:definition>
		<skos:prefLabel>California Verbal Learning Test</skos:prefLabel>
		<skos:altLabel></skos:altLabel>
</skos:Concept><skos:Concept rdf:about="http://cognitiveatlas.org/id/trm_4da63357e4999"> <dc:identifier>trm_4da63357e4999</dc:identifier>
		<dc:Title>Cognitive Atlas : Lexicon : Wechsler Memory Scale (revised)</dc:Title>
		<dc:Description>RDF output for 'Wechsler Memory Scale (revised)'</dc:Description>
		<dc:Type>InteractiveResource</dc:Type>
		<dc:Publisher>Cognitive Atlas</dc:Publisher>
		<dc:Creator>Cognitive Atlas RDF Generator</dc:Creator>
		<dc:Contributor>Natalie Picchetti</dc:Contributor>
		<dc:Date>2011-04-13 16:35:51</dc:Date>
		<dc:Format>text/rdf</dc:Format>
		<dc:Language>en</dc:Language>
		<skos:editorialNote>Generated by testgen.php on Thu Jun 9 14:25:25 PDT 2011.</skos:editorialNote>
		<skos:historyNote>No previous definition revisions.</skos:historyNote>
		<skos:changeNote>This is the first and only definition provided.</skos:changeNote>
		<skos:scopeNote>http://www.w3.org/2004/02/skos/core#Concept</skos:scopeNote>
		<skos:Note>SKOS properties defined in http://www.w3.org/TR/skos-primer/#secrel</skos:Note>
		<skos:inScheme rdf:resource="http://cognitiveatlas.org/tasks/"/>
		<skos:definition>No definition submitted yet.</skos:definition>
		<skos:prefLabel>Wechsler Memory Scale (revised)</skos:prefLabel>
		<skos:altLabel></skos:altLabel>
		<skos:related rdf:resource="http://cognitiveatlas.org/id/tsk_4a57abb949abc"/>
		<skos:example>immediate recall test is descended from Wechsler Memory Scale (revised)</skos:example>
</skos:Concept><skos:Concept rdf:about="http://cognitiveatlas.org/id/trm_4da6338803ed2"> <dc:identifier>trm_4da6338803ed2</dc:identifier>
		<dc:Title>Cognitive Atlas : Lexicon : Wechsler Intelligence Scale for Children - Revised</dc:Title>
		<dc:Description>RDF output for 'Wechsler Intelligence Scale for Children - Revised'</dc:Description>
		<dc:Type>InteractiveResource</dc:Type>
		<dc:Publisher>Cognitive Atlas</dc:Publisher>
		<dc:Creator>Cognitive Atlas RDF Generator</dc:Creator>
		<dc:Contributor>Natalie Picchetti</dc:Contributor>
		<dc:Date>2011-04-13 16:36:40</dc:Date>
		<dc:Format>text/rdf</dc:Format>
		<dc:Language>en</dc:Language>
		<skos:editorialNote>Generated by testgen.php on Thu Jun 9 14:25:25 PDT 2011.</skos:editorialNote>
		<skos:historyNote>No previous definition revisions.</skos:historyNote>
		<skos:changeNote>This is the first and only definition provided.</skos:changeNote>
		<skos:scopeNote>http://www.w3.org/2004/02/skos/core#Concept</skos:scopeNote>
		<skos:Note>SKOS properties defined in http://www.w3.org/TR/skos-primer/#secrel</skos:Note>
		<skos:inScheme rdf:resource="http://cognitiveatlas.org/tasks/"/>
		<skos:definition>No definition submitted yet.</skos:definition>
		<skos:prefLabel>Wechsler Intelligence Scale for Children - Revised</skos:prefLabel>
		<skos:altLabel></skos:altLabel>
</skos:Concept><skos:Concept rdf:about="http://cognitiveatlas.org/id/trm_4da633dbb5817"> <dc:identifier>trm_4da633dbb5817</dc:identifier>
		<dc:Title>Cognitive Atlas : Lexicon : word fluency test</dc:Title>
		<dc:Description>RDF output for 'word fluency test'</dc:Description>
		<dc:Type>InteractiveResource</dc:Type>
		<dc:Publisher>Cognitive Atlas</dc:Publisher>
		<dc:Creator>Cognitive Atlas RDF Generator</dc:Creator>
		<dc:Contributor>Natalie Picchetti</dc:Contributor>
		<dc:Date>2011-04-13 16:38:03</dc:Date>
		<dc:Format>text/rdf</dc:Format>
		<dc:Language>en</dc:Language>
		<skos:editorialNote>Generated by testgen.php on Thu Jun 9 14:25:25 PDT 2011.</skos:editorialNote>
		<skos:historyNote>No previous definition revisions.</skos:historyNote>
		<skos:changeNote>This is the first and only definition provided.</skos:changeNote>
		<skos:scopeNote>http://www.w3.org/2004/02/skos/core#Concept</skos:scopeNote>
		<skos:Note>SKOS properties defined in http://www.w3.org/TR/skos-primer/#secrel</skos:Note>
		<skos:inScheme rdf:resource="http://cognitiveatlas.org/tasks/"/>
		<skos:definition>No definition submitted yet.</skos:definition>
		<skos:prefLabel>word fluency test</skos:prefLabel>
		<skos:altLabel></skos:altLabel>
</skos:Concept><skos:Concept rdf:about="http://cognitiveatlas.org/id/trm_4da633fe917c4"> <dc:identifier>trm_4da633fe917c4</dc:identifier>
		<dc:Title>Cognitive Atlas : Lexicon : color trails test</dc:Title>
		<dc:Description>RDF output for 'color trails test'</dc:Description>
		<dc:Type>InteractiveResource</dc:Type>
		<dc:Publisher>Cognitive Atlas</dc:Publisher>
		<dc:Creator>Cognitive Atlas RDF Generator</dc:Creator>
		<dc:Contributor>Natalie Picchetti</dc:Contributor>
		<dc:Date>2011-04-13 16:38:38</dc:Date>
		<dc:Format>text/rdf</dc:Format>
		<dc:Language>en</dc:Language>
		<skos:editorialNote>Generated by testgen.php on Thu Jun 9 14:25:25 PDT 2011.</skos:editorialNote>
		<skos:historyNote>No previous definition revisions.</skos:historyNote>
		<skos:changeNote>This is the first and only definition provided.</skos:changeNote>
		<skos:scopeNote>http://www.w3.org/2004/02/skos/core#Concept</skos:scopeNote>
		<skos:Note>SKOS properties defined in http://www.w3.org/TR/skos-primer/#secrel</skos:Note>
		<skos:inScheme rdf:resource="http://cognitiveatlas.org/tasks/"/>
		<skos:definition>No definition submitted yet.</skos:definition>
		<skos:prefLabel>color trails test</skos:prefLabel>
		<skos:altLabel></skos:altLabel>
</skos:Concept><skos:Concept rdf:about="http://cognitiveatlas.org/id/trm_4da634216ebbc"> <dc:identifier>trm_4da634216ebbc</dc:identifier>
		<dc:Title>Cognitive Atlas : Lexicon : dual-task paradigm</dc:Title>
		<dc:Description>RDF output for 'dual-task paradigm'</dc:Description>
		<dc:Type>InteractiveResource</dc:Type>
		<dc:Publisher>Cognitive Atlas</dc:Publisher>
		<dc:Creator>Cognitive Atlas RDF Generator</dc:Creator>
		<dc:Contributor>Natalie Picchetti</dc:Contributor>
		<dc:Date>2011-04-13 16:39:13</dc:Date>
		<dc:Format>text/rdf</dc:Format>
		<dc:Language>en</dc:Language>
		<skos:editorialNote>Generated by testgen.php on Thu Jun 9 14:25:25 PDT 2011.</skos:editorialNote>
		<skos:historyNote>No previous definition revisions.</skos:historyNote>
		<skos:changeNote>This is the first and only definition provided.</skos:changeNote>
		<skos:scopeNote>http://www.w3.org/2004/02/skos/core#Concept</skos:scopeNote>
		<skos:Note>SKOS properties defined in http://www.w3.org/TR/skos-primer/#secrel</skos:Note>
		<skos:inScheme rdf:resource="http://cognitiveatlas.org/tasks/"/>
		<skos:definition>NO definition submitted yet.</skos:definition>
		<skos:prefLabel>dual-task paradigm</skos:prefLabel>
		<skos:altLabel></skos:altLabel>
</skos:Concept><skos:Concept rdf:about="http://cognitiveatlas.org/id/trm_4da869646e5d1"> <dc:identifier>trm_4da869646e5d1</dc:identifier>
		<dc:Title>Cognitive Atlas : Lexicon : item recognition task</dc:Title>
		<dc:Description>RDF output for 'item recognition task'</dc:Description>
		<dc:Type>InteractiveResource</dc:Type>
		<dc:Publisher>Cognitive Atlas</dc:Publisher>
		<dc:Creator>Cognitive Atlas RDF Generator</dc:Creator>
		<dc:Contributor>Natalie Picchetti</dc:Contributor>
		<dc:Date>2011-04-15 08:51:00</dc:Date>
		<dc:Format>text/rdf</dc:Format>
		<dc:Language>en</dc:Language>
		<skos:editorialNote>Generated by testgen.php on Thu Jun 9 14:25:25 PDT 2011.</skos:editorialNote>
		<skos:historyNote>No previous definition revisions.</skos:historyNote>
		<skos:changeNote>This is the first and only definition provided.</skos:changeNote>
		<skos:scopeNote>http://www.w3.org/2004/02/skos/core#Concept</skos:scopeNote>
		<skos:Note>SKOS properties defined in http://www.w3.org/TR/skos-primer/#secrel</skos:Note>
		<skos:inScheme rdf:resource="http://cognitiveatlas.org/tasks/"/>
		<skos:definition>No definition submitted yet.</skos:definition>
		<skos:prefLabel>item recognition task</skos:prefLabel>
		<skos:altLabel></skos:altLabel>
</skos:Concept><skos:Concept rdf:about="http://cognitiveatlas.org/id/trm_4da869e68b5c4"> <dc:identifier>trm_4da869e68b5c4</dc:identifier>
		<dc:Title>Cognitive Atlas : Lexicon : memory span test</dc:Title>
		<dc:Description>RDF output for 'memory span test'</dc:Description>
		<dc:Type>InteractiveResource</dc:Type>
		<dc:Publisher>Cognitive Atlas</dc:Publisher>
		<dc:Creator>Cognitive Atlas RDF Generator</dc:Creator>
		<dc:Contributor>Natalie Picchetti</dc:Contributor>
		<dc:Date>2011-04-15 08:53:10</dc:Date>
		<dc:Format>text/rdf</dc:Format>
		<dc:Language>en</dc:Language>
		<skos:editorialNote>Generated by testgen.php on Thu Jun 9 14:25:25 PDT 2011.</skos:editorialNote>
		<skos:historyNote>No previous definition revisions.</skos:historyNote>
		<skos:changeNote>This is the first and only definition provided.</skos:changeNote>
		<skos:scopeNote>http://www.w3.org/2004/02/skos/core#Concept</skos:scopeNote>
		<skos:Note>SKOS properties defined in http://www.w3.org/TR/skos-primer/#secrel</skos:Note>
		<skos:inScheme rdf:resource="http://cognitiveatlas.org/tasks/"/>
		<skos:definition>No definition submitted yet.</skos:definition>
		<skos:prefLabel>memory span test</skos:prefLabel>
		<skos:altLabel></skos:altLabel>
</skos:Concept><skos:Concept rdf:about="http://cognitiveatlas.org/id/trm_4da86a1bb7dd2"> <dc:identifier>trm_4da86a1bb7dd2</dc:identifier>
		<dc:Title>Cognitive Atlas : Lexicon : Reading Span Test</dc:Title>
		<dc:Description>RDF output for 'Reading Span Test'</dc:Description>
		<dc:Type>InteractiveResource</dc:Type>
		<dc:Publisher>Cognitive Atlas</dc:Publisher>
		<dc:Creator>Cognitive Atlas RDF Generator</dc:Creator>
		<dc:Contributor>Natalie Picchetti</dc:Contributor>
		<dc:Date>2011-04-15 08:54:03</dc:Date>
		<dc:Format>text/rdf</dc:Format>
		<dc:Language>en</dc:Language>
		<skos:editorialNote>Generated by testgen.php on Thu Jun 9 14:25:25 PDT 2011.</skos:editorialNote>
		<skos:historyNote>No previous definition revisions.</skos:historyNote>
		<skos:changeNote>This is the first and only definition provided.</skos:changeNote>
		<skos:scopeNote>http://www.w3.org/2004/02/skos/core#Concept</skos:scopeNote>
		<skos:Note>SKOS properties defined in http://www.w3.org/TR/skos-primer/#secrel</skos:Note>
		<skos:inScheme rdf:resource="http://cognitiveatlas.org/tasks/"/>
		<skos:definition>No definition submitted yet.</skos:definition>
		<skos:prefLabel>Reading Span Test</skos:prefLabel>
		<skos:altLabel></skos:altLabel>
</skos:Concept><skos:Concept rdf:about="http://cognitiveatlas.org/id/trm_4da86ad02b3ea"> <dc:identifier>trm_4da86ad02b3ea</dc:identifier>
		<dc:Title>Cognitive Atlas : Lexicon : complex span test</dc:Title>
		<dc:Description>RDF output for 'complex span test'</dc:Description>
		<dc:Type>InteractiveResource</dc:Type>
		<dc:Publisher>Cognitive Atlas</dc:Publisher>
		<dc:Creator>Cognitive Atlas RDF Generator</dc:Creator>
		<dc:Contributor>Natalie Picchetti</dc:Contributor>
		<dc:Date>2011-04-15 08:57:04</dc:Date>
		<dc:Format>text/rdf</dc:Format>
		<dc:Language>en</dc:Language>
		<skos:editorialNote>Generated by testgen.php on Thu Jun 9 14:25:25 PDT 2011.</skos:editorialNote>
		<skos:historyNote>No previous definition revisions.</skos:historyNote>
		<skos:changeNote>This is the first and only definition provided.</skos:changeNote>
		<skos:scopeNote>http://www.w3.org/2004/02/skos/core#Concept</skos:scopeNote>
		<skos:Note>SKOS properties defined in http://www.w3.org/TR/skos-primer/#secrel</skos:Note>
		<skos:inScheme rdf:resource="http://cognitiveatlas.org/tasks/"/>
		<skos:definition>No definition submitted yet.</skos:definition>
		<skos:prefLabel>complex span test</skos:prefLabel>
		<skos:altLabel></skos:altLabel>
</skos:Concept><skos:Concept rdf:about="http://cognitiveatlas.org/id/trm_4da86b2526726"> <dc:identifier>trm_4da86b2526726</dc:identifier>
		<dc:Title>Cognitive Atlas : Lexicon : operation span test</dc:Title>
		<dc:Description>RDF output for 'operation span test'</dc:Description>
		<dc:Type>InteractiveResource</dc:Type>
		<dc:Publisher>Cognitive Atlas</dc:Publisher>
		<dc:Creator>Cognitive Atlas RDF Generator</dc:Creator>
		<dc:Contributor>Natalie Picchetti</dc:Contributor>
		<dc:Date>2011-04-15 08:58:41</dc:Date>
		<dc:Format>text/rdf</dc:Format>
		<dc:Language>en</dc:Language>
		<skos:editorialNote>Generated by testgen.php on Thu Jun 9 14:25:25 PDT 2011.</skos:editorialNote>
		<skos:historyNote>Revision 2: 1 previous definitions.</skos:historyNote>
		<skos:changeNote>See http://cognitiveatlas.org/id/trm_4da86b2526726 for complete revision history.</skos:changeNote>
		<skos:scopeNote>http://www.w3.org/2004/02/skos/core#Concept</skos:scopeNote>
		<skos:Note>SKOS properties defined in http://www.w3.org/TR/skos-primer/#secrel</skos:Note>
		<skos:inScheme rdf:resource="http://cognitiveatlas.org/tasks/"/>
		<skos:definition>No definition submitted yet.</skos:definition>
		<skos:prefLabel>operation span test</skos:prefLabel>
		<skos:altLabel></skos:altLabel>
</skos:Concept><skos:Concept rdf:about="http://cognitiveatlas.org/id/trm_4da86b539924c"> <dc:identifier>trm_4da86b539924c</dc:identifier>
		<dc:Title>Cognitive Atlas : Lexicon : spatial span test</dc:Title>
		<dc:Description>RDF output for 'spatial span test'</dc:Description>
		<dc:Type>InteractiveResource</dc:Type>
		<dc:Publisher>Cognitive Atlas</dc:Publisher>
		<dc:Creator>Cognitive Atlas RDF Generator</dc:Creator>
		<dc:Contributor>Natalie Picchetti</dc:Contributor>
		<dc:Date>2011-04-15 08:59:15</dc:Date>
		<dc:Format>text/rdf</dc:Format>
		<dc:Language>en</dc:Language>
		<skos:editorialNote>Generated by testgen.php on Thu Jun 9 14:25:25 PDT 2011.</skos:editorialNote>
		<skos:historyNote>No previous definition revisions.</skos:historyNote>
		<skos:changeNote>This is the first and only definition provided.</skos:changeNote>
		<skos:scopeNote>http://www.w3.org/2004/02/skos/core#Concept</skos:scopeNote>
		<skos:Note>SKOS properties defined in http://www.w3.org/TR/skos-primer/#secrel</skos:Note>
		<skos:inScheme rdf:resource="http://cognitiveatlas.org/tasks/"/>
		<skos:definition>No definition submitted yet.</skos:definition>
		<skos:prefLabel>spatial span test</skos:prefLabel>
		<skos:altLabel></skos:altLabel>
</skos:Concept><skos:Concept rdf:about="http://cognitiveatlas.org/id/trm_4da86b75c6a5a"> <dc:identifier>trm_4da86b75c6a5a</dc:identifier>
		<dc:Title>Cognitive Atlas : Lexicon : letter-number sequencing</dc:Title>
		<dc:Description>RDF output for 'letter-number sequencing'</dc:Description>
		<dc:Type>InteractiveResource</dc:Type>
		<dc:Publisher>Cognitive Atlas</dc:Publisher>
		<dc:Creator>Cognitive Atlas RDF Generator</dc:Creator>
		<dc:Contributor>Natalie Picchetti</dc:Contributor>
		<dc:Date>2011-04-15 09:00:23</dc:Date>
		<dc:Format>text/rdf</dc:Format>
		<dc:Language>en</dc:Language>
		<skos:editorialNote>Generated by testgen.php on Thu Jun 9 14:25:25 PDT 2011.</skos:editorialNote>
		<skos:historyNote>Revision 2: 1 previous definitions.</skos:historyNote>
		<skos:changeNote>See http://cognitiveatlas.org/id/trm_4da86b75c6a5a for complete revision history.</skos:changeNote>
		<skos:scopeNote>http://www.w3.org/2004/02/skos/core#Concept</skos:scopeNote>
		<skos:Note>SKOS properties defined in http://www.w3.org/TR/skos-primer/#secrel</skos:Note>
		<skos:inScheme rdf:resource="http://cognitiveatlas.org/tasks/"/>
		<skos:definition>No definition submitted yet.</skos:definition>
		<skos:prefLabel>letter-number sequencing</skos:prefLabel>
		<skos:altLabel></skos:altLabel>
</skos:Concept><skos:Concept rdf:about="http://cognitiveatlas.org/id/trm_4da86c2a70a7d"> <dc:identifier>trm_4da86c2a70a7d</dc:identifier>
		<dc:Title>Cognitive Atlas : Lexicon : Dot Pattern Expectancy Task</dc:Title>
		<dc:Description>RDF output for 'Dot Pattern Expectancy Task'</dc:Description>
		<dc:Type>InteractiveResource</dc:Type>
		<dc:Publisher>Cognitive Atlas</dc:Publisher>
		<dc:Creator>Cognitive Atlas RDF Generator</dc:Creator>
		<dc:Contributor>Natalie Picchetti</dc:Contributor>
		<dc:Date>2011-04-15 09:02:50</dc:Date>
		<dc:Format>text/rdf</dc:Format>
		<dc:Language>en</dc:Language>
		<skos:editorialNote>Generated by testgen.php on Thu Jun 9 14:25:25 PDT 2011.</skos:editorialNote>
		<skos:historyNote>No previous definition revisions.</skos:historyNote>
		<skos:changeNote>This is the first and only definition provided.</skos:changeNote>
		<skos:scopeNote>http://www.w3.org/2004/02/skos/core#Concept</skos:scopeNote>
		<skos:Note>SKOS properties defined in http://www.w3.org/TR/skos-primer/#secrel</skos:Note>
		<skos:inScheme rdf:resource="http://cognitiveatlas.org/tasks/"/>
		<skos:definition>No definition submitted yet.</skos:definition>
		<skos:prefLabel>Dot Pattern Expectancy Task</skos:prefLabel>
		<skos:altLabel></skos:altLabel>
</skos:Concept><skos:Concept rdf:about="http://cognitiveatlas.org/id/trm_4da86c6808ddd"> <dc:identifier>trm_4da86c6808ddd</dc:identifier>
		<dc:Title>Cognitive Atlas : Lexicon : cattell culture fair intelligence test</dc:Title>
		<dc:Description>RDF output for 'cattell culture fair intelligence test'</dc:Description>
		<dc:Type>InteractiveResource</dc:Type>
		<dc:Publisher>Cognitive Atlas</dc:Publisher>
		<dc:Creator>Cognitive Atlas RDF Generator</dc:Creator>
		<dc:Contributor>Natalie Picchetti</dc:Contributor>
		<dc:Date>2011-04-15 09:03:52</dc:Date>
		<dc:Format>text/rdf</dc:Format>
		<dc:Language>en</dc:Language>
		<skos:editorialNote>Generated by testgen.php on Thu Jun 9 14:25:25 PDT 2011.</skos:editorialNote>
		<skos:historyNote>No previous definition revisions.</skos:historyNote>
		<skos:changeNote>This is the first and only definition provided.</skos:changeNote>
		<skos:scopeNote>http://www.w3.org/2004/02/skos/core#Concept</skos:scopeNote>
		<skos:Note>SKOS properties defined in http://www.w3.org/TR/skos-primer/#secrel</skos:Note>
		<skos:inScheme rdf:resource="http://cognitiveatlas.org/tasks/"/>
		<skos:definition>No definition submitted yet.</skos:definition>
		<skos:prefLabel>cattell culture fair intelligence test</skos:prefLabel>
		<skos:altLabel></skos:altLabel>
</skos:Concept><skos:Concept rdf:about="http://cognitiveatlas.org/id/trm_4da86c8bb3b04"> <dc:identifier>trm_4da86c8bb3b04</dc:identifier>
		<dc:Title>Cognitive Atlas : Lexicon : letter comparison</dc:Title>
		<dc:Description>RDF output for 'letter comparison'</dc:Description>
		<dc:Type>InteractiveResource</dc:Type>
		<dc:Publisher>Cognitive Atlas</dc:Publisher>
		<dc:Creator>Cognitive Atlas RDF Generator</dc:Creator>
		<dc:Contributor>Natalie Picchetti</dc:Contributor>
		<dc:Date>2011-04-15 09:04:27</dc:Date>
		<dc:Format>text/rdf</dc:Format>
		<dc:Language>en</dc:Language>
		<skos:editorialNote>Generated by testgen.php on Thu Jun 9 14:25:25 PDT 2011.</skos:editorialNote>
		<skos:historyNote>No previous definition revisions.</skos:historyNote>
		<skos:changeNote>This is the first and only definition provided.</skos:changeNote>
		<skos:scopeNote>http://www.w3.org/2004/02/skos/core#Concept</skos:scopeNote>
		<skos:Note>SKOS properties defined in http://www.w3.org/TR/skos-primer/#secrel</skos:Note>
		<skos:inScheme rdf:resource="http://cognitiveatlas.org/tasks/"/>
		<skos:definition>No definition submitted yet.</skos:definition>
		<skos:prefLabel>letter comparison</skos:prefLabel>
		<skos:altLabel></skos:altLabel>
</skos:Concept><skos:Concept rdf:about="http://cognitiveatlas.org/id/trm_4da86cb034ff6"> <dc:identifier>trm_4da86cb034ff6</dc:identifier>
		<dc:Title>Cognitive Atlas : Lexicon : pattern comparison</dc:Title>
		<dc:Description>RDF output for 'pattern comparison'</dc:Description>
		<dc:Type>InteractiveResource</dc:Type>
		<dc:Publisher>Cognitive Atlas</dc:Publisher>
		<dc:Creator>Cognitive Atlas RDF Generator</dc:Creator>
		<dc:Contributor>Natalie Picchetti</dc:Contributor>
		<dc:Date>2011-04-15 09:05:04</dc:Date>
		<dc:Format>text/rdf</dc:Format>
		<dc:Language>en</dc:Language>
		<skos:editorialNote>Generated by testgen.php on Thu Jun 9 14:25:25 PDT 2011.</skos:editorialNote>
		<skos:historyNote>No previous definition revisions.</skos:historyNote>
		<skos:changeNote>This is the first and only definition provided.</skos:changeNote>
		<skos:scopeNote>http://www.w3.org/2004/02/skos/core#Concept</skos:scopeNote>
		<skos:Note>SKOS properties defined in http://www.w3.org/TR/skos-primer/#secrel</skos:Note>
		<skos:inScheme rdf:resource="http://cognitiveatlas.org/tasks/"/>
		<skos:definition>No definition submitted yet.</skos:definition>
		<skos:prefLabel>pattern comparison</skos:prefLabel>
		<skos:altLabel></skos:altLabel>
</skos:Concept><skos:Concept rdf:about="http://cognitiveatlas.org/id/trm_4da86cdbd9eeb"> <dc:identifier>trm_4da86cdbd9eeb</dc:identifier>
		<dc:Title>Cognitive Atlas : Lexicon : test of variables of attention</dc:Title>
		<dc:Description>RDF output for 'test of variables of attention'</dc:Description>
		<dc:Type>InteractiveResource</dc:Type>
		<dc:Publisher>Cognitive Atlas</dc:Publisher>
		<dc:Creator>Cognitive Atlas RDF Generator</dc:Creator>
		<dc:Contributor>Natalie Picchetti</dc:Contributor>
		<dc:Date>2011-04-15 09:05:47</dc:Date>
		<dc:Format>text/rdf</dc:Format>
		<dc:Language>en</dc:Language>
		<skos:editorialNote>Generated by testgen.php on Thu Jun 9 14:25:25 PDT 2011.</skos:editorialNote>
		<skos:historyNote>No previous definition revisions.</skos:historyNote>
		<skos:changeNote>This is the first and only definition provided.</skos:changeNote>
		<skos:scopeNote>http://www.w3.org/2004/02/skos/core#Concept</skos:scopeNote>
		<skos:Note>SKOS properties defined in http://www.w3.org/TR/skos-primer/#secrel</skos:Note>
		<skos:inScheme rdf:resource="http://cognitiveatlas.org/tasks/"/>
		<skos:definition>No definition submitted yet.</skos:definition>
		<skos:prefLabel>test of variables of attention</skos:prefLabel>
		<skos:altLabel></skos:altLabel>
</skos:Concept><skos:Concept rdf:about="http://cognitiveatlas.org/id/trm_4da86cfe8cf1b"> <dc:identifier>trm_4da86cfe8cf1b</dc:identifier>
		<dc:Title>Cognitive Atlas : Lexicon : sustained attention to response task</dc:Title>
		<dc:Description>RDF output for 'sustained attention to response task'</dc:Description>
		<dc:Type>InteractiveResource</dc:Type>
		<dc:Publisher>Cognitive Atlas</dc:Publisher>
		<dc:Creator>Cognitive Atlas RDF Generator</dc:Creator>
		<dc:Contributor>Natalie Picchetti</dc:Contributor>
		<dc:Date>2011-04-15 09:06:22</dc:Date>
		<dc:Format>text/rdf</dc:Format>
		<dc:Language>en</dc:Language>
		<skos:editorialNote>Generated by testgen.php on Thu Jun 9 14:25:25 PDT 2011.</skos:editorialNote>
		<skos:historyNote>No previous definition revisions.</skos:historyNote>
		<skos:changeNote>This is the first and only definition provided.</skos:changeNote>
		<skos:scopeNote>http://www.w3.org/2004/02/skos/core#Concept</skos:scopeNote>
		<skos:Note>SKOS properties defined in http://www.w3.org/TR/skos-primer/#secrel</skos:Note>
		<skos:inScheme rdf:resource="http://cognitiveatlas.org/tasks/"/>
		<skos:definition>No definition submitted yet.</skos:definition>
		<skos:prefLabel>sustained attention to response task</skos:prefLabel>
		<skos:altLabel></skos:altLabel>
</skos:Concept><skos:Concept rdf:about="http://cognitiveatlas.org/id/trm_4da87b8bf1511"> <dc:identifier>trm_4da87b8bf1511</dc:identifier>
		<dc:Title>Cognitive Atlas : Lexicon : matching familiar figures test</dc:Title>
		<dc:Description>RDF output for 'matching familiar figures test'</dc:Description>
		<dc:Type>InteractiveResource</dc:Type>
		<dc:Publisher>Cognitive Atlas</dc:Publisher>
		<dc:Creator>Cognitive Atlas RDF Generator</dc:Creator>
		<dc:Contributor>Natalie Picchetti</dc:Contributor>
		<dc:Date>2011-04-15 10:08:27</dc:Date>
		<dc:Format>text/rdf</dc:Format>
		<dc:Language>en</dc:Language>
		<skos:editorialNote>Generated by testgen.php on Thu Jun 9 14:25:25 PDT 2011.</skos:editorialNote>
		<skos:historyNote>No previous definition revisions.</skos:historyNote>
		<skos:changeNote>This is the first and only definition provided.</skos:changeNote>
		<skos:scopeNote>http://www.w3.org/2004/02/skos/core#Concept</skos:scopeNote>
		<skos:Note>SKOS properties defined in http://www.w3.org/TR/skos-primer/#secrel</skos:Note>
		<skos:inScheme rdf:resource="http://cognitiveatlas.org/tasks/"/>
		<skos:definition>No definition submitted yet.</skos:definition>
		<skos:prefLabel>matching familiar figures test</skos:prefLabel>
		<skos:altLabel></skos:altLabel>
</skos:Concept><skos:Concept rdf:about="http://cognitiveatlas.org/id/trm_4da87e439c411"> <dc:identifier>trm_4da87e439c411</dc:identifier>
		<dc:Title>Cognitive Atlas : Lexicon : Tower of London</dc:Title>
		<dc:Description>RDF output for 'Tower of London'</dc:Description>
		<dc:Type>InteractiveResource</dc:Type>
		<dc:Publisher>Cognitive Atlas</dc:Publisher>
		<dc:Creator>Cognitive Atlas RDF Generator</dc:Creator>
		<dc:Contributor>Natalie Picchetti</dc:Contributor>
		<dc:Date>2011-04-15 10:20:03</dc:Date>
		<dc:Format>text/rdf</dc:Format>
		<dc:Language>en</dc:Language>
		<skos:editorialNote>Generated by testgen.php on Thu Jun 9 14:25:25 PDT 2011.</skos:editorialNote>
		<skos:historyNote>No previous definition revisions.</skos:historyNote>
		<skos:changeNote>This is the first and only definition provided.</skos:changeNote>
		<skos:scopeNote>http://www.w3.org/2004/02/skos/core#Concept</skos:scopeNote>
		<skos:Note>SKOS properties defined in http://www.w3.org/TR/skos-primer/#secrel</skos:Note>
		<skos:inScheme rdf:resource="http://cognitiveatlas.org/tasks/"/>
		<skos:definition>No definition submitted yet.</skos:definition>
		<skos:prefLabel>Tower of London</skos:prefLabel>
		<skos:altLabel></skos:altLabel>
</skos:Concept><skos:Concept rdf:about="http://cognitiveatlas.org/id/trm_4da87e7282f92"> <dc:identifier>trm_4da87e7282f92</dc:identifier>
		<dc:Title>Cognitive Atlas : Lexicon : Tower of Hanoi</dc:Title>
		<dc:Description>RDF output for 'Tower of Hanoi'</dc:Description>
		<dc:Type>InteractiveResource</dc:Type>
		<dc:Publisher>Cognitive Atlas</dc:Publisher>
		<dc:Creator>Cognitive Atlas RDF Generator</dc:Creator>
		<dc:Contributor>Natalie Picchetti</dc:Contributor>
		<dc:Date>2011-04-15 10:20:50</dc:Date>
		<dc:Format>text/rdf</dc:Format>
		<dc:Language>en</dc:Language>
		<skos:editorialNote>Generated by testgen.php on Thu Jun 9 14:25:25 PDT 2011.</skos:editorialNote>
		<skos:historyNote>No previous definition revisions.</skos:historyNote>
		<skos:changeNote>This is the first and only definition provided.</skos:changeNote>
		<skos:scopeNote>http://www.w3.org/2004/02/skos/core#Concept</skos:scopeNote>
		<skos:Note>SKOS properties defined in http://www.w3.org/TR/skos-primer/#secrel</skos:Note>
		<skos:inScheme rdf:resource="http://cognitiveatlas.org/tasks/"/>
		<skos:definition>No definition submitted yet.</skos:definition>
		<skos:prefLabel>Tower of Hanoi</skos:prefLabel>
		<skos:altLabel></skos:altLabel>
</skos:Concept><skos:Concept rdf:about="http://cognitiveatlas.org/id/trm_4da87e9c79847"> <dc:identifier>trm_4da87e9c79847</dc:identifier>
		<dc:Title>Cognitive Atlas : Lexicon : dichotic listening task</dc:Title>
		<dc:Description>RDF output for 'dichotic listening task'</dc:Description>
		<dc:Type>InteractiveResource</dc:Type>
		<dc:Publisher>Cognitive Atlas</dc:Publisher>
		<dc:Creator>Cognitive Atlas RDF Generator</dc:Creator>
		<dc:Contributor>Natalie Picchetti</dc:Contributor>
		<dc:Date>2011-04-15 10:21:32</dc:Date>
		<dc:Format>text/rdf</dc:Format>
		<dc:Language>en</dc:Language>
		<skos:editorialNote>Generated by testgen.php on Thu Jun 9 14:25:25 PDT 2011.</skos:editorialNote>
		<skos:historyNote>No previous definition revisions.</skos:historyNote>
		<skos:changeNote>This is the first and only definition provided.</skos:changeNote>
		<skos:scopeNote>http://www.w3.org/2004/02/skos/core#Concept</skos:scopeNote>
		<skos:Note>SKOS properties defined in http://www.w3.org/TR/skos-primer/#secrel</skos:Note>
		<skos:inScheme rdf:resource="http://cognitiveatlas.org/tasks/"/>
		<skos:definition>No definition submitted yet.</skos:definition>
		<skos:prefLabel>dichotic listening task</skos:prefLabel>
		<skos:altLabel></skos:altLabel>
</skos:Concept><skos:Concept rdf:about="http://cognitiveatlas.org/id/trm_4da87f383435b"> <dc:identifier>trm_4da87f383435b</dc:identifier>
		<dc:Title>Cognitive Atlas : Lexicon : directed forgetting task</dc:Title>
		<dc:Description>RDF output for 'directed forgetting task'</dc:Description>
		<dc:Type>InteractiveResource</dc:Type>
		<dc:Publisher>Cognitive Atlas</dc:Publisher>
		<dc:Creator>Cognitive Atlas RDF Generator</dc:Creator>
		<dc:Contributor>Natalie Picchetti</dc:Contributor>
		<dc:Date>2011-04-15 10:24:08</dc:Date>
		<dc:Format>text/rdf</dc:Format>
		<dc:Language>en</dc:Language>
		<skos:editorialNote>Generated by testgen.php on Thu Jun 9 14:25:25 PDT 2011.</skos:editorialNote>
		<skos:historyNote>No previous definition revisions.</skos:historyNote>
		<skos:changeNote>This is the first and only definition provided.</skos:changeNote>
		<skos:scopeNote>http://www.w3.org/2004/02/skos/core#Concept</skos:scopeNote>
		<skos:Note>SKOS properties defined in http://www.w3.org/TR/skos-primer/#secrel</skos:Note>
		<skos:inScheme rdf:resource="http://cognitiveatlas.org/tasks/"/>
		<skos:definition>No definition submitted yet.</skos:definition>
		<skos:prefLabel>directed forgetting task</skos:prefLabel>
		<skos:altLabel></skos:altLabel>
</skos:Concept><skos:Concept rdf:about="http://cognitiveatlas.org/id/trm_4da87f81bc2c8"> <dc:identifier>trm_4da87f81bc2c8</dc:identifier>
		<dc:Title>Cognitive Atlas : Lexicon : retrieval-induced forgetting task</dc:Title>
		<dc:Description>RDF output for 'retrieval-induced forgetting task'</dc:Description>
		<dc:Type>InteractiveResource</dc:Type>
		<dc:Publisher>Cognitive Atlas</dc:Publisher>
		<dc:Creator>Cognitive Atlas RDF Generator</dc:Creator>
		<dc:Contributor>Natalie Picchetti</dc:Contributor>
		<dc:Date>2011-04-15 10:25:21</dc:Date>
		<dc:Format>text/rdf</dc:Format>
		<dc:Language>en</dc:Language>
		<skos:editorialNote>Generated by testgen.php on Thu Jun 9 14:25:25 PDT 2011.</skos:editorialNote>
		<skos:historyNote>No previous definition revisions.</skos:historyNote>
		<skos:changeNote>This is the first and only definition provided.</skos:changeNote>
		<skos:scopeNote>http://www.w3.org/2004/02/skos/core#Concept</skos:scopeNote>
		<skos:Note>SKOS properties defined in http://www.w3.org/TR/skos-primer/#secrel</skos:Note>
		<skos:inScheme rdf:resource="http://cognitiveatlas.org/tasks/"/>
		<skos:definition>No definition submitted yet.</skos:definition>
		<skos:prefLabel>retrieval-induced forgetting task</skos:prefLabel>
		<skos:altLabel></skos:altLabel>
</skos:Concept><skos:Concept rdf:about="http://cognitiveatlas.org/id/trm_4da87fb28978e"> <dc:identifier>trm_4da87fb28978e</dc:identifier>
		<dc:Title>Cognitive Atlas : Lexicon : Paced Auditory Serial Addition Test</dc:Title>
		<dc:Description>RDF output for 'Paced Auditory Serial Addition Test'</dc:Description>
		<dc:Type>InteractiveResource</dc:Type>
		<dc:Publisher>Cognitive Atlas</dc:Publisher>
		<dc:Creator>Cognitive Atlas RDF Generator</dc:Creator>
		<dc:Contributor>Natalie Picchetti</dc:Contributor>
		<dc:Date>2011-04-15 10:26:10</dc:Date>
		<dc:Format>text/rdf</dc:Format>
		<dc:Language>en</dc:Language>
		<skos:editorialNote>Generated by testgen.php on Thu Jun 9 14:25:25 PDT 2011.</skos:editorialNote>
		<skos:historyNote>No previous definition revisions.</skos:historyNote>
		<skos:changeNote>This is the first and only definition provided.</skos:changeNote>
		<skos:scopeNote>http://www.w3.org/2004/02/skos/core#Concept</skos:scopeNote>
		<skos:Note>SKOS properties defined in http://www.w3.org/TR/skos-primer/#secrel</skos:Note>
		<skos:inScheme rdf:resource="http://cognitiveatlas.org/tasks/"/>
		<skos:definition>No definition submitted yet.</skos:definition>
		<skos:prefLabel>Paced Auditory Serial Addition Test</skos:prefLabel>
		<skos:altLabel></skos:altLabel>
</skos:Concept><skos:Concept rdf:about="http://cognitiveatlas.org/id/trm_4da87fdd7820e"> <dc:identifier>trm_4da87fdd7820e</dc:identifier>
		<dc:Title>Cognitive Atlas : Lexicon : Porteus maze test</dc:Title>
		<dc:Description>RDF output for 'Porteus maze test'</dc:Description>
		<dc:Type>InteractiveResource</dc:Type>
		<dc:Publisher>Cognitive Atlas</dc:Publisher>
		<dc:Creator>Cognitive Atlas RDF Generator</dc:Creator>
		<dc:Contributor>Natalie Picchetti</dc:Contributor>
		<dc:Date>2011-04-15 10:26:53</dc:Date>
		<dc:Format>text/rdf</dc:Format>
		<dc:Language>en</dc:Language>
		<skos:editorialNote>Generated by testgen.php on Thu Jun 9 14:25:25 PDT 2011.</skos:editorialNote>
		<skos:historyNote>No previous definition revisions.</skos:historyNote>
		<skos:changeNote>This is the first and only definition provided.</skos:changeNote>
		<skos:scopeNote>http://www.w3.org/2004/02/skos/core#Concept</skos:scopeNote>
		<skos:Note>SKOS properties defined in http://www.w3.org/TR/skos-primer/#secrel</skos:Note>
		<skos:inScheme rdf:resource="http://cognitiveatlas.org/tasks/"/>
		<skos:definition>No definition submitted yet.</skos:definition>
		<skos:prefLabel>Porteus maze test</skos:prefLabel>
		<skos:altLabel></skos:altLabel>
</skos:Concept><skos:Concept rdf:about="http://cognitiveatlas.org/id/trm_4da880396c76b"> <dc:identifier>trm_4da880396c76b</dc:identifier>
		<dc:Title>Cognitive Atlas : Lexicon : Rey-Ostereith Complex Figure Test</dc:Title>
		<dc:Description>RDF output for 'Rey-Ostereith Complex Figure Test'</dc:Description>
		<dc:Type>InteractiveResource</dc:Type>
		<dc:Publisher>Cognitive Atlas</dc:Publisher>
		<dc:Creator>Cognitive Atlas RDF Generator</dc:Creator>
		<dc:Contributor>Natalie Picchetti</dc:Contributor>
		<dc:Date>2011-04-15 10:28:25</dc:Date>
		<dc:Format>text/rdf</dc:Format>
		<dc:Language>en</dc:Language>
		<skos:editorialNote>Generated by testgen.php on Thu Jun 9 14:25:25 PDT 2011.</skos:editorialNote>
		<skos:historyNote>No previous definition revisions.</skos:historyNote>
		<skos:changeNote>This is the first and only definition provided.</skos:changeNote>
		<skos:scopeNote>http://www.w3.org/2004/02/skos/core#Concept</skos:scopeNote>
		<skos:Note>SKOS properties defined in http://www.w3.org/TR/skos-primer/#secrel</skos:Note>
		<skos:inScheme rdf:resource="http://cognitiveatlas.org/tasks/"/>
		<skos:definition>No definition submitted yet.</skos:definition>
		<skos:prefLabel>Rey-Ostereith Complex Figure Test</skos:prefLabel>
		<skos:altLabel></skos:altLabel>
</skos:Concept><skos:Concept rdf:about="http://cognitiveatlas.org/id/trm_4da880ff8fd4a"> <dc:identifier>trm_4da880ff8fd4a</dc:identifier>
		<dc:Title>Cognitive Atlas : Lexicon : Cambridge Neuropsychological Test Automated Battery </dc:Title>
		<dc:Description>RDF output for 'Cambridge Neuropsychological Test Automated Battery '</dc:Description>
		<dc:Type>InteractiveResource</dc:Type>
		<dc:Publisher>Cognitive Atlas</dc:Publisher>
		<dc:Creator>Cognitive Atlas RDF Generator</dc:Creator>
		<dc:Contributor>Natalie Picchetti</dc:Contributor>
		<dc:Date>2011-04-15 10:31:43</dc:Date>
		<dc:Format>text/rdf</dc:Format>
		<dc:Language>en</dc:Language>
		<skos:editorialNote>Generated by testgen.php on Thu Jun 9 14:25:25 PDT 2011.</skos:editorialNote>
		<skos:historyNote>No previous definition revisions.</skos:historyNote>
		<skos:changeNote>This is the first and only definition provided.</skos:changeNote>
		<skos:scopeNote>http://www.w3.org/2004/02/skos/core#Concept</skos:scopeNote>
		<skos:Note>SKOS properties defined in http://www.w3.org/TR/skos-primer/#secrel</skos:Note>
		<skos:inScheme rdf:resource="http://cognitiveatlas.org/tasks/"/>
		<skos:definition>is a computer-based cognitive assessment system consisting of a battery of neuropsychological tests, administered to subjects using a touch screen computer. The 22 tests in CANTAB examine various areas of cognitive function, including:

    * general memory and learning,
    * working memory and executive function,
    * visual memory,
    * attention and reaction time (RT),
    * semantic/verbal memory,
    * decision making and response control.

The CANTAB endeavours to import the accuracy and rigour of computerised psychological testing whilst retaining the wide range of ability measures demanded of a neuropsychological battery. It is suitable for young and old subjects, and aims to be culture and language independent through the use of non-verbal stimuli in the majority of the tests.</skos:definition>
		<skos:prefLabel>Cambridge Neuropsychological Test Automated Battery </skos:prefLabel>
		<skos:altLabel></skos:altLabel>
</skos:Concept><skos:Concept rdf:about="http://cognitiveatlas.org/id/trm_4da881dace79c"> <dc:identifier>trm_4da881dace79c</dc:identifier>
		<dc:Title>Cognitive Atlas : Lexicon : Corsi Blocks</dc:Title>
		<dc:Description>RDF output for 'Corsi Blocks'</dc:Description>
		<dc:Type>InteractiveResource</dc:Type>
		<dc:Publisher>Cognitive Atlas</dc:Publisher>
		<dc:Creator>Cognitive Atlas RDF Generator</dc:Creator>
		<dc:Contributor>Natalie Picchetti</dc:Contributor>
		<dc:Date>2011-04-15 10:35:51</dc:Date>
		<dc:Format>text/rdf</dc:Format>
		<dc:Language>en</dc:Language>
		<skos:editorialNote>Generated by testgen.php on Thu Jun 9 14:25:25 PDT 2011.</skos:editorialNote>
		<skos:historyNote>Revision 2: 1 previous definitions.</skos:historyNote>
		<skos:changeNote>See http://cognitiveatlas.org/id/trm_4da881dace79c for complete revision history.</skos:changeNote>
		<skos:scopeNote>http://www.w3.org/2004/02/skos/core#Concept</skos:scopeNote>
		<skos:Note>SKOS properties defined in http://www.w3.org/TR/skos-primer/#secrel</skos:Note>
		<skos:inScheme rdf:resource="http://cognitiveatlas.org/tasks/"/>
		<skos:definition>was developed in the early 1970s as a visuospatial counterpart to the verbal-memory span task (Milner, 1971). Over the years, it has frequently been used to assess visuospatial short-term memory performance in adults (e.g. Smyth &amp; Scholey, 1992), children (e.g. Orsini, Schiappa, &amp; Grossi, 1981), and patients with neuropsychological deficits (e.g. Vilkki &amp; Holst, 1989). 

The original Corsi apparatus consisted of a set of nine identical blocks (3 X 3 X 3 cm) irregularly positioned on a wooden board (23 X 28 cm). The experimenter points to a series of blocks at a rate of one block per second. Subsequently, the participant is required to point to the same blocks in their order of presentation. The length of the block sequences increases until recall is no longer correct. 

Numerous variations have since been employed in both display characteristics (e.g. colour, number and size of the blocks, block placement, size of the board) and test administration (e.g. presentation rate, block sequences, recall order, scoring technique) (for a review, see Berch, Krikorian, &amp; Huha, 1998).</skos:definition>
		<skos:prefLabel>Corsi Blocks</skos:prefLabel>
		<skos:altLabel></skos:altLabel>
		<skos:related rdf:resource="http://cognitiveatlas.org/id/tsk_4a57abb9498df"/>
		<skos:example>Block Tapping Test is descended from Corsi Blocks</skos:example>
</skos:Concept><skos:Concept rdf:about="http://cognitiveatlas.org/id/trm_4da886fc2bc46"> <dc:identifier>trm_4da886fc2bc46</dc:identifier>
		<dc:Title>Cognitive Atlas : Lexicon : Visual Patterns Test</dc:Title>
		<dc:Description>RDF output for 'Visual Patterns Test'</dc:Description>
		<dc:Type>InteractiveResource</dc:Type>
		<dc:Publisher>Cognitive Atlas</dc:Publisher>
		<dc:Creator>Cognitive Atlas RDF Generator</dc:Creator>
		<dc:Contributor>Natalie Picchetti</dc:Contributor>
		<dc:Date>2011-04-15 10:57:16</dc:Date>
		<dc:Format>text/rdf</dc:Format>
		<dc:Language>en</dc:Language>
		<skos:editorialNote>Generated by testgen.php on Thu Jun 9 14:25:25 PDT 2011.</skos:editorialNote>
		<skos:historyNote>No previous definition revisions.</skos:historyNote>
		<skos:changeNote>This is the first and only definition provided.</skos:changeNote>
		<skos:scopeNote>http://www.w3.org/2004/02/skos/core#Concept</skos:scopeNote>
		<skos:Note>SKOS properties defined in http://www.w3.org/TR/skos-primer/#secrel</skos:Note>
		<skos:inScheme rdf:resource="http://cognitiveatlas.org/tasks/"/>
		<skos:definition>is a measure of short term visual memory that has been designed for use both as a clinical tool and a research instrument.  In the VPT, the subject is presented with matrix patterns of black and white squares in grids of varying size and required to memorize a series of black and white checkerboard-like patterns of increasing complexity. Such matrix patterns are virtually impossible to code verbally.</skos:definition>
		<skos:prefLabel>Visual Patterns Test</skos:prefLabel>
		<skos:altLabel></skos:altLabel>
</skos:Concept><skos:Concept rdf:about="http://cognitiveatlas.org/id/trm_4da887bdd8908"> <dc:identifier>trm_4da887bdd8908</dc:identifier>
		<dc:Title>Cognitive Atlas : Lexicon : mirror tracing test</dc:Title>
		<dc:Description>RDF output for 'mirror tracing test'</dc:Description>
		<dc:Type>InteractiveResource</dc:Type>
		<dc:Publisher>Cognitive Atlas</dc:Publisher>
		<dc:Creator>Cognitive Atlas RDF Generator</dc:Creator>
		<dc:Contributor>Natalie Picchetti</dc:Contributor>
		<dc:Date>2011-04-15 11:00:29</dc:Date>
		<dc:Format>text/rdf</dc:Format>
		<dc:Language>en</dc:Language>
		<skos:editorialNote>Generated by testgen.php on Thu Jun 9 14:25:25 PDT 2011.</skos:editorialNote>
		<skos:historyNote>No previous definition revisions.</skos:historyNote>
		<skos:changeNote>This is the first and only definition provided.</skos:changeNote>
		<skos:scopeNote>http://www.w3.org/2004/02/skos/core#Concept</skos:scopeNote>
		<skos:Note>SKOS properties defined in http://www.w3.org/TR/skos-primer/#secrel</skos:Note>
		<skos:inScheme rdf:resource="http://cognitiveatlas.org/tasks/"/>
		<skos:definition>No definition submitted yet.</skos:definition>
		<skos:prefLabel>mirror tracing test</skos:prefLabel>
		<skos:altLabel></skos:altLabel>
</skos:Concept><skos:Concept rdf:about="http://cognitiveatlas.org/id/trm_4da8885b33375"> <dc:identifier>trm_4da8885b33375</dc:identifier>
		<dc:Title>Cognitive Atlas : Lexicon : Rivermead Behavioural Memory Test</dc:Title>
		<dc:Description>RDF output for 'Rivermead Behavioural Memory Test'</dc:Description>
		<dc:Type>InteractiveResource</dc:Type>
		<dc:Publisher>Cognitive Atlas</dc:Publisher>
		<dc:Creator>Cognitive Atlas RDF Generator</dc:Creator>
		<dc:Contributor>Natalie Picchetti</dc:Contributor>
		<dc:Date>2011-04-15 11:03:07</dc:Date>
		<dc:Format>text/rdf</dc:Format>
		<dc:Language>en</dc:Language>
		<skos:editorialNote>Generated by testgen.php on Thu Jun 9 14:25:25 PDT 2011.</skos:editorialNote>
		<skos:historyNote>No previous definition revisions.</skos:historyNote>
		<skos:changeNote>This is the first and only definition provided.</skos:changeNote>
		<skos:scopeNote>http://www.w3.org/2004/02/skos/core#Concept</skos:scopeNote>
		<skos:Note>SKOS properties defined in http://www.w3.org/TR/skos-primer/#secrel</skos:Note>
		<skos:inScheme rdf:resource="http://cognitiveatlas.org/tasks/"/>
		<skos:definition>comprises a number of subtests focused on providing objective measures of everyday memory performance in people with observed and/or reported memory difficulties.</skos:definition>
		<skos:prefLabel>Rivermead Behavioural Memory Test</skos:prefLabel>
		<skos:altLabel></skos:altLabel>
</skos:Concept><skos:Concept rdf:about="http://cognitiveatlas.org/id/trm_4da88a2a63d97"> <dc:identifier>trm_4da88a2a63d97</dc:identifier>
		<dc:Title>Cognitive Atlas : Lexicon : Paired Associate Learning</dc:Title>
		<dc:Description>RDF output for 'Paired Associate Learning'</dc:Description>
		<dc:Type>InteractiveResource</dc:Type>
		<dc:Publisher>Cognitive Atlas</dc:Publisher>
		<dc:Creator>Cognitive Atlas RDF Generator</dc:Creator>
		<dc:Contributor>Natalie Picchetti</dc:Contributor>
		<dc:Date>2011-04-15 11:10:50</dc:Date>
		<dc:Format>text/rdf</dc:Format>
		<dc:Language>en</dc:Language>
		<skos:editorialNote>Generated by testgen.php on Thu Jun 9 14:25:25 PDT 2011.</skos:editorialNote>
		<skos:historyNote>No previous definition revisions.</skos:historyNote>
		<skos:changeNote>This is the first and only definition provided.</skos:changeNote>
		<skos:scopeNote>http://www.w3.org/2004/02/skos/core#Concept</skos:scopeNote>
		<skos:Note>SKOS properties defined in http://www.w3.org/TR/skos-primer/#secrel</skos:Note>
		<skos:inScheme rdf:resource="http://cognitiveatlas.org/tasks/"/>
		<skos:definition>was invented by Mary Whiton Calkins in 1894 and involves the pairing of two items (usually words)—a stimulus and a response. For example, words such as calendar (stimulus) and shoe (response) may be paired, and when the learner is prompted with the stimulus, he responds with the appropriate word (shoe).</skos:definition>
		<skos:prefLabel>Paired Associate Learning</skos:prefLabel>
		<skos:altLabel></skos:altLabel>
</skos:Concept><skos:Concept rdf:about="http://cognitiveatlas.org/id/trm_4da88a8e13f26"> <dc:identifier>trm_4da88a8e13f26</dc:identifier>
		<dc:Title>Cognitive Atlas : Lexicon : Vigilance</dc:Title>
		<dc:Description>RDF output for 'Vigilance'</dc:Description>
		<dc:Type>InteractiveResource</dc:Type>
		<dc:Publisher>Cognitive Atlas</dc:Publisher>
		<dc:Creator>Cognitive Atlas RDF Generator</dc:Creator>
		<dc:Contributor>Natalie Picchetti</dc:Contributor>
		<dc:Date>2011-04-15 11:12:30</dc:Date>
		<dc:Format>text/rdf</dc:Format>
		<dc:Language>en</dc:Language>
		<skos:editorialNote>Generated by testgen.php on Thu Jun 9 14:25:25 PDT 2011.</skos:editorialNote>
		<skos:historyNote>No previous definition revisions.</skos:historyNote>
		<skos:changeNote>This is the first and only definition provided.</skos:changeNote>
		<skos:scopeNote>http://www.w3.org/2004/02/skos/core#Concept</skos:scopeNote>
		<skos:Note>SKOS properties defined in http://www.w3.org/TR/skos-primer/#secrel</skos:Note>
		<skos:inScheme rdf:resource="http://cognitiveatlas.org/tasks/"/>
		<skos:definition>No definition submitted yet.</skos:definition>
		<skos:prefLabel>Vigilance</skos:prefLabel>
		<skos:altLabel></skos:altLabel>
</skos:Concept><skos:Concept rdf:about="http://cognitiveatlas.org/id/trm_4da88ae0f2952"> <dc:identifier>trm_4da88ae0f2952</dc:identifier>
		<dc:Title>Cognitive Atlas : Lexicon : Rey Auditory Verbal Learning Task</dc:Title>
		<dc:Description>RDF output for 'Rey Auditory Verbal Learning Task'</dc:Description>
		<dc:Type>InteractiveResource</dc:Type>
		<dc:Publisher>Cognitive Atlas</dc:Publisher>
		<dc:Creator>Cognitive Atlas RDF Generator</dc:Creator>
		<dc:Contributor>Natalie Picchetti</dc:Contributor>
		<dc:Date>2011-04-15 11:13:52</dc:Date>
		<dc:Format>text/rdf</dc:Format>
		<dc:Language>en</dc:Language>
		<skos:editorialNote>Generated by testgen.php on Thu Jun 9 14:25:25 PDT 2011.</skos:editorialNote>
		<skos:historyNote>No previous definition revisions.</skos:historyNote>
		<skos:changeNote>This is the first and only definition provided.</skos:changeNote>
		<skos:scopeNote>http://www.w3.org/2004/02/skos/core#Concept</skos:scopeNote>
		<skos:Note>SKOS properties defined in http://www.w3.org/TR/skos-primer/#secrel</skos:Note>
		<skos:inScheme rdf:resource="http://cognitiveatlas.org/tasks/"/>
		<skos:definition>No definition submitted yet.</skos:definition>
		<skos:prefLabel>Rey Auditory Verbal Learning Task</skos:prefLabel>
		<skos:altLabel></skos:altLabel>
</skos:Concept><skos:Concept rdf:about="http://cognitiveatlas.org/id/trm_4da88b17b985b"> <dc:identifier>trm_4da88b17b985b</dc:identifier>
		<dc:Title>Cognitive Atlas : Lexicon : Nonword Repetition Task</dc:Title>
		<dc:Description>RDF output for 'Nonword Repetition Task'</dc:Description>
		<dc:Type>InteractiveResource</dc:Type>
		<dc:Publisher>Cognitive Atlas</dc:Publisher>
		<dc:Creator>Cognitive Atlas RDF Generator</dc:Creator>
		<dc:Contributor>Natalie Picchetti</dc:Contributor>
		<dc:Date>2011-04-15 11:14:47</dc:Date>
		<dc:Format>text/rdf</dc:Format>
		<dc:Language>en</dc:Language>
		<skos:editorialNote>Generated by testgen.php on Thu Jun 9 14:25:25 PDT 2011.</skos:editorialNote>
		<skos:historyNote>No previous definition revisions.</skos:historyNote>
		<skos:changeNote>This is the first and only definition provided.</skos:changeNote>
		<skos:scopeNote>http://www.w3.org/2004/02/skos/core#Concept</skos:scopeNote>
		<skos:Note>SKOS properties defined in http://www.w3.org/TR/skos-primer/#secrel</skos:Note>
		<skos:inScheme rdf:resource="http://cognitiveatlas.org/tasks/"/>
		<skos:definition>No definition submitted yet.</skos:definition>
		<skos:prefLabel>Nonword Repetition Task</skos:prefLabel>
		<skos:altLabel></skos:altLabel>
</skos:Concept><skos:Concept rdf:about="http://cognitiveatlas.org/id/trm_4da88b3b0cbcc"> <dc:identifier>trm_4da88b3b0cbcc</dc:identifier>
		<dc:Title>Cognitive Atlas : Lexicon : Response Mapping Task</dc:Title>
		<dc:Description>RDF output for 'Response Mapping Task'</dc:Description>
		<dc:Type>InteractiveResource</dc:Type>
		<dc:Publisher>Cognitive Atlas</dc:Publisher>
		<dc:Creator>Cognitive Atlas RDF Generator</dc:Creator>
		<dc:Contributor>Natalie Picchetti</dc:Contributor>
		<dc:Date>2011-04-15 11:15:23</dc:Date>
		<dc:Format>text/rdf</dc:Format>
		<dc:Language>en</dc:Language>
		<skos:editorialNote>Generated by testgen.php on Thu Jun 9 14:25:25 PDT 2011.</skos:editorialNote>
		<skos:historyNote>No previous definition revisions.</skos:historyNote>
		<skos:changeNote>This is the first and only definition provided.</skos:changeNote>
		<skos:scopeNote>http://www.w3.org/2004/02/skos/core#Concept</skos:scopeNote>
		<skos:Note>SKOS properties defined in http://www.w3.org/TR/skos-primer/#secrel</skos:Note>
		<skos:inScheme rdf:resource="http://cognitiveatlas.org/tasks/"/>
		<skos:definition>No definition submitted yet.</skos:definition>
		<skos:prefLabel>Response Mapping Task</skos:prefLabel>
		<skos:altLabel></skos:altLabel>
</skos:Concept><skos:Concept rdf:about="http://cognitiveatlas.org/id/trm_4da88b63787d6"> <dc:identifier>trm_4da88b63787d6</dc:identifier>
		<dc:Title>Cognitive Atlas : Lexicon : Pursuit Rotor Task</dc:Title>
		<dc:Description>RDF output for 'Pursuit Rotor Task'</dc:Description>
		<dc:Type>InteractiveResource</dc:Type>
		<dc:Publisher>Cognitive Atlas</dc:Publisher>
		<dc:Creator>Cognitive Atlas RDF Generator</dc:Creator>
		<dc:Contributor>Natalie Picchetti</dc:Contributor>
		<dc:Date>2011-05-19 14:20:24</dc:Date>
		<dc:Format>text/rdf</dc:Format>
		<dc:Language>en</dc:Language>
		<skos:editorialNote>Generated by testgen.php on Thu Jun 9 14:25:25 PDT 2011.</skos:editorialNote>
		<skos:historyNote>Revision 2: 1 previous definitions.</skos:historyNote>
		<skos:changeNote>See http://cognitiveatlas.org/id/trm_4da88b63787d6 for complete revision history.</skos:changeNote>
		<skos:scopeNote>http://www.w3.org/2004/02/skos/core#Concept</skos:scopeNote>
		<skos:Note>SKOS properties defined in http://www.w3.org/TR/skos-primer/#secrel</skos:Note>
		<skos:inScheme rdf:resource="http://cognitiveatlas.org/tasks/"/>
		<skos:definition>The pursuit rotor task is a task used in common use in the mid 20th century which involved a participant trying to follow (pursue) a small disc on a rotating turntable. Original mechanical versions had typical rotation rates of 60 RPM, which is probably too fast for mouse-controlled versions. The PEBL version offers a simple version with multiple trials and controllable parameters that can be used as a test of hand-eye coordination. </skos:definition>
		<skos:prefLabel>Pursuit Rotor Task</skos:prefLabel>
		<skos:altLabel></skos:altLabel>
</skos:Concept><skos:Concept rdf:about="http://cognitiveatlas.org/id/trm_4da88b8b60ffb"> <dc:identifier>trm_4da88b8b60ffb</dc:identifier>
		<dc:Title>Cognitive Atlas : Lexicon : alternating runs paradigm</dc:Title>
		<dc:Description>RDF output for 'alternating runs paradigm'</dc:Description>
		<dc:Type>InteractiveResource</dc:Type>
		<dc:Publisher>Cognitive Atlas</dc:Publisher>
		<dc:Creator>Cognitive Atlas RDF Generator</dc:Creator>
		<dc:Contributor>Natalie Picchetti</dc:Contributor>
		<dc:Date>2011-04-15 11:16:43</dc:Date>
		<dc:Format>text/rdf</dc:Format>
		<dc:Language>en</dc:Language>
		<skos:editorialNote>Generated by testgen.php on Thu Jun 9 14:25:25 PDT 2011.</skos:editorialNote>
		<skos:historyNote>No previous definition revisions.</skos:historyNote>
		<skos:changeNote>This is the first and only definition provided.</skos:changeNote>
		<skos:scopeNote>http://www.w3.org/2004/02/skos/core#Concept</skos:scopeNote>
		<skos:Note>SKOS properties defined in http://www.w3.org/TR/skos-primer/#secrel</skos:Note>
		<skos:inScheme rdf:resource="http://cognitiveatlas.org/tasks/"/>
		<skos:definition>No definition submitted yet.</skos:definition>
		<skos:prefLabel>alternating runs paradigm</skos:prefLabel>
		<skos:altLabel></skos:altLabel>
</skos:Concept><skos:Concept rdf:about="http://cognitiveatlas.org/id/trm_4da88bb3c2462"> <dc:identifier>trm_4da88bb3c2462</dc:identifier>
		<dc:Title>Cognitive Atlas : Lexicon : object alternation task</dc:Title>
		<dc:Description>RDF output for 'object alternation task'</dc:Description>
		<dc:Type>InteractiveResource</dc:Type>
		<dc:Publisher>Cognitive Atlas</dc:Publisher>
		<dc:Creator>Cognitive Atlas RDF Generator</dc:Creator>
		<dc:Contributor>Natalie Picchetti</dc:Contributor>
		<dc:Date>2011-04-15 11:17:23</dc:Date>
		<dc:Format>text/rdf</dc:Format>
		<dc:Language>en</dc:Language>
		<skos:editorialNote>Generated by testgen.php on Thu Jun 9 14:25:25 PDT 2011.</skos:editorialNote>
		<skos:historyNote>No previous definition revisions.</skos:historyNote>
		<skos:changeNote>This is the first and only definition provided.</skos:changeNote>
		<skos:scopeNote>http://www.w3.org/2004/02/skos/core#Concept</skos:scopeNote>
		<skos:Note>SKOS properties defined in http://www.w3.org/TR/skos-primer/#secrel</skos:Note>
		<skos:inScheme rdf:resource="http://cognitiveatlas.org/tasks/"/>
		<skos:definition>No definition submitted yet.</skos:definition>
		<skos:prefLabel>object alternation task</skos:prefLabel>
		<skos:altLabel></skos:altLabel>
</skos:Concept><skos:Concept rdf:about="http://cognitiveatlas.org/id/trm_4da88bd4412da"> <dc:identifier>trm_4da88bd4412da</dc:identifier>
		<dc:Title>Cognitive Atlas : Lexicon : animal naming task</dc:Title>
		<dc:Description>RDF output for 'animal naming task'</dc:Description>
		<dc:Type>InteractiveResource</dc:Type>
		<dc:Publisher>Cognitive Atlas</dc:Publisher>
		<dc:Creator>Cognitive Atlas RDF Generator</dc:Creator>
		<dc:Contributor>Natalie Picchetti</dc:Contributor>
		<dc:Date>2011-04-15 11:17:56</dc:Date>
		<dc:Format>text/rdf</dc:Format>
		<dc:Language>en</dc:Language>
		<skos:editorialNote>Generated by testgen.php on Thu Jun 9 14:25:25 PDT 2011.</skos:editorialNote>
		<skos:historyNote>No previous definition revisions.</skos:historyNote>
		<skos:changeNote>This is the first and only definition provided.</skos:changeNote>
		<skos:scopeNote>http://www.w3.org/2004/02/skos/core#Concept</skos:scopeNote>
		<skos:Note>SKOS properties defined in http://www.w3.org/TR/skos-primer/#secrel</skos:Note>
		<skos:inScheme rdf:resource="http://cognitiveatlas.org/tasks/"/>
		<skos:definition>No definition submitted yet.</skos:definition>
		<skos:prefLabel>animal naming task</skos:prefLabel>
		<skos:altLabel></skos:altLabel>
</skos:Concept><skos:Concept rdf:about="http://cognitiveatlas.org/id/trm_4da88bff0507c"> <dc:identifier>trm_4da88bff0507c</dc:identifier>
		<dc:Title>Cognitive Atlas : Lexicon : CatBat task</dc:Title>
		<dc:Description>RDF output for 'CatBat task'</dc:Description>
		<dc:Type>InteractiveResource</dc:Type>
		<dc:Publisher>Cognitive Atlas</dc:Publisher>
		<dc:Creator>Cognitive Atlas RDF Generator</dc:Creator>
		<dc:Contributor>Natalie Picchetti</dc:Contributor>
		<dc:Date>2011-04-15 11:18:39</dc:Date>
		<dc:Format>text/rdf</dc:Format>
		<dc:Language>en</dc:Language>
		<skos:editorialNote>Generated by testgen.php on Thu Jun 9 14:25:25 PDT 2011.</skos:editorialNote>
		<skos:historyNote>No previous definition revisions.</skos:historyNote>
		<skos:changeNote>This is the first and only definition provided.</skos:changeNote>
		<skos:scopeNote>http://www.w3.org/2004/02/skos/core#Concept</skos:scopeNote>
		<skos:Note>SKOS properties defined in http://www.w3.org/TR/skos-primer/#secrel</skos:Note>
		<skos:inScheme rdf:resource="http://cognitiveatlas.org/tasks/"/>
		<skos:definition>No definition submitted yet.</skos:definition>
		<skos:prefLabel>CatBat task</skos:prefLabel>
		<skos:altLabel></skos:altLabel>
</skos:Concept><skos:Concept rdf:about="http://cognitiveatlas.org/id/trm_4da88c205b16b"> <dc:identifier>trm_4da88c205b16b</dc:identifier>
		<dc:Title>Cognitive Atlas : Lexicon : Haptic Illusion Task</dc:Title>
		<dc:Description>RDF output for 'Haptic Illusion Task'</dc:Description>
		<dc:Type>InteractiveResource</dc:Type>
		<dc:Publisher>Cognitive Atlas</dc:Publisher>
		<dc:Creator>Cognitive Atlas RDF Generator</dc:Creator>
		<dc:Contributor>Natalie Picchetti</dc:Contributor>
		<dc:Date>2011-04-15 11:19:12</dc:Date>
		<dc:Format>text/rdf</dc:Format>
		<dc:Language>en</dc:Language>
		<skos:editorialNote>Generated by testgen.php on Thu Jun 9 14:25:25 PDT 2011.</skos:editorialNote>
		<skos:historyNote>No previous definition revisions.</skos:historyNote>
		<skos:changeNote>This is the first and only definition provided.</skos:changeNote>
		<skos:scopeNote>http://www.w3.org/2004/02/skos/core#Concept</skos:scopeNote>
		<skos:Note>SKOS properties defined in http://www.w3.org/TR/skos-primer/#secrel</skos:Note>
		<skos:inScheme rdf:resource="http://cognitiveatlas.org/tasks/"/>
		<skos:definition>No definition submitted yet.</skos:definition>
		<skos:prefLabel>Haptic Illusion Task</skos:prefLabel>
		<skos:altLabel></skos:altLabel>
</skos:Concept><skos:Concept rdf:about="http://cognitiveatlas.org/id/trm_4da88c5302e06"> <dc:identifier>trm_4da88c5302e06</dc:identifier>
		<dc:Title>Cognitive Atlas : Lexicon : Brixton Spatial Anticipation Test</dc:Title>
		<dc:Description>RDF output for 'Brixton Spatial Anticipation Test'</dc:Description>
		<dc:Type>InteractiveResource</dc:Type>
		<dc:Publisher>Cognitive Atlas</dc:Publisher>
		<dc:Creator>Cognitive Atlas RDF Generator</dc:Creator>
		<dc:Contributor>Natalie Picchetti</dc:Contributor>
		<dc:Date>2011-04-15 11:20:03</dc:Date>
		<dc:Format>text/rdf</dc:Format>
		<dc:Language>en</dc:Language>
		<skos:editorialNote>Generated by testgen.php on Thu Jun 9 14:25:25 PDT 2011.</skos:editorialNote>
		<skos:historyNote>No previous definition revisions.</skos:historyNote>
		<skos:changeNote>This is the first and only definition provided.</skos:changeNote>
		<skos:scopeNote>http://www.w3.org/2004/02/skos/core#Concept</skos:scopeNote>
		<skos:Note>SKOS properties defined in http://www.w3.org/TR/skos-primer/#secrel</skos:Note>
		<skos:inScheme rdf:resource="http://cognitiveatlas.org/tasks/"/>
		<skos:definition>No definition submitted yet.</skos:definition>
		<skos:prefLabel>Brixton Spatial Anticipation Test</skos:prefLabel>
		<skos:altLabel></skos:altLabel>
</skos:Concept><skos:Concept rdf:about="http://cognitiveatlas.org/id/trm_4da88c904862b"> <dc:identifier>trm_4da88c904862b</dc:identifier>
		<dc:Title>Cognitive Atlas : Lexicon : Hayling Sentence Completion Test</dc:Title>
		<dc:Description>RDF output for 'Hayling Sentence Completion Test'</dc:Description>
		<dc:Type>InteractiveResource</dc:Type>
		<dc:Publisher>Cognitive Atlas</dc:Publisher>
		<dc:Creator>Cognitive Atlas RDF Generator</dc:Creator>
		<dc:Contributor>Natalie Picchetti</dc:Contributor>
		<dc:Date>2011-04-15 11:21:04</dc:Date>
		<dc:Format>text/rdf</dc:Format>
		<dc:Language>en</dc:Language>
		<skos:editorialNote>Generated by testgen.php on Thu Jun 9 14:25:25 PDT 2011.</skos:editorialNote>
		<skos:historyNote>No previous definition revisions.</skos:historyNote>
		<skos:changeNote>This is the first and only definition provided.</skos:changeNote>
		<skos:scopeNote>http://www.w3.org/2004/02/skos/core#Concept</skos:scopeNote>
		<skos:Note>SKOS properties defined in http://www.w3.org/TR/skos-primer/#secrel</skos:Note>
		<skos:inScheme rdf:resource="http://cognitiveatlas.org/tasks/"/>
		<skos:definition>No definition submitted yet.</skos:definition>
		<skos:prefLabel>Hayling Sentence Completion Test</skos:prefLabel>
		<skos:altLabel></skos:altLabel>
</skos:Concept><skos:Concept rdf:about="http://cognitiveatlas.org/id/trm_4da88cb222308"> <dc:identifier>trm_4da88cb222308</dc:identifier>
		<dc:Title>Cognitive Atlas : Lexicon : Picture Set Test</dc:Title>
		<dc:Description>RDF output for 'Picture Set Test'</dc:Description>
		<dc:Type>InteractiveResource</dc:Type>
		<dc:Publisher>Cognitive Atlas</dc:Publisher>
		<dc:Creator>Cognitive Atlas RDF Generator</dc:Creator>
		<dc:Contributor>Natalie Picchetti</dc:Contributor>
		<dc:Date>2011-04-15 11:21:38</dc:Date>
		<dc:Format>text/rdf</dc:Format>
		<dc:Language>en</dc:Language>
		<skos:editorialNote>Generated by testgen.php on Thu Jun 9 14:25:25 PDT 2011.</skos:editorialNote>
		<skos:historyNote>No previous definition revisions.</skos:historyNote>
		<skos:changeNote>This is the first and only definition provided.</skos:changeNote>
		<skos:scopeNote>http://www.w3.org/2004/02/skos/core#Concept</skos:scopeNote>
		<skos:Note>SKOS properties defined in http://www.w3.org/TR/skos-primer/#secrel</skos:Note>
		<skos:inScheme rdf:resource="http://cognitiveatlas.org/tasks/"/>
		<skos:definition>No definition submitted yet.</skos:definition>
		<skos:prefLabel>Picture Set Test</skos:prefLabel>
		<skos:altLabel></skos:altLabel>
</skos:Concept><skos:Concept rdf:about="http://cognitiveatlas.org/id/trm_4da88ec6735ad"> <dc:identifier>trm_4da88ec6735ad</dc:identifier>
		<dc:Title>Cognitive Atlas : Lexicon : Uznadze Haptic Illusion Task</dc:Title>
		<dc:Description>RDF output for 'Uznadze Haptic Illusion Task'</dc:Description>
		<dc:Type>InteractiveResource</dc:Type>
		<dc:Publisher>Cognitive Atlas</dc:Publisher>
		<dc:Creator>Cognitive Atlas RDF Generator</dc:Creator>
		<dc:Contributor>Natalie Picchetti</dc:Contributor>
		<dc:Date>2011-04-15 11:30:30</dc:Date>
		<dc:Format>text/rdf</dc:Format>
		<dc:Language>en</dc:Language>
		<skos:editorialNote>Generated by testgen.php on Thu Jun 9 14:25:25 PDT 2011.</skos:editorialNote>
		<skos:historyNote>No previous definition revisions.</skos:historyNote>
		<skos:changeNote>This is the first and only definition provided.</skos:changeNote>
		<skos:scopeNote>http://www.w3.org/2004/02/skos/core#Concept</skos:scopeNote>
		<skos:Note>SKOS properties defined in http://www.w3.org/TR/skos-primer/#secrel</skos:Note>
		<skos:inScheme rdf:resource="http://cognitiveatlas.org/tasks/"/>
		<skos:definition>No definition submitted yet.</skos:definition>
		<skos:prefLabel>Uznadze Haptic Illusion Task</skos:prefLabel>
		<skos:altLabel></skos:altLabel>
</skos:Concept><skos:Concept rdf:about="http://cognitiveatlas.org/id/trm_4da890594742a"> <dc:identifier>trm_4da890594742a</dc:identifier>
		<dc:Title>Cognitive Atlas : Lexicon : emotional regulation task</dc:Title>
		<dc:Description>RDF output for 'emotional regulation task'</dc:Description>
		<dc:Type>InteractiveResource</dc:Type>
		<dc:Publisher>Cognitive Atlas</dc:Publisher>
		<dc:Creator>Cognitive Atlas RDF Generator</dc:Creator>
		<dc:Contributor>Natalie Picchetti</dc:Contributor>
		<dc:Date>2011-04-15 11:37:13</dc:Date>
		<dc:Format>text/rdf</dc:Format>
		<dc:Language>en</dc:Language>
		<skos:editorialNote>Generated by testgen.php on Thu Jun 9 14:25:25 PDT 2011.</skos:editorialNote>
		<skos:historyNote>No previous definition revisions.</skos:historyNote>
		<skos:changeNote>This is the first and only definition provided.</skos:changeNote>
		<skos:scopeNote>http://www.w3.org/2004/02/skos/core#Concept</skos:scopeNote>
		<skos:Note>SKOS properties defined in http://www.w3.org/TR/skos-primer/#secrel</skos:Note>
		<skos:inScheme rdf:resource="http://cognitiveatlas.org/tasks/"/>
		<skos:definition>No definition submitted yet.</skos:definition>
		<skos:prefLabel>emotional regulation task</skos:prefLabel>
		<skos:altLabel></skos:altLabel>
</skos:Concept><skos:Concept rdf:about="http://cognitiveatlas.org/id/trm_4da89077f19ae"> <dc:identifier>trm_4da89077f19ae</dc:identifier>
		<dc:Title>Cognitive Atlas : Lexicon : Digit Cancellation Task</dc:Title>
		<dc:Description>RDF output for 'Digit Cancellation Task'</dc:Description>
		<dc:Type>InteractiveResource</dc:Type>
		<dc:Publisher>Cognitive Atlas</dc:Publisher>
		<dc:Creator>Cognitive Atlas RDF Generator</dc:Creator>
		<dc:Contributor>Natalie Picchetti</dc:Contributor>
		<dc:Date>2011-04-15 11:37:43</dc:Date>
		<dc:Format>text/rdf</dc:Format>
		<dc:Language>en</dc:Language>
		<skos:editorialNote>Generated by testgen.php on Thu Jun 9 14:25:25 PDT 2011.</skos:editorialNote>
		<skos:historyNote>No previous definition revisions.</skos:historyNote>
		<skos:changeNote>This is the first and only definition provided.</skos:changeNote>
		<skos:scopeNote>http://www.w3.org/2004/02/skos/core#Concept</skos:scopeNote>
		<skos:Note>SKOS properties defined in http://www.w3.org/TR/skos-primer/#secrel</skos:Note>
		<skos:inScheme rdf:resource="http://cognitiveatlas.org/tasks/"/>
		<skos:definition>No definition submitted yet.</skos:definition>
		<skos:prefLabel>Digit Cancellation Task</skos:prefLabel>
		<skos:altLabel></skos:altLabel>
</skos:Concept><skos:Concept rdf:about="http://cognitiveatlas.org/id/trm_4da89089ce0af"> <dc:identifier>trm_4da89089ce0af</dc:identifier>
		<dc:Title>Cognitive Atlas : Lexicon : Zoo Map Test</dc:Title>
		<dc:Description>RDF output for 'Zoo Map Test'</dc:Description>
		<dc:Type>InteractiveResource</dc:Type>
		<dc:Publisher>Cognitive Atlas</dc:Publisher>
		<dc:Creator>Cognitive Atlas RDF Generator</dc:Creator>
		<dc:Contributor>Natalie Picchetti</dc:Contributor>
		<dc:Date>2011-04-15 11:38:01</dc:Date>
		<dc:Format>text/rdf</dc:Format>
		<dc:Language>en</dc:Language>
		<skos:editorialNote>Generated by testgen.php on Thu Jun 9 14:25:25 PDT 2011.</skos:editorialNote>
		<skos:historyNote>No previous definition revisions.</skos:historyNote>
		<skos:changeNote>This is the first and only definition provided.</skos:changeNote>
		<skos:scopeNote>http://www.w3.org/2004/02/skos/core#Concept</skos:scopeNote>
		<skos:Note>SKOS properties defined in http://www.w3.org/TR/skos-primer/#secrel</skos:Note>
		<skos:inScheme rdf:resource="http://cognitiveatlas.org/tasks/"/>
		<skos:prefLabel>Zoo Map Test</skos:prefLabel>
		<skos:altLabel></skos:altLabel>
</skos:Concept><skos:Concept rdf:about="http://cognitiveatlas.org/id/trm_4da890a9bd7a3"> <dc:identifier>trm_4da890a9bd7a3</dc:identifier>
		<dc:Title>Cognitive Atlas : Lexicon : Morris Water Maze</dc:Title>
		<dc:Description>RDF output for 'Morris Water Maze'</dc:Description>
		<dc:Type>InteractiveResource</dc:Type>
		<dc:Publisher>Cognitive Atlas</dc:Publisher>
		<dc:Creator>Cognitive Atlas RDF Generator</dc:Creator>
		<dc:Contributor>Natalie Picchetti</dc:Contributor>
		<dc:Date>2011-04-15 11:38:33</dc:Date>
		<dc:Format>text/rdf</dc:Format>
		<dc:Language>en</dc:Language>
		<skos:editorialNote>Generated by testgen.php on Thu Jun 9 14:25:25 PDT 2011.</skos:editorialNote>
		<skos:historyNote>No previous definition revisions.</skos:historyNote>
		<skos:changeNote>This is the first and only definition provided.</skos:changeNote>
		<skos:scopeNote>http://www.w3.org/2004/02/skos/core#Concept</skos:scopeNote>
		<skos:Note>SKOS properties defined in http://www.w3.org/TR/skos-primer/#secrel</skos:Note>
		<skos:inScheme rdf:resource="http://cognitiveatlas.org/tasks/"/>
		<skos:definition>No definition submitted yet.</skos:definition>
		<skos:prefLabel>Morris Water Maze</skos:prefLabel>
		<skos:altLabel></skos:altLabel>
</skos:Concept><skos:Concept rdf:about="http://cognitiveatlas.org/id/trm_4da890cf99b9e"> <dc:identifier>trm_4da890cf99b9e</dc:identifier>
		<dc:Title>Cognitive Atlas : Lexicon : Stockings of Cambridge Task</dc:Title>
		<dc:Description>RDF output for 'Stockings of Cambridge Task'</dc:Description>
		<dc:Type>InteractiveResource</dc:Type>
		<dc:Publisher>Cognitive Atlas</dc:Publisher>
		<dc:Creator>Cognitive Atlas RDF Generator</dc:Creator>
		<dc:Contributor>Natalie Picchetti</dc:Contributor>
		<dc:Date>2011-04-15 11:39:11</dc:Date>
		<dc:Format>text/rdf</dc:Format>
		<dc:Language>en</dc:Language>
		<skos:editorialNote>Generated by testgen.php on Thu Jun 9 14:25:25 PDT 2011.</skos:editorialNote>
		<skos:historyNote>No previous definition revisions.</skos:historyNote>
		<skos:changeNote>This is the first and only definition provided.</skos:changeNote>
		<skos:scopeNote>http://www.w3.org/2004/02/skos/core#Concept</skos:scopeNote>
		<skos:Note>SKOS properties defined in http://www.w3.org/TR/skos-primer/#secrel</skos:Note>
		<skos:inScheme rdf:resource="http://cognitiveatlas.org/tasks/"/>
		<skos:definition>No definition submitted yet.</skos:definition>
		<skos:prefLabel>Stockings of Cambridge Task</skos:prefLabel>
		<skos:altLabel></skos:altLabel>
</skos:Concept><skos:Concept rdf:about="http://cognitiveatlas.org/id/trm_4da890f978492"> <dc:identifier>trm_4da890f978492</dc:identifier>
		<dc:Title>Cognitive Atlas : Lexicon : Glasgow Coma Scale</dc:Title>
		<dc:Description>RDF output for 'Glasgow Coma Scale'</dc:Description>
		<dc:Type>InteractiveResource</dc:Type>
		<dc:Publisher>Cognitive Atlas</dc:Publisher>
		<dc:Creator>Cognitive Atlas RDF Generator</dc:Creator>
		<dc:Contributor>Natalie Picchetti</dc:Contributor>
		<dc:Date>2011-04-20 16:58:30</dc:Date>
		<dc:Format>text/rdf</dc:Format>
		<dc:Language>en</dc:Language>
		<skos:editorialNote>Generated by testgen.php on Thu Jun 9 14:25:25 PDT 2011.</skos:editorialNote>
		<skos:historyNote>Revision 2: 1 previous definitions.</skos:historyNote>
		<skos:changeNote>See http://cognitiveatlas.org/id/trm_4da890f978492 for complete revision history.</skos:changeNote>
		<skos:scopeNote>http://www.w3.org/2004/02/skos/core#Concept</skos:scopeNote>
		<skos:Note>SKOS properties defined in http://www.w3.org/TR/skos-primer/#secrel</skos:Note>
		<skos:inScheme rdf:resource="http://cognitiveatlas.org/tasks/"/>
		<skos:definition>is a neurological scale that aims to give a reliable, objective way of recording the conscious state of a person for initial as well as subsequent assessment. A patient is assessed against the criteria of the scale, and the resulting points give a patient score between 3 (indicating deep unconsciousness) and either 14 (original scale) or 15 (the more widely used modified or revised scale).</skos:definition>
		<skos:prefLabel>Glasgow Coma Scale</skos:prefLabel>
		<skos:altLabel></skos:altLabel>
</skos:Concept><skos:Concept rdf:about="http://cognitiveatlas.org/id/trm_4da8911e715e3"> <dc:identifier>trm_4da8911e715e3</dc:identifier>
		<dc:Title>Cognitive Atlas : Lexicon : Early Social Communications Scales</dc:Title>
		<dc:Description>RDF output for 'Early Social Communications Scales'</dc:Description>
		<dc:Type>InteractiveResource</dc:Type>
		<dc:Publisher>Cognitive Atlas</dc:Publisher>
		<dc:Creator>Cognitive Atlas RDF Generator</dc:Creator>
		<dc:Contributor>Natalie Picchetti</dc:Contributor>
		<dc:Date>2011-04-15 11:40:30</dc:Date>
		<dc:Format>text/rdf</dc:Format>
		<dc:Language>en</dc:Language>
		<skos:editorialNote>Generated by testgen.php on Thu Jun 9 14:25:25 PDT 2011.</skos:editorialNote>
		<skos:historyNote>No previous definition revisions.</skos:historyNote>
		<skos:changeNote>This is the first and only definition provided.</skos:changeNote>
		<skos:scopeNote>http://www.w3.org/2004/02/skos/core#Concept</skos:scopeNote>
		<skos:Note>SKOS properties defined in http://www.w3.org/TR/skos-primer/#secrel</skos:Note>
		<skos:inScheme rdf:resource="http://cognitiveatlas.org/tasks/"/>
		<skos:definition>No definition submitted yet.</skos:definition>
		<skos:prefLabel>Early Social Communications Scales</skos:prefLabel>
		<skos:altLabel></skos:altLabel>
</skos:Concept><skos:Concept rdf:about="http://cognitiveatlas.org/id/trm_4da8914987ee2"> <dc:identifier>trm_4da8914987ee2</dc:identifier>
		<dc:Title>Cognitive Atlas : Lexicon : Reynell Developmental Language Scales</dc:Title>
		<dc:Description>RDF output for 'Reynell Developmental Language Scales'</dc:Description>
		<dc:Type>InteractiveResource</dc:Type>
		<dc:Publisher>Cognitive Atlas</dc:Publisher>
		<dc:Creator>Cognitive Atlas RDF Generator</dc:Creator>
		<dc:Contributor>Natalie Picchetti</dc:Contributor>
		<dc:Date>2011-04-15 11:41:13</dc:Date>
		<dc:Format>text/rdf</dc:Format>
		<dc:Language>en</dc:Language>
		<skos:editorialNote>Generated by testgen.php on Thu Jun 9 14:25:25 PDT 2011.</skos:editorialNote>
		<skos:historyNote>No previous definition revisions.</skos:historyNote>
		<skos:changeNote>This is the first and only definition provided.</skos:changeNote>
		<skos:scopeNote>http://www.w3.org/2004/02/skos/core#Concept</skos:scopeNote>
		<skos:Note>SKOS properties defined in http://www.w3.org/TR/skos-primer/#secrel</skos:Note>
		<skos:inScheme rdf:resource="http://cognitiveatlas.org/tasks/"/>
		<skos:definition>No definition submitted yet.</skos:definition>
		<skos:prefLabel>Reynell Developmental Language Scales</skos:prefLabel>
		<skos:altLabel></skos:altLabel>
</skos:Concept><skos:Concept rdf:about="http://cognitiveatlas.org/id/trm_4da891794859f"> <dc:identifier>trm_4da891794859f</dc:identifier>
		<dc:Title>Cognitive Atlas : Lexicon : MacAuthur Communicative Development Inventory</dc:Title>
		<dc:Description>RDF output for 'MacAuthur Communicative Development Inventory'</dc:Description>
		<dc:Type>InteractiveResource</dc:Type>
		<dc:Publisher>Cognitive Atlas</dc:Publisher>
		<dc:Creator>Cognitive Atlas RDF Generator</dc:Creator>
		<dc:Contributor>Natalie Picchetti</dc:Contributor>
		<dc:Date>2011-04-15 11:42:01</dc:Date>
		<dc:Format>text/rdf</dc:Format>
		<dc:Language>en</dc:Language>
		<skos:editorialNote>Generated by testgen.php on Thu Jun 9 14:25:25 PDT 2011.</skos:editorialNote>
		<skos:historyNote>No previous definition revisions.</skos:historyNote>
		<skos:changeNote>This is the first and only definition provided.</skos:changeNote>
		<skos:scopeNote>http://www.w3.org/2004/02/skos/core#Concept</skos:scopeNote>
		<skos:Note>SKOS properties defined in http://www.w3.org/TR/skos-primer/#secrel</skos:Note>
		<skos:inScheme rdf:resource="http://cognitiveatlas.org/tasks/"/>
		<skos:definition>No definition submitted yet.</skos:definition>
		<skos:prefLabel>MacAuthur Communicative Development Inventory</skos:prefLabel>
		<skos:altLabel></skos:altLabel>
</skos:Concept><skos:Concept rdf:about="http://cognitiveatlas.org/id/trm_4da891a546d8c"> <dc:identifier>trm_4da891a546d8c</dc:identifier>
		<dc:Title>Cognitive Atlas : Lexicon : Autism Diagnostic Observation Schedule</dc:Title>
		<dc:Description>RDF output for 'Autism Diagnostic Observation Schedule'</dc:Description>
		<dc:Type>InteractiveResource</dc:Type>
		<dc:Publisher>Cognitive Atlas</dc:Publisher>
		<dc:Creator>Cognitive Atlas RDF Generator</dc:Creator>
		<dc:Contributor>Natalie Picchetti</dc:Contributor>
		<dc:Date>2011-04-15 11:42:45</dc:Date>
		<dc:Format>text/rdf</dc:Format>
		<dc:Language>en</dc:Language>
		<skos:editorialNote>Generated by testgen.php on Thu Jun 9 14:25:25 PDT 2011.</skos:editorialNote>
		<skos:historyNote>No previous definition revisions.</skos:historyNote>
		<skos:changeNote>This is the first and only definition provided.</skos:changeNote>
		<skos:scopeNote>http://www.w3.org/2004/02/skos/core#Concept</skos:scopeNote>
		<skos:Note>SKOS properties defined in http://www.w3.org/TR/skos-primer/#secrel</skos:Note>
		<skos:inScheme rdf:resource="http://cognitiveatlas.org/tasks/"/>
		<skos:definition>No definition submitted yet.</skos:definition>
		<skos:prefLabel>Autism Diagnostic Observation Schedule</skos:prefLabel>
		<skos:altLabel></skos:altLabel>
</skos:Concept><skos:Concept rdf:about="http://cognitiveatlas.org/id/trm_4da891d43240c"> <dc:identifier>trm_4da891d43240c</dc:identifier>
		<dc:Title>Cognitive Atlas : Lexicon : Modified Erikson Scale of Communication Attitudes</dc:Title>
		<dc:Description>RDF output for 'Modified Erikson Scale of Communication Attitudes'</dc:Description>
		<dc:Type>InteractiveResource</dc:Type>
		<dc:Publisher>Cognitive Atlas</dc:Publisher>
		<dc:Creator>Cognitive Atlas RDF Generator</dc:Creator>
		<dc:Contributor>Natalie Picchetti</dc:Contributor>
		<dc:Date>2011-04-15 11:43:32</dc:Date>
		<dc:Format>text/rdf</dc:Format>
		<dc:Language>en</dc:Language>
		<skos:editorialNote>Generated by testgen.php on Thu Jun 9 14:25:25 PDT 2011.</skos:editorialNote>
		<skos:historyNote>No previous definition revisions.</skos:historyNote>
		<skos:changeNote>This is the first and only definition provided.</skos:changeNote>
		<skos:scopeNote>http://www.w3.org/2004/02/skos/core#Concept</skos:scopeNote>
		<skos:Note>SKOS properties defined in http://www.w3.org/TR/skos-primer/#secrel</skos:Note>
		<skos:inScheme rdf:resource="http://cognitiveatlas.org/tasks/"/>
		<skos:definition>No definition submitted yet.</skos:definition>
		<skos:prefLabel>Modified Erikson Scale of Communication Attitudes</skos:prefLabel>
		<skos:altLabel></skos:altLabel>
</skos:Concept><skos:Concept rdf:about="http://cognitiveatlas.org/id/trm_4dadbdd0b2b8c"> <dc:identifier>trm_4dadbdd0b2b8c</dc:identifier>
		<dc:Title>Cognitive Atlas : Lexicon : delayed response task</dc:Title>
		<dc:Description>RDF output for 'delayed response task'</dc:Description>
		<dc:Type>InteractiveResource</dc:Type>
		<dc:Publisher>Cognitive Atlas</dc:Publisher>
		<dc:Creator>Cognitive Atlas RDF Generator</dc:Creator>
		<dc:Contributor>Natalie Picchetti</dc:Contributor>
		<dc:Date>2011-04-19 09:52:32</dc:Date>
		<dc:Format>text/rdf</dc:Format>
		<dc:Language>en</dc:Language>
		<skos:editorialNote>Generated by testgen.php on Thu Jun 9 14:25:25 PDT 2011.</skos:editorialNote>
		<skos:historyNote>No previous definition revisions.</skos:historyNote>
		<skos:changeNote>This is the first and only definition provided.</skos:changeNote>
		<skos:scopeNote>http://www.w3.org/2004/02/skos/core#Concept</skos:scopeNote>
		<skos:Note>SKOS properties defined in http://www.w3.org/TR/skos-primer/#secrel</skos:Note>
		<skos:inScheme rdf:resource="http://cognitiveatlas.org/tasks/"/>
		<skos:definition>No definition submitted yet.</skos:definition>
		<skos:prefLabel>delayed response task</skos:prefLabel>
		<skos:altLabel></skos:altLabel>
		<skos:related rdf:resource="http://cognitiveatlas.org/id/trm_4dadbe225bdf1"/>
		<skos:example>spatial delayed response task is descended from delayed response task</skos:example>
</skos:Concept><skos:Concept rdf:about="http://cognitiveatlas.org/id/trm_4dadbe225bdf1"> <dc:identifier>trm_4dadbe225bdf1</dc:identifier>
		<dc:Title>Cognitive Atlas : Lexicon : spatial delayed response task</dc:Title>
		<dc:Description>RDF output for 'spatial delayed response task'</dc:Description>
		<dc:Type>InteractiveResource</dc:Type>
		<dc:Publisher>Cognitive Atlas</dc:Publisher>
		<dc:Creator>Cognitive Atlas RDF Generator</dc:Creator>
		<dc:Contributor>Natalie Picchetti</dc:Contributor>
		<dc:Date>2011-04-19 09:53:54</dc:Date>
		<dc:Format>text/rdf</dc:Format>
		<dc:Language>en</dc:Language>
		<skos:editorialNote>Generated by testgen.php on Thu Jun 9 14:25:25 PDT 2011.</skos:editorialNote>
		<skos:historyNote>No previous definition revisions.</skos:historyNote>
		<skos:changeNote>This is the first and only definition provided.</skos:changeNote>
		<skos:scopeNote>http://www.w3.org/2004/02/skos/core#Concept</skos:scopeNote>
		<skos:Note>SKOS properties defined in http://www.w3.org/TR/skos-primer/#secrel</skos:Note>
		<skos:inScheme rdf:resource="http://cognitiveatlas.org/tasks/"/>
		<skos:definition>No definition submitted yet.</skos:definition>
		<skos:prefLabel>spatial delayed response task</skos:prefLabel>
		<skos:altLabel></skos:altLabel>
		<skos:related rdf:resource="http://cognitiveatlas.org/id/trm_4dadbdd0b2b8c"/>
		<skos:example>spatial delayed response task is descended from delayed response task</skos:example>
</skos:Concept><skos:Concept rdf:about="http://cognitiveatlas.org/id/trm_4dadbfd771a54"> <dc:identifier>trm_4dadbfd771a54</dc:identifier>
		<dc:Title>Cognitive Atlas : Lexicon : Picture-word Stroop task</dc:Title>
		<dc:Description>RDF output for 'Picture-word Stroop task'</dc:Description>
		<dc:Type>InteractiveResource</dc:Type>
		<dc:Publisher>Cognitive Atlas</dc:Publisher>
		<dc:Creator>Cognitive Atlas RDF Generator</dc:Creator>
		<dc:Contributor>Natalie Picchetti</dc:Contributor>
		<dc:Date>2011-04-19 10:01:11</dc:Date>
		<dc:Format>text/rdf</dc:Format>
		<dc:Language>en</dc:Language>
		<skos:editorialNote>Generated by testgen.php on Thu Jun 9 14:25:25 PDT 2011.</skos:editorialNote>
		<skos:historyNote>No previous definition revisions.</skos:historyNote>
		<skos:changeNote>This is the first and only definition provided.</skos:changeNote>
		<skos:scopeNote>http://www.w3.org/2004/02/skos/core#Concept</skos:scopeNote>
		<skos:Note>SKOS properties defined in http://www.w3.org/TR/skos-primer/#secrel</skos:Note>
		<skos:inScheme rdf:resource="http://cognitiveatlas.org/tasks/"/>
		<skos:definition>No definition submitted yet.</skos:definition>
		<skos:prefLabel>Picture-word Stroop task</skos:prefLabel>
		<skos:altLabel></skos:altLabel>
		<skos:related rdf:resource="http://cognitiveatlas.org/id/tsk_4a57abb949e27"/>
		<skos:example>Picture-word Stroop task is descended from Stroop task</skos:example>
</skos:Concept></rdf:RDF>